<?xml version="1.0" encoding="UTF-8"?>
<rdf:RDF
   xmlns:ns1="https://w3id.org/omop/ontology/"
   xmlns:ns2="http://www.lesfleursdunormal.fr/static/_downloads/owlready_ontology.owl#"
   xmlns:owl="http://www.w3.org/2002/07/owl#"
   xmlns:rdf="http://www.w3.org/1999/02/22-rdf-syntax-ns#"
   xmlns:rdfs="http://www.w3.org/2000/01/rdf-schema#"
>
  <rdf:Description rdf:about="https://w3id.org/omop/ontology/end_datetime">
    <rdf:type rdf:resource="http://www.w3.org/2002/07/owl#DatatypeProperty"/>
    <rdf:type rdf:resource="http://www.w3.org/2002/07/owl#FunctionalProperty"/>
    <rdfs:comment xml:lang="en">(for ConditionEra:) The end date for the Condition Era
constructed from the individual
instances of Condition Occurrences.
It is the end date of the final
continuously recorded instance of the
Condition.</rdfs:comment>
    <rdfs:comment xml:lang="en">(for ConditionOccurrence:) If a source does not specify datetime the convention is to set the time to midnight (00:00:0000)</rdfs:comment>
    <rdfs:comment xml:lang="en">(for DeviceExposure:) If a source does not specify datetime the convention is to set the time to midnight (00:00:0000)</rdfs:comment>
    <rdfs:comment xml:lang="en">(for DoseEra:) The date the Person was no longer exposed to the dosage of the specific drug ingredient. An era is ended if there are 31 days or more between dosage records.</rdfs:comment>
    <rdfs:comment xml:lang="en">(for DrugEra:) The Drug Era End Date is the end date of the last Drug Exposure. The End Date of each Drug Exposure is either taken from the field drug_exposure_end_date or, as it is typically not available, inferred using the following rules:
For pharmacy prescription data, the date when the drug was dispensed plus the number of days of supply are used to extrapolate the End Date for the Drug Exposure. Depending on the country-specific healthcare system, this supply information is either explicitly provided in the day_supply field or inferred from package size or similar information.
For Procedure Drugs, usually the drug is administered on a single date (i.e., the administration date).
A standard Persistence Window of 30 days (gap, slack) is permitted between two subsequent such extrapolated DRUG_EXPOSURE records to be considered to be merged into a single Drug Era.</rdfs:comment>
    <rdfs:comment xml:lang="en">(for DrugExposure:) This is not required, though it is in v6. If a source does not specify datetime the convention is to set the time to midnight (00:00:0000)</rdfs:comment>
    <rdfs:comment xml:lang="en">(for VisitDetail:) If no time is given for the end date of a visit, set it to midnight (00:00:0000).</rdfs:comment>
    <rdfs:comment xml:lang="en">(for VisitOccurrence:) If no time is given for the end date of a visit, set it to midnight (00:00:0000).</rdfs:comment>
    <rdfs:domain rdf:resource="https://w3id.org/omop/ontology/DatetimeDuration"/>
    <rdfs:range rdf:resource="http://www.w3.org/2001/XMLSchema#dateTime"/>
    <ns1:omop_cdm_name rdf:datatype="http://www.w3.org/2001/XMLSchema#string">condition_era.condition_era_end_datetime#343 AS datetime</ns1:omop_cdm_name>
    <ns1:omop_cdm_name rdf:datatype="http://www.w3.org/2001/XMLSchema#string">condition_occurrence.condition_end_datetime#67 AS datetime</ns1:omop_cdm_name>
    <ns1:omop_cdm_name rdf:datatype="http://www.w3.org/2001/XMLSchema#string">device_exposure.device_exposure_end_datetime#120 AS datetime</ns1:omop_cdm_name>
    <ns1:omop_cdm_name rdf:datatype="http://www.w3.org/2001/XMLSchema#string">dose_era.dose_era_end_datetime#338 AS datetime</ns1:omop_cdm_name>
    <ns1:omop_cdm_name rdf:datatype="http://www.w3.org/2001/XMLSchema#string">drug_era.drug_era_end_datetime#329 AS datetime</ns1:omop_cdm_name>
    <ns1:omop_cdm_name rdf:datatype="http://www.w3.org/2001/XMLSchema#string">drug_exposure.drug_exposure_end_datetime#83 AS datetime</ns1:omop_cdm_name>
    <ns1:omop_cdm_name rdf:datatype="http://www.w3.org/2001/XMLSchema#string">visit_detail.visit_detail_end_datetime#48 AS datetime</ns1:omop_cdm_name>
    <ns1:omop_cdm_name rdf:datatype="http://www.w3.org/2001/XMLSchema#string">visit_occurrence.visit_end_datetime#31 AS datetime</ns1:omop_cdm_name>
  </rdf:Description>
  <rdf:Description rdf:about="https://w3id.org/omop/ontology/Event">
    <rdf:type rdf:resource="http://www.w3.org/2002/07/owl#Class"/>
    <rdfs:subClassOf rdf:nodeID="nde7e53d44aa94269b5c0c83d6d8798ccb285"/>
    <rdfs:subClassOf rdf:nodeID="nde7e53d44aa94269b5c0c83d6d8798ccb286"/>
    <rdfs:subClassOf rdf:resource="https://w3id.org/omop/ontology/OmopCDMThing"/>
  </rdf:Description>
  <rdf:Description rdf:about="https://w3id.org/omop/ontology/survey_source_identifier">
    <rdf:type rdf:resource="http://www.w3.org/2002/07/owl#DatatypeProperty"/>
    <rdf:type rdf:resource="http://www.w3.org/2002/07/owl#FunctionalProperty"/>
    <rdfs:comment xml:lang="en">(for SurveyConduct:) Unique identifier for each completed survey in source system.</rdfs:comment>
    <rdfs:domain rdf:resource="https://w3id.org/omop/ontology/SurveyConduct"/>
    <rdfs:range rdf:resource="http://www.w3.org/2001/XMLSchema#string"/>
    <ns1:omop_cdm_name rdf:datatype="http://www.w3.org/2001/XMLSchema#string">survey_conduct.survey_source_identifier#245 AS str</ns1:omop_cdm_name>
  </rdf:Description>
  <rdf:Description rdf:nodeID="nde7e53d44aa94269b5c0c83d6d8798ccb580">
    <rdf:first rdf:resource="https://w3id.org/omop/ontology/Metadata"/>
    <rdf:rest rdf:nodeID="nde7e53d44aa94269b5c0c83d6d8798ccb581"/>
  </rdf:Description>
  <rdf:Description rdf:nodeID="nde7e53d44aa94269b5c0c83d6d8798ccb71">
    <rdf:first rdf:resource="https://w3id.org/omop/ontology/Observation"/>
    <rdf:rest rdf:nodeID="nde7e53d44aa94269b5c0c83d6d8798ccb72"/>
  </rdf:Description>
  <rdf:Description rdf:about="https://w3id.org/omop/ontology/has_respondent_type">
    <rdf:type rdf:resource="http://www.w3.org/2002/07/owl#FunctionalProperty"/>
    <rdf:type rdf:resource="http://www.w3.org/2002/07/owl#ObjectProperty"/>
    <ns2:python_name rdf:datatype="http://www.w3.org/2001/XMLSchema#string">respondent_type</ns2:python_name>
    <rdfs:comment xml:lang="en">(for SurveyConduct:) This is a Concept that represents who actually recorded the answers to the survey. For example, this could be the patient or a research associate.
There is no specific domain or class for this field, just choose the one that best represents the value given in the source.</rdfs:comment>
    <rdfs:domain rdf:resource="https://w3id.org/omop/ontology/SurveyConduct"/>
    <rdfs:range rdf:resource="https://w3id.org/omop/ontology/Concept"/>
    <ns1:omop_cdm_name rdf:datatype="http://www.w3.org/2001/XMLSchema#string">survey_conduct.respondent_type_concept_id#236 AS Concept</ns1:omop_cdm_name>
  </rdf:Description>
  <rdf:Description rdf:nodeID="nde7e53d44aa94269b5c0c83d6d8798ccb45">
    <rdf:type rdf:resource="http://www.w3.org/2002/07/owl#Class"/>
    <owl:unionOf rdf:nodeID="nde7e53d44aa94269b5c0c83d6d8798ccb46"/>
  </rdf:Description>
  <rdf:Description rdf:about="https://w3id.org/omop/ontology/has_event">
    <rdf:type rdf:resource="http://www.w3.org/2002/07/owl#FunctionalProperty"/>
    <rdf:type rdf:resource="http://www.w3.org/2002/07/owl#ObjectProperty"/>
    <ns2:python_name rdf:datatype="http://www.w3.org/2001/XMLSchema#string">event</ns2:python_name>
    <rdfs:comment xml:lang="en">(for Cost:) If the Cost record is related to another record in the database, this field is the primary key of the linked record.
Put the primary key of the linked record, if applicable, here.</rdfs:comment>
    <rdfs:comment xml:lang="en">(for Observation:) If the Observation record is related to another record in the database, this field is the primary key of the linked record.
Put the primary key of the linked record, if applicable, here. See the [ETL Conventions for the OBSERVATION](https://ohdsi.github.io/CommonDataModel/cdm60.html#observation) table for more details.</rdfs:comment>
    <rdfs:domain rdf:nodeID="nde7e53d44aa94269b5c0c83d6d8798ccb118"/>
    <ns1:omop_cdm_name rdf:datatype="http://www.w3.org/2001/XMLSchema#string">cost.cost_event_id#309 AS Thing</ns1:omop_cdm_name>
    <ns1:omop_cdm_name rdf:datatype="http://www.w3.org/2001/XMLSchema#string">note.note_event_id#179 AS Thing</ns1:omop_cdm_name>
    <ns1:omop_cdm_name rdf:datatype="http://www.w3.org/2001/XMLSchema#string">observation.observation_event_id#167 AS Thing</ns1:omop_cdm_name>
  </rdf:Description>
  <rdf:Description rdf:nodeID="nde7e53d44aa94269b5c0c83d6d8798ccb15">
    <rdf:first rdf:resource="https://w3id.org/omop/ontology/Measurement"/>
    <rdf:rest rdf:nodeID="nde7e53d44aa94269b5c0c83d6d8798ccb16"/>
  </rdf:Description>
  <rdf:Description rdf:nodeID="nde7e53d44aa94269b5c0c83d6d8798ccb181">
    <rdf:type rdf:resource="http://www.w3.org/2002/07/owl#Restriction"/>
    <owl:onProperty rdf:resource="https://w3id.org/omop/ontology/valid_end_date"/>
    <owl:someValuesFrom rdf:resource="http://www.w3.org/2001/XMLSchema#date"/>
  </rdf:Description>
  <rdf:Description rdf:about="https://w3id.org/omop/ontology/Observation">
    <rdf:type rdf:resource="http://www.w3.org/2002/07/owl#Class"/>
    <rdfs:subClassOf rdf:nodeID="nde7e53d44aa94269b5c0c83d6d8798ccb512"/>
    <rdfs:subClassOf rdf:nodeID="nde7e53d44aa94269b5c0c83d6d8798ccb513"/>
    <rdfs:subClassOf rdf:nodeID="nde7e53d44aa94269b5c0c83d6d8798ccb514"/>
    <rdfs:subClassOf rdf:nodeID="nde7e53d44aa94269b5c0c83d6d8798ccb515"/>
    <rdfs:subClassOf rdf:nodeID="nde7e53d44aa94269b5c0c83d6d8798ccb516"/>
    <rdfs:subClassOf rdf:nodeID="nde7e53d44aa94269b5c0c83d6d8798ccb517"/>
    <rdfs:subClassOf rdf:nodeID="nde7e53d44aa94269b5c0c83d6d8798ccb518"/>
    <rdfs:subClassOf rdf:nodeID="nde7e53d44aa94269b5c0c83d6d8798ccb519"/>
    <rdfs:subClassOf rdf:nodeID="nde7e53d44aa94269b5c0c83d6d8798ccb520"/>
    <rdfs:subClassOf rdf:nodeID="nde7e53d44aa94269b5c0c83d6d8798ccb521"/>
    <rdfs:subClassOf rdf:nodeID="nde7e53d44aa94269b5c0c83d6d8798ccb522"/>
    <rdfs:subClassOf rdf:nodeID="nde7e53d44aa94269b5c0c83d6d8798ccb523"/>
    <rdfs:subClassOf rdf:nodeID="nde7e53d44aa94269b5c0c83d6d8798ccb524"/>
    <rdfs:subClassOf rdf:nodeID="nde7e53d44aa94269b5c0c83d6d8798ccb526"/>
    <rdfs:subClassOf rdf:nodeID="nde7e53d44aa94269b5c0c83d6d8798ccb527"/>
    <rdfs:subClassOf rdf:nodeID="nde7e53d44aa94269b5c0c83d6d8798ccb528"/>
    <rdfs:subClassOf rdf:nodeID="nde7e53d44aa94269b5c0c83d6d8798ccb529"/>
    <rdfs:subClassOf rdf:nodeID="nde7e53d44aa94269b5c0c83d6d8798ccb530"/>
    <rdfs:subClassOf rdf:nodeID="nde7e53d44aa94269b5c0c83d6d8798ccb531"/>
    <rdfs:subClassOf rdf:resource="https://w3id.org/omop/ontology/Event"/>
    <ns1:omop_cdm_name rdf:datatype="http://www.w3.org/2001/XMLSchema#string">observation</ns1:omop_cdm_name>
  </rdf:Description>
  <rdf:Description rdf:about="https://w3id.org/omop/ontology/SurveyConduct">
    <rdf:type rdf:resource="http://www.w3.org/2002/07/owl#Class"/>
    <rdfs:subClassOf rdf:nodeID="nde7e53d44aa94269b5c0c83d6d8798ccb591"/>
    <rdfs:subClassOf rdf:nodeID="nde7e53d44aa94269b5c0c83d6d8798ccb592"/>
    <rdfs:subClassOf rdf:nodeID="nde7e53d44aa94269b5c0c83d6d8798ccb593"/>
    <rdfs:subClassOf rdf:nodeID="nde7e53d44aa94269b5c0c83d6d8798ccb594"/>
    <rdfs:subClassOf rdf:nodeID="nde7e53d44aa94269b5c0c83d6d8798ccb595"/>
    <rdfs:subClassOf rdf:nodeID="nde7e53d44aa94269b5c0c83d6d8798ccb596"/>
    <rdfs:subClassOf rdf:nodeID="nde7e53d44aa94269b5c0c83d6d8798ccb597"/>
    <rdfs:subClassOf rdf:nodeID="nde7e53d44aa94269b5c0c83d6d8798ccb598"/>
    <rdfs:subClassOf rdf:nodeID="nde7e53d44aa94269b5c0c83d6d8798ccb599"/>
    <rdfs:subClassOf rdf:nodeID="nde7e53d44aa94269b5c0c83d6d8798ccb600"/>
    <rdfs:subClassOf rdf:nodeID="nde7e53d44aa94269b5c0c83d6d8798ccb601"/>
    <rdfs:subClassOf rdf:nodeID="nde7e53d44aa94269b5c0c83d6d8798ccb602"/>
    <rdfs:subClassOf rdf:nodeID="nde7e53d44aa94269b5c0c83d6d8798ccb603"/>
    <rdfs:subClassOf rdf:nodeID="nde7e53d44aa94269b5c0c83d6d8798ccb604"/>
    <rdfs:subClassOf rdf:nodeID="nde7e53d44aa94269b5c0c83d6d8798ccb605"/>
    <rdfs:subClassOf rdf:nodeID="nde7e53d44aa94269b5c0c83d6d8798ccb606"/>
    <rdfs:subClassOf rdf:nodeID="nde7e53d44aa94269b5c0c83d6d8798ccb607"/>
    <rdfs:subClassOf rdf:nodeID="nde7e53d44aa94269b5c0c83d6d8798ccb609"/>
    <rdfs:subClassOf rdf:nodeID="nde7e53d44aa94269b5c0c83d6d8798ccb610"/>
    <rdfs:subClassOf rdf:nodeID="nde7e53d44aa94269b5c0c83d6d8798ccb611"/>
    <rdfs:subClassOf rdf:nodeID="nde7e53d44aa94269b5c0c83d6d8798ccb612"/>
    <rdfs:subClassOf rdf:nodeID="nde7e53d44aa94269b5c0c83d6d8798ccb613"/>
    <rdfs:subClassOf rdf:nodeID="nde7e53d44aa94269b5c0c83d6d8798ccb614"/>
    <rdfs:subClassOf rdf:nodeID="nde7e53d44aa94269b5c0c83d6d8798ccb615"/>
    <rdfs:subClassOf rdf:nodeID="nde7e53d44aa94269b5c0c83d6d8798ccb616"/>
    <rdfs:subClassOf rdf:nodeID="nde7e53d44aa94269b5c0c83d6d8798ccb617"/>
    <rdfs:subClassOf rdf:nodeID="nde7e53d44aa94269b5c0c83d6d8798ccb618"/>
    <rdfs:subClassOf rdf:nodeID="nde7e53d44aa94269b5c0c83d6d8798ccb619"/>
    <rdfs:subClassOf rdf:nodeID="nde7e53d44aa94269b5c0c83d6d8798ccb620"/>
    <rdfs:subClassOf rdf:nodeID="nde7e53d44aa94269b5c0c83d6d8798ccb621"/>
    <rdfs:subClassOf rdf:resource="https://w3id.org/omop/ontology/OmopCDMThing"/>
    <ns1:omop_cdm_name rdf:datatype="http://www.w3.org/2001/XMLSchema#string">survey_conduct</ns1:omop_cdm_name>
  </rdf:Description>
  <rdf:Description rdf:nodeID="nde7e53d44aa94269b5c0c83d6d8798ccb280">
    <rdf:type rdf:resource="http://www.w3.org/2002/07/owl#Restriction"/>
    <owl:onProperty rdf:resource="https://w3id.org/omop/ontology/name"/>
    <owl:someValuesFrom rdf:resource="http://www.w3.org/2001/XMLSchema#string"/>
  </rdf:Description>
  <rdf:Description rdf:about="https://w3id.org/omop/ontology/Cost">
    <rdf:type rdf:resource="http://www.w3.org/2002/07/owl#Class"/>
    <rdfs:subClassOf rdf:nodeID="nde7e53d44aa94269b5c0c83d6d8798ccb492"/>
    <rdfs:subClassOf rdf:nodeID="nde7e53d44aa94269b5c0c83d6d8798ccb493"/>
    <rdfs:subClassOf rdf:nodeID="nde7e53d44aa94269b5c0c83d6d8798ccb494"/>
    <rdfs:subClassOf rdf:nodeID="nde7e53d44aa94269b5c0c83d6d8798ccb495"/>
    <rdfs:subClassOf rdf:nodeID="nde7e53d44aa94269b5c0c83d6d8798ccb496"/>
    <rdfs:subClassOf rdf:nodeID="nde7e53d44aa94269b5c0c83d6d8798ccb497"/>
    <rdfs:subClassOf rdf:nodeID="nde7e53d44aa94269b5c0c83d6d8798ccb498"/>
    <rdfs:subClassOf rdf:nodeID="nde7e53d44aa94269b5c0c83d6d8798ccb499"/>
    <rdfs:subClassOf rdf:nodeID="nde7e53d44aa94269b5c0c83d6d8798ccb500"/>
    <rdfs:subClassOf rdf:nodeID="nde7e53d44aa94269b5c0c83d6d8798ccb501"/>
    <rdfs:subClassOf rdf:nodeID="nde7e53d44aa94269b5c0c83d6d8798ccb502"/>
    <rdfs:subClassOf rdf:nodeID="nde7e53d44aa94269b5c0c83d6d8798ccb503"/>
    <rdfs:subClassOf rdf:nodeID="nde7e53d44aa94269b5c0c83d6d8798ccb505"/>
    <rdfs:subClassOf rdf:nodeID="nde7e53d44aa94269b5c0c83d6d8798ccb506"/>
    <rdfs:subClassOf rdf:nodeID="nde7e53d44aa94269b5c0c83d6d8798ccb507"/>
    <rdfs:subClassOf rdf:nodeID="nde7e53d44aa94269b5c0c83d6d8798ccb508"/>
    <rdfs:subClassOf rdf:nodeID="nde7e53d44aa94269b5c0c83d6d8798ccb509"/>
    <rdfs:subClassOf rdf:nodeID="nde7e53d44aa94269b5c0c83d6d8798ccb510"/>
    <rdfs:subClassOf rdf:nodeID="nde7e53d44aa94269b5c0c83d6d8798ccb511"/>
    <rdfs:subClassOf rdf:resource="https://w3id.org/omop/ontology/OmopCDMThing"/>
    <ns1:omop_cdm_name rdf:datatype="http://www.w3.org/2001/XMLSchema#string">cost</ns1:omop_cdm_name>
  </rdf:Description>
  <rdf:Description rdf:nodeID="nde7e53d44aa94269b5c0c83d6d8798ccb189">
    <rdf:type rdf:resource="http://www.w3.org/2002/07/owl#Restriction"/>
    <owl:allValuesFrom rdf:resource="https://w3id.org/omop/ontology/Concept"/>
    <owl:onProperty rdf:resource="https://w3id.org/omop/ontology/has_cause"/>
  </rdf:Description>
  <rdf:Description rdf:nodeID="nde7e53d44aa94269b5c0c83d6d8798ccb102">
    <rdf:type rdf:resource="http://www.w3.org/2002/07/owl#Restriction"/>
    <owl:allValuesFrom rdf:resource="https://w3id.org/omop/ontology/Concept"/>
    <owl:onProperty rdf:resource="https://w3id.org/omop/ontology/has_concept"/>
  </rdf:Description>
  <rdf:Description rdf:nodeID="nde7e53d44aa94269b5c0c83d6d8798ccb282">
    <rdf:type rdf:resource="http://www.w3.org/2002/07/owl#Restriction"/>
    <owl:allValuesFrom rdf:resource="http://www.w3.org/2001/XMLSchema#date"/>
    <owl:onProperty rdf:resource="https://w3id.org/omop/ontology/cdm_release_date"/>
  </rdf:Description>
  <rdf:Description rdf:about="https://w3id.org/omop/ontology/value_as_datetime">
    <rdf:type rdf:resource="http://www.w3.org/2002/07/owl#DatatypeProperty"/>
    <rdf:type rdf:resource="http://www.w3.org/2002/07/owl#FunctionalProperty"/>
    <rdfs:comment xml:lang="en">(for Observation:) It is possible that some Observation records might store a result as a date value.</rdfs:comment>
    <rdfs:domain rdf:resource="https://w3id.org/omop/ontology/Observation"/>
    <rdfs:range rdf:resource="http://www.w3.org/2001/XMLSchema#dateTime"/>
    <ns1:omop_cdm_name rdf:datatype="http://www.w3.org/2001/XMLSchema#string">observation.value_as_datetime#169 AS datetime</ns1:omop_cdm_name>
  </rdf:Description>
  <rdf:Description rdf:nodeID="nde7e53d44aa94269b5c0c83d6d8798ccb605">
    <rdf:type rdf:resource="http://www.w3.org/2002/07/owl#Restriction"/>
    <owl:allValuesFrom rdf:resource="http://www.w3.org/2001/XMLSchema#integer"/>
    <owl:onProperty rdf:resource="https://w3id.org/omop/ontology/validated_survey_source_value"/>
  </rdf:Description>
  <rdf:Description rdf:about="https://w3id.org/omop/ontology/Measurement">
    <rdf:type rdf:resource="http://www.w3.org/2002/07/owl#Class"/>
    <rdfs:subClassOf rdf:nodeID="nde7e53d44aa94269b5c0c83d6d8798ccb453"/>
    <rdfs:subClassOf rdf:nodeID="nde7e53d44aa94269b5c0c83d6d8798ccb454"/>
    <rdfs:subClassOf rdf:nodeID="nde7e53d44aa94269b5c0c83d6d8798ccb455"/>
    <rdfs:subClassOf rdf:nodeID="nde7e53d44aa94269b5c0c83d6d8798ccb456"/>
    <rdfs:subClassOf rdf:nodeID="nde7e53d44aa94269b5c0c83d6d8798ccb457"/>
    <rdfs:subClassOf rdf:nodeID="nde7e53d44aa94269b5c0c83d6d8798ccb458"/>
    <rdfs:subClassOf rdf:nodeID="nde7e53d44aa94269b5c0c83d6d8798ccb459"/>
    <rdfs:subClassOf rdf:nodeID="nde7e53d44aa94269b5c0c83d6d8798ccb460"/>
    <rdfs:subClassOf rdf:nodeID="nde7e53d44aa94269b5c0c83d6d8798ccb461"/>
    <rdfs:subClassOf rdf:nodeID="nde7e53d44aa94269b5c0c83d6d8798ccb462"/>
    <rdfs:subClassOf rdf:nodeID="nde7e53d44aa94269b5c0c83d6d8798ccb464"/>
    <rdfs:subClassOf rdf:nodeID="nde7e53d44aa94269b5c0c83d6d8798ccb465"/>
    <rdfs:subClassOf rdf:nodeID="nde7e53d44aa94269b5c0c83d6d8798ccb466"/>
    <rdfs:subClassOf rdf:nodeID="nde7e53d44aa94269b5c0c83d6d8798ccb467"/>
    <rdfs:subClassOf rdf:nodeID="nde7e53d44aa94269b5c0c83d6d8798ccb468"/>
    <rdfs:subClassOf rdf:nodeID="nde7e53d44aa94269b5c0c83d6d8798ccb469"/>
    <rdfs:subClassOf rdf:nodeID="nde7e53d44aa94269b5c0c83d6d8798ccb470"/>
    <rdfs:subClassOf rdf:nodeID="nde7e53d44aa94269b5c0c83d6d8798ccb471"/>
    <rdfs:subClassOf rdf:resource="https://w3id.org/omop/ontology/Event"/>
    <rdfs:subClassOf rdf:resource="https://w3id.org/omop/ontology/Occurrence"/>
    <ns1:omop_cdm_name rdf:datatype="http://www.w3.org/2001/XMLSchema#string">measurement</ns1:omop_cdm_name>
  </rdf:Description>
  <rdf:Description rdf:nodeID="nde7e53d44aa94269b5c0c83d6d8798ccb689">
    <rdf:type rdf:resource="http://www.w3.org/2002/07/owl#Restriction"/>
    <owl:onProperty rdf:resource="https://w3id.org/omop/ontology/code"/>
    <owl:someValuesFrom rdf:resource="http://www.w3.org/2001/XMLSchema#string"/>
  </rdf:Description>
  <rdf:Description rdf:nodeID="nde7e53d44aa94269b5c0c83d6d8798ccb184">
    <rdf:type rdf:resource="http://www.w3.org/2002/07/owl#Restriction"/>
    <owl:onProperty rdf:resource="https://w3id.org/omop/ontology/concept_id_2"/>
    <owl:someValuesFrom rdf:resource="http://www.w3.org/2001/XMLSchema#integer"/>
  </rdf:Description>
  <rdf:Description rdf:about="https://w3id.org/omop/ontology/admitted_from_source_value">
    <rdf:type rdf:resource="http://www.w3.org/2002/07/owl#DatatypeProperty"/>
    <rdf:type rdf:resource="http://www.w3.org/2002/07/owl#FunctionalProperty"/>
    <rdfs:comment xml:lang="en">(for VisitDetail:) Use this field to determine where the patient was admitted from. This concept is part of the visit domain and can indicate if a patient was admitted to the hospital from a long-term care facility, for example.
If available, map the admitted_from_source_value to a standard concept in the visit domain. If not available, map to 0. [Accepted Concepts](https://athena.ohdsi.org/search-terms/terms?domain=Visit&amp;standardConcept=Standard&amp;page=1&amp;pageSize=15&amp;query=).</rdfs:comment>
    <rdfs:comment xml:lang="en">(for VisitOccurrence:) This information may be called something different in the source data but the field is meant to contain a value indicating where a person was admitted from. Typically this applies only to visits that have a length of stay, like inpatient visits or long-term care visits.</rdfs:comment>
    <rdfs:domain rdf:nodeID="nde7e53d44aa94269b5c0c83d6d8798ccb33"/>
    <ns1:omop_cdm_name rdf:datatype="http://www.w3.org/2001/XMLSchema#string">visit_detail.admitted_from_source_value#55 AS int</ns1:omop_cdm_name>
    <ns1:omop_cdm_name rdf:datatype="http://www.w3.org/2001/XMLSchema#string">visit_occurrence.admitted_from_source_value#38 AS str</ns1:omop_cdm_name>
  </rdf:Description>
  <rdf:Description rdf:about="https://w3id.org/omop/ontology/start_datetime">
    <rdf:type rdf:resource="http://www.w3.org/2002/07/owl#DatatypeProperty"/>
    <rdf:type rdf:resource="http://www.w3.org/2002/07/owl#FunctionalProperty"/>
    <rdfs:comment xml:lang="en">(for ConditionEra:) The start date for the Condition Era
constructed from the individual
instances of Condition Occurrences.
It is the start date of the very first
chronologically recorded instance of
the condition with at least 31 days since any prior record of the same Condition.</rdfs:comment>
    <rdfs:comment xml:lang="en">(for ConditionOccurrence:) If a source does not specify datetime the convention is to set the time to midnight (00:00:0000)</rdfs:comment>
    <rdfs:comment xml:lang="en">(for DeviceExposure:) This is not required, though it is in v6. If a source does not specify datetime the convention is to set the time to midnight (00:00:0000)</rdfs:comment>
    <rdfs:comment xml:lang="en">(for DoseEra:) The date the Person started on the specific dosage, with at least 31 days since any prior exposure.</rdfs:comment>
    <rdfs:comment xml:lang="en">(for DrugEra:) The Drug Era Start Date is the start date of the first Drug Exposure for a given ingredient, with at least 31 days since the previous exposure.</rdfs:comment>
    <rdfs:comment xml:lang="en">(for DrugExposure:) This is not required, though it is in v6. If a source does not specify datetime the convention is to set the time to midnight (00:00:0000)</rdfs:comment>
    <rdfs:comment xml:lang="en">(for VisitDetail:) If no time is given for the start date of a visit, set it to midnight (00:00:0000).</rdfs:comment>
    <rdfs:comment xml:lang="en">(for VisitOccurrence:) If no time is given for the start date of a visit, set it to midnight (00:00:0000).</rdfs:comment>
    <rdfs:domain rdf:resource="https://w3id.org/omop/ontology/DatetimeDuration"/>
    <rdfs:range rdf:resource="http://www.w3.org/2001/XMLSchema#dateTime"/>
    <ns1:omop_cdm_name rdf:datatype="http://www.w3.org/2001/XMLSchema#string">condition_era.condition_era_start_datetime#342 AS datetime</ns1:omop_cdm_name>
    <ns1:omop_cdm_name rdf:datatype="http://www.w3.org/2001/XMLSchema#string">condition_occurrence.condition_start_datetime#65 AS datetime</ns1:omop_cdm_name>
    <ns1:omop_cdm_name rdf:datatype="http://www.w3.org/2001/XMLSchema#string">device_exposure.device_exposure_start_datetime#118 AS datetime</ns1:omop_cdm_name>
    <ns1:omop_cdm_name rdf:datatype="http://www.w3.org/2001/XMLSchema#string">dose_era.dose_era_start_datetime#337 AS datetime</ns1:omop_cdm_name>
    <ns1:omop_cdm_name rdf:datatype="http://www.w3.org/2001/XMLSchema#string">drug_era.drug_era_start_datetime#328 AS datetime</ns1:omop_cdm_name>
    <ns1:omop_cdm_name rdf:datatype="http://www.w3.org/2001/XMLSchema#string">drug_exposure.drug_exposure_start_datetime#81 AS datetime</ns1:omop_cdm_name>
    <ns1:omop_cdm_name rdf:datatype="http://www.w3.org/2001/XMLSchema#string">visit_detail.visit_detail_start_datetime#46 AS datetime</ns1:omop_cdm_name>
    <ns1:omop_cdm_name rdf:datatype="http://www.w3.org/2001/XMLSchema#string">visit_occurrence.visit_start_datetime#29 AS datetime</ns1:omop_cdm_name>
  </rdf:Description>
  <rdf:Description rdf:about="https://w3id.org/omop/ontology/Death">
    <rdf:type rdf:resource="http://www.w3.org/2002/07/owl#Class"/>
    <rdfs:subClassOf rdf:nodeID="nde7e53d44aa94269b5c0c83d6d8798ccb188"/>
    <rdfs:subClassOf rdf:nodeID="nde7e53d44aa94269b5c0c83d6d8798ccb189"/>
    <rdfs:subClassOf rdf:nodeID="nde7e53d44aa94269b5c0c83d6d8798ccb190"/>
    <rdfs:subClassOf rdf:nodeID="nde7e53d44aa94269b5c0c83d6d8798ccb191"/>
    <rdfs:subClassOf rdf:resource="https://w3id.org/omop/ontology/Event"/>
    <ns1:omop_cdm_name rdf:datatype="http://www.w3.org/2001/XMLSchema#string">death</ns1:omop_cdm_name>
  </rdf:Description>
  <rdf:Description rdf:nodeID="nde7e53d44aa94269b5c0c83d6d8798ccb382">
    <rdf:type rdf:resource="http://www.w3.org/2002/07/owl#Restriction"/>
    <owl:allValuesFrom rdf:resource="http://www.w3.org/2001/XMLSchema#string"/>
    <owl:onProperty rdf:resource="https://w3id.org/omop/ontology/stop_reason"/>
  </rdf:Description>
  <rdf:Description rdf:about="https://w3id.org/omop/ontology/fact_id_1">
    <rdf:type rdf:resource="http://www.w3.org/2002/07/owl#DatatypeProperty"/>
    <rdf:type rdf:resource="http://www.w3.org/2002/07/owl#FunctionalProperty"/>
    <rdfs:domain rdf:resource="https://w3id.org/omop/ontology/FactRelationship"/>
    <rdfs:range rdf:resource="http://www.w3.org/2001/XMLSchema#integer"/>
    <ns1:omop_cdm_name rdf:datatype="http://www.w3.org/2001/XMLSchema#string">fact_relationship.fact_id_1#223 AS int</ns1:omop_cdm_name>
  </rdf:Description>
  <rdf:Description rdf:about="https://w3id.org/omop/ontology/Concept">
    <rdf:type rdf:resource="http://www.w3.org/2002/07/owl#Class"/>
    <rdfs:subClassOf rdf:nodeID="nde7e53d44aa94269b5c0c83d6d8798ccb676"/>
    <rdfs:subClassOf rdf:nodeID="nde7e53d44aa94269b5c0c83d6d8798ccb677"/>
    <rdfs:subClassOf rdf:nodeID="nde7e53d44aa94269b5c0c83d6d8798ccb678"/>
    <rdfs:subClassOf rdf:nodeID="nde7e53d44aa94269b5c0c83d6d8798ccb679"/>
    <rdfs:subClassOf rdf:nodeID="nde7e53d44aa94269b5c0c83d6d8798ccb680"/>
    <rdfs:subClassOf rdf:nodeID="nde7e53d44aa94269b5c0c83d6d8798ccb681"/>
    <rdfs:subClassOf rdf:nodeID="nde7e53d44aa94269b5c0c83d6d8798ccb682"/>
    <rdfs:subClassOf rdf:nodeID="nde7e53d44aa94269b5c0c83d6d8798ccb683"/>
    <rdfs:subClassOf rdf:nodeID="nde7e53d44aa94269b5c0c83d6d8798ccb684"/>
    <rdfs:subClassOf rdf:nodeID="nde7e53d44aa94269b5c0c83d6d8798ccb685"/>
    <rdfs:subClassOf rdf:nodeID="nde7e53d44aa94269b5c0c83d6d8798ccb686"/>
    <rdfs:subClassOf rdf:nodeID="nde7e53d44aa94269b5c0c83d6d8798ccb687"/>
    <rdfs:subClassOf rdf:nodeID="nde7e53d44aa94269b5c0c83d6d8798ccb688"/>
    <rdfs:subClassOf rdf:nodeID="nde7e53d44aa94269b5c0c83d6d8798ccb689"/>
    <rdfs:subClassOf rdf:nodeID="nde7e53d44aa94269b5c0c83d6d8798ccb690"/>
    <rdfs:subClassOf rdf:nodeID="nde7e53d44aa94269b5c0c83d6d8798ccb691"/>
    <rdfs:subClassOf rdf:resource="https://w3id.org/omop/ontology/OmopCDMThing"/>
    <ns1:omop_cdm_name rdf:datatype="http://www.w3.org/2001/XMLSchema#string">concept</ns1:omop_cdm_name>
  </rdf:Description>
  <rdf:Description rdf:about="https://w3id.org/omop/ontology/has_relationship">
    <rdf:type rdf:resource="http://www.w3.org/2002/07/owl#FunctionalProperty"/>
    <rdf:type rdf:resource="http://www.w3.org/2002/07/owl#ObjectProperty"/>
    <ns2:python_name rdf:datatype="http://www.w3.org/2001/XMLSchema#string">relationship</ns2:python_name>
    <rdfs:comment xml:lang="en">(for ConceptRelationship:) The relationship between CONCEPT_ID_1 and CONCEPT_ID_2. Please see the [Vocabulary Conventions](https://ohdsi.github.io/CommonDataModel/dataModelConventions.html#concept_relationships). for more information.</rdfs:comment>
    <rdfs:domain rdf:nodeID="nde7e53d44aa94269b5c0c83d6d8798ccb129"/>
    <ns1:omop_cdm_name rdf:datatype="http://www.w3.org/2001/XMLSchema#string">concept_relationship.relationship_id#385 AS Relationship</ns1:omop_cdm_name>
    <ns1:omop_cdm_name rdf:datatype="http://www.w3.org/2001/XMLSchema#string">fact_relationship.relationship_concept_id#226 AS Concept</ns1:omop_cdm_name>
  </rdf:Description>
  <rdf:Description rdf:nodeID="nde7e53d44aa94269b5c0c83d6d8798ccb578">
    <rdf:first rdf:resource="https://w3id.org/omop/ontology/CohortDefinition"/>
    <rdf:rest rdf:nodeID="nde7e53d44aa94269b5c0c83d6d8798ccb579"/>
  </rdf:Description>
  <rdf:Description rdf:nodeID="nde7e53d44aa94269b5c0c83d6d8798ccb393">
    <rdf:type rdf:resource="http://www.w3.org/2002/07/owl#Restriction"/>
    <owl:onProperty rdf:nodeID="nde7e53d44aa94269b5c0c83d6d8798ccb394"/>
    <owl:someValuesFrom rdf:resource="https://w3id.org/omop/ontology/Person"/>
  </rdf:Description>
  <rdf:Description rdf:about="https://w3id.org/omop/ontology/has_payer_source">
    <rdf:type rdf:resource="http://www.w3.org/2002/07/owl#FunctionalProperty"/>
    <rdf:type rdf:resource="http://www.w3.org/2002/07/owl#ObjectProperty"/>
    <ns2:python_name rdf:datatype="http://www.w3.org/2001/XMLSchema#string">payer_source</ns2:python_name>
    <rdfs:comment xml:lang="en">(for PayerPlanPeriod:) If the source data codes the Payer in an OMOP supported vocabulary store the concept_id here. If not available, set to 0.</rdfs:comment>
    <rdfs:domain rdf:resource="https://w3id.org/omop/ontology/PayerPlanPeriod"/>
    <rdfs:range rdf:resource="https://w3id.org/omop/ontology/Concept"/>
    <ns1:omop_cdm_name rdf:datatype="http://www.w3.org/2001/XMLSchema#string">payer_plan_period.payer_source_concept_id#293 AS Concept</ns1:omop_cdm_name>
  </rdf:Description>
  <rdf:Description rdf:nodeID="nde7e53d44aa94269b5c0c83d6d8798ccb104">
    <rdf:type rdf:resource="http://www.w3.org/2002/07/owl#Restriction"/>
    <owl:onProperty rdf:resource="https://w3id.org/omop/ontology/has_location"/>
    <owl:someValuesFrom rdf:resource="https://w3id.org/omop/ontology/Location"/>
  </rdf:Description>
  <rdf:Description rdf:about="https://w3id.org/omop/ontology/Exposure">
    <rdf:type rdf:resource="http://www.w3.org/2002/07/owl#Class"/>
    <rdfs:subClassOf rdf:nodeID="nde7e53d44aa94269b5c0c83d6d8798ccb203"/>
    <rdfs:subClassOf rdf:nodeID="nde7e53d44aa94269b5c0c83d6d8798ccb204"/>
    <rdfs:subClassOf rdf:nodeID="nde7e53d44aa94269b5c0c83d6d8798ccb205"/>
    <rdfs:subClassOf rdf:nodeID="nde7e53d44aa94269b5c0c83d6d8798ccb206"/>
    <rdfs:subClassOf rdf:nodeID="nde7e53d44aa94269b5c0c83d6d8798ccb207"/>
    <rdfs:subClassOf rdf:nodeID="nde7e53d44aa94269b5c0c83d6d8798ccb208"/>
    <rdfs:subClassOf rdf:nodeID="nde7e53d44aa94269b5c0c83d6d8798ccb209"/>
    <rdfs:subClassOf rdf:nodeID="nde7e53d44aa94269b5c0c83d6d8798ccb210"/>
    <rdfs:subClassOf rdf:resource="https://w3id.org/omop/ontology/ClinicalElement"/>
    <rdfs:subClassOf rdf:resource="https://w3id.org/omop/ontology/DateDuration"/>
    <rdfs:subClassOf rdf:resource="https://w3id.org/omop/ontology/DatetimeDuration"/>
  </rdf:Description>
  <rdf:Description rdf:nodeID="nde7e53d44aa94269b5c0c83d6d8798ccb161">
    <rdf:type rdf:resource="http://www.w3.org/2002/07/owl#Restriction"/>
    <owl:onProperty rdf:resource="https://w3id.org/omop/ontology/has_relationship"/>
    <owl:someValuesFrom rdf:resource="https://w3id.org/omop/ontology/Concept"/>
  </rdf:Description>
  <rdf:Description rdf:about="https://w3id.org/omop/ontology/numerator_value">
    <rdf:type rdf:resource="http://www.w3.org/2002/07/owl#DatatypeProperty"/>
    <rdf:type rdf:resource="http://www.w3.org/2002/07/owl#FunctionalProperty"/>
    <rdfs:comment xml:lang="en">(for DrugStrength:) The concentration of the active ingredient contained within the drug product.</rdfs:comment>
    <rdfs:domain rdf:resource="https://w3id.org/omop/ontology/DrugStrength"/>
    <rdfs:range rdf:resource="http://www.w3.org/2001/XMLSchema#decimal"/>
    <ns1:omop_cdm_name rdf:datatype="http://www.w3.org/2001/XMLSchema#string">drug_strength.numerator_value#415 AS float</ns1:omop_cdm_name>
  </rdf:Description>
  <rdf:Description rdf:about="https://w3id.org/omop/ontology/BaseVisit">
    <rdf:type rdf:resource="http://www.w3.org/2002/07/owl#Class"/>
    <rdfs:subClassOf rdf:nodeID="nde7e53d44aa94269b5c0c83d6d8798ccb434"/>
    <rdfs:subClassOf rdf:nodeID="nde7e53d44aa94269b5c0c83d6d8798ccb435"/>
    <rdfs:subClassOf rdf:nodeID="nde7e53d44aa94269b5c0c83d6d8798ccb436"/>
    <rdfs:subClassOf rdf:nodeID="nde7e53d44aa94269b5c0c83d6d8798ccb437"/>
    <rdfs:subClassOf rdf:nodeID="nde7e53d44aa94269b5c0c83d6d8798ccb438"/>
    <rdfs:subClassOf rdf:nodeID="nde7e53d44aa94269b5c0c83d6d8798ccb439"/>
    <rdfs:subClassOf rdf:nodeID="nde7e53d44aa94269b5c0c83d6d8798ccb440"/>
    <rdfs:subClassOf rdf:nodeID="nde7e53d44aa94269b5c0c83d6d8798ccb441"/>
    <rdfs:subClassOf rdf:nodeID="nde7e53d44aa94269b5c0c83d6d8798ccb442"/>
    <rdfs:subClassOf rdf:nodeID="nde7e53d44aa94269b5c0c83d6d8798ccb443"/>
    <rdfs:subClassOf rdf:nodeID="nde7e53d44aa94269b5c0c83d6d8798ccb444"/>
    <rdfs:subClassOf rdf:nodeID="nde7e53d44aa94269b5c0c83d6d8798ccb445"/>
    <rdfs:subClassOf rdf:nodeID="nde7e53d44aa94269b5c0c83d6d8798ccb446"/>
    <rdfs:subClassOf rdf:nodeID="nde7e53d44aa94269b5c0c83d6d8798ccb447"/>
    <rdfs:subClassOf rdf:nodeID="nde7e53d44aa94269b5c0c83d6d8798ccb448"/>
    <rdfs:subClassOf rdf:nodeID="nde7e53d44aa94269b5c0c83d6d8798ccb449"/>
    <rdfs:subClassOf rdf:nodeID="nde7e53d44aa94269b5c0c83d6d8798ccb450"/>
    <rdfs:subClassOf rdf:nodeID="nde7e53d44aa94269b5c0c83d6d8798ccb451"/>
    <rdfs:subClassOf rdf:nodeID="nde7e53d44aa94269b5c0c83d6d8798ccb452"/>
    <rdfs:subClassOf rdf:resource="https://w3id.org/omop/ontology/DateDuration"/>
    <rdfs:subClassOf rdf:resource="https://w3id.org/omop/ontology/DatetimeDuration"/>
    <rdfs:subClassOf rdf:resource="https://w3id.org/omop/ontology/Occurrence"/>
  </rdf:Description>
  <rdf:Description rdf:nodeID="nde7e53d44aa94269b5c0c83d6d8798ccb544">
    <rdf:type rdf:resource="http://www.w3.org/2002/07/owl#Restriction"/>
    <owl:onProperty rdf:nodeID="nde7e53d44aa94269b5c0c83d6d8798ccb545"/>
    <owl:someValuesFrom rdf:resource="https://w3id.org/omop/ontology/Person"/>
  </rdf:Description>
  <rdf:Description rdf:about="https://w3id.org/omop/ontology/Note">
    <rdf:type rdf:resource="http://www.w3.org/2002/07/owl#Class"/>
    <rdfs:subClassOf rdf:nodeID="nde7e53d44aa94269b5c0c83d6d8798ccb416"/>
    <rdfs:subClassOf rdf:nodeID="nde7e53d44aa94269b5c0c83d6d8798ccb417"/>
    <rdfs:subClassOf rdf:nodeID="nde7e53d44aa94269b5c0c83d6d8798ccb418"/>
    <rdfs:subClassOf rdf:nodeID="nde7e53d44aa94269b5c0c83d6d8798ccb420"/>
    <rdfs:subClassOf rdf:nodeID="nde7e53d44aa94269b5c0c83d6d8798ccb421"/>
    <rdfs:subClassOf rdf:nodeID="nde7e53d44aa94269b5c0c83d6d8798ccb422"/>
    <rdfs:subClassOf rdf:nodeID="nde7e53d44aa94269b5c0c83d6d8798ccb423"/>
    <rdfs:subClassOf rdf:nodeID="nde7e53d44aa94269b5c0c83d6d8798ccb424"/>
    <rdfs:subClassOf rdf:nodeID="nde7e53d44aa94269b5c0c83d6d8798ccb425"/>
    <rdfs:subClassOf rdf:nodeID="nde7e53d44aa94269b5c0c83d6d8798ccb426"/>
    <rdfs:subClassOf rdf:nodeID="nde7e53d44aa94269b5c0c83d6d8798ccb427"/>
    <rdfs:subClassOf rdf:nodeID="nde7e53d44aa94269b5c0c83d6d8798ccb428"/>
    <rdfs:subClassOf rdf:nodeID="nde7e53d44aa94269b5c0c83d6d8798ccb429"/>
    <rdfs:subClassOf rdf:nodeID="nde7e53d44aa94269b5c0c83d6d8798ccb430"/>
    <rdfs:subClassOf rdf:nodeID="nde7e53d44aa94269b5c0c83d6d8798ccb431"/>
    <rdfs:subClassOf rdf:nodeID="nde7e53d44aa94269b5c0c83d6d8798ccb432"/>
    <rdfs:subClassOf rdf:nodeID="nde7e53d44aa94269b5c0c83d6d8798ccb433"/>
    <rdfs:subClassOf rdf:resource="https://w3id.org/omop/ontology/ClinicalElement"/>
    <rdfs:subClassOf rdf:resource="https://w3id.org/omop/ontology/Event"/>
    <ns1:omop_cdm_name rdf:datatype="http://www.w3.org/2001/XMLSchema#string">note</ns1:omop_cdm_name>
  </rdf:Description>
  <rdf:Description rdf:nodeID="nde7e53d44aa94269b5c0c83d6d8798ccb298">
    <rdf:type rdf:resource="http://www.w3.org/2002/07/owl#Restriction"/>
    <owl:allValuesFrom rdf:resource="http://www.w3.org/2001/XMLSchema#string"/>
    <owl:onProperty rdf:resource="https://w3id.org/omop/ontology/source_value"/>
  </rdf:Description>
  <rdf:Description rdf:about="https://w3id.org/omop/ontology/SourceToConceptMap">
    <rdf:type rdf:resource="http://www.w3.org/2002/07/owl#Class"/>
    <rdfs:subClassOf rdf:nodeID="nde7e53d44aa94269b5c0c83d6d8798ccb248"/>
    <rdfs:subClassOf rdf:nodeID="nde7e53d44aa94269b5c0c83d6d8798ccb249"/>
    <rdfs:subClassOf rdf:nodeID="nde7e53d44aa94269b5c0c83d6d8798ccb250"/>
    <rdfs:subClassOf rdf:nodeID="nde7e53d44aa94269b5c0c83d6d8798ccb251"/>
    <rdfs:subClassOf rdf:nodeID="nde7e53d44aa94269b5c0c83d6d8798ccb252"/>
    <rdfs:subClassOf rdf:nodeID="nde7e53d44aa94269b5c0c83d6d8798ccb253"/>
    <rdfs:subClassOf rdf:nodeID="nde7e53d44aa94269b5c0c83d6d8798ccb254"/>
    <rdfs:subClassOf rdf:nodeID="nde7e53d44aa94269b5c0c83d6d8798ccb255"/>
    <rdfs:subClassOf rdf:nodeID="nde7e53d44aa94269b5c0c83d6d8798ccb256"/>
    <rdfs:subClassOf rdf:nodeID="nde7e53d44aa94269b5c0c83d6d8798ccb257"/>
    <rdfs:subClassOf rdf:nodeID="nde7e53d44aa94269b5c0c83d6d8798ccb258"/>
    <rdfs:subClassOf rdf:nodeID="nde7e53d44aa94269b5c0c83d6d8798ccb259"/>
    <rdfs:subClassOf rdf:nodeID="nde7e53d44aa94269b5c0c83d6d8798ccb260"/>
    <rdfs:subClassOf rdf:nodeID="nde7e53d44aa94269b5c0c83d6d8798ccb261"/>
    <rdfs:subClassOf rdf:nodeID="nde7e53d44aa94269b5c0c83d6d8798ccb262"/>
    <rdfs:subClassOf rdf:nodeID="nde7e53d44aa94269b5c0c83d6d8798ccb263"/>
    <rdfs:subClassOf rdf:resource="https://w3id.org/omop/ontology/OmopCDMThing"/>
    <ns1:omop_cdm_name rdf:datatype="http://www.w3.org/2001/XMLSchema#string">source_to_concept_map</ns1:omop_cdm_name>
  </rdf:Description>
  <rdf:Description rdf:nodeID="nde7e53d44aa94269b5c0c83d6d8798ccb641">
    <rdf:type rdf:resource="http://www.w3.org/2002/07/owl#Restriction"/>
    <owl:onProperty rdf:resource="https://w3id.org/omop/ontology/has_race"/>
    <owl:someValuesFrom rdf:resource="https://w3id.org/omop/ontology/Concept"/>
  </rdf:Description>
  <rdf:Description rdf:nodeID="nde7e53d44aa94269b5c0c83d6d8798ccb645">
    <rdf:type rdf:resource="http://www.w3.org/2002/07/owl#Restriction"/>
    <owl:onProperty rdf:resource="https://w3id.org/omop/ontology/has_ethnicity_source"/>
    <owl:someValuesFrom rdf:resource="https://w3id.org/omop/ontology/Concept"/>
  </rdf:Description>
  <rdf:Description rdf:nodeID="nde7e53d44aa94269b5c0c83d6d8798ccb385">
    <rdf:type rdf:resource="http://www.w3.org/2002/07/owl#Restriction"/>
    <owl:allValuesFrom rdf:resource="https://w3id.org/omop/ontology/Concept"/>
    <owl:onProperty rdf:resource="https://w3id.org/omop/ontology/has_anatomic_site"/>
  </rdf:Description>
  <rdf:Description rdf:nodeID="nde7e53d44aa94269b5c0c83d6d8798ccb256">
    <rdf:type rdf:resource="http://www.w3.org/2002/07/owl#Restriction"/>
    <owl:onProperty rdf:resource="https://w3id.org/omop/ontology/has_target_vocabulary"/>
    <owl:someValuesFrom rdf:resource="https://w3id.org/omop/ontology/Vocabulary"/>
  </rdf:Description>
  <rdf:Description rdf:about="https://w3id.org/omop/ontology/Specimen">
    <rdf:type rdf:resource="http://www.w3.org/2002/07/owl#Class"/>
    <rdfs:subClassOf rdf:nodeID="nde7e53d44aa94269b5c0c83d6d8798ccb385"/>
    <rdfs:subClassOf rdf:nodeID="nde7e53d44aa94269b5c0c83d6d8798ccb386"/>
    <rdfs:subClassOf rdf:nodeID="nde7e53d44aa94269b5c0c83d6d8798ccb387"/>
    <rdfs:subClassOf rdf:nodeID="nde7e53d44aa94269b5c0c83d6d8798ccb388"/>
    <rdfs:subClassOf rdf:nodeID="nde7e53d44aa94269b5c0c83d6d8798ccb389"/>
    <rdfs:subClassOf rdf:nodeID="nde7e53d44aa94269b5c0c83d6d8798ccb390"/>
    <rdfs:subClassOf rdf:nodeID="nde7e53d44aa94269b5c0c83d6d8798ccb391"/>
    <rdfs:subClassOf rdf:nodeID="nde7e53d44aa94269b5c0c83d6d8798ccb392"/>
    <rdfs:subClassOf rdf:nodeID="nde7e53d44aa94269b5c0c83d6d8798ccb393"/>
    <rdfs:subClassOf rdf:nodeID="nde7e53d44aa94269b5c0c83d6d8798ccb395"/>
    <rdfs:subClassOf rdf:nodeID="nde7e53d44aa94269b5c0c83d6d8798ccb396"/>
    <rdfs:subClassOf rdf:nodeID="nde7e53d44aa94269b5c0c83d6d8798ccb397"/>
    <rdfs:subClassOf rdf:nodeID="nde7e53d44aa94269b5c0c83d6d8798ccb398"/>
    <rdfs:subClassOf rdf:nodeID="nde7e53d44aa94269b5c0c83d6d8798ccb399"/>
    <rdfs:subClassOf rdf:resource="https://w3id.org/omop/ontology/Event"/>
    <ns1:omop_cdm_name rdf:datatype="http://www.w3.org/2001/XMLSchema#string">specimen</ns1:omop_cdm_name>
  </rdf:Description>
  <rdf:Description rdf:nodeID="nde7e53d44aa94269b5c0c83d6d8798ccb182">
    <rdf:type rdf:resource="http://www.w3.org/2002/07/owl#Restriction"/>
    <owl:onProperty rdf:resource="https://w3id.org/omop/ontology/valid_start_date"/>
    <owl:someValuesFrom rdf:resource="http://www.w3.org/2001/XMLSchema#date"/>
  </rdf:Description>
  <rdf:Description rdf:nodeID="nde7e53d44aa94269b5c0c83d6d8798ccb530">
    <rdf:type rdf:resource="http://www.w3.org/2002/07/owl#Restriction"/>
    <owl:onProperty rdf:resource="https://w3id.org/omop/ontology/has_source"/>
    <owl:someValuesFrom rdf:resource="https://w3id.org/omop/ontology/Concept"/>
  </rdf:Description>
  <rdf:Description rdf:about="https://w3id.org/omop/ontology/sig">
    <rdf:type rdf:resource="http://www.w3.org/2002/07/owl#DatatypeProperty"/>
    <rdf:type rdf:resource="http://www.w3.org/2002/07/owl#FunctionalProperty"/>
    <rdfs:comment xml:lang="en">(for DrugExposure:) This is the verbatim instruction for the drug as written by the provider.
Put the written out instructions for the drug as it is verbatim in the source, if available.</rdfs:comment>
    <rdfs:domain rdf:resource="https://w3id.org/omop/ontology/DrugExposure"/>
    <rdfs:range rdf:resource="http://www.w3.org/2001/XMLSchema#string"/>
    <ns1:omop_cdm_name rdf:datatype="http://www.w3.org/2001/XMLSchema#string">drug_exposure.sig#90 AS str</ns1:omop_cdm_name>
  </rdf:Description>
  <rdf:Description rdf:about="https://w3id.org/omop/ontology/FactRelationship">
    <rdf:type rdf:resource="http://www.w3.org/2002/07/owl#Class"/>
    <rdfs:subClassOf rdf:nodeID="nde7e53d44aa94269b5c0c83d6d8798ccb152"/>
    <rdfs:subClassOf rdf:nodeID="nde7e53d44aa94269b5c0c83d6d8798ccb153"/>
    <rdfs:subClassOf rdf:nodeID="nde7e53d44aa94269b5c0c83d6d8798ccb154"/>
    <rdfs:subClassOf rdf:nodeID="nde7e53d44aa94269b5c0c83d6d8798ccb155"/>
    <rdfs:subClassOf rdf:nodeID="nde7e53d44aa94269b5c0c83d6d8798ccb156"/>
    <rdfs:subClassOf rdf:nodeID="nde7e53d44aa94269b5c0c83d6d8798ccb157"/>
    <rdfs:subClassOf rdf:nodeID="nde7e53d44aa94269b5c0c83d6d8798ccb158"/>
    <rdfs:subClassOf rdf:nodeID="nde7e53d44aa94269b5c0c83d6d8798ccb159"/>
    <rdfs:subClassOf rdf:nodeID="nde7e53d44aa94269b5c0c83d6d8798ccb160"/>
    <rdfs:subClassOf rdf:nodeID="nde7e53d44aa94269b5c0c83d6d8798ccb161"/>
    <rdfs:subClassOf rdf:resource="https://w3id.org/omop/ontology/OmopCDMThing"/>
    <ns1:omop_cdm_name rdf:datatype="http://www.w3.org/2001/XMLSchema#string">fact_relationship</ns1:omop_cdm_name>
  </rdf:Description>
  <rdf:Description rdf:nodeID="nde7e53d44aa94269b5c0c83d6d8798ccb599">
    <rdf:type rdf:resource="http://www.w3.org/2002/07/owl#Restriction"/>
    <owl:allValuesFrom rdf:resource="https://w3id.org/omop/ontology/Concept"/>
    <owl:onProperty rdf:resource="https://w3id.org/omop/ontology/has_respondent_type"/>
  </rdf:Description>
  <rdf:Description rdf:about="https://w3id.org/omop/ontology/has_concept">
    <rdf:type rdf:resource="http://www.w3.org/2002/07/owl#FunctionalProperty"/>
    <rdf:type rdf:resource="http://www.w3.org/2002/07/owl#ObjectProperty"/>
    <ns2:python_name rdf:datatype="http://www.w3.org/2001/XMLSchema#string">concept</ns2:python_name>
    <rdfs:comment xml:lang="en">(for ConceptClass:) A Concept that represents the Concept Class.</rdfs:comment>
    <rdfs:comment xml:lang="en">(for ConditionEra:) The Concept Id representing the Condition.</rdfs:comment>
    <rdfs:comment xml:lang="en">(for ConditionOccurrence:) The CONDITION_CONCEPT_ID field is recommended for primary use in analyses, and must be used for network studies. This is the standard concept mapped from the source value which represents a condition
The CONCEPT_ID that the CONDITION_SOURCE_VALUE maps to. Only records whose source values map to concepts with a domain of "Condition" should go in this table. [Accepted Concepts](https://athena.ohdsi.org/search-terms/terms?domain=Condition&amp;standardConcept=Standard&amp;page=1&amp;pageSize=15&amp;query=).</rdfs:comment>
    <rdfs:comment xml:lang="en">(for Cost:) A foreign key that refers to a Standard Cost Concept identifier in the Standardized Vocabularies belonging to the 'Cost' vocabulary.</rdfs:comment>
    <rdfs:comment xml:lang="en">(for DeviceExposure:) The DEVICE_CONCEPT_ID field is recommended for primary use in analyses, and must be used for network studies. This is the standard concept mapped from the source concept id which represents a foreign object or instrument the person was exposed to.
The CONCEPT_ID that the DEVICE_SOURCE_VALUE maps to.</rdfs:comment>
    <rdfs:comment xml:lang="en">(for Domain:) A Concept representing the Domain Concept the DOMAIN record belongs to.</rdfs:comment>
    <rdfs:comment xml:lang="en">(for DoseEra:) The Concept Id representing the specific drug ingredient.</rdfs:comment>
    <rdfs:comment xml:lang="en">(for DrugEra:) The Concept Id representing the specific drug ingredient.</rdfs:comment>
    <rdfs:comment xml:lang="en">(for DrugExposure:) The DRUG_CONCEPT_ID field is recommended for primary use in analyses, and must be used for network studies. This is the standard concept mapped from the source concept id which represents a drug product or molecule otherwise introduced to the body. The drug concepts can have a varying degree of information about drug strength and dose. This information is relevant in the context of quantity and administration information in the subsequent fields plus strength information from the DRUG_STRENGTH table, provided as part of the standard vocabulary download.
The CONCEPT_ID that the DRUG_SOURCE_VALUE maps to. The concept id should be derived either from mapping from the source concept id or by picking the drug concept representing the most amount of detail you have. Records whose source values map to standard concepts with a domain of Drug should go in this table. When the Drug Source Value of the code cannot be translated into Standard Drug Concept IDs, a Drug exposure entry is stored with only the corresponding SOURCE_CONCEPT_ID and DRUG_SOURCE_VALUE and a DRUG_CONCEPT_ID of 0. The Drug Concept with the most detailed content of information is preferred during the mapping process. These are indicated in the CONCEPT_CLASS_ID field of the Concept and are recorded in the following order of precedence: 'Branded Pack', 'Clinical Pack', 'Branded Drug', 'Clinical Drug', 'Branded Drug Component', 'Clinical Drug Component', 'Branded Drug Form', 'Clinical Drug Form', and only if no other information is available 'Ingredient'. Note: If only the drug class is known, the DRUG_CONCEPT_ID field should contain 0. [Accepted Concepts](https://athena.ohdsi.org/search-terms/terms?domain=Drug&amp;standardConcept=Standard&amp;page=1&amp;pageSize=15&amp;query=).</rdfs:comment>
    <rdfs:comment xml:lang="en">(for DrugStrength:) The Concept representing the Branded Drug or Clinical Drug Product.</rdfs:comment>
    <rdfs:comment xml:lang="en">(for Measurement:) The MEASUREMENT_CONCEPT_ID field is recommended for primary use in analyses, and must be used for network studies.
The CONCEPT_ID that the MEASUREMENT_SOURCE_CONCEPT_ID maps to. Only records whose SOURCE_CONCEPT_IDs map to Standard Concepts with a domain of "Measurement" should go in this table.</rdfs:comment>
    <rdfs:comment xml:lang="en">(for Observation:) The OBSERVATION_CONCEPT_ID field is recommended for primary use in analyses, and must be used for network studies.
The CONCEPT_ID that the OBSERVATION_SOURCE_CONCEPT_ID maps to. There is no specified domain that the Concepts in this table must adhere to. The only rule is that records with Concepts in the Condition, Procedure, Drug, Measurement, or Device domains MUST go to the corresponding table.</rdfs:comment>
    <rdfs:comment xml:lang="en">(for ProcedureOccurrence:) The PROCEDURE_CONCEPT_ID field is recommended for primary use in analyses, and must be used for network studies. This is the standard concept mapped from the source value which represents a procedure
The CONCEPT_ID that the PROCEDURE_SOURCE_VALUE maps to. Only records whose source values map to standard concepts with a domain of "Procedure" should go in this table. [Accepted Concepts](https://athena.ohdsi.org/search-terms/terms?domain=Procedure&amp;standardConcept=Standard&amp;page=1&amp;pageSize=15&amp;query=).</rdfs:comment>
    <rdfs:comment xml:lang="en">(for Specimen:) The standard CONCEPT_ID that the SPECIMEN_SOURCE_VALUE maps to in the specimen domain. [Accepted Concepts](https://athena.ohdsi.org/search-terms/terms?domain=Specimen&amp;standardConcept=Standard&amp;page=1&amp;pageSize=15&amp;query=)</rdfs:comment>
    <rdfs:comment xml:lang="en">(for VisitDetail:) This field contains a concept id representing the kind of visit detail, like inpatient or outpatient. All concepts in this field should be standard and belong to the Visit domain.
Populate this field based on the kind of visit that took place for the person. For example this could be "Inpatient Visit", "Outpatient Visit", "Ambulatory Visit", etc. This table will contain standard concepts in the Visit domain. These concepts are arranged in a hierarchical structure to facilitate cohort definitions by rolling up to generally familiar Visits adopted in most healthcare systems worldwide. [Accepted Concepts](https://athena.ohdsi.org/search-terms/terms?domain=Visit&amp;standardConcept=Standard&amp;page=1&amp;pageSize=15&amp;query=).</rdfs:comment>
    <rdfs:comment xml:lang="en">(for VisitOccurrence:) This field contains a concept id representing the kind of visit, like inpatient or outpatient. All concepts in this field should be standard and belong to the Visit domain.
Populate this field based on the kind of visit that took place for the person. For example this could be "Inpatient Visit", "Outpatient Visit", "Ambulatory Visit", etc. This table will contain standard concepts in the Visit domain. These concepts are arranged in a hierarchical structure to facilitate cohort definitions by rolling up to generally familiar Visits adopted in most healthcare systems worldwide.</rdfs:comment>
    <rdfs:comment xml:lang="en">(for Vocabulary:) A Concept that represents the Vocabulary the VOCABULARY record belongs to.</rdfs:comment>
    <rdfs:domain rdf:nodeID="nde7e53d44aa94269b5c0c83d6d8798ccb622"/>
    <rdfs:range rdf:resource="https://w3id.org/omop/ontology/Concept"/>
    <ns1:omop_cdm_name rdf:datatype="http://www.w3.org/2001/XMLSchema#string">concept_class.concept_class_concept_id#382 AS Concept</ns1:omop_cdm_name>
    <ns1:omop_cdm_name rdf:datatype="http://www.w3.org/2001/XMLSchema#string">concept_synonym.concept_id#395 AS Concept</ns1:omop_cdm_name>
    <ns1:omop_cdm_name rdf:datatype="http://www.w3.org/2001/XMLSchema#string">condition_era.condition_concept_id#341 AS Concept</ns1:omop_cdm_name>
    <ns1:omop_cdm_name rdf:datatype="http://www.w3.org/2001/XMLSchema#string">condition_occurrence.condition_concept_id#63 AS Concept</ns1:omop_cdm_name>
    <ns1:omop_cdm_name rdf:datatype="http://www.w3.org/2001/XMLSchema#string">cost.cost_concept_id#311 AS Concept</ns1:omop_cdm_name>
    <ns1:omop_cdm_name rdf:datatype="http://www.w3.org/2001/XMLSchema#string">device_exposure.device_concept_id#116 AS Concept</ns1:omop_cdm_name>
    <ns1:omop_cdm_name rdf:datatype="http://www.w3.org/2001/XMLSchema#string">domain.domain_concept_id#379 AS Concept</ns1:omop_cdm_name>
    <ns1:omop_cdm_name rdf:datatype="http://www.w3.org/2001/XMLSchema#string">dose_era.drug_concept_id#334 AS Concept</ns1:omop_cdm_name>
    <ns1:omop_cdm_name rdf:datatype="http://www.w3.org/2001/XMLSchema#string">drug_era.drug_concept_id#327 AS Concept</ns1:omop_cdm_name>
    <ns1:omop_cdm_name rdf:datatype="http://www.w3.org/2001/XMLSchema#string">drug_exposure.drug_concept_id#79 AS Concept</ns1:omop_cdm_name>
    <ns1:omop_cdm_name rdf:datatype="http://www.w3.org/2001/XMLSchema#string">drug_strength.drug_concept_id#411 AS Concept</ns1:omop_cdm_name>
    <ns1:omop_cdm_name rdf:datatype="http://www.w3.org/2001/XMLSchema#string">measurement.measurement_concept_id#131 AS Concept</ns1:omop_cdm_name>
    <ns1:omop_cdm_name rdf:datatype="http://www.w3.org/2001/XMLSchema#string">metadata.metadata_concept_id#345 AS Concept</ns1:omop_cdm_name>
    <ns1:omop_cdm_name rdf:datatype="http://www.w3.org/2001/XMLSchema#string">note_nlp.note_nlp_concept_id#199 AS Concept</ns1:omop_cdm_name>
    <ns1:omop_cdm_name rdf:datatype="http://www.w3.org/2001/XMLSchema#string">observation.observation_concept_id#151 AS Concept</ns1:omop_cdm_name>
    <ns1:omop_cdm_name rdf:datatype="http://www.w3.org/2001/XMLSchema#string">procedure_occurrence.procedure_concept_id#102 AS Concept</ns1:omop_cdm_name>
    <ns1:omop_cdm_name rdf:datatype="http://www.w3.org/2001/XMLSchema#string">relationship.relationship_concept_id#394 AS Concept</ns1:omop_cdm_name>
    <ns1:omop_cdm_name rdf:datatype="http://www.w3.org/2001/XMLSchema#string">specimen.specimen_concept_id#209 AS Concept</ns1:omop_cdm_name>
    <ns1:omop_cdm_name rdf:datatype="http://www.w3.org/2001/XMLSchema#string">visit_detail.visit_detail_concept_id#44 AS Concept</ns1:omop_cdm_name>
    <ns1:omop_cdm_name rdf:datatype="http://www.w3.org/2001/XMLSchema#string">visit_occurrence.visit_concept_id#27 AS Concept</ns1:omop_cdm_name>
    <ns1:omop_cdm_name rdf:datatype="http://www.w3.org/2001/XMLSchema#string">vocabulary.vocabulary_concept_id#376 AS Concept</ns1:omop_cdm_name>
  </rdf:Description>
  <rdf:Description rdf:about="https://w3id.org/omop/ontology/vocabulary_version">
    <rdf:type rdf:resource="http://www.w3.org/2002/07/owl#DatatypeProperty"/>
    <rdf:type rdf:resource="http://www.w3.org/2002/07/owl#FunctionalProperty"/>
    <rdfs:domain rdf:resource="https://w3id.org/omop/ontology/CdmSource"/>
    <rdfs:range rdf:resource="http://www.w3.org/2001/XMLSchema#string"/>
    <ns1:omop_cdm_name rdf:datatype="http://www.w3.org/2001/XMLSchema#string">cdm_source.vocabulary_version#361 AS str</ns1:omop_cdm_name>
  </rdf:Description>
  <rdf:Description rdf:nodeID="nde7e53d44aa94269b5c0c83d6d8798ccb301">
    <rdf:type rdf:resource="http://www.w3.org/2002/07/owl#Restriction"/>
    <owl:allValuesFrom rdf:resource="https://w3id.org/omop/ontology/Concept"/>
    <owl:onProperty rdf:resource="https://w3id.org/omop/ontology/has_concept"/>
  </rdf:Description>
  <rdf:Description rdf:about="https://w3id.org/omop/ontology/has_plan_source">
    <rdf:type rdf:resource="http://www.w3.org/2002/07/owl#FunctionalProperty"/>
    <rdf:type rdf:resource="http://www.w3.org/2002/07/owl#ObjectProperty"/>
    <ns2:python_name rdf:datatype="http://www.w3.org/2001/XMLSchema#string">plan_source</ns2:python_name>
    <rdfs:comment xml:lang="en">(for PayerPlanPeriod:) If the source data codes the Plan in an OMOP supported vocabulary store the concept_id here. If not available, set to 0.</rdfs:comment>
    <rdfs:domain rdf:resource="https://w3id.org/omop/ontology/PayerPlanPeriod"/>
    <rdfs:range rdf:resource="https://w3id.org/omop/ontology/Concept"/>
    <ns1:omop_cdm_name rdf:datatype="http://www.w3.org/2001/XMLSchema#string">payer_plan_period.plan_source_concept_id#296 AS Concept</ns1:omop_cdm_name>
  </rdf:Description>
  <rdf:Description rdf:nodeID="nde7e53d44aa94269b5c0c83d6d8798ccb494">
    <rdf:type rdf:resource="http://www.w3.org/2002/07/owl#Restriction"/>
    <owl:allValuesFrom rdf:resource="http://www.w3.org/2001/XMLSchema#string"/>
    <owl:onProperty rdf:resource="https://w3id.org/omop/ontology/revenue_code_source_value"/>
  </rdf:Description>
  <rdf:Description rdf:about="https://w3id.org/omop/ontology/collection_method_source_value">
    <rdf:type rdf:resource="http://www.w3.org/2002/07/owl#DatatypeProperty"/>
    <rdf:type rdf:resource="http://www.w3.org/2002/07/owl#FunctionalProperty"/>
    <rdfs:comment xml:lang="en">(for SurveyConduct:) The collection method as it appears in the source data.</rdfs:comment>
    <rdfs:domain rdf:resource="https://w3id.org/omop/ontology/SurveyConduct"/>
    <rdfs:range rdf:resource="http://www.w3.org/2001/XMLSchema#string"/>
    <ns1:omop_cdm_name rdf:datatype="http://www.w3.org/2001/XMLSchema#string">survey_conduct.collection_method_source_value#242 AS str</ns1:omop_cdm_name>
  </rdf:Description>
  <rdf:Description rdf:about="https://w3id.org/omop/ontology/valid_end_date">
    <rdf:type rdf:resource="http://www.w3.org/2002/07/owl#DatatypeProperty"/>
    <rdf:type rdf:resource="http://www.w3.org/2002/07/owl#FunctionalProperty"/>
    <rdfs:comment xml:lang="en">(for Concept:) The date when the Concept became
invalid because it was deleted or
superseded (updated) by a new concept.
The default value is 31-Dec-2099,
meaning, the Concept is valid until it
becomes deprecated.</rdfs:comment>
    <rdfs:comment xml:lang="en">(for ConceptRelationship:) The date when the relationship is invalidated.</rdfs:comment>
    <rdfs:comment xml:lang="en">(for DrugStrength:) The date when then Concept became invalid.</rdfs:comment>
    <rdfs:comment xml:lang="en">(for SourceToConceptMap:) The date when the mapping
instance became invalid because it
was deleted or superseded
(updated) by a new relationship.
Default value is 31-Dec-2099.</rdfs:comment>
    <rdfs:domain rdf:nodeID="nde7e53d44aa94269b5c0c83d6d8798ccb227"/>
    <rdfs:range rdf:resource="http://www.w3.org/2001/XMLSchema#date"/>
    <ns1:omop_cdm_name rdf:datatype="http://www.w3.org/2001/XMLSchema#string">concept.valid_end_date#370 AS date</ns1:omop_cdm_name>
    <ns1:omop_cdm_name rdf:datatype="http://www.w3.org/2001/XMLSchema#string">concept_relationship.valid_end_date#387 AS date</ns1:omop_cdm_name>
    <ns1:omop_cdm_name rdf:datatype="http://www.w3.org/2001/XMLSchema#string">drug_strength.valid_end_date#421 AS date</ns1:omop_cdm_name>
    <ns1:omop_cdm_name rdf:datatype="http://www.w3.org/2001/XMLSchema#string">source_to_concept_map.valid_end_date#409 AS date</ns1:omop_cdm_name>
  </rdf:Description>
  <rdf:Description rdf:nodeID="nde7e53d44aa94269b5c0c83d6d8798ccb640">
    <rdf:type rdf:resource="http://www.w3.org/2002/07/owl#Restriction"/>
    <owl:allValuesFrom rdf:resource="https://w3id.org/omop/ontology/DrugEra"/>
    <owl:onProperty rdf:resource="https://w3id.org/omop/ontology/has_drug_era"/>
  </rdf:Description>
  <rdf:Description rdf:about="https://w3id.org/omop/ontology/CdmSource">
    <rdf:type rdf:resource="http://www.w3.org/2002/07/owl#Class"/>
    <rdfs:subClassOf rdf:nodeID="nde7e53d44aa94269b5c0c83d6d8798ccb274"/>
    <rdfs:subClassOf rdf:nodeID="nde7e53d44aa94269b5c0c83d6d8798ccb275"/>
    <rdfs:subClassOf rdf:nodeID="nde7e53d44aa94269b5c0c83d6d8798ccb276"/>
    <rdfs:subClassOf rdf:nodeID="nde7e53d44aa94269b5c0c83d6d8798ccb277"/>
    <rdfs:subClassOf rdf:nodeID="nde7e53d44aa94269b5c0c83d6d8798ccb278"/>
    <rdfs:subClassOf rdf:nodeID="nde7e53d44aa94269b5c0c83d6d8798ccb279"/>
    <rdfs:subClassOf rdf:nodeID="nde7e53d44aa94269b5c0c83d6d8798ccb280"/>
    <rdfs:subClassOf rdf:nodeID="nde7e53d44aa94269b5c0c83d6d8798ccb281"/>
    <rdfs:subClassOf rdf:nodeID="nde7e53d44aa94269b5c0c83d6d8798ccb282"/>
    <rdfs:subClassOf rdf:nodeID="nde7e53d44aa94269b5c0c83d6d8798ccb283"/>
    <rdfs:subClassOf rdf:nodeID="nde7e53d44aa94269b5c0c83d6d8798ccb284"/>
    <rdfs:subClassOf rdf:resource="https://w3id.org/omop/ontology/OmopCDMThing"/>
    <ns1:omop_cdm_name rdf:datatype="http://www.w3.org/2001/XMLSchema#string">cdm_source</ns1:omop_cdm_name>
  </rdf:Description>
  <rdf:Description rdf:about="https://w3id.org/omop/ontology/CohortDefinition">
    <rdf:type rdf:resource="http://www.w3.org/2002/07/owl#Class"/>
    <rdfs:subClassOf rdf:nodeID="nde7e53d44aa94269b5c0c83d6d8798ccb237"/>
    <rdfs:subClassOf rdf:nodeID="nde7e53d44aa94269b5c0c83d6d8798ccb238"/>
    <rdfs:subClassOf rdf:nodeID="nde7e53d44aa94269b5c0c83d6d8798ccb239"/>
    <rdfs:subClassOf rdf:nodeID="nde7e53d44aa94269b5c0c83d6d8798ccb240"/>
    <rdfs:subClassOf rdf:nodeID="nde7e53d44aa94269b5c0c83d6d8798ccb241"/>
    <rdfs:subClassOf rdf:nodeID="nde7e53d44aa94269b5c0c83d6d8798ccb242"/>
    <rdfs:subClassOf rdf:nodeID="nde7e53d44aa94269b5c0c83d6d8798ccb243"/>
    <rdfs:subClassOf rdf:nodeID="nde7e53d44aa94269b5c0c83d6d8798ccb244"/>
    <rdfs:subClassOf rdf:nodeID="nde7e53d44aa94269b5c0c83d6d8798ccb245"/>
    <rdfs:subClassOf rdf:resource="https://w3id.org/omop/ontology/OmopCDMThing"/>
    <ns1:omop_cdm_name rdf:datatype="http://www.w3.org/2001/XMLSchema#string">cohort_definition</ns1:omop_cdm_name>
  </rdf:Description>
  <rdf:Description rdf:about="https://w3id.org/omop/ontology/defines_ancestry">
    <rdf:type rdf:resource="http://www.w3.org/2002/07/owl#DatatypeProperty"/>
    <rdf:type rdf:resource="http://www.w3.org/2002/07/owl#FunctionalProperty"/>
    <rdfs:domain rdf:resource="https://w3id.org/omop/ontology/Relationship"/>
    <rdfs:range rdf:resource="http://www.w3.org/2001/XMLSchema#string"/>
    <ns1:omop_cdm_name rdf:datatype="http://www.w3.org/2001/XMLSchema#string">relationship.defines_ancestry#392 AS str</ns1:omop_cdm_name>
  </rdf:Description>
  <rdf:Description rdf:about="https://w3id.org/omop/ontology/days_supply">
    <rdf:type rdf:resource="http://www.w3.org/2002/07/owl#DatatypeProperty"/>
    <rdf:type rdf:resource="http://www.w3.org/2002/07/owl#FunctionalProperty"/>
    <rdfs:comment xml:lang="en">(for DrugExposure:) Days supply of the drug. This should be the verbatim days_supply as given on the prescription. If the drug is physician administered use duration end date if given or set to 1 as default if duration is not available.</rdfs:comment>
    <rdfs:domain rdf:resource="https://w3id.org/omop/ontology/DrugExposure"/>
    <rdfs:range rdf:resource="http://www.w3.org/2001/XMLSchema#integer"/>
    <ns1:omop_cdm_name rdf:datatype="http://www.w3.org/2001/XMLSchema#string">drug_exposure.days_supply#89 AS int</ns1:omop_cdm_name>
  </rdf:Description>
  <rdf:Description rdf:nodeID="nde7e53d44aa94269b5c0c83d6d8798ccb520">
    <rdf:type rdf:resource="http://www.w3.org/2002/07/owl#Restriction"/>
    <owl:allValuesFrom rdf:resource="http://www.w3.org/2001/XMLSchema#dateTime"/>
    <owl:onProperty rdf:resource="https://w3id.org/omop/ontology/value_as_datetime"/>
  </rdf:Description>
  <rdf:Description rdf:about="https://w3id.org/omop/ontology/has_section">
    <rdf:type rdf:resource="http://www.w3.org/2002/07/owl#FunctionalProperty"/>
    <rdf:type rdf:resource="http://www.w3.org/2002/07/owl#ObjectProperty"/>
    <ns2:python_name rdf:datatype="http://www.w3.org/2001/XMLSchema#string">section</ns2:python_name>
    <rdfs:comment xml:lang="en">(for NoteNlp:) The SECTION_CONCEPT_ID should be used to represent the note section contained in the NOTE_NLP record. These concepts can be found as parts of document panels and are based on the type of note written, i.e. a discharge summary. These panels can be found as concepts with the relationship 'Subsumes' to CONCEPT_ID [45875957](https://athena.ohdsi.org/search-terms/terms/45875957).</rdfs:comment>
    <rdfs:domain rdf:resource="https://w3id.org/omop/ontology/NoteNlp"/>
    <rdfs:range rdf:resource="https://w3id.org/omop/ontology/Concept"/>
    <ns1:omop_cdm_name rdf:datatype="http://www.w3.org/2001/XMLSchema#string">note_nlp.section_concept_id#195 AS Concept</ns1:omop_cdm_name>
  </rdf:Description>
  <rdf:Description rdf:about="https://w3id.org/omop/ontology/has_sponsor">
    <rdf:type rdf:resource="http://www.w3.org/2002/07/owl#FunctionalProperty"/>
    <rdf:type rdf:resource="http://www.w3.org/2002/07/owl#ObjectProperty"/>
    <ns2:python_name rdf:datatype="http://www.w3.org/2001/XMLSchema#string">sponsor</ns2:python_name>
    <rdfs:comment xml:lang="en">(for PayerPlanPeriod:) This field represents the sponsor of the Plan who finances the Plan. This includes self-insured, small group health plan and large group health plan.
Map the sponsor directly to a standard CONCEPT_ID. If one does not exists please contact the vocabulary team. There is no global controlled vocabulary available for this information. The point is to stratify on this information and identify if Persons have the same sponsor though the name of the sponsor is not necessary. If not available, set to 0. [Accepted Concepts](http://athena.ohdsi.org/search-terms/terms?domain=Sponsor&amp;standardConcept=Standard&amp;page=1&amp;pageSize=15&amp;query=).</rdfs:comment>
    <rdfs:domain rdf:resource="https://w3id.org/omop/ontology/PayerPlanPeriod"/>
    <rdfs:range rdf:resource="https://w3id.org/omop/ontology/Concept"/>
    <ns1:omop_cdm_name rdf:datatype="http://www.w3.org/2001/XMLSchema#string">payer_plan_period.sponsor_concept_id#300 AS Concept</ns1:omop_cdm_name>
  </rdf:Description>
  <rdf:Description rdf:nodeID="nde7e53d44aa94269b5c0c83d6d8798ccb155">
    <rdf:type rdf:resource="http://www.w3.org/2002/07/owl#Restriction"/>
    <owl:allValuesFrom rdf:resource="https://w3id.org/omop/ontology/Concept"/>
    <owl:onProperty rdf:resource="https://w3id.org/omop/ontology/has_relationship"/>
  </rdf:Description>
  <rdf:Description rdf:about="https://w3id.org/omop/ontology/family_source_value">
    <rdf:type rdf:resource="http://www.w3.org/2002/07/owl#DatatypeProperty"/>
    <rdf:type rdf:resource="http://www.w3.org/2002/07/owl#FunctionalProperty"/>
    <rdfs:comment xml:lang="en">(for PayerPlanPeriod:) The common identifier for all people (often a family) that covered by the same policy.
Often these are the common digits of the enrollment id of the policy members.</rdfs:comment>
    <rdfs:domain rdf:resource="https://w3id.org/omop/ontology/PayerPlanPeriod"/>
    <rdfs:range rdf:resource="http://www.w3.org/2001/XMLSchema#string"/>
    <ns1:omop_cdm_name rdf:datatype="http://www.w3.org/2001/XMLSchema#string">payer_plan_period.family_source_value#303 AS str</ns1:omop_cdm_name>
  </rdf:Description>
  <rdf:Description rdf:about="https://w3id.org/omop/ontology/has_entity">
    <rdf:type rdf:resource="http://www.w3.org/2002/07/owl#FunctionalProperty"/>
    <rdf:type rdf:resource="http://www.w3.org/2002/07/owl#ObjectProperty"/>
    <ns2:python_name rdf:datatype="http://www.w3.org/2001/XMLSchema#string">entity</ns2:python_name>
    <rdfs:comment xml:lang="en">(for LocationHistory:) The unique identifier for the entity. References either person_id, provider_id, or care_site_id, depending on domain_id.</rdfs:comment>
    <rdfs:domain rdf:resource="https://w3id.org/omop/ontology/LocationHistory"/>
    <ns1:omop_cdm_name rdf:datatype="http://www.w3.org/2001/XMLSchema#string">location_history.entity_id#264 AS Thing</ns1:omop_cdm_name>
  </rdf:Description>
  <rdf:Description rdf:nodeID="nde7e53d44aa94269b5c0c83d6d8798ccb479">
    <rdf:type rdf:resource="http://www.w3.org/2002/07/owl#Restriction"/>
    <owl:onProperty rdf:resource="https://w3id.org/omop/ontology/has_specialty"/>
    <owl:someValuesFrom rdf:resource="https://w3id.org/omop/ontology/Concept"/>
  </rdf:Description>
  <rdf:Description rdf:about="https://w3id.org/omop/ontology/Era">
    <rdf:type rdf:resource="http://www.w3.org/2002/07/owl#Class"/>
    <rdfs:subClassOf rdf:nodeID="nde7e53d44aa94269b5c0c83d6d8798ccb102"/>
    <rdfs:subClassOf rdf:nodeID="nde7e53d44aa94269b5c0c83d6d8798ccb103"/>
    <rdfs:subClassOf rdf:resource="https://w3id.org/omop/ontology/ClinicalElement"/>
    <rdfs:subClassOf rdf:resource="https://w3id.org/omop/ontology/DatetimeDuration"/>
  </rdf:Description>
  <rdf:Description rdf:about="https://w3id.org/omop/ontology/has_source">
    <rdf:type rdf:resource="http://www.w3.org/2002/07/owl#FunctionalProperty"/>
    <rdf:type rdf:resource="http://www.w3.org/2002/07/owl#ObjectProperty"/>
    <ns2:python_name rdf:datatype="http://www.w3.org/2001/XMLSchema#string">source</ns2:python_name>
    <rdfs:comment xml:lang="en">(for ConditionOccurrence:) This is the concept representing the condition source value and may not necessarily be standard. This field is discouraged from use in analysis because it is not required to contain Standard Concepts that are used across the OHDSI community, and should only be used when Standard Concepts do not adequately represent the source detail for the Condition necessary for a given analytic use case. Consider using CONDITION_CONCEPT_ID instead to enable standardized analytics that can be consistent across the network.
If the CONDITION_SOURCE_VALUE is coded in the source data using an OMOP supported vocabulary put the concept id representing the source value here. If not available, set to 0.</rdfs:comment>
    <rdfs:comment xml:lang="en">(for Cost:) A foreign key to a Cost Concept that refers to the code used in the source.</rdfs:comment>
    <rdfs:comment xml:lang="en">(for DeviceExposure:) This is the concept representing the device source value and may not necessarily be standard. This field is discouraged from use in analysis because it is not required to contain Standard Concepts that are used across the OHDSI community, and should only be used when Standard Concepts do not adequately represent the source detail for the Device necessary for a given analytic use case. Consider using DEVICE_CONCEPT_ID instead to enable standardized analytics that can be consistent across the network.
If the DEVICE_SOURCE_VALUE is coded in the source data using an OMOP supported vocabulary put the concept id representing the source value here. If unavailable, set to 0.</rdfs:comment>
    <rdfs:comment xml:lang="en">(for DrugExposure:) This is the concept representing the drug source value and may not necessarily be standard. This field is discouraged from use in analysis because it is not required to contain Standard Concepts that are used across the OHDSI community, and should only be used when Standard Concepts do not adequately represent the source detail for the Drug necessary for a given analytic use case. Consider using DRUG_CONCEPT_ID instead to enable standardized analytics that can be consistent across the network.
If the DRUG_SOURCE_VALUE is coded in the source data using an OMOP supported vocabulary put the concept id representing the source value here. If unavailable, set to 0.</rdfs:comment>
    <rdfs:comment xml:lang="en">(for Measurement:) This is the concept representing the MEASUREMENT_SOURCE_VALUE and may not necessarily be standard. This field is discouraged from use in analysis because it is not required to contain Standard Concepts that are used across the OHDSI community, and should only be used when Standard Concepts do not adequately represent the source detail for the Measurement necessary for a given analytic use case. Consider using MEASUREMENT_CONCEPT_ID instead to enable standardized analytics that can be consistent across the network.
If the MEASUREMENT_SOURCE_VALUE is coded in the source data using an OMOP supported vocabulary put the concept id representing the source value here. If not available, set to 0.</rdfs:comment>
    <rdfs:comment xml:lang="en">(for Observation:) This is the concept representing the OBSERVATION_SOURCE_VALUE and may not necessarily be standard. This field is discouraged from use in analysis because it is not required to contain Standard Concepts that are used across the OHDSI community, and should only be used when Standard Concepts do not adequately represent the source detail for the Observation necessary for a given analytic use case. Consider using OBSERVATION_CONCEPT_ID instead to enable standardized analytics that can be consistent across the network.
If the OBSERVATION_SOURCE_VALUE is coded in the source data using an OMOP supported vocabulary put the concept id representing the source value here. If not available, set to 0.</rdfs:comment>
    <rdfs:comment xml:lang="en">(for ProcedureOccurrence:) This is the concept representing the procedure source value and may not necessarily be standard. This field is discouraged from use in analysis because it is not required to contain Standard Concepts that are used across the OHDSI community, and should only be used when Standard Concepts do not adequately represent the source detail for the Procedure necessary for a given analytic use case. Consider using PROCEDURE_CONCEPT_ID instead to enable standardized analytics that can be consistent across the network.
If the PROCEDURE_SOURCE_VALUE is coded in the source data using an OMOP supported vocabulary put the concept id representing the source value here. If not available, set to 0.</rdfs:comment>
    <rdfs:comment xml:lang="en">(for SourceToConceptMap:) A foreign key to the Source
Concept that is being translated
into a Standard Concept.
This is either 0 or should be a number above 2 billion, which are the Concepts reserved for site-specific codes and mappings.</rdfs:comment>
    <rdfs:comment xml:lang="en">(for Specimen:) This is the identifier for the specimen from the source system.</rdfs:comment>
    <rdfs:comment xml:lang="en">(for VisitDetail:) If the VISIT_DETAIL_SOURCE_VALUE is coded in the source data using an OMOP supported vocabulary put the concept id representing the source value here. If not available, map to 0.</rdfs:comment>
    <rdfs:comment xml:lang="en">(for VisitOccurrence:) If the visit source value is coded in the source data using an OMOP supported vocabulary put the concept id representing the source value here. If not available set to 0.</rdfs:comment>
    <rdfs:domain rdf:nodeID="nde7e53d44aa94269b5c0c83d6d8798ccb481"/>
    <ns1:omop_cdm_name rdf:datatype="http://www.w3.org/2001/XMLSchema#string">condition_occurrence.condition_source_concept_id#75 AS Concept</ns1:omop_cdm_name>
    <ns1:omop_cdm_name rdf:datatype="http://www.w3.org/2001/XMLSchema#string">cost.cost_source_concept_id#313 AS Concept</ns1:omop_cdm_name>
    <ns1:omop_cdm_name rdf:datatype="http://www.w3.org/2001/XMLSchema#string">device_exposure.device_source_concept_id#128 AS Concept</ns1:omop_cdm_name>
    <ns1:omop_cdm_name rdf:datatype="http://www.w3.org/2001/XMLSchema#string">drug_exposure.drug_source_concept_id#97 AS Concept</ns1:omop_cdm_name>
    <ns1:omop_cdm_name rdf:datatype="http://www.w3.org/2001/XMLSchema#string">measurement.measurement_source_concept_id#146 AS Concept</ns1:omop_cdm_name>
    <ns1:omop_cdm_name rdf:datatype="http://www.w3.org/2001/XMLSchema#string">note_nlp.note_nlp_source_concept_id#200 AS Concept</ns1:omop_cdm_name>
    <ns1:omop_cdm_name rdf:datatype="http://www.w3.org/2001/XMLSchema#string">observation.observation_source_concept_id#164 AS Concept</ns1:omop_cdm_name>
    <ns1:omop_cdm_name rdf:datatype="http://www.w3.org/2001/XMLSchema#string">procedure_occurrence.procedure_source_concept_id#112 AS Concept</ns1:omop_cdm_name>
    <ns1:omop_cdm_name rdf:datatype="http://www.w3.org/2001/XMLSchema#string">source_to_concept_map.source_concept_id#403 AS Concept</ns1:omop_cdm_name>
    <ns1:omop_cdm_name rdf:datatype="http://www.w3.org/2001/XMLSchema#string">specimen.specimen_source_id#217 AS Thing</ns1:omop_cdm_name>
    <ns1:omop_cdm_name rdf:datatype="http://www.w3.org/2001/XMLSchema#string">visit_detail.visit_detail_source_concept_id#53 AS Concept</ns1:omop_cdm_name>
    <ns1:omop_cdm_name rdf:datatype="http://www.w3.org/2001/XMLSchema#string">visit_occurrence.visit_source_concept_id#36 AS Concept</ns1:omop_cdm_name>
  </rdf:Description>
  <rdf:Description rdf:about="https://w3id.org/omop/ontology/has_ethnicity">
    <rdf:type rdf:resource="http://www.w3.org/2002/07/owl#FunctionalProperty"/>
    <rdf:type rdf:resource="http://www.w3.org/2002/07/owl#ObjectProperty"/>
    <ns2:python_name rdf:datatype="http://www.w3.org/2001/XMLSchema#string">ethnicity</ns2:python_name>
    <rdfs:comment xml:lang="en">(for Person:) This field captures Ethnicity as defined by the Office of Management and Budget (OMB) of the US Government: it distinguishes only between "Hispanic" and "Not Hispanic". Races and ethnic backgrounds are not stored here.
Only use this field if you have US-based data and a source of this information. Do not attempt to infer Ethnicity from the race or ethnic background of the Person. [Accepted ethnicity concepts](http://athena.ohdsi.org/search-terms/terms?domain=Ethnicity&amp;standardConcept=Standard&amp;page=1&amp;pageSize=15&amp;query=)</rdfs:comment>
    <rdfs:domain rdf:resource="https://w3id.org/omop/ontology/Person"/>
    <rdfs:range rdf:resource="https://w3id.org/omop/ontology/Concept"/>
    <ns1:omop_cdm_name rdf:datatype="http://www.w3.org/2001/XMLSchema#string">person.ethnicity_concept_id#9 AS Concept</ns1:omop_cdm_name>
  </rdf:Description>
  <rdf:Description rdf:about="https://w3id.org/omop/ontology/respondent_type_source_value">
    <rdf:type rdf:resource="http://www.w3.org/2002/07/owl#DatatypeProperty"/>
    <rdf:type rdf:resource="http://www.w3.org/2002/07/owl#FunctionalProperty"/>
    <rdfs:comment xml:lang="en">(for SurveyConduct:) Source code representing role of person who completed the survey.</rdfs:comment>
    <rdfs:domain rdf:resource="https://w3id.org/omop/ontology/SurveyConduct"/>
    <rdfs:range rdf:resource="http://www.w3.org/2001/XMLSchema#string"/>
    <ns1:omop_cdm_name rdf:datatype="http://www.w3.org/2001/XMLSchema#string">survey_conduct.respondent_type_source_value#240 AS str</ns1:omop_cdm_name>
  </rdf:Description>
  <rdf:Description rdf:nodeID="nde7e53d44aa94269b5c0c83d6d8798ccb327">
    <rdf:type rdf:resource="http://www.w3.org/2002/07/owl#Restriction"/>
    <owl:allValuesFrom rdf:resource="https://w3id.org/omop/ontology/Concept"/>
    <owl:onProperty rdf:resource="https://w3id.org/omop/ontology/has_ingredient"/>
  </rdf:Description>
  <rdf:Description rdf:about="https://w3id.org/omop/ontology/DrugEra">
    <rdf:type rdf:resource="http://www.w3.org/2002/07/owl#Class"/>
    <rdfs:subClassOf rdf:nodeID="nde7e53d44aa94269b5c0c83d6d8798ccb98"/>
    <rdfs:subClassOf rdf:nodeID="nde7e53d44aa94269b5c0c83d6d8798ccb100"/>
    <rdfs:subClassOf rdf:nodeID="nde7e53d44aa94269b5c0c83d6d8798ccb101"/>
    <rdfs:subClassOf rdf:resource="https://w3id.org/omop/ontology/Era"/>
    <ns1:omop_cdm_name rdf:datatype="http://www.w3.org/2001/XMLSchema#string">drug_era</ns1:omop_cdm_name>
  </rdf:Description>
  <rdf:Description rdf:nodeID="nde7e53d44aa94269b5c0c83d6d8798ccb405">
    <rdf:type rdf:resource="http://www.w3.org/2002/07/owl#Restriction"/>
    <owl:allValuesFrom rdf:resource="https://w3id.org/omop/ontology/Concept"/>
    <owl:onProperty rdf:resource="https://w3id.org/omop/ontology/has_concept"/>
  </rdf:Description>
  <rdf:Description rdf:nodeID="nde7e53d44aa94269b5c0c83d6d8798ccb390">
    <rdf:type rdf:resource="http://www.w3.org/2002/07/owl#Restriction"/>
    <owl:allValuesFrom rdf:resource="https://w3id.org/omop/ontology/Concept"/>
    <owl:onProperty rdf:resource="https://w3id.org/omop/ontology/has_unit"/>
  </rdf:Description>
  <rdf:Description rdf:nodeID="nde7e53d44aa94269b5c0c83d6d8798ccb408">
    <rdf:type rdf:resource="http://www.w3.org/2002/07/owl#Restriction"/>
    <owl:allValuesFrom rdf:resource="http://www.w3.org/2001/XMLSchema#string"/>
    <owl:onProperty rdf:resource="https://w3id.org/omop/ontology/city"/>
  </rdf:Description>
  <rdf:Description rdf:about="https://w3id.org/omop/ontology/cause_source_value">
    <rdf:type rdf:resource="http://www.w3.org/2002/07/owl#DatatypeProperty"/>
    <rdf:type rdf:resource="http://www.w3.org/2002/07/owl#FunctionalProperty"/>
    <rdfs:domain rdf:resource="https://w3id.org/omop/ontology/Death"/>
    <rdfs:range rdf:resource="http://www.w3.org/2001/XMLSchema#string"/>
    <ns1:omop_cdm_name rdf:datatype="http://www.w3.org/2001/XMLSchema#string">death.cause_source_value#175 AS str</ns1:omop_cdm_name>
  </rdf:Description>
  <rdf:Description rdf:nodeID="nde7e53d44aa94269b5c0c83d6d8798ccb152">
    <rdf:type rdf:resource="http://www.w3.org/2002/07/owl#Restriction"/>
    <owl:onProperty rdf:resource="https://w3id.org/omop/ontology/fact_id_1"/>
    <owl:someValuesFrom rdf:resource="http://www.w3.org/2001/XMLSchema#integer"/>
  </rdf:Description>
  <rdf:Description rdf:about="https://w3id.org/omop/ontology/has_operator">
    <rdf:type rdf:resource="http://www.w3.org/2002/07/owl#FunctionalProperty"/>
    <rdf:type rdf:resource="http://www.w3.org/2002/07/owl#ObjectProperty"/>
    <ns2:python_name rdf:datatype="http://www.w3.org/2001/XMLSchema#string">operator</ns2:python_name>
    <rdfs:comment xml:lang="en">(for Measurement:) The meaning of Concept [4172703](https://athena.ohdsi.org/search-terms/terms/4172703) for '=' is identical to omission of a OPERATOR_CONCEPT_ID value. Since the use of this field is rare, it's important when devising analyses to not to forget testing for the content of this field for values different from =.
Operators are &lt;, &lt;=, =, &gt;=, &gt; and these concepts belong to the 'Meas Value Operator' domain. [Accepted Concepts](https://athena.ohdsi.org/search-terms/terms?domain=Meas+Value+Operator&amp;standardConcept=Standard&amp;page=1&amp;pageSize=15&amp;query=).</rdfs:comment>
    <rdfs:domain rdf:resource="https://w3id.org/omop/ontology/Measurement"/>
    <rdfs:range rdf:resource="https://w3id.org/omop/ontology/Concept"/>
    <ns1:omop_cdm_name rdf:datatype="http://www.w3.org/2001/XMLSchema#string">measurement.operator_concept_id#136 AS Concept</ns1:omop_cdm_name>
  </rdf:Description>
  <rdf:Description rdf:about="https://w3id.org/omop/ontology/gender_source_value">
    <rdf:type rdf:resource="http://www.w3.org/2002/07/owl#DatatypeProperty"/>
    <rdf:type rdf:resource="http://www.w3.org/2002/07/owl#FunctionalProperty"/>
    <rdfs:comment xml:lang="en">(for Person:) This field is used to store the biological sex of the person from the source data. It is not intended for use in standard analytics but for reference only.
Put the biological sex of the person as it appears in the source data.</rdfs:comment>
    <rdfs:comment xml:lang="en">(for Provider:) This is provider's gender as it appears in the source data.
Put the provider's gender as it appears in the source data. This field is up to the discretion of the ETL-er as to whether this should be the coded value from the source or the text description of the lookup value.</rdfs:comment>
    <rdfs:domain rdf:resource="https://w3id.org/omop/ontology/BasePerson"/>
    <rdfs:range rdf:resource="http://www.w3.org/2001/XMLSchema#string"/>
    <ns1:omop_cdm_name rdf:datatype="http://www.w3.org/2001/XMLSchema#string">person.gender_source_value#14 AS str</ns1:omop_cdm_name>
    <ns1:omop_cdm_name rdf:datatype="http://www.w3.org/2001/XMLSchema#string">provider.gender_source_value#284 AS str</ns1:omop_cdm_name>
  </rdf:Description>
  <rdf:Description rdf:nodeID="nde7e53d44aa94269b5c0c83d6d8798ccb312">
    <rdf:type rdf:resource="http://www.w3.org/2002/07/owl#Restriction"/>
    <owl:allValuesFrom rdf:resource="https://w3id.org/omop/ontology/Concept"/>
    <owl:onProperty rdf:resource="https://w3id.org/omop/ontology/has_source"/>
  </rdf:Description>
  <rdf:Description rdf:about="https://w3id.org/omop/ontology/latitude">
    <rdf:type rdf:resource="http://www.w3.org/2002/07/owl#DatatypeProperty"/>
    <rdf:type rdf:resource="http://www.w3.org/2002/07/owl#FunctionalProperty"/>
    <rdfs:comment xml:lang="en">(for Location:) The geocoded latitude.</rdfs:comment>
    <rdfs:domain rdf:resource="https://w3id.org/omop/ontology/Location"/>
    <rdfs:range rdf:resource="http://www.w3.org/2001/XMLSchema#decimal"/>
    <ns1:omop_cdm_name rdf:datatype="http://www.w3.org/2001/XMLSchema#string">location.latitude#259 AS float</ns1:omop_cdm_name>
  </rdf:Description>
  <rdf:Description rdf:nodeID="nde7e53d44aa94269b5c0c83d6d8798ccb21">
    <rdf:type rdf:resource="http://www.w3.org/2002/07/owl#Restriction"/>
    <owl:onProperty rdf:resource="https://w3id.org/omop/ontology/has_language"/>
    <owl:someValuesFrom rdf:resource="https://w3id.org/omop/ontology/Concept"/>
  </rdf:Description>
  <rdf:Description rdf:about="https://w3id.org/omop/ontology/Person">
    <rdf:type rdf:resource="http://www.w3.org/2002/07/owl#Class"/>
    <rdfs:subClassOf rdf:nodeID="nde7e53d44aa94269b5c0c83d6d8798ccb640"/>
    <rdfs:subClassOf rdf:nodeID="nde7e53d44aa94269b5c0c83d6d8798ccb641"/>
    <rdfs:subClassOf rdf:nodeID="nde7e53d44aa94269b5c0c83d6d8798ccb642"/>
    <rdfs:subClassOf rdf:nodeID="nde7e53d44aa94269b5c0c83d6d8798ccb643"/>
    <rdfs:subClassOf rdf:nodeID="nde7e53d44aa94269b5c0c83d6d8798ccb644"/>
    <rdfs:subClassOf rdf:nodeID="nde7e53d44aa94269b5c0c83d6d8798ccb645"/>
    <rdfs:subClassOf rdf:nodeID="nde7e53d44aa94269b5c0c83d6d8798ccb646"/>
    <rdfs:subClassOf rdf:nodeID="nde7e53d44aa94269b5c0c83d6d8798ccb647"/>
    <rdfs:subClassOf rdf:nodeID="nde7e53d44aa94269b5c0c83d6d8798ccb648"/>
    <rdfs:subClassOf rdf:nodeID="nde7e53d44aa94269b5c0c83d6d8798ccb649"/>
    <rdfs:subClassOf rdf:nodeID="nde7e53d44aa94269b5c0c83d6d8798ccb650"/>
    <rdfs:subClassOf rdf:nodeID="nde7e53d44aa94269b5c0c83d6d8798ccb651"/>
    <rdfs:subClassOf rdf:nodeID="nde7e53d44aa94269b5c0c83d6d8798ccb652"/>
    <rdfs:subClassOf rdf:nodeID="nde7e53d44aa94269b5c0c83d6d8798ccb653"/>
    <rdfs:subClassOf rdf:nodeID="nde7e53d44aa94269b5c0c83d6d8798ccb654"/>
    <rdfs:subClassOf rdf:nodeID="nde7e53d44aa94269b5c0c83d6d8798ccb655"/>
    <rdfs:subClassOf rdf:nodeID="nde7e53d44aa94269b5c0c83d6d8798ccb656"/>
    <rdfs:subClassOf rdf:nodeID="nde7e53d44aa94269b5c0c83d6d8798ccb657"/>
    <rdfs:subClassOf rdf:nodeID="nde7e53d44aa94269b5c0c83d6d8798ccb658"/>
    <rdfs:subClassOf rdf:nodeID="nde7e53d44aa94269b5c0c83d6d8798ccb659"/>
    <rdfs:subClassOf rdf:nodeID="nde7e53d44aa94269b5c0c83d6d8798ccb660"/>
    <rdfs:subClassOf rdf:nodeID="nde7e53d44aa94269b5c0c83d6d8798ccb661"/>
    <rdfs:subClassOf rdf:nodeID="nde7e53d44aa94269b5c0c83d6d8798ccb662"/>
    <rdfs:subClassOf rdf:nodeID="nde7e53d44aa94269b5c0c83d6d8798ccb663"/>
    <rdfs:subClassOf rdf:nodeID="nde7e53d44aa94269b5c0c83d6d8798ccb664"/>
    <rdfs:subClassOf rdf:nodeID="nde7e53d44aa94269b5c0c83d6d8798ccb665"/>
    <rdfs:subClassOf rdf:nodeID="nde7e53d44aa94269b5c0c83d6d8798ccb666"/>
    <rdfs:subClassOf rdf:nodeID="nde7e53d44aa94269b5c0c83d6d8798ccb667"/>
    <rdfs:subClassOf rdf:nodeID="nde7e53d44aa94269b5c0c83d6d8798ccb668"/>
    <rdfs:subClassOf rdf:nodeID="nde7e53d44aa94269b5c0c83d6d8798ccb669"/>
    <rdfs:subClassOf rdf:nodeID="nde7e53d44aa94269b5c0c83d6d8798ccb670"/>
    <rdfs:subClassOf rdf:nodeID="nde7e53d44aa94269b5c0c83d6d8798ccb671"/>
    <rdfs:subClassOf rdf:nodeID="nde7e53d44aa94269b5c0c83d6d8798ccb672"/>
    <rdfs:subClassOf rdf:nodeID="nde7e53d44aa94269b5c0c83d6d8798ccb673"/>
    <rdfs:subClassOf rdf:nodeID="nde7e53d44aa94269b5c0c83d6d8798ccb674"/>
    <rdfs:subClassOf rdf:nodeID="nde7e53d44aa94269b5c0c83d6d8798ccb675"/>
    <rdfs:subClassOf rdf:resource="https://w3id.org/omop/ontology/BasePerson"/>
    <ns1:omop_cdm_name rdf:datatype="http://www.w3.org/2001/XMLSchema#string">person</ns1:omop_cdm_name>
  </rdf:Description>
  <rdf:Description rdf:nodeID="nde7e53d44aa94269b5c0c83d6d8798ccb460">
    <rdf:type rdf:resource="http://www.w3.org/2002/07/owl#Restriction"/>
    <owl:allValuesFrom rdf:resource="http://www.w3.org/2001/XMLSchema#string"/>
    <owl:onProperty rdf:resource="https://w3id.org/omop/ontology/unit_source_value"/>
  </rdf:Description>
  <rdf:Description rdf:nodeID="nde7e53d44aa94269b5c0c83d6d8798ccb337">
    <rdf:type rdf:resource="http://www.w3.org/2002/07/owl#Restriction"/>
    <owl:allValuesFrom rdf:resource="https://w3id.org/omop/ontology/Concept"/>
    <owl:onProperty rdf:resource="https://w3id.org/omop/ontology/has_concept"/>
  </rdf:Description>
  <rdf:Description rdf:about="https://w3id.org/omop/ontology/value">
    <rdf:type rdf:resource="http://www.w3.org/2002/07/owl#DatatypeProperty"/>
    <rdf:type rdf:resource="http://www.w3.org/2002/07/owl#FunctionalProperty"/>
    <rdfs:comment xml:lang="en">(for DoseEra:) The numeric value of the dosage of the drug_ingredient.</rdfs:comment>
    <rdfs:domain rdf:resource="https://w3id.org/omop/ontology/DoseEra"/>
    <rdfs:range rdf:resource="http://www.w3.org/2001/XMLSchema#decimal"/>
    <ns1:omop_cdm_name rdf:datatype="http://www.w3.org/2001/XMLSchema#string">dose_era.dose_value#336 AS float</ns1:omop_cdm_name>
  </rdf:Description>
  <rdf:Description rdf:nodeID="nde7e53d44aa94269b5c0c83d6d8798ccb73">
    <rdf:type rdf:resource="http://www.w3.org/2002/07/owl#Class"/>
    <owl:unionOf rdf:nodeID="nde7e53d44aa94269b5c0c83d6d8798ccb74"/>
  </rdf:Description>
  <rdf:Description rdf:about="https://w3id.org/omop/ontology/has_ethnicity_source">
    <rdf:type rdf:resource="http://www.w3.org/2002/07/owl#FunctionalProperty"/>
    <rdf:type rdf:resource="http://www.w3.org/2002/07/owl#ObjectProperty"/>
    <ns2:python_name rdf:datatype="http://www.w3.org/2001/XMLSchema#string">ethnicity_source</ns2:python_name>
    <rdfs:comment xml:lang="en">(for Person:) Due to the small number of options, this tends to be zero.
If the source data codes ethnicity in an OMOP supported vocabulary, store the concept_id here, otherwise set to 0.</rdfs:comment>
    <rdfs:domain rdf:resource="https://w3id.org/omop/ontology/Person"/>
    <rdfs:range rdf:resource="https://w3id.org/omop/ontology/Concept"/>
    <ns1:omop_cdm_name rdf:datatype="http://www.w3.org/2001/XMLSchema#string">person.ethnicity_source_concept_id#19 AS Concept</ns1:omop_cdm_name>
  </rdf:Description>
  <rdf:Description rdf:about="https://w3id.org/omop/ontology/denominator_value">
    <rdf:type rdf:resource="http://www.w3.org/2002/07/owl#DatatypeProperty"/>
    <rdf:type rdf:resource="http://www.w3.org/2002/07/owl#FunctionalProperty"/>
    <rdfs:comment xml:lang="en">(for DrugStrength:) The amount of total liquid (or other divisible product, such as ointment, gel, spray, etc.).</rdfs:comment>
    <rdfs:domain rdf:resource="https://w3id.org/omop/ontology/DrugStrength"/>
    <rdfs:range rdf:resource="http://www.w3.org/2001/XMLSchema#decimal"/>
    <ns1:omop_cdm_name rdf:datatype="http://www.w3.org/2001/XMLSchema#string">drug_strength.denominator_value#417 AS float</ns1:omop_cdm_name>
  </rdf:Description>
  <rdf:Description rdf:about="https://w3id.org/omop/ontology/datetime">
    <rdf:type rdf:resource="http://www.w3.org/2002/07/owl#DatatypeProperty"/>
    <rdf:type rdf:resource="http://www.w3.org/2002/07/owl#FunctionalProperty"/>
    <rdfs:comment xml:lang="en">(for Measurement:) This is not required, though it is in v6. If a source does not specify datetime the convention is to set the time to midnight (00:00:0000)</rdfs:comment>
    <rdfs:comment xml:lang="en">(for Note:) If time is not given set the time to midnight.</rdfs:comment>
    <rdfs:comment xml:lang="en">(for NoteNlp:) The date and time of the note processing.</rdfs:comment>
    <rdfs:comment xml:lang="en">(for Observation:) If no time is given set to midnight (00:00:00).</rdfs:comment>
    <rdfs:comment xml:lang="en">(for ProcedureOccurrence:) This is not required, though it is in v6. If a source does not specify datetime the convention is to set the time to midnight (00:00:0000)</rdfs:comment>
    <rdfs:domain rdf:resource="https://w3id.org/omop/ontology/Event"/>
    <rdfs:range rdf:resource="http://www.w3.org/2001/XMLSchema#dateTime"/>
    <ns1:omop_cdm_name rdf:datatype="http://www.w3.org/2001/XMLSchema#string">death.death_datetime#172 AS datetime</ns1:omop_cdm_name>
    <ns1:omop_cdm_name rdf:datatype="http://www.w3.org/2001/XMLSchema#string">measurement.measurement_datetime#133 AS datetime</ns1:omop_cdm_name>
    <ns1:omop_cdm_name rdf:datatype="http://www.w3.org/2001/XMLSchema#string">metadata.metadata_datetime#351 AS datetime</ns1:omop_cdm_name>
    <ns1:omop_cdm_name rdf:datatype="http://www.w3.org/2001/XMLSchema#string">note.note_datetime#182 AS datetime</ns1:omop_cdm_name>
    <ns1:omop_cdm_name rdf:datatype="http://www.w3.org/2001/XMLSchema#string">note_nlp.nlp_datetime#203 AS datetime</ns1:omop_cdm_name>
    <ns1:omop_cdm_name rdf:datatype="http://www.w3.org/2001/XMLSchema#string">observation.observation_datetime#153 AS datetime</ns1:omop_cdm_name>
    <ns1:omop_cdm_name rdf:datatype="http://www.w3.org/2001/XMLSchema#string">procedure_occurrence.procedure_datetime#104 AS datetime</ns1:omop_cdm_name>
    <ns1:omop_cdm_name rdf:datatype="http://www.w3.org/2001/XMLSchema#string">specimen.specimen_datetime#212 AS datetime</ns1:omop_cdm_name>
  </rdf:Description>
  <rdf:Description rdf:about="https://w3id.org/omop/ontology/unit_source_value">
    <rdf:type rdf:resource="http://www.w3.org/2002/07/owl#DatatypeProperty"/>
    <rdf:type rdf:resource="http://www.w3.org/2002/07/owl#FunctionalProperty"/>
    <rdfs:comment xml:lang="en">(for Measurement:) This field houses the verbatim value from the source data representing the unit of the Measurement that occurred.
This code is mapped to a Standard Condition Concept in the Standardized Vocabularies and the original code is stored here for reference.</rdfs:comment>
    <rdfs:comment xml:lang="en">(for Observation:) This field houses the verbatim value from the source data representing the unit of the Observation that occurred.
This code is mapped to a Standard Condition Concept in the Standardized Vocabularies and the original code is stored here for reference.</rdfs:comment>
    <rdfs:comment xml:lang="en">(for Specimen:) This unit for the quantity of the specimen, as represented in the source.</rdfs:comment>
    <rdfs:domain rdf:nodeID="nde7e53d44aa94269b5c0c83d6d8798ccb73"/>
    <rdfs:range rdf:resource="http://www.w3.org/2001/XMLSchema#string"/>
    <ns1:omop_cdm_name rdf:datatype="http://www.w3.org/2001/XMLSchema#string">measurement.unit_source_value#147 AS str</ns1:omop_cdm_name>
    <ns1:omop_cdm_name rdf:datatype="http://www.w3.org/2001/XMLSchema#string">observation.unit_source_value#165 AS str</ns1:omop_cdm_name>
    <ns1:omop_cdm_name rdf:datatype="http://www.w3.org/2001/XMLSchema#string">specimen.unit_source_value#219 AS str</ns1:omop_cdm_name>
  </rdf:Description>
  <rdf:Description rdf:about="https://w3id.org/omop/ontology/has_admitted_from">
    <rdf:type rdf:resource="http://www.w3.org/2002/07/owl#FunctionalProperty"/>
    <rdf:type rdf:resource="http://www.w3.org/2002/07/owl#ObjectProperty"/>
    <ns2:python_name rdf:datatype="http://www.w3.org/2001/XMLSchema#string">admitted_from</ns2:python_name>
    <rdfs:comment xml:lang="en">(for VisitDetail:) This information may be called something different in the source data but the field is meant to contain a value indicating where a person was admitted from. Typically this applies only to visits that have a length of stay, like inpatient visits or long-term care visits.</rdfs:comment>
    <rdfs:comment xml:lang="en">(for VisitOccurrence:) Use this field to determine where the patient was admitted from. This concept is part of the visit domain and can indicate if a patient was admitted to the hospital from a long-term care facility, for example.
If available, map the admitted_from_source_value to a standard concept in the visit domain. If not available set to 0.</rdfs:comment>
    <rdfs:domain rdf:nodeID="nde7e53d44aa94269b5c0c83d6d8798ccb36"/>
    <rdfs:range rdf:resource="https://w3id.org/omop/ontology/Concept"/>
    <ns1:omop_cdm_name rdf:datatype="http://www.w3.org/2001/XMLSchema#string">visit_detail.admitted_from_concept_id#54 AS Concept</ns1:omop_cdm_name>
    <ns1:omop_cdm_name rdf:datatype="http://www.w3.org/2001/XMLSchema#string">visit_occurrence.admitted_from_concept_id#37 AS Concept</ns1:omop_cdm_name>
  </rdf:Description>
  <rdf:Description rdf:nodeID="nde7e53d44aa94269b5c0c83d6d8798ccb166">
    <rdf:type rdf:resource="http://www.w3.org/2002/07/owl#Restriction"/>
    <owl:allValuesFrom rdf:resource="http://www.w3.org/2001/XMLSchema#string"/>
    <owl:onProperty rdf:resource="https://w3id.org/omop/ontology/name"/>
  </rdf:Description>
  <rdf:Description rdf:about="https://w3id.org/omop/ontology/Duration">
    <rdf:type rdf:resource="http://www.w3.org/2002/07/owl#Class"/>
    <rdfs:subClassOf rdf:resource="https://w3id.org/omop/ontology/OmopCDMThing"/>
  </rdf:Description>
  <rdf:Description rdf:about="https://w3id.org/omop/ontology/refills">
    <rdf:type rdf:resource="http://www.w3.org/2002/07/owl#DatatypeProperty"/>
    <rdf:type rdf:resource="http://www.w3.org/2002/07/owl#FunctionalProperty"/>
    <rdfs:comment xml:lang="en">(for DrugExposure:) This is only filled in when the record is coming from a prescription written this field is meant to represent intended refills at time of the prescription.</rdfs:comment>
    <rdfs:domain rdf:resource="https://w3id.org/omop/ontology/DrugExposure"/>
    <rdfs:range rdf:resource="http://www.w3.org/2001/XMLSchema#integer"/>
    <ns1:omop_cdm_name rdf:datatype="http://www.w3.org/2001/XMLSchema#string">drug_exposure.refills#87 AS int</ns1:omop_cdm_name>
  </rdf:Description>
  <rdf:Description rdf:about="https://w3id.org/omop/ontology/has_payer_plan_period">
    <rdf:type rdf:resource="http://www.w3.org/2002/07/owl#FunctionalProperty"/>
    <rdf:type rdf:resource="http://www.w3.org/2002/07/owl#ObjectProperty"/>
    <ns2:python_name rdf:datatype="http://www.w3.org/2001/XMLSchema#string">payer_plan_period</ns2:python_name>
    <rdfs:comment xml:lang="en">(for Cost:) A foreign key to the PAYER_PLAN_PERIOD table, where the details of the Payer, Plan and Family are stored. Record the payer_plan_id that relates to the payer who contributed to the paid_by_payer field.</rdfs:comment>
    <rdfs:comment xml:lang="en">(reversed relation, for PayerPlanPeriod:) The Person covered by the Plan.
A single Person can have multiple, overlapping, PAYER_PLAN_PERIOD records</rdfs:comment>
    <rdfs:domain rdf:nodeID="nde7e53d44aa94269b5c0c83d6d8798ccb60"/>
    <rdfs:range rdf:resource="https://w3id.org/omop/ontology/PayerPlanPeriod"/>
    <ns1:omop_cdm_name rdf:datatype="http://www.w3.org/2001/XMLSchema#string">cost.payer_plan_period_id#324 AS PayerPlanPeriod</ns1:omop_cdm_name>
    <ns1:omop_cdm_name rdf:datatype="http://www.w3.org/2001/XMLSchema#string">payer_plan_period.person_id#287 AS Person</ns1:omop_cdm_name>
  </rdf:Description>
  <rdf:Description rdf:about="https://w3id.org/omop/ontology/LocationHistory">
    <rdf:type rdf:resource="http://www.w3.org/2002/07/owl#Class"/>
    <rdfs:subClassOf rdf:nodeID="nde7e53d44aa94269b5c0c83d6d8798ccb104"/>
    <rdfs:subClassOf rdf:nodeID="nde7e53d44aa94269b5c0c83d6d8798ccb105"/>
    <rdfs:subClassOf rdf:nodeID="nde7e53d44aa94269b5c0c83d6d8798ccb106"/>
    <rdfs:subClassOf rdf:nodeID="nde7e53d44aa94269b5c0c83d6d8798ccb107"/>
    <rdfs:subClassOf rdf:nodeID="nde7e53d44aa94269b5c0c83d6d8798ccb108"/>
    <rdfs:subClassOf rdf:nodeID="nde7e53d44aa94269b5c0c83d6d8798ccb109"/>
    <rdfs:subClassOf rdf:nodeID="nde7e53d44aa94269b5c0c83d6d8798ccb110"/>
    <rdfs:subClassOf rdf:nodeID="nde7e53d44aa94269b5c0c83d6d8798ccb111"/>
    <rdfs:subClassOf rdf:resource="https://w3id.org/omop/ontology/DateDuration"/>
    <ns1:omop_cdm_name rdf:datatype="http://www.w3.org/2001/XMLSchema#string">location_history</ns1:omop_cdm_name>
  </rdf:Description>
  <rdf:Description rdf:nodeID="nde7e53d44aa94269b5c0c83d6d8798ccb223">
    <rdf:type rdf:resource="http://www.w3.org/2002/07/owl#Restriction"/>
    <owl:allValuesFrom rdf:resource="https://w3id.org/omop/ontology/Location"/>
    <owl:onProperty rdf:resource="https://w3id.org/omop/ontology/has_location"/>
  </rdf:Description>
  <rdf:Description rdf:about="https://w3id.org/omop/ontology/has_ancestor">
    <rdf:type rdf:resource="http://www.w3.org/2002/07/owl#FunctionalProperty"/>
    <rdf:type rdf:resource="http://www.w3.org/2002/07/owl#ObjectProperty"/>
    <ns2:python_name rdf:datatype="http://www.w3.org/2001/XMLSchema#string">ancestor</ns2:python_name>
    <rdfs:comment xml:lang="en">(for ConceptAncestor:) The Concept Id for the higher-level concept
that forms the ancestor in the relationship.</rdfs:comment>
    <rdfs:domain rdf:resource="https://w3id.org/omop/ontology/ConceptAncestor"/>
    <rdfs:range rdf:resource="https://w3id.org/omop/ontology/Concept"/>
    <ns1:omop_cdm_name rdf:datatype="http://www.w3.org/2001/XMLSchema#string">concept_ancestor.ancestor_concept_id#398 AS Concept</ns1:omop_cdm_name>
  </rdf:Description>
  <rdf:Description rdf:about="https://w3id.org/omop/ontology/npi">
    <rdf:type rdf:resource="http://www.w3.org/2002/07/owl#DatatypeProperty"/>
    <rdf:type rdf:resource="http://www.w3.org/2002/07/owl#FunctionalProperty"/>
    <rdfs:comment xml:lang="en">(for Provider:) This is the National Provider Number issued to health care providers in the US by the Centers for Medicare and Medicaid Services (CMS).</rdfs:comment>
    <rdfs:domain rdf:resource="https://w3id.org/omop/ontology/Provider"/>
    <rdfs:range rdf:resource="http://www.w3.org/2001/XMLSchema#string"/>
    <ns1:omop_cdm_name rdf:datatype="http://www.w3.org/2001/XMLSchema#string">provider.npi#275 AS str</ns1:omop_cdm_name>
  </rdf:Description>
  <rdf:Description rdf:nodeID="nde7e53d44aa94269b5c0c83d6d8798ccb510">
    <rdf:type rdf:resource="http://www.w3.org/2002/07/owl#Restriction"/>
    <owl:allValuesFrom rdf:resource="http://www.w3.org/2002/07/owl#Thing"/>
    <owl:onProperty rdf:resource="https://w3id.org/omop/ontology/has_event"/>
  </rdf:Description>
  <rdf:Description rdf:nodeID="nde7e53d44aa94269b5c0c83d6d8798ccb477">
    <rdf:type rdf:resource="http://www.w3.org/2002/07/owl#Restriction"/>
    <owl:allValuesFrom rdf:resource="https://w3id.org/omop/ontology/Concept"/>
    <owl:onProperty rdf:resource="https://w3id.org/omop/ontology/has_specialty"/>
  </rdf:Description>
  <rdf:Description rdf:about="https://w3id.org/omop/ontology/has_device_exposure">
    <rdf:type rdf:resource="http://www.w3.org/2002/07/owl#ObjectProperty"/>
    <ns2:python_name rdf:datatype="http://www.w3.org/2001/XMLSchema#string">device_exposures</ns2:python_name>
    <rdfs:comment xml:lang="en">(reversed relation, for DeviceExposure:) The Visit Detail during which the device was prescribed or given.
To populate this field device exposures must be explicitly initiated in the visit detail record.</rdfs:comment>
    <rdfs:comment xml:lang="en">(reversed relation, for DeviceExposure:) The Visit during which the device was prescribed or given.
To populate this field device exposures must be explicitly initiated in the visit.</rdfs:comment>
    <rdfs:domain rdf:nodeID="nde7e53d44aa94269b5c0c83d6d8798ccb42"/>
    <rdfs:range rdf:resource="https://w3id.org/omop/ontology/DeviceExposure"/>
    <ns1:omop_cdm_name rdf:datatype="http://www.w3.org/2001/XMLSchema#string">device_exposure.person_id#115 AS Person</ns1:omop_cdm_name>
    <ns1:omop_cdm_name rdf:datatype="http://www.w3.org/2001/XMLSchema#string">device_exposure.visit_detail_id#126 AS VisitDetail</ns1:omop_cdm_name>
    <ns1:omop_cdm_name rdf:datatype="http://www.w3.org/2001/XMLSchema#string">device_exposure.visit_occurrence_id#125 AS VisitOccurrence</ns1:omop_cdm_name>
  </rdf:Description>
  <rdf:Description rdf:about="https://w3id.org/omop/ontology/county">
    <rdf:type rdf:resource="http://www.w3.org/2002/07/owl#DatatypeProperty"/>
    <rdf:type rdf:resource="http://www.w3.org/2002/07/owl#FunctionalProperty"/>
    <rdfs:domain rdf:resource="https://w3id.org/omop/ontology/Location"/>
    <rdfs:range rdf:resource="http://www.w3.org/2001/XMLSchema#string"/>
    <ns1:omop_cdm_name rdf:datatype="http://www.w3.org/2001/XMLSchema#string">location.county#257 AS str</ns1:omop_cdm_name>
  </rdf:Description>
  <rdf:Description rdf:about="https://w3id.org/omop/ontology/specialty_source_value">
    <rdf:type rdf:resource="http://www.w3.org/2002/07/owl#DatatypeProperty"/>
    <rdf:type rdf:resource="http://www.w3.org/2002/07/owl#FunctionalProperty"/>
    <rdfs:comment xml:lang="en">(for Provider:) This is the kind of provider or specialty as it appears in the source data. This includes physician specialties such as internal medicine, emergency medicine, etc. and allied health professionals such as nurses, midwives, and pharmacists.
Put the kind of provider as it appears in the source data. This field is up to the discretion of the ETL-er as to whether this should be the coded value from the source or the text description of the lookup value.</rdfs:comment>
    <rdfs:domain rdf:resource="https://w3id.org/omop/ontology/Provider"/>
    <rdfs:range rdf:resource="http://www.w3.org/2001/XMLSchema#string"/>
    <ns1:omop_cdm_name rdf:datatype="http://www.w3.org/2001/XMLSchema#string">provider.specialty_source_value#282 AS str</ns1:omop_cdm_name>
  </rdf:Description>
  <rdf:Description rdf:nodeID="nde7e53d44aa94269b5c0c83d6d8798ccb529">
    <rdf:type rdf:resource="http://www.w3.org/2002/07/owl#Restriction"/>
    <owl:allValuesFrom rdf:resource="https://w3id.org/omop/ontology/Concept"/>
    <owl:onProperty rdf:resource="https://w3id.org/omop/ontology/has_concept"/>
  </rdf:Description>
  <rdf:Description rdf:about="https://w3id.org/omop/ontology/lot_number">
    <rdf:type rdf:resource="http://www.w3.org/2002/07/owl#DatatypeProperty"/>
    <rdf:type rdf:resource="http://www.w3.org/2002/07/owl#FunctionalProperty"/>
    <rdfs:domain rdf:resource="https://w3id.org/omop/ontology/DrugExposure"/>
    <rdfs:range rdf:resource="http://www.w3.org/2001/XMLSchema#string"/>
    <ns1:omop_cdm_name rdf:datatype="http://www.w3.org/2001/XMLSchema#string">drug_exposure.lot_number#92 AS str</ns1:omop_cdm_name>
  </rdf:Description>
  <rdf:Description rdf:about="https://w3id.org/omop/ontology/has_payer">
    <rdf:type rdf:resource="http://www.w3.org/2002/07/owl#FunctionalProperty"/>
    <rdf:type rdf:resource="http://www.w3.org/2002/07/owl#ObjectProperty"/>
    <ns2:python_name rdf:datatype="http://www.w3.org/2001/XMLSchema#string">payer</ns2:python_name>
    <rdfs:comment xml:lang="en">(for PayerPlanPeriod:) This field represents the organization who reimburses the provider which administers care to the Person.
Map the Payer directly to a standard CONCEPT_ID. If one does not exists please contact the vocabulary team. There is no global controlled vocabulary available for this information. The point is to stratify on this information and identify if Persons have the same payer, though the name of the Payer is not necessary. If not available, set to 0. [Accepted Concepts](http://athena.ohdsi.org/search-terms/terms?domain=Payer&amp;standardConcept=Standard&amp;page=1&amp;pageSize=15&amp;query=).</rdfs:comment>
    <rdfs:domain rdf:resource="https://w3id.org/omop/ontology/PayerPlanPeriod"/>
    <rdfs:range rdf:resource="https://w3id.org/omop/ontology/Concept"/>
    <ns1:omop_cdm_name rdf:datatype="http://www.w3.org/2001/XMLSchema#string">payer_plan_period.payer_concept_id#291 AS Concept</ns1:omop_cdm_name>
  </rdf:Description>
  <rdf:Description rdf:about="https://w3id.org/omop/ontology/Vocabulary">
    <rdf:type rdf:resource="http://www.w3.org/2002/07/owl#Class"/>
    <rdfs:subClassOf rdf:nodeID="nde7e53d44aa94269b5c0c83d6d8798ccb400"/>
    <rdfs:subClassOf rdf:nodeID="nde7e53d44aa94269b5c0c83d6d8798ccb401"/>
    <rdfs:subClassOf rdf:nodeID="nde7e53d44aa94269b5c0c83d6d8798ccb402"/>
    <rdfs:subClassOf rdf:nodeID="nde7e53d44aa94269b5c0c83d6d8798ccb403"/>
    <rdfs:subClassOf rdf:nodeID="nde7e53d44aa94269b5c0c83d6d8798ccb404"/>
    <rdfs:subClassOf rdf:nodeID="nde7e53d44aa94269b5c0c83d6d8798ccb405"/>
    <rdfs:subClassOf rdf:nodeID="nde7e53d44aa94269b5c0c83d6d8798ccb406"/>
    <rdfs:subClassOf rdf:resource="https://w3id.org/omop/ontology/OmopCDMThing"/>
    <ns1:omop_cdm_name rdf:datatype="http://www.w3.org/2001/XMLSchema#string">vocabulary</ns1:omop_cdm_name>
  </rdf:Description>
  <rdf:Description rdf:nodeID="nde7e53d44aa94269b5c0c83d6d8798ccb561">
    <rdf:first rdf:resource="https://w3id.org/omop/ontology/Death"/>
    <rdf:rest rdf:nodeID="nde7e53d44aa94269b5c0c83d6d8798ccb562"/>
  </rdf:Description>
  <rdf:Description rdf:about="https://w3id.org/omop/ontology/has_unit">
    <rdf:type rdf:resource="http://www.w3.org/2002/07/owl#FunctionalProperty"/>
    <rdf:type rdf:resource="http://www.w3.org/2002/07/owl#ObjectProperty"/>
    <ns2:python_name rdf:datatype="http://www.w3.org/2001/XMLSchema#string">unit</ns2:python_name>
    <rdfs:comment xml:lang="en">(for DoseEra:) The Concept Id representing the unit of the specific drug ingredient.</rdfs:comment>
    <rdfs:comment xml:lang="en">(for Measurement:) There is currently no recommended unit for individual measurements, i.e. it is not mandatory to represent Hemoglobin a1C measurements as a percentage. UNIT_SOURCE_VALUES should be mapped to a Standard Concept in the Unit domain that best represents the unit as given in the source data.
There is no standardization requirement for units associated with MEASUREMENT_CONCEPT_IDs, however, it is the responsibility of the ETL to choose the most plausible unit.</rdfs:comment>
    <rdfs:comment xml:lang="en">(for Observation:) There is currently no recommended unit for individual observation concepts. UNIT_SOURCE_VALUES should be mapped to a Standard Concept in the Unit domain that best represents the unit as given in the source data.
There is no standardization requirement for units associated with OBSERVATION_CONCEPT_IDs, however, it is the responsibility of the ETL to choose the most plausible unit.</rdfs:comment>
    <rdfs:comment xml:lang="en">(for Specimen:) The unit for the quantity of the specimen.
Map the UNIT_SOURCE_VALUE to a Standard Concept in the Unit domain. [Accepted Concepts](https://athena.ohdsi.org/search-terms/terms?domain=Unit&amp;standardConcept=Standard&amp;page=1&amp;pageSize=15&amp;query=)</rdfs:comment>
    <rdfs:domain rdf:nodeID="nde7e53d44aa94269b5c0c83d6d8798ccb170"/>
    <rdfs:range rdf:resource="https://w3id.org/omop/ontology/Concept"/>
    <ns1:omop_cdm_name rdf:datatype="http://www.w3.org/2001/XMLSchema#string">dose_era.unit_concept_id#335 AS Concept</ns1:omop_cdm_name>
    <ns1:omop_cdm_name rdf:datatype="http://www.w3.org/2001/XMLSchema#string">measurement.unit_concept_id#139 AS Concept</ns1:omop_cdm_name>
    <ns1:omop_cdm_name rdf:datatype="http://www.w3.org/2001/XMLSchema#string">observation.unit_concept_id#159 AS Concept</ns1:omop_cdm_name>
    <ns1:omop_cdm_name rdf:datatype="http://www.w3.org/2001/XMLSchema#string">specimen.unit_concept_id#214 AS Concept</ns1:omop_cdm_name>
  </rdf:Description>
  <rdf:Description rdf:about="https://w3id.org/omop/ontology/ConceptRelationship">
    <rdf:type rdf:resource="http://www.w3.org/2002/07/owl#Class"/>
    <rdfs:subClassOf rdf:nodeID="nde7e53d44aa94269b5c0c83d6d8798ccb175"/>
    <rdfs:subClassOf rdf:nodeID="nde7e53d44aa94269b5c0c83d6d8798ccb176"/>
    <rdfs:subClassOf rdf:nodeID="nde7e53d44aa94269b5c0c83d6d8798ccb177"/>
    <rdfs:subClassOf rdf:nodeID="nde7e53d44aa94269b5c0c83d6d8798ccb178"/>
    <rdfs:subClassOf rdf:nodeID="nde7e53d44aa94269b5c0c83d6d8798ccb179"/>
    <rdfs:subClassOf rdf:nodeID="nde7e53d44aa94269b5c0c83d6d8798ccb180"/>
    <rdfs:subClassOf rdf:nodeID="nde7e53d44aa94269b5c0c83d6d8798ccb181"/>
    <rdfs:subClassOf rdf:nodeID="nde7e53d44aa94269b5c0c83d6d8798ccb182"/>
    <rdfs:subClassOf rdf:nodeID="nde7e53d44aa94269b5c0c83d6d8798ccb183"/>
    <rdfs:subClassOf rdf:nodeID="nde7e53d44aa94269b5c0c83d6d8798ccb184"/>
    <rdfs:subClassOf rdf:nodeID="nde7e53d44aa94269b5c0c83d6d8798ccb185"/>
    <rdfs:subClassOf rdf:resource="https://w3id.org/omop/ontology/OmopCDMThing"/>
    <ns1:omop_cdm_name rdf:datatype="http://www.w3.org/2001/XMLSchema#string">concept_relationship</ns1:omop_cdm_name>
  </rdf:Description>
  <rdf:Description rdf:about="https://w3id.org/omop/ontology/has_anatomic_site">
    <rdf:type rdf:resource="http://www.w3.org/2002/07/owl#FunctionalProperty"/>
    <rdf:type rdf:resource="http://www.w3.org/2002/07/owl#ObjectProperty"/>
    <ns2:python_name rdf:datatype="http://www.w3.org/2001/XMLSchema#string">anatomic_site</ns2:python_name>
    <rdfs:comment xml:lang="en">(for Specimen:) This is the site on the body where the specimen is from.
Map the ANATOMIC_SITE_SOURCE_VALUE to a Standard Concept in the Spec Anatomic Site domain. This should be coded at the lowest level of granularity [Accepted Concepts](https://athena.ohdsi.org/search-terms/terms?standardConcept=Standard&amp;domain=Spec+Anatomic+Site&amp;conceptClass=Body+Structure&amp;page=4&amp;pageSize=15&amp;query=)</rdfs:comment>
    <rdfs:domain rdf:resource="https://w3id.org/omop/ontology/Specimen"/>
    <rdfs:range rdf:resource="https://w3id.org/omop/ontology/Concept"/>
    <ns1:omop_cdm_name rdf:datatype="http://www.w3.org/2001/XMLSchema#string">specimen.anatomic_site_concept_id#215 AS Concept</ns1:omop_cdm_name>
  </rdf:Description>
  <rdf:Description rdf:about="https://w3id.org/omop/ontology/Metadata">
    <rdf:type rdf:resource="http://www.w3.org/2002/07/owl#Class"/>
    <rdfs:subClassOf rdf:nodeID="nde7e53d44aa94269b5c0c83d6d8798ccb162"/>
    <rdfs:subClassOf rdf:nodeID="nde7e53d44aa94269b5c0c83d6d8798ccb163"/>
    <rdfs:subClassOf rdf:nodeID="nde7e53d44aa94269b5c0c83d6d8798ccb164"/>
    <rdfs:subClassOf rdf:nodeID="nde7e53d44aa94269b5c0c83d6d8798ccb165"/>
    <rdfs:subClassOf rdf:nodeID="nde7e53d44aa94269b5c0c83d6d8798ccb166"/>
    <rdfs:subClassOf rdf:nodeID="nde7e53d44aa94269b5c0c83d6d8798ccb167"/>
    <rdfs:subClassOf rdf:nodeID="nde7e53d44aa94269b5c0c83d6d8798ccb168"/>
    <rdfs:subClassOf rdf:nodeID="nde7e53d44aa94269b5c0c83d6d8798ccb169"/>
    <rdfs:subClassOf rdf:resource="https://w3id.org/omop/ontology/Event"/>
    <ns1:omop_cdm_name rdf:datatype="http://www.w3.org/2001/XMLSchema#string">metadata</ns1:omop_cdm_name>
  </rdf:Description>
  <rdf:Description rdf:about="https://w3id.org/omop/ontology/DoseEra">
    <rdf:type rdf:resource="http://www.w3.org/2002/07/owl#Class"/>
    <rdfs:subClassOf rdf:nodeID="nde7e53d44aa94269b5c0c83d6d8798ccb92"/>
    <rdfs:subClassOf rdf:nodeID="nde7e53d44aa94269b5c0c83d6d8798ccb93"/>
    <rdfs:subClassOf rdf:nodeID="nde7e53d44aa94269b5c0c83d6d8798ccb95"/>
    <rdfs:subClassOf rdf:nodeID="nde7e53d44aa94269b5c0c83d6d8798ccb96"/>
    <rdfs:subClassOf rdf:nodeID="nde7e53d44aa94269b5c0c83d6d8798ccb97"/>
    <rdfs:subClassOf rdf:resource="https://w3id.org/omop/ontology/Era"/>
    <ns1:omop_cdm_name rdf:datatype="http://www.w3.org/2001/XMLSchema#string">dose_era</ns1:omop_cdm_name>
  </rdf:Description>
  <rdf:Description rdf:about="https://w3id.org/omop/ontology/has_drug_era">
    <rdf:type rdf:resource="http://www.w3.org/2002/07/owl#ObjectProperty"/>
    <ns2:python_name rdf:datatype="http://www.w3.org/2001/XMLSchema#string">drug_eras</ns2:python_name>
    <rdfs:domain rdf:resource="https://w3id.org/omop/ontology/Person"/>
    <rdfs:range rdf:resource="https://w3id.org/omop/ontology/DrugEra"/>
    <ns1:omop_cdm_name rdf:datatype="http://www.w3.org/2001/XMLSchema#string">drug_era.person_id#326 AS Person</ns1:omop_cdm_name>
  </rdf:Description>
  <rdf:Description rdf:nodeID="nde7e53d44aa94269b5c0c83d6d8798ccb478">
    <rdf:type rdf:resource="http://www.w3.org/2002/07/owl#Restriction"/>
    <owl:allValuesFrom rdf:resource="http://www.w3.org/2001/XMLSchema#string"/>
    <owl:onProperty rdf:resource="https://w3id.org/omop/ontology/npi"/>
  </rdf:Description>
  <rdf:Description rdf:nodeID="nde7e53d44aa94269b5c0c83d6d8798ccb624">
    <rdf:first rdf:resource="https://w3id.org/omop/ontology/NoteNlp"/>
    <rdf:rest rdf:nodeID="nde7e53d44aa94269b5c0c83d6d8798ccb625"/>
  </rdf:Description>
  <rdf:Description rdf:about="https://w3id.org/omop/ontology/date">
    <rdf:type rdf:resource="http://www.w3.org/2002/07/owl#DatatypeProperty"/>
    <rdf:type rdf:resource="http://www.w3.org/2002/07/owl#FunctionalProperty"/>
    <rdfs:comment xml:lang="en">(for Measurement:) Use this date to determine the date of the measurement.
If there are multiple dates in the source data associated with a record such as order_date, draw_date, and result_date, choose the one that is closest to the date the sample was drawn from the patient.</rdfs:comment>
    <rdfs:comment xml:lang="en">(for Note:) The date the note was recorded.</rdfs:comment>
    <rdfs:comment xml:lang="en">(for NoteNlp:) The date of the note processing.</rdfs:comment>
    <rdfs:comment xml:lang="en">(for Observation:) The date of the Observation. Depending on what the Observation represents this could be the date of a lab test, the date of a survey, or the date a patient's family history was taken.
For some observations the ETL may need to make a choice as to which date to choose.</rdfs:comment>
    <rdfs:comment xml:lang="en">(for ProcedureOccurrence:) Use this date to determine the date the procedure occurred.
If a procedure lasts more than a day, then it should be recorded as a separate record for each day the procedure occurred, this logic is in lieu of the procedure_end_date, which will be added in a future version of the CDM.</rdfs:comment>
    <rdfs:comment xml:lang="en">(for Specimen:) The date the specimen was collected.</rdfs:comment>
    <rdfs:domain rdf:resource="https://w3id.org/omop/ontology/Event"/>
    <rdfs:range rdf:resource="http://www.w3.org/2001/XMLSchema#date"/>
    <ns1:omop_cdm_name rdf:datatype="http://www.w3.org/2001/XMLSchema#string">death.death_date#171 AS date</ns1:omop_cdm_name>
    <ns1:omop_cdm_name rdf:datatype="http://www.w3.org/2001/XMLSchema#string">measurement.measurement_date#132 AS date</ns1:omop_cdm_name>
    <ns1:omop_cdm_name rdf:datatype="http://www.w3.org/2001/XMLSchema#string">metadata.metadata_date#350 AS date</ns1:omop_cdm_name>
    <ns1:omop_cdm_name rdf:datatype="http://www.w3.org/2001/XMLSchema#string">note.note_date#181 AS date</ns1:omop_cdm_name>
    <ns1:omop_cdm_name rdf:datatype="http://www.w3.org/2001/XMLSchema#string">note_nlp.nlp_date#202 AS date</ns1:omop_cdm_name>
    <ns1:omop_cdm_name rdf:datatype="http://www.w3.org/2001/XMLSchema#string">observation.observation_date#152 AS date</ns1:omop_cdm_name>
    <ns1:omop_cdm_name rdf:datatype="http://www.w3.org/2001/XMLSchema#string">procedure_occurrence.procedure_date#103 AS date</ns1:omop_cdm_name>
    <ns1:omop_cdm_name rdf:datatype="http://www.w3.org/2001/XMLSchema#string">specimen.specimen_date#211 AS date</ns1:omop_cdm_name>
  </rdf:Description>
  <rdf:Description rdf:about="https://w3id.org/omop/ontology/has_cause">
    <rdf:type rdf:resource="http://www.w3.org/2002/07/owl#FunctionalProperty"/>
    <rdf:type rdf:resource="http://www.w3.org/2002/07/owl#ObjectProperty"/>
    <ns2:python_name rdf:datatype="http://www.w3.org/2001/XMLSchema#string">cause</ns2:python_name>
    <rdfs:domain rdf:resource="https://w3id.org/omop/ontology/Death"/>
    <rdfs:range rdf:resource="https://w3id.org/omop/ontology/Concept"/>
    <ns1:omop_cdm_name rdf:datatype="http://www.w3.org/2001/XMLSchema#string">death.cause_concept_id#174 AS Concept</ns1:omop_cdm_name>
  </rdf:Description>
  <rdf:Description rdf:about="https://w3id.org/omop/ontology/cdm_release_date">
    <rdf:type rdf:resource="http://www.w3.org/2002/07/owl#DatatypeProperty"/>
    <rdf:type rdf:resource="http://www.w3.org/2002/07/owl#FunctionalProperty"/>
    <rdfs:comment xml:lang="en">(for CdmSource:) The release data of the CDM instance.</rdfs:comment>
    <rdfs:domain rdf:resource="https://w3id.org/omop/ontology/CdmSource"/>
    <rdfs:range rdf:resource="http://www.w3.org/2001/XMLSchema#date"/>
    <ns1:omop_cdm_name rdf:datatype="http://www.w3.org/2001/XMLSchema#string">cdm_source.cdm_release_date#359 AS date</ns1:omop_cdm_name>
  </rdf:Description>
  <rdf:Description rdf:nodeID="nde7e53d44aa94269b5c0c83d6d8798ccb648">
    <rdf:type rdf:resource="http://www.w3.org/2002/07/owl#Restriction"/>
    <owl:allValuesFrom rdf:resource="https://w3id.org/omop/ontology/Death"/>
    <owl:onProperty rdf:resource="https://w3id.org/omop/ontology/has_death"/>
  </rdf:Description>
  <rdf:Description rdf:nodeID="nde7e53d44aa94269b5c0c83d6d8798ccb426">
    <rdf:type rdf:resource="http://www.w3.org/2002/07/owl#Restriction"/>
    <owl:allValuesFrom rdf:resource="https://w3id.org/omop/ontology/Concept"/>
    <owl:onProperty rdf:resource="https://w3id.org/omop/ontology/has_language"/>
  </rdf:Description>
  <rdf:Description rdf:nodeID="nde7e53d44aa94269b5c0c83d6d8798ccb379">
    <rdf:type rdf:resource="http://www.w3.org/2002/07/owl#Restriction"/>
    <owl:allValuesFrom rdf:resource="http://www.w3.org/2001/XMLSchema#integer"/>
    <owl:onProperty rdf:resource="https://w3id.org/omop/ontology/refills"/>
  </rdf:Description>
  <rdf:Description rdf:about="https://w3id.org/omop/ontology/has_timing">
    <rdf:type rdf:resource="http://www.w3.org/2002/07/owl#FunctionalProperty"/>
    <rdf:type rdf:resource="http://www.w3.org/2002/07/owl#ObjectProperty"/>
    <ns2:python_name rdf:datatype="http://www.w3.org/2001/XMLSchema#string">timing</ns2:python_name>
    <rdfs:comment xml:lang="en">(for SurveyConduct:) This is a Concept that represents the timing of the survey. For example this could be the 3-month follow-up appointment.
There is no specific domain or class for this field, just choose the one that best represents the value given in the source.</rdfs:comment>
    <rdfs:domain rdf:resource="https://w3id.org/omop/ontology/SurveyConduct"/>
    <rdfs:range rdf:resource="https://w3id.org/omop/ontology/Concept"/>
    <ns1:omop_cdm_name rdf:datatype="http://www.w3.org/2001/XMLSchema#string">survey_conduct.timing_concept_id#237 AS Concept</ns1:omop_cdm_name>
  </rdf:Description>
  <rdf:Description rdf:nodeID="nde7e53d44aa94269b5c0c83d6d8798ccb389">
    <rdf:type rdf:resource="http://www.w3.org/2002/07/owl#Restriction"/>
    <owl:allValuesFrom rdf:resource="https://w3id.org/omop/ontology/Concept"/>
    <owl:onProperty rdf:resource="https://w3id.org/omop/ontology/has_disease_status"/>
  </rdf:Description>
  <rdf:Description rdf:about="https://w3id.org/omop/ontology/has_condition_occurrence">
    <rdf:type rdf:resource="http://www.w3.org/2002/07/owl#ObjectProperty"/>
    <ns2:python_name rdf:datatype="http://www.w3.org/2001/XMLSchema#string">condition_occurrences</ns2:python_name>
    <rdfs:comment xml:lang="en">(reversed relation, for ConditionOccurrence:) The PERSON_ID of the PERSON for whom the condition is recorded.</rdfs:comment>
    <rdfs:comment xml:lang="en">(reversed relation, for ConditionOccurrence:) The VISIT_DETAIL record during which the condition occurred. For example, if the person was in the ICU at the time of the diagnosis the VISIT_OCCURRENCE record would reflect the overall hospital stay and the VISIT_DETAIL record would reflect the ICU stay during the hospital visit.
Same rules apply as for the VISIT_OCCURRENCE_ID.</rdfs:comment>
    <rdfs:comment xml:lang="en">(reversed relation, for ConditionOccurrence:) The visit during which the condition occurred.
Depending on the structure of the source data, this may have to be determined based on dates. If a CONDITION_START_DATE occurs within the start and end date of a Visit it is a valid ETL choice to choose the VISIT_OCCURRENCE_ID from the Visit that subsumes it, even if not explicitly stated in the data. While not required, an attempt should be made to locate the VISIT_OCCURRENCE_ID of the CONDITION_OCCURRENCE record.</rdfs:comment>
    <rdfs:domain rdf:nodeID="nde7e53d44aa94269b5c0c83d6d8798ccb39"/>
    <rdfs:range rdf:resource="https://w3id.org/omop/ontology/ConditionOccurrence"/>
    <ns1:omop_cdm_name rdf:datatype="http://www.w3.org/2001/XMLSchema#string">condition_occurrence.person_id#62 AS Person</ns1:omop_cdm_name>
    <ns1:omop_cdm_name rdf:datatype="http://www.w3.org/2001/XMLSchema#string">condition_occurrence.visit_detail_id#73 AS VisitDetail</ns1:omop_cdm_name>
    <ns1:omop_cdm_name rdf:datatype="http://www.w3.org/2001/XMLSchema#string">condition_occurrence.visit_occurrence_id#72 AS VisitOccurrence</ns1:omop_cdm_name>
  </rdf:Description>
  <rdf:Description rdf:nodeID="nde7e53d44aa94269b5c0c83d6d8798ccb413">
    <rdf:type rdf:resource="http://www.w3.org/2002/07/owl#Restriction"/>
    <owl:allValuesFrom rdf:resource="http://www.w3.org/2001/XMLSchema#string"/>
    <owl:onProperty rdf:resource="https://w3id.org/omop/ontology/state"/>
  </rdf:Description>
  <rdf:Description rdf:nodeID="nde7e53d44aa94269b5c0c83d6d8798ccb81">
    <rdf:type rdf:resource="http://www.w3.org/2002/07/owl#Restriction"/>
    <owl:onProperty rdf:resource="https://w3id.org/omop/ontology/min_levels_of_separation"/>
    <owl:someValuesFrom rdf:resource="http://www.w3.org/2001/XMLSchema#integer"/>
  </rdf:Description>
  <rdf:Description rdf:about="https://w3id.org/omop/ontology/DrugStrength">
    <rdf:type rdf:resource="http://www.w3.org/2002/07/owl#Class"/>
    <rdfs:subClassOf rdf:nodeID="nde7e53d44aa94269b5c0c83d6d8798ccb323"/>
    <rdfs:subClassOf rdf:nodeID="nde7e53d44aa94269b5c0c83d6d8798ccb324"/>
    <rdfs:subClassOf rdf:nodeID="nde7e53d44aa94269b5c0c83d6d8798ccb325"/>
    <rdfs:subClassOf rdf:nodeID="nde7e53d44aa94269b5c0c83d6d8798ccb326"/>
    <rdfs:subClassOf rdf:nodeID="nde7e53d44aa94269b5c0c83d6d8798ccb327"/>
    <rdfs:subClassOf rdf:nodeID="nde7e53d44aa94269b5c0c83d6d8798ccb328"/>
    <rdfs:subClassOf rdf:nodeID="nde7e53d44aa94269b5c0c83d6d8798ccb329"/>
    <rdfs:subClassOf rdf:nodeID="nde7e53d44aa94269b5c0c83d6d8798ccb330"/>
    <rdfs:subClassOf rdf:nodeID="nde7e53d44aa94269b5c0c83d6d8798ccb331"/>
    <rdfs:subClassOf rdf:nodeID="nde7e53d44aa94269b5c0c83d6d8798ccb332"/>
    <rdfs:subClassOf rdf:nodeID="nde7e53d44aa94269b5c0c83d6d8798ccb333"/>
    <rdfs:subClassOf rdf:nodeID="nde7e53d44aa94269b5c0c83d6d8798ccb334"/>
    <rdfs:subClassOf rdf:nodeID="nde7e53d44aa94269b5c0c83d6d8798ccb335"/>
    <rdfs:subClassOf rdf:nodeID="nde7e53d44aa94269b5c0c83d6d8798ccb336"/>
    <rdfs:subClassOf rdf:nodeID="nde7e53d44aa94269b5c0c83d6d8798ccb337"/>
    <rdfs:subClassOf rdf:nodeID="nde7e53d44aa94269b5c0c83d6d8798ccb338"/>
    <rdfs:subClassOf rdf:resource="https://w3id.org/omop/ontology/OmopCDMThing"/>
    <ns1:omop_cdm_name rdf:datatype="http://www.w3.org/2001/XMLSchema#string">drug_strength</ns1:omop_cdm_name>
  </rdf:Description>
  <rdf:Description rdf:nodeID="nde7e53d44aa94269b5c0c83d6d8798ccb192">
    <rdf:type rdf:resource="http://www.w3.org/2002/07/owl#Restriction"/>
    <owl:allValuesFrom rdf:resource="https://w3id.org/omop/ontology/Concept"/>
    <owl:onProperty rdf:resource="https://w3id.org/omop/ontology/has_gender_source"/>
  </rdf:Description>
  <rdf:Description rdf:about="https://w3id.org/omop/ontology/version">
    <rdf:type rdf:resource="http://www.w3.org/2002/07/owl#DatatypeProperty"/>
    <rdf:type rdf:resource="http://www.w3.org/2002/07/owl#FunctionalProperty"/>
    <rdfs:comment xml:lang="en">(for Vocabulary:) Version of the Vocabulary as indicated in
the source.</rdfs:comment>
    <rdfs:domain rdf:resource="https://w3id.org/omop/ontology/Vocabulary"/>
    <rdfs:range rdf:resource="http://www.w3.org/2001/XMLSchema#string"/>
    <ns1:omop_cdm_name rdf:datatype="http://www.w3.org/2001/XMLSchema#string">vocabulary.vocabulary_version#375 AS str</ns1:omop_cdm_name>
  </rdf:Description>
  <rdf:Description rdf:about="https://w3id.org/omop/ontology/is_hierarchical">
    <rdf:type rdf:resource="http://www.w3.org/2002/07/owl#DatatypeProperty"/>
    <rdf:type rdf:resource="http://www.w3.org/2002/07/owl#FunctionalProperty"/>
    <rdfs:domain rdf:resource="https://w3id.org/omop/ontology/Relationship"/>
    <rdfs:range rdf:resource="http://www.w3.org/2001/XMLSchema#string"/>
    <ns1:omop_cdm_name rdf:datatype="http://www.w3.org/2001/XMLSchema#string">relationship.is_hierarchical#391 AS str</ns1:omop_cdm_name>
  </rdf:Description>
  <rdf:Description rdf:nodeID="nde7e53d44aa94269b5c0c83d6d8798ccb258">
    <rdf:type rdf:resource="http://www.w3.org/2002/07/owl#Restriction"/>
    <owl:allValuesFrom rdf:resource="https://w3id.org/omop/ontology/Concept"/>
    <owl:onProperty rdf:resource="https://w3id.org/omop/ontology/has_source"/>
  </rdf:Description>
  <rdf:Description rdf:about="https://w3id.org/omop/ontology/discharge_to_source_value">
    <rdf:type rdf:resource="http://www.w3.org/2002/07/owl#DatatypeProperty"/>
    <rdf:type rdf:resource="http://www.w3.org/2002/07/owl#FunctionalProperty"/>
    <rdfs:comment xml:lang="en">(for VisitDetail:) This information may be called something different in the source data but the field is meant to contain a value indicating where a person was discharged to after a visit, as in they went home or were moved to long-term care. Typically this applies only to visits that have a length of stay of a day or more.</rdfs:comment>
    <rdfs:comment xml:lang="en">(for VisitOccurrence:) This information may be called something different in the source data but the field is meant to contain a value indicating where a person was discharged to after a visit, as in they went home or were moved to long-term care. Typically this applies only to visits that have a length of stay of a day or more.</rdfs:comment>
    <rdfs:domain rdf:resource="https://w3id.org/omop/ontology/BaseVisit"/>
    <rdfs:range rdf:resource="http://www.w3.org/2001/XMLSchema#string"/>
    <ns1:omop_cdm_name rdf:datatype="http://www.w3.org/2001/XMLSchema#string">visit_detail.discharge_to_source_value#56 AS str</ns1:omop_cdm_name>
    <ns1:omop_cdm_name rdf:datatype="http://www.w3.org/2001/XMLSchema#string">visit_occurrence.discharge_to_source_value#40 AS str</ns1:omop_cdm_name>
  </rdf:Description>
  <rdf:Description rdf:nodeID="nde7e53d44aa94269b5c0c83d6d8798ccb683">
    <rdf:type rdf:resource="http://www.w3.org/2002/07/owl#Restriction"/>
    <owl:allValuesFrom rdf:resource="https://w3id.org/omop/ontology/ConceptClass"/>
    <owl:onProperty rdf:resource="https://w3id.org/omop/ontology/has_class"/>
  </rdf:Description>
  <rdf:Description rdf:about="https://w3id.org/omop/ontology/has_care_site">
    <rdf:type rdf:resource="http://www.w3.org/2002/07/owl#FunctionalProperty"/>
    <rdf:type rdf:resource="http://www.w3.org/2002/07/owl#ObjectProperty"/>
    <ns2:python_name rdf:datatype="http://www.w3.org/2001/XMLSchema#string">care_site</ns2:python_name>
    <rdfs:comment xml:lang="en">(for Person:) The Care Site refers to where the Provider typically provides the primary care.</rdfs:comment>
    <rdfs:comment xml:lang="en">(for Provider:) This is the CARE_SITE_ID for the location that the provider primarily practices in.
If a Provider has more than one Care Site, the main or most often exerted CARE_SITE_ID should be recorded.</rdfs:comment>
    <rdfs:comment xml:lang="en">(for VisitDetail:) This field provides information about the Care Site where the Visit Detail took place.
There should only be one Care Site associated with a Visit Detail.</rdfs:comment>
    <rdfs:comment xml:lang="en">(for VisitOccurrence:) This field provides information about the care site where the visit took place.
There should only be one care site associated with a visit.</rdfs:comment>
    <rdfs:domain rdf:nodeID="nde7e53d44aa94269b5c0c83d6d8798ccb5"/>
    <rdfs:range rdf:resource="https://w3id.org/omop/ontology/CareSite"/>
    <ns1:omop_cdm_name rdf:datatype="http://www.w3.org/2001/XMLSchema#string">person.care_site_id#12 AS CareSite</ns1:omop_cdm_name>
    <ns1:omop_cdm_name rdf:datatype="http://www.w3.org/2001/XMLSchema#string">provider.care_site_id#278 AS CareSite</ns1:omop_cdm_name>
    <ns1:omop_cdm_name rdf:datatype="http://www.w3.org/2001/XMLSchema#string">visit_detail.care_site_id#51 AS CareSite</ns1:omop_cdm_name>
    <ns1:omop_cdm_name rdf:datatype="http://www.w3.org/2001/XMLSchema#string">visit_occurrence.care_site_id#34 AS CareSite</ns1:omop_cdm_name>
  </rdf:Description>
  <rdf:Description rdf:about="https://w3id.org/omop/ontology/ConceptAncestor">
    <rdf:type rdf:resource="http://www.w3.org/2002/07/owl#Class"/>
    <rdfs:subClassOf rdf:nodeID="nde7e53d44aa94269b5c0c83d6d8798ccb80"/>
    <rdfs:subClassOf rdf:nodeID="nde7e53d44aa94269b5c0c83d6d8798ccb81"/>
    <rdfs:subClassOf rdf:nodeID="nde7e53d44aa94269b5c0c83d6d8798ccb82"/>
    <rdfs:subClassOf rdf:nodeID="nde7e53d44aa94269b5c0c83d6d8798ccb83"/>
    <rdfs:subClassOf rdf:nodeID="nde7e53d44aa94269b5c0c83d6d8798ccb84"/>
    <rdfs:subClassOf rdf:nodeID="nde7e53d44aa94269b5c0c83d6d8798ccb85"/>
    <rdfs:subClassOf rdf:nodeID="nde7e53d44aa94269b5c0c83d6d8798ccb86"/>
    <rdfs:subClassOf rdf:nodeID="nde7e53d44aa94269b5c0c83d6d8798ccb87"/>
    <rdfs:subClassOf rdf:resource="https://w3id.org/omop/ontology/OmopCDMThing"/>
    <ns1:omop_cdm_name rdf:datatype="http://www.w3.org/2001/XMLSchema#string">concept_ancestor</ns1:omop_cdm_name>
  </rdf:Description>
  <rdf:Description rdf:about="https://w3id.org/omop/ontology/survey_start_date">
    <rdf:type rdf:resource="http://www.w3.org/2002/07/owl#DatatypeProperty"/>
    <rdf:type rdf:resource="http://www.w3.org/2002/07/owl#FunctionalProperty"/>
    <rdfs:comment xml:lang="en">(for SurveyConduct:) Date on which the survey was started.</rdfs:comment>
    <rdfs:domain rdf:resource="https://w3id.org/omop/ontology/SurveyConduct"/>
    <rdfs:range rdf:resource="http://www.w3.org/2001/XMLSchema#date"/>
    <ns1:omop_cdm_name rdf:datatype="http://www.w3.org/2001/XMLSchema#string">survey_conduct.survey_start_date#230 AS date</ns1:omop_cdm_name>
  </rdf:Description>
  <rdf:Description rdf:about="https://w3id.org/omop/ontology/Provider">
    <rdf:type rdf:resource="http://www.w3.org/2002/07/owl#Class"/>
    <rdfs:subClassOf rdf:nodeID="nde7e53d44aa94269b5c0c83d6d8798ccb472"/>
    <rdfs:subClassOf rdf:nodeID="nde7e53d44aa94269b5c0c83d6d8798ccb473"/>
    <rdfs:subClassOf rdf:nodeID="nde7e53d44aa94269b5c0c83d6d8798ccb474"/>
    <rdfs:subClassOf rdf:nodeID="nde7e53d44aa94269b5c0c83d6d8798ccb475"/>
    <rdfs:subClassOf rdf:nodeID="nde7e53d44aa94269b5c0c83d6d8798ccb476"/>
    <rdfs:subClassOf rdf:nodeID="nde7e53d44aa94269b5c0c83d6d8798ccb477"/>
    <rdfs:subClassOf rdf:nodeID="nde7e53d44aa94269b5c0c83d6d8798ccb478"/>
    <rdfs:subClassOf rdf:nodeID="nde7e53d44aa94269b5c0c83d6d8798ccb479"/>
    <rdfs:subClassOf rdf:nodeID="nde7e53d44aa94269b5c0c83d6d8798ccb480"/>
    <rdfs:subClassOf rdf:resource="https://w3id.org/omop/ontology/BasePerson"/>
    <ns1:omop_cdm_name rdf:datatype="http://www.w3.org/2001/XMLSchema#string">provider</ns1:omop_cdm_name>
  </rdf:Description>
  <rdf:Description rdf:nodeID="nde7e53d44aa94269b5c0c83d6d8798ccb469">
    <rdf:type rdf:resource="http://www.w3.org/2002/07/owl#Restriction"/>
    <owl:allValuesFrom rdf:resource="https://w3id.org/omop/ontology/Concept"/>
    <owl:onProperty rdf:resource="https://w3id.org/omop/ontology/has_unit"/>
  </rdf:Description>
  <rdf:Description rdf:nodeID="nde7e53d44aa94269b5c0c83d6d8798ccb476">
    <rdf:type rdf:resource="http://www.w3.org/2002/07/owl#Restriction"/>
    <owl:allValuesFrom rdf:resource="http://www.w3.org/2001/XMLSchema#string"/>
    <owl:onProperty rdf:resource="https://w3id.org/omop/ontology/name"/>
  </rdf:Description>
  <rdf:Description rdf:nodeID="nde7e53d44aa94269b5c0c83d6d8798ccb54">
    <rdf:type rdf:resource="http://www.w3.org/2002/07/owl#Class"/>
    <owl:unionOf rdf:nodeID="nde7e53d44aa94269b5c0c83d6d8798ccb55"/>
  </rdf:Description>
  <rdf:Description rdf:about="https://w3id.org/omop/ontology/NoteNlp">
    <rdf:type rdf:resource="http://www.w3.org/2002/07/owl#Class"/>
    <rdfs:subClassOf rdf:nodeID="nde7e53d44aa94269b5c0c83d6d8798ccb339"/>
    <rdfs:subClassOf rdf:nodeID="nde7e53d44aa94269b5c0c83d6d8798ccb340"/>
    <rdfs:subClassOf rdf:nodeID="nde7e53d44aa94269b5c0c83d6d8798ccb341"/>
    <rdfs:subClassOf rdf:nodeID="nde7e53d44aa94269b5c0c83d6d8798ccb342"/>
    <rdfs:subClassOf rdf:nodeID="nde7e53d44aa94269b5c0c83d6d8798ccb343"/>
    <rdfs:subClassOf rdf:nodeID="nde7e53d44aa94269b5c0c83d6d8798ccb344"/>
    <rdfs:subClassOf rdf:nodeID="nde7e53d44aa94269b5c0c83d6d8798ccb346"/>
    <rdfs:subClassOf rdf:nodeID="nde7e53d44aa94269b5c0c83d6d8798ccb347"/>
    <rdfs:subClassOf rdf:nodeID="nde7e53d44aa94269b5c0c83d6d8798ccb348"/>
    <rdfs:subClassOf rdf:nodeID="nde7e53d44aa94269b5c0c83d6d8798ccb349"/>
    <rdfs:subClassOf rdf:nodeID="nde7e53d44aa94269b5c0c83d6d8798ccb350"/>
    <rdfs:subClassOf rdf:nodeID="nde7e53d44aa94269b5c0c83d6d8798ccb351"/>
    <rdfs:subClassOf rdf:resource="https://w3id.org/omop/ontology/Event"/>
    <ns1:omop_cdm_name rdf:datatype="http://www.w3.org/2001/XMLSchema#string">note_nlp</ns1:omop_cdm_name>
  </rdf:Description>
  <rdf:Description rdf:nodeID="nde7e53d44aa94269b5c0c83d6d8798ccb86">
    <rdf:type rdf:resource="http://www.w3.org/2002/07/owl#Restriction"/>
    <owl:allValuesFrom rdf:resource="https://w3id.org/omop/ontology/Concept"/>
    <owl:onProperty rdf:resource="https://w3id.org/omop/ontology/has_descendant"/>
  </rdf:Description>
  <rdf:Description rdf:about="https://w3id.org/omop/ontology/has_location">
    <rdf:type rdf:resource="http://www.w3.org/2002/07/owl#FunctionalProperty"/>
    <rdf:type rdf:resource="http://www.w3.org/2002/07/owl#ObjectProperty"/>
    <ns2:python_name rdf:datatype="http://www.w3.org/2001/XMLSchema#string">location</ns2:python_name>
    <rdfs:comment xml:lang="en">(for CareSite:) The location_id from the LOCATION table representing the physical location of the care_site.</rdfs:comment>
    <rdfs:comment xml:lang="en">(for LocationHistory:) This is the LOCATION_ID for the LOCATION_HISTORY record.</rdfs:comment>
    <rdfs:comment xml:lang="en">(for Person:) The location refers to the physical address of the person. This field should capture the last known location of the person.  Any prior locations are captured in the [LOCATION_HISTORY](https://ohdsi.github.io/CommonDataModel/cdm60.html#location_history) table.
Put the location_id from the LOCATION table here that represents the most granular location information for the person. This could represent anything from postal code or parts thereof, state, or county for example. Since many databases contain deidentified data, it is common that the precision of the location is reduced to prevent re-identification. This field should capture the last known location. Any prior locations are captured in the [LOCATION_HISTORY](https://ohdsi.github.io/CommonDataModel/cdm60.html#location_history) table.</rdfs:comment>
    <rdfs:domain rdf:nodeID="nde7e53d44aa94269b5c0c83d6d8798ccb125"/>
    <rdfs:range rdf:resource="https://w3id.org/omop/ontology/Location"/>
    <ns1:omop_cdm_name rdf:datatype="http://www.w3.org/2001/XMLSchema#string">care_site.location_id#270 AS Location</ns1:omop_cdm_name>
    <ns1:omop_cdm_name rdf:datatype="http://www.w3.org/2001/XMLSchema#string">location_history.location_id#261 AS Location</ns1:omop_cdm_name>
    <ns1:omop_cdm_name rdf:datatype="http://www.w3.org/2001/XMLSchema#string">person.location_id#10 AS Location</ns1:omop_cdm_name>
  </rdf:Description>
  <rdf:Description rdf:nodeID="nde7e53d44aa94269b5c0c83d6d8798ccb194">
    <rdf:type rdf:resource="http://www.w3.org/2002/07/owl#Restriction"/>
    <owl:onProperty rdf:resource="https://w3id.org/omop/ontology/has_gender"/>
    <owl:someValuesFrom rdf:resource="https://w3id.org/omop/ontology/Concept"/>
  </rdf:Description>
  <rdf:Description rdf:about="https://w3id.org/omop/ontology/source_description">
    <rdf:type rdf:resource="http://www.w3.org/2002/07/owl#DatatypeProperty"/>
    <rdf:type rdf:resource="http://www.w3.org/2002/07/owl#FunctionalProperty"/>
    <rdfs:comment xml:lang="en">(for CdmSource:) The description of the CDM instance.</rdfs:comment>
    <rdfs:domain rdf:resource="https://w3id.org/omop/ontology/CdmSource"/>
    <rdfs:range rdf:resource="http://www.w3.org/2001/XMLSchema#string"/>
    <ns1:omop_cdm_name rdf:datatype="http://www.w3.org/2001/XMLSchema#string">cdm_source.source_description#355 AS str</ns1:omop_cdm_name>
  </rdf:Description>
  <rdf:Description rdf:nodeID="nde7e53d44aa94269b5c0c83d6d8798ccb124">
    <rdf:first rdf:resource="https://w3id.org/omop/ontology/Note"/>
    <rdf:rest rdf:resource="http://www.w3.org/1999/02/22-rdf-syntax-ns#nil"/>
  </rdf:Description>
  <rdf:Description rdf:nodeID="nde7e53d44aa94269b5c0c83d6d8798ccb542">
    <rdf:type rdf:resource="http://www.w3.org/2002/07/owl#Restriction"/>
    <owl:allValuesFrom rdf:resource="https://w3id.org/omop/ontology/Concept"/>
    <owl:onProperty rdf:resource="https://w3id.org/omop/ontology/has_stop_reason_source"/>
  </rdf:Description>
  <rdf:Description rdf:about="https://w3id.org/omop/ontology/id">
    <rdf:type rdf:resource="http://www.w3.org/2002/07/owl#DatatypeProperty"/>
    <rdf:type rdf:resource="http://www.w3.org/2002/07/owl#FunctionalProperty"/>
    <rdfs:comment xml:lang="en">(for CareSite:) Assign an id to each unique combination of location_id and place_of_service_source_value.</rdfs:comment>
    <rdfs:comment xml:lang="en">(for CohortDefinition:) This is the identifier given to the cohort, usually by the ATLAS application</rdfs:comment>
    <rdfs:comment xml:lang="en">(for Concept:) A unique identifier for each Concept across all domains.</rdfs:comment>
    <rdfs:comment xml:lang="en">(for ConceptClass:) A unique key for each class.</rdfs:comment>
    <rdfs:comment xml:lang="en">(for ConditionOccurrence:) The unique key given to a condition record for a person. Refer to the ETL for how duplicate conditions during the same visit were handled.
Each instance of a condition present in the source data should be assigned this unique key. In some cases, a person can have multiple records of the same condition within the same visit. It is valid to keep these duplicates and assign them individual, unique, CONDITION_OCCURRENCE_IDs, though it is up to the ETL how they should be handled.</rdfs:comment>
    <rdfs:comment xml:lang="en">(for Cost:) A unique identifier for each COST record.</rdfs:comment>
    <rdfs:comment xml:lang="en">(for DeviceExposure:) The unique key given to records a person's exposure to a foreign physical object or instrument.
Each instance of an exposure to a foreign object or device present in the source data should be assigned this unique key.</rdfs:comment>
    <rdfs:comment xml:lang="en">(for Domain:) A unique key for each domain.</rdfs:comment>
    <rdfs:comment xml:lang="en">(for DrugExposure:) The unique key given to records of drug dispensings or administrations for a person. Refer to the ETL for how duplicate drugs during the same visit were handled.
Each instance of a drug dispensing or administration present in the source data should be assigned this unique key. In some cases, a person can have multiple records of the same drug within the same visit. It is valid to keep these duplicates and assign them individual, unique, DRUG_EXPOSURE_IDs, though it is up to the ETL how they should be handled.</rdfs:comment>
    <rdfs:comment xml:lang="en">(for Location:) The unique key given to a unique Location.
Each instance of a Location in the source data should be assigned this unique key.</rdfs:comment>
    <rdfs:comment xml:lang="en">(for Measurement:) The unique key given to a Measurement record for a Person. Refer to the ETL for how duplicate Measurements during the same Visit were handled.
Each instance of a measurement present in the source data should be assigned this unique key. In some cases, a person can have multiple records of the same measurement within the same visit. It is valid to keep these duplicates and assign them individual, unique, MEASUREMENT_IDs, though it is up to the ETL how they should be handled.</rdfs:comment>
    <rdfs:comment xml:lang="en">(for Note:) A unique identifier for each note.</rdfs:comment>
    <rdfs:comment xml:lang="en">(for NoteNlp:) A unique identifier for the NLP record.</rdfs:comment>
    <rdfs:comment xml:lang="en">(for Observation:) The unique key given to an Observation record for a Person. Refer to the ETL for how duplicate Observations during the same Visit were handled.
Each instance of an observation present in the source data should be assigned this unique key.</rdfs:comment>
    <rdfs:comment xml:lang="en">(for ObservationPeriod:) A Person can have multiple discrete Observation Periods which are identified by the Observation_Period_Id.
Assign a unique observation_period_id to each discrete Observation Period for a Person.</rdfs:comment>
    <rdfs:comment xml:lang="en">(for PayerPlanPeriod:) A unique identifier for each unique combination of a Person, Payer, Plan, and Period of time.</rdfs:comment>
    <rdfs:comment xml:lang="en">(for Person:) It is assumed that every person with a different unique identifier is in fact a different person and should be treated independently.
Any person linkage that needs to occur to uniquely identify Persons ought to be done prior to writing this table. This identifier can be the original id from the source data provided if it is an integer, otherwise it can be an autogenerated number.</rdfs:comment>
    <rdfs:comment xml:lang="en">(for ProcedureOccurrence:) The unique key given to a procedure record for a person. Refer to the ETL for how duplicate procedures during the same visit were handled.
Each instance of a procedure occurrence in the source data should be assigned this unique key. In some cases, a person can have multiple records of the same procedure within the same visit. It is valid to keep these duplicates and assign them individual, unique, PROCEDURE_OCCURRENCE_IDs, though it is up to the ETL how they should be handled.</rdfs:comment>
    <rdfs:comment xml:lang="en">(for Provider:) It is assumed that every provider with a different unique identifier is in fact a different person and should be treated independently.
This identifier can be the original id from the source data provided it is an integer, otherwise it can be an autogenerated number.</rdfs:comment>
    <rdfs:comment xml:lang="en">(for Specimen:) Unique identifier for each specimen.</rdfs:comment>
    <rdfs:comment xml:lang="en">(for SurveyConduct:) Unique identifier for each completed survey.
For each instance of a survey completion create a unique identifier.</rdfs:comment>
    <rdfs:comment xml:lang="en">(for VisitDetail:) Use this to identify unique interactions between a person and the health care system. This identifier links across the other CDM event tables to associate events with a visit detail.
This should be populated by creating a unique identifier for each unique interaction between a person and the healthcare system where the person receives a medical good or service over a span of time.</rdfs:comment>
    <rdfs:comment xml:lang="en">(for VisitOccurrence:) Use this to identify unique interactions between a person and the health care system. This identifier links across the other CDM event tables to associate events with a visit.
This should be populated by creating a unique identifier for each unique interaction between a person and the healthcare system where the person receives a medical good or service over a span of time.</rdfs:comment>
    <rdfs:comment xml:lang="en">(for Vocabulary:) A unique identifier for each Vocabulary, such
as ICD9CM, SNOMED, Visit.</rdfs:comment>
    <rdfs:domain rdf:resource="https://w3id.org/omop/ontology/OmopCDMThing"/>
    <rdfs:range rdf:nodeID="nde7e53d44aa94269b5c0c83d6d8798ccb8"/>
    <ns1:omop_cdm_name rdf:datatype="http://www.w3.org/2001/XMLSchema#string">care_site.care_site_id#267 AS int|str</ns1:omop_cdm_name>
    <ns1:omop_cdm_name rdf:datatype="http://www.w3.org/2001/XMLSchema#string">cohort_definition.cohort_definition_id#427 AS int|str</ns1:omop_cdm_name>
    <ns1:omop_cdm_name rdf:datatype="http://www.w3.org/2001/XMLSchema#string">concept.concept_id#362 AS int|str</ns1:omop_cdm_name>
    <ns1:omop_cdm_name rdf:datatype="http://www.w3.org/2001/XMLSchema#string">concept_class.concept_class_id#380 AS int|str</ns1:omop_cdm_name>
    <ns1:omop_cdm_name rdf:datatype="http://www.w3.org/2001/XMLSchema#string">condition_era.condition_era_id#339 AS int|str</ns1:omop_cdm_name>
    <ns1:omop_cdm_name rdf:datatype="http://www.w3.org/2001/XMLSchema#string">condition_occurrence.condition_occurrence_id#61 AS int|str</ns1:omop_cdm_name>
    <ns1:omop_cdm_name rdf:datatype="http://www.w3.org/2001/XMLSchema#string">cost.cost_id#307 AS int|str</ns1:omop_cdm_name>
    <ns1:omop_cdm_name rdf:datatype="http://www.w3.org/2001/XMLSchema#string">device_exposure.device_exposure_id#114 AS int|str</ns1:omop_cdm_name>
    <ns1:omop_cdm_name rdf:datatype="http://www.w3.org/2001/XMLSchema#string">domain.domain_id#377 AS int|str</ns1:omop_cdm_name>
    <ns1:omop_cdm_name rdf:datatype="http://www.w3.org/2001/XMLSchema#string">dose_era.dose_era_id#332 AS int|str</ns1:omop_cdm_name>
    <ns1:omop_cdm_name rdf:datatype="http://www.w3.org/2001/XMLSchema#string">drug_era.drug_era_id#325 AS int|str</ns1:omop_cdm_name>
    <ns1:omop_cdm_name rdf:datatype="http://www.w3.org/2001/XMLSchema#string">drug_exposure.drug_exposure_id#77 AS int|str</ns1:omop_cdm_name>
    <ns1:omop_cdm_name rdf:datatype="http://www.w3.org/2001/XMLSchema#string">location.location_id#251 AS int|str</ns1:omop_cdm_name>
    <ns1:omop_cdm_name rdf:datatype="http://www.w3.org/2001/XMLSchema#string">measurement.measurement_id#129 AS int|str</ns1:omop_cdm_name>
    <ns1:omop_cdm_name rdf:datatype="http://www.w3.org/2001/XMLSchema#string">note.note_id#177 AS int|str</ns1:omop_cdm_name>
    <ns1:omop_cdm_name rdf:datatype="http://www.w3.org/2001/XMLSchema#string">note_nlp.note_nlp_id#193 AS int|str</ns1:omop_cdm_name>
    <ns1:omop_cdm_name rdf:datatype="http://www.w3.org/2001/XMLSchema#string">observation.observation_id#149 AS int|str</ns1:omop_cdm_name>
    <ns1:omop_cdm_name rdf:datatype="http://www.w3.org/2001/XMLSchema#string">observation_period.observation_period_id#20 AS int|str</ns1:omop_cdm_name>
    <ns1:omop_cdm_name rdf:datatype="http://www.w3.org/2001/XMLSchema#string">payer_plan_period.payer_plan_period_id#286 AS int|str</ns1:omop_cdm_name>
    <ns1:omop_cdm_name rdf:datatype="http://www.w3.org/2001/XMLSchema#string">person.person_id#1 AS int|str</ns1:omop_cdm_name>
    <ns1:omop_cdm_name rdf:datatype="http://www.w3.org/2001/XMLSchema#string">procedure_occurrence.procedure_occurrence_id#100 AS int|str</ns1:omop_cdm_name>
    <ns1:omop_cdm_name rdf:datatype="http://www.w3.org/2001/XMLSchema#string">provider.provider_id#273 AS int|str</ns1:omop_cdm_name>
    <ns1:omop_cdm_name rdf:datatype="http://www.w3.org/2001/XMLSchema#string">relationship.relationship_id#389 AS int|str</ns1:omop_cdm_name>
    <ns1:omop_cdm_name rdf:datatype="http://www.w3.org/2001/XMLSchema#string">specimen.specimen_id#207 AS int|str</ns1:omop_cdm_name>
    <ns1:omop_cdm_name rdf:datatype="http://www.w3.org/2001/XMLSchema#string">survey_conduct.survey_conduct_id#227 AS int|str</ns1:omop_cdm_name>
    <ns1:omop_cdm_name rdf:datatype="http://www.w3.org/2001/XMLSchema#string">visit_detail.visit_detail_id#42 AS int|str</ns1:omop_cdm_name>
    <ns1:omop_cdm_name rdf:datatype="http://www.w3.org/2001/XMLSchema#string">visit_occurrence.visit_occurrence_id#25 AS int|str</ns1:omop_cdm_name>
    <ns1:omop_cdm_name rdf:datatype="http://www.w3.org/2001/XMLSchema#string">vocabulary.vocabulary_id#372 AS int|str</ns1:omop_cdm_name>
  </rdf:Description>
  <rdf:Description rdf:about="https://w3id.org/omop/ontology/stop_reason">
    <rdf:type rdf:resource="http://www.w3.org/2002/07/owl#DatatypeProperty"/>
    <rdf:type rdf:resource="http://www.w3.org/2002/07/owl#FunctionalProperty"/>
    <rdfs:comment xml:lang="en">(for ConditionOccurrence:) The Stop Reason indicates why a Condition is no longer valid with respect to the purpose within the source data. Note that a Stop Reason does not necessarily imply that the condition is no longer occurring.
This information is often not populated in source data and it is a valid etl choice to leave it blank if the information does not exist.</rdfs:comment>
    <rdfs:comment xml:lang="en">(for DrugExposure:) The reason a person stopped a medication as it is represented in the source. Reasons include regimen completed, changed, removed, etc. This field will be retired in v6.0.
This information is often not populated in source data and it is a valid etl choice to leave it blank if the information does not exist.</rdfs:comment>
    <rdfs:domain rdf:nodeID="nde7e53d44aa94269b5c0c83d6d8798ccb11"/>
    <rdfs:range rdf:resource="http://www.w3.org/2001/XMLSchema#string"/>
    <ns1:omop_cdm_name rdf:datatype="http://www.w3.org/2001/XMLSchema#string">condition_occurrence.stop_reason#70 AS str</ns1:omop_cdm_name>
    <ns1:omop_cdm_name rdf:datatype="http://www.w3.org/2001/XMLSchema#string">drug_exposure.stop_reason#86 AS str</ns1:omop_cdm_name>
  </rdf:Description>
  <rdf:Description rdf:about="https://w3id.org/omop/ontology/has_stop_reason_source">
    <rdf:type rdf:resource="http://www.w3.org/2002/07/owl#FunctionalProperty"/>
    <rdf:type rdf:resource="http://www.w3.org/2002/07/owl#ObjectProperty"/>
    <ns2:python_name rdf:datatype="http://www.w3.org/2001/XMLSchema#string">stop_reason_source</ns2:python_name>
    <rdfs:comment xml:lang="en">(for PayerPlanPeriod:) If the source data codes the stop reason in an OMOP supported vocabulary store the concept_id here.</rdfs:comment>
    <rdfs:domain rdf:resource="https://w3id.org/omop/ontology/PayerPlanPeriod"/>
    <rdfs:range rdf:resource="https://w3id.org/omop/ontology/Concept"/>
    <ns1:omop_cdm_name rdf:datatype="http://www.w3.org/2001/XMLSchema#string">payer_plan_period.stop_reason_source_concept_id#306 AS Concept</ns1:omop_cdm_name>
  </rdf:Description>
  <rdf:Description rdf:about="https://w3id.org/omop/ontology/source_release_date">
    <rdf:type rdf:resource="http://www.w3.org/2002/07/owl#DatatypeProperty"/>
    <rdf:type rdf:resource="http://www.w3.org/2002/07/owl#FunctionalProperty"/>
    <rdfs:comment xml:lang="en">(for CdmSource:) The release date of the source data.</rdfs:comment>
    <rdfs:domain rdf:resource="https://w3id.org/omop/ontology/CdmSource"/>
    <rdfs:range rdf:resource="http://www.w3.org/2001/XMLSchema#date"/>
    <ns1:omop_cdm_name rdf:datatype="http://www.w3.org/2001/XMLSchema#string">cdm_source.source_release_date#358 AS date</ns1:omop_cdm_name>
  </rdf:Description>
  <rdf:Description rdf:about="https://w3id.org/omop/ontology/has_reverse_relationship">
    <rdf:type rdf:resource="http://www.w3.org/2002/07/owl#FunctionalProperty"/>
    <rdf:type rdf:resource="http://www.w3.org/2002/07/owl#ObjectProperty"/>
    <ns2:python_name rdf:datatype="http://www.w3.org/2001/XMLSchema#string">reverse_relationship</ns2:python_name>
    <rdfs:domain rdf:resource="https://w3id.org/omop/ontology/Relationship"/>
    <ns1:omop_cdm_name rdf:datatype="http://www.w3.org/2001/XMLSchema#string">relationship.reverse_relationship_id#393 AS Thing</ns1:omop_cdm_name>
  </rdf:Description>
  <rdf:Description rdf:about="https://w3id.org/omop/ontology/PayerPlanPeriod">
    <rdf:type rdf:resource="http://www.w3.org/2002/07/owl#Class"/>
    <rdfs:subClassOf rdf:nodeID="nde7e53d44aa94269b5c0c83d6d8798ccb532"/>
    <rdfs:subClassOf rdf:nodeID="nde7e53d44aa94269b5c0c83d6d8798ccb533"/>
    <rdfs:subClassOf rdf:nodeID="nde7e53d44aa94269b5c0c83d6d8798ccb534"/>
    <rdfs:subClassOf rdf:nodeID="nde7e53d44aa94269b5c0c83d6d8798ccb535"/>
    <rdfs:subClassOf rdf:nodeID="nde7e53d44aa94269b5c0c83d6d8798ccb536"/>
    <rdfs:subClassOf rdf:nodeID="nde7e53d44aa94269b5c0c83d6d8798ccb537"/>
    <rdfs:subClassOf rdf:nodeID="nde7e53d44aa94269b5c0c83d6d8798ccb538"/>
    <rdfs:subClassOf rdf:nodeID="nde7e53d44aa94269b5c0c83d6d8798ccb539"/>
    <rdfs:subClassOf rdf:nodeID="nde7e53d44aa94269b5c0c83d6d8798ccb540"/>
    <rdfs:subClassOf rdf:nodeID="nde7e53d44aa94269b5c0c83d6d8798ccb541"/>
    <rdfs:subClassOf rdf:nodeID="nde7e53d44aa94269b5c0c83d6d8798ccb542"/>
    <rdfs:subClassOf rdf:nodeID="nde7e53d44aa94269b5c0c83d6d8798ccb543"/>
    <rdfs:subClassOf rdf:nodeID="nde7e53d44aa94269b5c0c83d6d8798ccb544"/>
    <rdfs:subClassOf rdf:nodeID="nde7e53d44aa94269b5c0c83d6d8798ccb546"/>
    <rdfs:subClassOf rdf:nodeID="nde7e53d44aa94269b5c0c83d6d8798ccb547"/>
    <rdfs:subClassOf rdf:nodeID="nde7e53d44aa94269b5c0c83d6d8798ccb548"/>
    <rdfs:subClassOf rdf:nodeID="nde7e53d44aa94269b5c0c83d6d8798ccb549"/>
    <rdfs:subClassOf rdf:nodeID="nde7e53d44aa94269b5c0c83d6d8798ccb550"/>
    <rdfs:subClassOf rdf:nodeID="nde7e53d44aa94269b5c0c83d6d8798ccb551"/>
    <rdfs:subClassOf rdf:nodeID="nde7e53d44aa94269b5c0c83d6d8798ccb552"/>
    <rdfs:subClassOf rdf:nodeID="nde7e53d44aa94269b5c0c83d6d8798ccb553"/>
    <rdfs:subClassOf rdf:nodeID="nde7e53d44aa94269b5c0c83d6d8798ccb554"/>
    <rdfs:subClassOf rdf:nodeID="nde7e53d44aa94269b5c0c83d6d8798ccb555"/>
    <rdfs:subClassOf rdf:nodeID="nde7e53d44aa94269b5c0c83d6d8798ccb556"/>
    <rdfs:subClassOf rdf:nodeID="nde7e53d44aa94269b5c0c83d6d8798ccb557"/>
    <rdfs:subClassOf rdf:nodeID="nde7e53d44aa94269b5c0c83d6d8798ccb558"/>
    <rdfs:subClassOf rdf:resource="https://w3id.org/omop/ontology/DateDuration"/>
    <ns1:omop_cdm_name rdf:datatype="http://www.w3.org/2001/XMLSchema#string">payer_plan_period</ns1:omop_cdm_name>
  </rdf:Description>
  <rdf:Description rdf:about="https://w3id.org/omop/ontology/VisitOccurrence">
    <rdf:type rdf:resource="http://www.w3.org/2002/07/owl#Class"/>
    <rdfs:subClassOf rdf:nodeID="nde7e53d44aa94269b5c0c83d6d8798ccb352"/>
    <rdfs:subClassOf rdf:nodeID="nde7e53d44aa94269b5c0c83d6d8798ccb353"/>
    <rdfs:subClassOf rdf:nodeID="nde7e53d44aa94269b5c0c83d6d8798ccb354"/>
    <rdfs:subClassOf rdf:nodeID="nde7e53d44aa94269b5c0c83d6d8798ccb355"/>
    <rdfs:subClassOf rdf:nodeID="nde7e53d44aa94269b5c0c83d6d8798ccb356"/>
    <rdfs:subClassOf rdf:nodeID="nde7e53d44aa94269b5c0c83d6d8798ccb357"/>
    <rdfs:subClassOf rdf:nodeID="nde7e53d44aa94269b5c0c83d6d8798ccb358"/>
    <rdfs:subClassOf rdf:resource="https://w3id.org/omop/ontology/BaseVisit"/>
    <ns1:omop_cdm_name rdf:datatype="http://www.w3.org/2001/XMLSchema#string">visit_occurrence</ns1:omop_cdm_name>
  </rdf:Description>
  <rdf:Description rdf:about="https://w3id.org/omop/ontology/has_race_source">
    <rdf:type rdf:resource="http://www.w3.org/2002/07/owl#FunctionalProperty"/>
    <rdf:type rdf:resource="http://www.w3.org/2002/07/owl#ObjectProperty"/>
    <ns2:python_name rdf:datatype="http://www.w3.org/2001/XMLSchema#string">race_source</ns2:python_name>
    <rdfs:comment xml:lang="en">(for Person:) Due to the small number of options, this tends to be zero.
If the source data codes race in an OMOP supported vocabulary store the concept_id here, otherwise set to 0.</rdfs:comment>
    <rdfs:domain rdf:resource="https://w3id.org/omop/ontology/Person"/>
    <rdfs:range rdf:resource="https://w3id.org/omop/ontology/Concept"/>
    <ns1:omop_cdm_name rdf:datatype="http://www.w3.org/2001/XMLSchema#string">person.race_source_concept_id#17 AS Concept</ns1:omop_cdm_name>
  </rdf:Description>
  <rdf:Description rdf:nodeID="nde7e53d44aa94269b5c0c83d6d8798ccb134">
    <rdf:first rdf:resource="https://w3id.org/omop/ontology/CohortDefinition"/>
    <rdf:rest rdf:resource="http://www.w3.org/1999/02/22-rdf-syntax-ns#nil"/>
  </rdf:Description>
  <rdf:Description rdf:about="https://w3id.org/omop/ontology/stop_reason_source_value">
    <rdf:type rdf:resource="http://www.w3.org/2002/07/owl#DatatypeProperty"/>
    <rdf:type rdf:resource="http://www.w3.org/2002/07/owl#FunctionalProperty"/>
    <rdfs:comment xml:lang="en">(for PayerPlanPeriod:) The Plan stop reason as it appears in the source data.</rdfs:comment>
    <rdfs:domain rdf:resource="https://w3id.org/omop/ontology/PayerPlanPeriod"/>
    <rdfs:range rdf:resource="http://www.w3.org/2001/XMLSchema#string"/>
    <ns1:omop_cdm_name rdf:datatype="http://www.w3.org/2001/XMLSchema#string">payer_plan_period.stop_reason_source_value#305 AS str</ns1:omop_cdm_name>
  </rdf:Description>
  <rdf:Description rdf:about="https://w3id.org/omop/ontology/has_stop_reason_concept">
    <rdf:type rdf:resource="http://www.w3.org/2002/07/owl#FunctionalProperty"/>
    <rdf:type rdf:resource="http://www.w3.org/2002/07/owl#ObjectProperty"/>
    <ns2:python_name rdf:datatype="http://www.w3.org/2001/XMLSchema#string">stop_reason_concept</ns2:python_name>
    <rdfs:comment xml:lang="en">(for PayerPlanPeriod:) This field represents the reason the Person left the Plan, if known.
Map the stop reason directly to a standard CONCEPT_ID. If one does not exists please contact the vocabulary team. There is no global controlled vocabulary available for this information. [Accepted Concepts](http://athena.ohdsi.org/search-terms/terms?domain=Plan+Stop+Reason&amp;standardConcept=Standard&amp;page=1&amp;pageSize=15&amp;query=).</rdfs:comment>
    <rdfs:domain rdf:resource="https://w3id.org/omop/ontology/PayerPlanPeriod"/>
    <rdfs:range rdf:resource="https://w3id.org/omop/ontology/Concept"/>
    <ns1:omop_cdm_name rdf:datatype="http://www.w3.org/2001/XMLSchema#string">payer_plan_period.stop_reason_concept_id#304 AS Concept</ns1:omop_cdm_name>
  </rdf:Description>
  <rdf:Description rdf:about="https://w3id.org/omop/ontology/sponsor_source_value">
    <rdf:type rdf:resource="http://www.w3.org/2002/07/owl#DatatypeProperty"/>
    <rdf:type rdf:resource="http://www.w3.org/2002/07/owl#FunctionalProperty"/>
    <rdfs:comment xml:lang="en">(for PayerPlanPeriod:) The Plan sponsor as it appears in the source data.</rdfs:comment>
    <rdfs:domain rdf:resource="https://w3id.org/omop/ontology/PayerPlanPeriod"/>
    <rdfs:range rdf:resource="http://www.w3.org/2001/XMLSchema#string"/>
    <ns1:omop_cdm_name rdf:datatype="http://www.w3.org/2001/XMLSchema#string">payer_plan_period.sponsor_source_value#301 AS str</ns1:omop_cdm_name>
  </rdf:Description>
  <rdf:Description rdf:about="https://w3id.org/omop/ontology/has_dose_era">
    <rdf:type rdf:resource="http://www.w3.org/2002/07/owl#ObjectProperty"/>
    <ns2:python_name rdf:datatype="http://www.w3.org/2001/XMLSchema#string">dose_eras</ns2:python_name>
    <rdfs:domain rdf:resource="https://w3id.org/omop/ontology/Person"/>
    <rdfs:range rdf:resource="https://w3id.org/omop/ontology/DoseEra"/>
    <ns1:omop_cdm_name rdf:datatype="http://www.w3.org/2001/XMLSchema#string">dose_era.person_id#333 AS Person</ns1:omop_cdm_name>
  </rdf:Description>
  <rdf:Description rdf:about="https://w3id.org/omop/ontology/DeviceExposure">
    <rdf:type rdf:resource="http://www.w3.org/2002/07/owl#Class"/>
    <rdfs:subClassOf rdf:nodeID="nde7e53d44aa94269b5c0c83d6d8798ccb148"/>
    <rdfs:subClassOf rdf:nodeID="nde7e53d44aa94269b5c0c83d6d8798ccb150"/>
    <rdfs:subClassOf rdf:nodeID="nde7e53d44aa94269b5c0c83d6d8798ccb151"/>
    <rdfs:subClassOf rdf:resource="https://w3id.org/omop/ontology/Exposure"/>
    <ns1:omop_cdm_name rdf:datatype="http://www.w3.org/2001/XMLSchema#string">device_exposure</ns1:omop_cdm_name>
  </rdf:Description>
  <rdf:Description rdf:nodeID="nde7e53d44aa94269b5c0c83d6d8798ccb100">
    <rdf:type rdf:resource="http://www.w3.org/2002/07/owl#Restriction"/>
    <owl:allValuesFrom rdf:resource="http://www.w3.org/2001/XMLSchema#integer"/>
    <owl:onProperty rdf:resource="https://w3id.org/omop/ontology/exposure_count"/>
  </rdf:Description>
  <rdf:Description rdf:about="https://w3id.org/omop/ontology/has_definition_type">
    <rdf:type rdf:resource="http://www.w3.org/2002/07/owl#FunctionalProperty"/>
    <rdf:type rdf:resource="http://www.w3.org/2002/07/owl#ObjectProperty"/>
    <ns2:python_name rdf:datatype="http://www.w3.org/2001/XMLSchema#string">definition_type</ns2:python_name>
    <rdfs:comment xml:lang="en">(for CohortDefinition:) Type defining what kind of Cohort Definition the record represents and how the syntax may be executed.</rdfs:comment>
    <rdfs:domain rdf:resource="https://w3id.org/omop/ontology/CohortDefinition"/>
    <rdfs:range rdf:resource="https://w3id.org/omop/ontology/Concept"/>
    <ns1:omop_cdm_name rdf:datatype="http://www.w3.org/2001/XMLSchema#string">cohort_definition.definition_type_concept_id#430 AS Concept</ns1:omop_cdm_name>
  </rdf:Description>
  <rdf:Description rdf:nodeID="nde7e53d44aa94269b5c0c83d6d8798ccb246">
    <rdf:type rdf:resource="http://www.w3.org/2002/07/owl#Restriction"/>
    <owl:allValuesFrom rdf:resource="http://www.w3.org/2001/XMLSchema#date"/>
    <owl:onProperty rdf:resource="https://w3id.org/omop/ontology/end_date"/>
  </rdf:Description>
  <rdf:Description rdf:nodeID="nde7e53d44aa94269b5c0c83d6d8798ccb583">
    <rdf:type rdf:resource="http://www.w3.org/2002/07/owl#Restriction"/>
    <owl:allValuesFrom rdf:nodeID="nde7e53d44aa94269b5c0c83d6d8798ccb584"/>
    <owl:onProperty rdf:resource="https://w3id.org/omop/ontology/id"/>
  </rdf:Description>
  <rdf:Description rdf:about="https://w3id.org/omop/ontology/has_gender">
    <rdf:type rdf:resource="http://www.w3.org/2002/07/owl#FunctionalProperty"/>
    <rdf:type rdf:resource="http://www.w3.org/2002/07/owl#ObjectProperty"/>
    <ns2:python_name rdf:datatype="http://www.w3.org/2001/XMLSchema#string">gender</ns2:python_name>
    <rdfs:comment xml:lang="en">(for Person:) This field is meant to capture the biological sex at birth of the Person. This field should not be used to study gender identity issues.
Use the gender or sex value present in the data under the assumption that it is the biological sex at birth. If the source data captures gender identity it should be stored in the [OBSERVATION](https://ohdsi.github.io/CommonDataModel/cdm60.html#observation) table. [Accepted gender concepts](http://athena.ohdsi.org/search-terms/terms?domain=Gender&amp;standardConcept=Standard&amp;page=1&amp;pageSize=15&amp;query=)</rdfs:comment>
    <rdfs:comment xml:lang="en">(for Provider:) This field represents the recorded gender of the provider in the source data.
If given, put a concept from the gender domain representing the recorded gender of the provider. If not available, set to 0. [Accepted Concepts](http://athena.ohdsi.org/search-terms/terms?domain=Gender&amp;standardConcept=Standard&amp;page=1&amp;pageSize=15&amp;query=).</rdfs:comment>
    <rdfs:domain rdf:resource="https://w3id.org/omop/ontology/BasePerson"/>
    <rdfs:range rdf:resource="https://w3id.org/omop/ontology/Concept"/>
    <ns1:omop_cdm_name rdf:datatype="http://www.w3.org/2001/XMLSchema#string">person.gender_concept_id#2 AS Concept</ns1:omop_cdm_name>
    <ns1:omop_cdm_name rdf:datatype="http://www.w3.org/2001/XMLSchema#string">provider.gender_concept_id#280 AS Concept</ns1:omop_cdm_name>
  </rdf:Description>
  <rdf:Description rdf:about="https://w3id.org/omop/ontology/has_gender_source">
    <rdf:type rdf:resource="http://www.w3.org/2002/07/owl#FunctionalProperty"/>
    <rdf:type rdf:resource="http://www.w3.org/2002/07/owl#ObjectProperty"/>
    <ns2:python_name rdf:datatype="http://www.w3.org/2001/XMLSchema#string">gender_source</ns2:python_name>
    <rdfs:comment xml:lang="en">(for Person:) Due to the small number of options, this tends to be zero.
If the source data codes biological sex in a non-standard vocabulary, store the concept_id here, otherwise set to 0.</rdfs:comment>
    <rdfs:comment xml:lang="en">(for Provider:) This is often zero as many sites use proprietary codes to store provider gender.
If the source data codes provider gender in an OMOP supported vocabulary store the concept_id here. If not available, set to 0.</rdfs:comment>
    <rdfs:domain rdf:resource="https://w3id.org/omop/ontology/BasePerson"/>
    <rdfs:range rdf:resource="https://w3id.org/omop/ontology/Concept"/>
    <ns1:omop_cdm_name rdf:datatype="http://www.w3.org/2001/XMLSchema#string">person.gender_source_concept_id#15 AS Concept</ns1:omop_cdm_name>
    <ns1:omop_cdm_name rdf:datatype="http://www.w3.org/2001/XMLSchema#string">provider.gender_source_concept_id#285 AS Concept</ns1:omop_cdm_name>
  </rdf:Description>
  <rdf:Description rdf:nodeID="nde7e53d44aa94269b5c0c83d6d8798ccb610">
    <rdf:type rdf:resource="http://www.w3.org/2002/07/owl#Restriction"/>
    <owl:allValuesFrom rdf:resource="http://www.w3.org/2001/XMLSchema#string"/>
    <owl:onProperty rdf:resource="https://w3id.org/omop/ontology/assisted_source_value"/>
  </rdf:Description>
  <rdf:Description rdf:about="https://w3id.org/omop/ontology/has_class">
    <rdf:type rdf:resource="http://www.w3.org/2002/07/owl#FunctionalProperty"/>
    <rdf:type rdf:resource="http://www.w3.org/2002/07/owl#ObjectProperty"/>
    <ns2:python_name rdf:datatype="http://www.w3.org/2001/XMLSchema#string">class</ns2:python_name>
    <rdfs:comment xml:lang="en">(for Concept:) The attribute or concept class of the
Concept. Examples are 'Clinical Drug',
'Ingredient', 'Clinical Finding' etc.</rdfs:comment>
    <rdfs:comment xml:lang="en">(for Note:) A Standard Concept Id representing the HL7 LOINC
Document Type Vocabulary classification of the note.
Map the note classification to a Standard Concept. For more information see the ETL Conventions in the description of the NOTE table. [AcceptedConcepts](https://athena.ohdsi.org/search-terms/terms?standardConcept=Standard&amp;conceptClass=Doc+Kind&amp;conceptClass=Doc+Role&amp;conceptClass=Doc+Setting&amp;conceptClass=Doc+Subject+Matter&amp;conceptClass=Doc+Type+of+Service&amp;domain=Meas+Value&amp;page=1&amp;pageSize=15&amp;query=). This Concept can alternatively be represented by concepts with the relationship 'Kind of (LOINC)' to [706391](https://athena.ohdsi.org/search-terms/terms/706391) (Note).</rdfs:comment>
    <rdfs:domain rdf:nodeID="nde7e53d44aa94269b5c0c83d6d8798ccb112"/>
    <ns1:omop_cdm_name rdf:datatype="http://www.w3.org/2001/XMLSchema#string">concept.concept_class_id#366 AS ConceptClass</ns1:omop_cdm_name>
    <ns1:omop_cdm_name rdf:datatype="http://www.w3.org/2001/XMLSchema#string">note.note_class_concept_id#184 AS Concept</ns1:omop_cdm_name>
  </rdf:Description>
  <rdf:Description rdf:about="https://w3id.org/omop/ontology/DrugExposure">
    <rdf:type rdf:resource="http://www.w3.org/2002/07/owl#Class"/>
    <rdfs:subClassOf rdf:nodeID="nde7e53d44aa94269b5c0c83d6d8798ccb373"/>
    <rdfs:subClassOf rdf:nodeID="nde7e53d44aa94269b5c0c83d6d8798ccb374"/>
    <rdfs:subClassOf rdf:nodeID="nde7e53d44aa94269b5c0c83d6d8798ccb375"/>
    <rdfs:subClassOf rdf:nodeID="nde7e53d44aa94269b5c0c83d6d8798ccb376"/>
    <rdfs:subClassOf rdf:nodeID="nde7e53d44aa94269b5c0c83d6d8798ccb378"/>
    <rdfs:subClassOf rdf:nodeID="nde7e53d44aa94269b5c0c83d6d8798ccb379"/>
    <rdfs:subClassOf rdf:nodeID="nde7e53d44aa94269b5c0c83d6d8798ccb380"/>
    <rdfs:subClassOf rdf:nodeID="nde7e53d44aa94269b5c0c83d6d8798ccb381"/>
    <rdfs:subClassOf rdf:nodeID="nde7e53d44aa94269b5c0c83d6d8798ccb382"/>
    <rdfs:subClassOf rdf:nodeID="nde7e53d44aa94269b5c0c83d6d8798ccb383"/>
    <rdfs:subClassOf rdf:nodeID="nde7e53d44aa94269b5c0c83d6d8798ccb384"/>
    <rdfs:subClassOf rdf:resource="https://w3id.org/omop/ontology/Exposure"/>
    <ns1:omop_cdm_name rdf:datatype="http://www.w3.org/2001/XMLSchema#string">drug_exposure</ns1:omop_cdm_name>
  </rdf:Description>
  <rdf:Description rdf:nodeID="nde7e53d44aa94269b5c0c83d6d8798ccb197">
    <rdf:type rdf:resource="http://www.w3.org/2002/07/owl#Restriction"/>
    <owl:allValuesFrom rdf:resource="https://w3id.org/omop/ontology/CareSite"/>
    <owl:onProperty rdf:resource="https://w3id.org/omop/ontology/has_care_site"/>
  </rdf:Description>
  <rdf:Description rdf:about="https://w3id.org/omop/ontology/BasePerson">
    <rdf:type rdf:resource="http://www.w3.org/2002/07/owl#Class"/>
    <rdfs:subClassOf rdf:nodeID="nde7e53d44aa94269b5c0c83d6d8798ccb192"/>
    <rdfs:subClassOf rdf:nodeID="nde7e53d44aa94269b5c0c83d6d8798ccb193"/>
    <rdfs:subClassOf rdf:nodeID="nde7e53d44aa94269b5c0c83d6d8798ccb194"/>
    <rdfs:subClassOf rdf:nodeID="nde7e53d44aa94269b5c0c83d6d8798ccb195"/>
    <rdfs:subClassOf rdf:nodeID="nde7e53d44aa94269b5c0c83d6d8798ccb196"/>
    <rdfs:subClassOf rdf:nodeID="nde7e53d44aa94269b5c0c83d6d8798ccb197"/>
    <rdfs:subClassOf rdf:nodeID="nde7e53d44aa94269b5c0c83d6d8798ccb198"/>
    <rdfs:subClassOf rdf:resource="https://w3id.org/omop/ontology/OmopCDMThing"/>
  </rdf:Description>
  <rdf:Description rdf:about="https://w3id.org/omop/ontology/has_numerator_unit">
    <rdf:type rdf:resource="http://www.w3.org/2002/07/owl#FunctionalProperty"/>
    <rdf:type rdf:resource="http://www.w3.org/2002/07/owl#ObjectProperty"/>
    <ns2:python_name rdf:datatype="http://www.w3.org/2001/XMLSchema#string">numerator_unit</ns2:python_name>
    <rdfs:comment xml:lang="en">(for DrugStrength:) The Concept representing the Unit of measure for the concentration of active ingredient.</rdfs:comment>
    <rdfs:domain rdf:resource="https://w3id.org/omop/ontology/DrugStrength"/>
    <rdfs:range rdf:resource="https://w3id.org/omop/ontology/Concept"/>
    <ns1:omop_cdm_name rdf:datatype="http://www.w3.org/2001/XMLSchema#string">drug_strength.numerator_unit_concept_id#416 AS Concept</ns1:omop_cdm_name>
  </rdf:Description>
  <rdf:Description rdf:about="https://w3id.org/omop/ontology/has_ingredient">
    <rdf:type rdf:resource="http://www.w3.org/2002/07/owl#FunctionalProperty"/>
    <rdf:type rdf:resource="http://www.w3.org/2002/07/owl#ObjectProperty"/>
    <ns2:python_name rdf:datatype="http://www.w3.org/2001/XMLSchema#string">ingredient</ns2:python_name>
    <rdfs:comment xml:lang="en">(for DrugStrength:) The Concept representing the active ingredient contained within the drug product.
Combination Drugs will have more than one record in this table, one for each active Ingredient.</rdfs:comment>
    <rdfs:domain rdf:resource="https://w3id.org/omop/ontology/DrugStrength"/>
    <rdfs:range rdf:resource="https://w3id.org/omop/ontology/Concept"/>
    <ns1:omop_cdm_name rdf:datatype="http://www.w3.org/2001/XMLSchema#string">drug_strength.ingredient_concept_id#412 AS Concept</ns1:omop_cdm_name>
  </rdf:Description>
  <rdf:Description rdf:about="https://w3id.org/omop/ontology/paid_date">
    <rdf:type rdf:resource="http://www.w3.org/2002/07/owl#DatatypeProperty"/>
    <rdf:type rdf:resource="http://www.w3.org/2002/07/owl#FunctionalProperty"/>
    <rdfs:comment xml:lang="en">(for Cost:) The date payment was received for a service or encounter</rdfs:comment>
    <rdfs:domain rdf:resource="https://w3id.org/omop/ontology/Cost"/>
    <rdfs:range rdf:resource="http://www.w3.org/2001/XMLSchema#date"/>
    <ns1:omop_cdm_name rdf:datatype="http://www.w3.org/2001/XMLSchema#string">cost.paid_date#319 AS date</ns1:omop_cdm_name>
  </rdf:Description>
  <rdf:Description rdf:nodeID="nde7e53d44aa94269b5c0c83d6d8798ccb23">
    <rdf:type rdf:resource="http://www.w3.org/2002/07/owl#Restriction"/>
    <owl:allValuesFrom rdf:resource="https://w3id.org/omop/ontology/Concept"/>
    <owl:onProperty rdf:resource="https://w3id.org/omop/ontology/has_language"/>
  </rdf:Description>
  <rdf:Description rdf:nodeID="nde7e53d44aa94269b5c0c83d6d8798ccb373">
    <rdf:type rdf:resource="http://www.w3.org/2002/07/owl#Restriction"/>
    <owl:allValuesFrom rdf:resource="http://www.w3.org/2001/XMLSchema#string"/>
    <owl:onProperty rdf:resource="https://w3id.org/omop/ontology/sig"/>
  </rdf:Description>
  <rdf:Description rdf:about="https://w3id.org/omop/ontology/has_vocabulary">
    <rdf:type rdf:resource="http://www.w3.org/2002/07/owl#FunctionalProperty"/>
    <rdf:type rdf:resource="http://www.w3.org/2002/07/owl#ObjectProperty"/>
    <ns2:python_name rdf:datatype="http://www.w3.org/2001/XMLSchema#string">vocabulary</ns2:python_name>
    <rdfs:comment xml:lang="en">(for Concept:) A foreign key to the [VOCABULARY](https://ohdsi.github.io/CommonDataModel/cdm531.html#vocabulary)
table indicating from which source the
Concept has been adapted.</rdfs:comment>
    <rdfs:domain rdf:resource="https://w3id.org/omop/ontology/Concept"/>
    <rdfs:range rdf:resource="https://w3id.org/omop/ontology/Vocabulary"/>
    <ns1:omop_cdm_name rdf:datatype="http://www.w3.org/2001/XMLSchema#string">concept.vocabulary_id#365 AS Vocabulary</ns1:omop_cdm_name>
  </rdf:Description>
  <rdf:Description rdf:about="https://w3id.org/omop/ontology/has_procedure_occurrence">
    <rdf:type rdf:resource="http://www.w3.org/2002/07/owl#ObjectProperty"/>
    <ns2:python_name rdf:datatype="http://www.w3.org/2001/XMLSchema#string">procedure_occurrences</ns2:python_name>
    <rdfs:comment xml:lang="en">(reversed relation, for ProcedureOccurrence:) The PERSON_ID of the PERSON for whom the procedure is recorded. This may be a system generated code.</rdfs:comment>
    <rdfs:comment xml:lang="en">(reversed relation, for ProcedureOccurrence:) The VISIT_DETAIL record during which the Procedure occurred. For example, if the Person was in the ICU at the time of the Procedure the VISIT_OCCURRENCE record would reflect the overall hospital stay and the VISIT_DETAIL record would reflect the ICU stay during the hospital visit.
Same rules apply as for the VISIT_OCCURRENCE_ID.</rdfs:comment>
    <rdfs:comment xml:lang="en">(reversed relation, for ProcedureOccurrence:) The visit during which the procedure occurred.
Depending on the structure of the source data, this may have to be determined based on dates. If a PROCEDURE_DATE occurs within the start and end date of a Visit it is a valid ETL choice to choose the VISIT_OCCURRENCE_ID from the Visit that subsumes it, even if not explicitly stated in the data. While not required, an attempt should be made to locate the VISIT_OCCURRENCE_ID of the PROCEDURE_OCCURRENCE record.</rdfs:comment>
    <rdfs:domain rdf:nodeID="nde7e53d44aa94269b5c0c83d6d8798ccb63"/>
    <rdfs:range rdf:resource="https://w3id.org/omop/ontology/ProcedureOccurrence"/>
    <ns1:omop_cdm_name rdf:datatype="http://www.w3.org/2001/XMLSchema#string">procedure_occurrence.person_id#101 AS Person</ns1:omop_cdm_name>
    <ns1:omop_cdm_name rdf:datatype="http://www.w3.org/2001/XMLSchema#string">procedure_occurrence.visit_detail_id#110 AS VisitDetail</ns1:omop_cdm_name>
    <ns1:omop_cdm_name rdf:datatype="http://www.w3.org/2001/XMLSchema#string">procedure_occurrence.visit_occurrence_id#109 AS VisitOccurrence</ns1:omop_cdm_name>
  </rdf:Description>
  <rdf:Description rdf:nodeID="nde7e53d44aa94269b5c0c83d6d8798ccb70">
    <rdf:first rdf:resource="https://w3id.org/omop/ontology/Measurement"/>
    <rdf:rest rdf:nodeID="nde7e53d44aa94269b5c0c83d6d8798ccb71"/>
  </rdf:Description>
  <rdf:Description rdf:nodeID="nde7e53d44aa94269b5c0c83d6d8798ccb423">
    <rdf:type rdf:resource="http://www.w3.org/2002/07/owl#Restriction"/>
    <owl:onProperty rdf:resource="https://w3id.org/omop/ontology/has_language"/>
    <owl:someValuesFrom rdf:resource="https://w3id.org/omop/ontology/Concept"/>
  </rdf:Description>
  <rdf:Description rdf:nodeID="nde7e53d44aa94269b5c0c83d6d8798ccb443">
    <rdf:type rdf:resource="http://www.w3.org/2002/07/owl#Restriction"/>
    <owl:allValuesFrom rdf:resource="https://w3id.org/omop/ontology/DeviceExposure"/>
    <owl:onProperty rdf:resource="https://w3id.org/omop/ontology/has_device_exposure"/>
  </rdf:Description>
  <rdf:Description rdf:nodeID="nde7e53d44aa94269b5c0c83d6d8798ccb105">
    <rdf:type rdf:resource="http://www.w3.org/2002/07/owl#Restriction"/>
    <owl:allValuesFrom rdf:resource="http://www.w3.org/2002/07/owl#Thing"/>
    <owl:onProperty rdf:resource="https://w3id.org/omop/ontology/has_entity"/>
  </rdf:Description>
  <rdf:Description rdf:nodeID="nde7e53d44aa94269b5c0c83d6d8798ccb35">
    <rdf:first rdf:resource="https://w3id.org/omop/ontology/VisitDetail"/>
    <rdf:rest rdf:resource="http://www.w3.org/1999/02/22-rdf-syntax-ns#nil"/>
  </rdf:Description>
  <rdf:Description rdf:nodeID="nde7e53d44aa94269b5c0c83d6d8798ccb202">
    <rdf:type rdf:resource="http://www.w3.org/2002/07/owl#Restriction"/>
    <owl:onProperty rdf:resource="https://w3id.org/omop/ontology/name"/>
    <owl:someValuesFrom rdf:resource="http://www.w3.org/2001/XMLSchema#string"/>
  </rdf:Description>
  <rdf:Description rdf:nodeID="nde7e53d44aa94269b5c0c83d6d8798ccb439">
    <rdf:type rdf:resource="http://www.w3.org/2002/07/owl#Restriction"/>
    <owl:allValuesFrom rdf:resource="http://www.w3.org/2001/XMLSchema#string"/>
    <owl:onProperty rdf:resource="https://w3id.org/omop/ontology/discharge_to_source_value"/>
  </rdf:Description>
  <rdf:Description rdf:about="https://w3id.org/omop/ontology/VisitDetail">
    <rdf:type rdf:resource="http://www.w3.org/2002/07/owl#Class"/>
    <rdfs:subClassOf rdf:nodeID="nde7e53d44aa94269b5c0c83d6d8798ccb314"/>
    <rdfs:subClassOf rdf:nodeID="nde7e53d44aa94269b5c0c83d6d8798ccb316"/>
    <rdfs:subClassOf rdf:nodeID="nde7e53d44aa94269b5c0c83d6d8798ccb317"/>
    <rdfs:subClassOf rdf:nodeID="nde7e53d44aa94269b5c0c83d6d8798ccb318"/>
    <rdfs:subClassOf rdf:nodeID="nde7e53d44aa94269b5c0c83d6d8798ccb319"/>
    <rdfs:subClassOf rdf:nodeID="nde7e53d44aa94269b5c0c83d6d8798ccb321"/>
    <rdfs:subClassOf rdf:nodeID="nde7e53d44aa94269b5c0c83d6d8798ccb322"/>
    <rdfs:subClassOf rdf:resource="https://w3id.org/omop/ontology/BaseVisit"/>
    <ns1:omop_cdm_name rdf:datatype="http://www.w3.org/2001/XMLSchema#string">visit_detail</ns1:omop_cdm_name>
  </rdf:Description>
  <rdf:Description rdf:nodeID="nde7e53d44aa94269b5c0c83d6d8798ccb421">
    <rdf:type rdf:resource="http://www.w3.org/2002/07/owl#Restriction"/>
    <owl:onProperty rdf:resource="https://w3id.org/omop/ontology/has_encoding"/>
    <owl:someValuesFrom rdf:resource="https://w3id.org/omop/ontology/Concept"/>
  </rdf:Description>
  <rdf:Description rdf:nodeID="nde7e53d44aa94269b5c0c83d6d8798ccb674">
    <rdf:type rdf:resource="http://www.w3.org/2002/07/owl#Restriction"/>
    <owl:allValuesFrom rdf:resource="https://w3id.org/omop/ontology/ConditionEra"/>
    <owl:onProperty rdf:resource="https://w3id.org/omop/ontology/has_condition_era"/>
  </rdf:Description>
  <rdf:Description rdf:nodeID="nde7e53d44aa94269b5c0c83d6d8798ccb342">
    <rdf:type rdf:resource="http://www.w3.org/2002/07/owl#Restriction"/>
    <owl:allValuesFrom rdf:resource="http://www.w3.org/2001/XMLSchema#string"/>
    <owl:onProperty rdf:resource="https://w3id.org/omop/ontology/term_exists"/>
  </rdf:Description>
  <rdf:Description rdf:nodeID="nde7e53d44aa94269b5c0c83d6d8798ccb448">
    <rdf:type rdf:resource="http://www.w3.org/2002/07/owl#Restriction"/>
    <owl:allValuesFrom rdf:resource="https://w3id.org/omop/ontology/ConditionOccurrence"/>
    <owl:onProperty rdf:resource="https://w3id.org/omop/ontology/has_condition_occurrence"/>
  </rdf:Description>
  <rdf:Description rdf:about="https://w3id.org/omop/ontology/drg_source_value">
    <rdf:type rdf:resource="http://www.w3.org/2002/07/owl#DatatypeProperty"/>
    <rdf:type rdf:resource="http://www.w3.org/2002/07/owl#FunctionalProperty"/>
    <rdfs:comment xml:lang="en">(for Cost:) The source value for the 3-digit DRG source code as it appears in the source data, stored here for reference.</rdfs:comment>
    <rdfs:domain rdf:resource="https://w3id.org/omop/ontology/Cost"/>
    <rdfs:range rdf:resource="http://www.w3.org/2001/XMLSchema#string"/>
    <ns1:omop_cdm_name rdf:datatype="http://www.w3.org/2001/XMLSchema#string">cost.drg_source_value#323 AS str</ns1:omop_cdm_name>
  </rdf:Description>
  <rdf:Description rdf:nodeID="nde7e53d44aa94269b5c0c83d6d8798ccb467">
    <rdf:type rdf:resource="http://www.w3.org/2002/07/owl#Restriction"/>
    <owl:allValuesFrom rdf:resource="http://www.w3.org/2001/XMLSchema#string"/>
    <owl:onProperty rdf:resource="https://w3id.org/omop/ontology/source_value"/>
  </rdf:Description>
  <rdf:Description rdf:about="https://w3id.org/omop/ontology/assisted_source_value">
    <rdf:type rdf:resource="http://www.w3.org/2002/07/owl#DatatypeProperty"/>
    <rdf:type rdf:resource="http://www.w3.org/2002/07/owl#FunctionalProperty"/>
    <rdfs:comment xml:lang="en">(for SurveyConduct:) Source value representing whether patient required assistance to complete the survey. Example: 'Completed without assistance', 'Completed with assistance'.</rdfs:comment>
    <rdfs:domain rdf:resource="https://w3id.org/omop/ontology/SurveyConduct"/>
    <rdfs:range rdf:resource="http://www.w3.org/2001/XMLSchema#string"/>
    <ns1:omop_cdm_name rdf:datatype="http://www.w3.org/2001/XMLSchema#string">survey_conduct.assisted_source_value#239 AS str</ns1:omop_cdm_name>
  </rdf:Description>
  <rdf:Description rdf:about="https://w3id.org/omop/ontology/revenue_code_source_value">
    <rdf:type rdf:resource="http://www.w3.org/2002/07/owl#DatatypeProperty"/>
    <rdf:type rdf:resource="http://www.w3.org/2002/07/owl#FunctionalProperty"/>
    <rdfs:comment xml:lang="en">(for Cost:) The source value for the Revenue code as it appears in the source data, stored here for reference.</rdfs:comment>
    <rdfs:domain rdf:resource="https://w3id.org/omop/ontology/Cost"/>
    <rdfs:range rdf:resource="http://www.w3.org/2001/XMLSchema#string"/>
    <ns1:omop_cdm_name rdf:datatype="http://www.w3.org/2001/XMLSchema#string">cost.revenue_code_source_value#322 AS str</ns1:omop_cdm_name>
  </rdf:Description>
  <rdf:Description rdf:about="https://w3id.org/omop/ontology/amount_value">
    <rdf:type rdf:resource="http://www.w3.org/2002/07/owl#DatatypeProperty"/>
    <rdf:type rdf:resource="http://www.w3.org/2002/07/owl#FunctionalProperty"/>
    <rdfs:comment xml:lang="en">(for DrugStrength:) The numeric value or the amount of active ingredient contained within the drug product.</rdfs:comment>
    <rdfs:domain rdf:resource="https://w3id.org/omop/ontology/DrugStrength"/>
    <rdfs:range rdf:resource="http://www.w3.org/2001/XMLSchema#decimal"/>
    <ns1:omop_cdm_name rdf:datatype="http://www.w3.org/2001/XMLSchema#string">drug_strength.amount_value#413 AS float</ns1:omop_cdm_name>
  </rdf:Description>
  <rdf:Description rdf:about="https://w3id.org/omop/ontology/min_levels_of_separation">
    <rdf:type rdf:resource="http://www.w3.org/2002/07/owl#DatatypeProperty"/>
    <rdf:type rdf:resource="http://www.w3.org/2002/07/owl#FunctionalProperty"/>
    <rdfs:comment xml:lang="en">(for ConceptAncestor:) The minimum separation in number of
levels of hierarchy between ancestor and
descendant concepts. This is an attribute
that is used to simplify hierarchic analysis.</rdfs:comment>
    <rdfs:domain rdf:resource="https://w3id.org/omop/ontology/ConceptAncestor"/>
    <rdfs:range rdf:resource="http://www.w3.org/2001/XMLSchema#integer"/>
    <ns1:omop_cdm_name rdf:datatype="http://www.w3.org/2001/XMLSchema#string">concept_ancestor.min_levels_of_separation#400 AS int</ns1:omop_cdm_name>
  </rdf:Description>
  <rdf:Description rdf:about="https://w3id.org/omop/ontology/has_type">
    <rdf:type rdf:resource="http://www.w3.org/2002/07/owl#FunctionalProperty"/>
    <rdf:type rdf:resource="http://www.w3.org/2002/07/owl#ObjectProperty"/>
    <ns2:python_name rdf:datatype="http://www.w3.org/2001/XMLSchema#string">type</ns2:python_name>
    <rdfs:comment xml:lang="en">(for ConditionOccurrence:) This field can be used to determine the provenance of the Condition record, as in whether the condition was from an EHR system, insurance claim, registry, or other sources.
Choose the condition_type_concept_id that best represents the provenance of the record. [Accepted Concepts](https://athena.ohdsi.org/search-terms/terms?domain=Type+Concept&amp;standardConcept=Standard&amp;page=1&amp;pageSize=15&amp;query=).</rdfs:comment>
    <rdfs:comment xml:lang="en">(for Cost:) A foreign key identifier to a concept in the CONCEPT table for the provenance or the source of the COST data and belonging to the 'Type Concept' vocabulary</rdfs:comment>
    <rdfs:comment xml:lang="en">(for DeviceExposure:) You can use the TYPE_CONCEPT_ID to denote the provenance of the record, as in whether the record is from administrative claims or EHR. [Accepted Concepts](https://athena.ohdsi.org/search-terms/terms?domain=Type+Concept&amp;standardConcept=Standard&amp;page=1&amp;pageSize=15&amp;query=).
Choose the drug_type_concept_id that best represents the provenance of the record, for example whether it came from a record of a prescription written or physician administered drug.</rdfs:comment>
    <rdfs:comment xml:lang="en">(for DrugExposure:) You can use the TYPE_CONCEPT_ID to delineate between prescriptions written vs. prescriptions dispensed vs. medication history vs. patient-reported exposure, etc.
Choose the drug_type_concept_id that best represents the provenance of the record, for example whether it came from a record of a prescription written or physician administered drug. [Accepted Concepts](https://athena.ohdsi.org/search-terms/terms?domain=Type+Concept&amp;standardConcept=Standard&amp;page=1&amp;pageSize=15&amp;query=).</rdfs:comment>
    <rdfs:comment xml:lang="en">(for Measurement:) This field can be used to determine the provenance of the Measurement record, as in whether the measurement was from an EHR system, insurance claim, registry, or other sources.
Choose the MEASUREMENT_TYPE_CONCEPT_ID that best represents the provenance of the record, for example whether it came from an EHR record or billing claim. [Accepted Concepts](https://athena.ohdsi.org/search-terms/terms?domain=Type+Concept&amp;standardConcept=Standard&amp;page=1&amp;pageSize=15&amp;query=).</rdfs:comment>
    <rdfs:comment xml:lang="en">(for Note:) The provenance of the note. Most likely this will be EHR.
Put the source system of the note, as in EHR record. [Accepted Concepts](https://athena.ohdsi.org/search-terms/terms?standardConcept=Standard&amp;domain=Type+Concept&amp;page=1&amp;pageSize=15&amp;query=).</rdfs:comment>
    <rdfs:comment xml:lang="en">(for Observation:) This field can be used to determine the provenance of the Observation record, as in whether the measurement was from an EHR system, insurance claim, registry, or other sources.
Choose the OBSERVATION_TYPE_CONCEPT_ID that best represents the provenance of the record, for example whether it came from an EHR record or billing claim. [Accepted Concepts](https://athena.ohdsi.org/search-terms/terms?domain=Type+Concept&amp;standardConcept=Standard&amp;page=1&amp;pageSize=15&amp;query=).</rdfs:comment>
    <rdfs:comment xml:lang="en">(for ProcedureOccurrence:) This field can be used to determine the provenance of the Procedure record, as in whether the procedure was from an EHR system, insurance claim, registry, or other sources.
Choose the PROCEDURE_TYPE_CONCEPT_ID that best represents the provenance of the record, for example whether it came from an EHR record or billing claim. If a procedure is recorded as an EHR encounter, the PROCEDURE_TYPE_CONCEPT would be 'EHR encounter record'. [Accepted Concepts](https://athena.ohdsi.org/search-terms/terms?domain=Type+Concept&amp;standardConcept=Standard&amp;page=1&amp;pageSize=15&amp;query=).</rdfs:comment>
    <rdfs:comment xml:lang="en">(for Specimen:) Put the source of the specimen record, as in an EHR system. [Accepted Concepts](https://athena.ohdsi.org/search-terms/terms?standardConcept=Standard&amp;domain=Type+Concept&amp;page=1&amp;pageSize=15&amp;query=).</rdfs:comment>
    <rdfs:comment xml:lang="en">(for VisitDetail:) Use this field to understand the provenance of the visit detail record, or where the record comes from.
Populate this field based on the provenance of the visit detail record, as in whether it came from an EHR record or billing claim. [Accepted Concepts](https://athena.ohdsi.org/search-terms/terms?domain=Type+Concept&amp;standardConcept=Standard&amp;page=1&amp;pageSize=15&amp;query=).</rdfs:comment>
    <rdfs:comment xml:lang="en">(for VisitOccurrence:) Use this field to understand the provenance of the visit record, or where the record comes from.
Populate this field based on the provenance of the visit record, as in whether it came from an EHR record or billing claim.</rdfs:comment>
    <rdfs:domain rdf:nodeID="nde7e53d44aa94269b5c0c83d6d8798ccb559"/>
    <rdfs:range rdf:resource="https://w3id.org/omop/ontology/Concept"/>
    <ns1:omop_cdm_name rdf:datatype="http://www.w3.org/2001/XMLSchema#string">condition_occurrence.condition_type_concept_id#68 AS Concept</ns1:omop_cdm_name>
    <ns1:omop_cdm_name rdf:datatype="http://www.w3.org/2001/XMLSchema#string">cost.cost_type_concept_id#312 AS Concept</ns1:omop_cdm_name>
    <ns1:omop_cdm_name rdf:datatype="http://www.w3.org/2001/XMLSchema#string">death.death_type_concept_id#173 AS Concept</ns1:omop_cdm_name>
    <ns1:omop_cdm_name rdf:datatype="http://www.w3.org/2001/XMLSchema#string">device_exposure.device_type_concept_id#121 AS Concept</ns1:omop_cdm_name>
    <ns1:omop_cdm_name rdf:datatype="http://www.w3.org/2001/XMLSchema#string">drug_exposure.drug_type_concept_id#85 AS Concept</ns1:omop_cdm_name>
    <ns1:omop_cdm_name rdf:datatype="http://www.w3.org/2001/XMLSchema#string">measurement.measurement_type_concept_id#135 AS Concept</ns1:omop_cdm_name>
    <ns1:omop_cdm_name rdf:datatype="http://www.w3.org/2001/XMLSchema#string">metadata.metadata_type_concept_id#346 AS Concept</ns1:omop_cdm_name>
    <ns1:omop_cdm_name rdf:datatype="http://www.w3.org/2001/XMLSchema#string">note.note_type_concept_id#183 AS Concept</ns1:omop_cdm_name>
    <ns1:omop_cdm_name rdf:datatype="http://www.w3.org/2001/XMLSchema#string">observation.observation_type_concept_id#154 AS Concept</ns1:omop_cdm_name>
    <ns1:omop_cdm_name rdf:datatype="http://www.w3.org/2001/XMLSchema#string">procedure_occurrence.procedure_type_concept_id#105 AS Concept</ns1:omop_cdm_name>
    <ns1:omop_cdm_name rdf:datatype="http://www.w3.org/2001/XMLSchema#string">specimen.specimen_type_concept_id#210 AS Concept</ns1:omop_cdm_name>
    <ns1:omop_cdm_name rdf:datatype="http://www.w3.org/2001/XMLSchema#string">visit_detail.visit_detail_type_concept_id#49 AS Concept</ns1:omop_cdm_name>
    <ns1:omop_cdm_name rdf:datatype="http://www.w3.org/2001/XMLSchema#string">visit_occurrence.visit_type_concept_id#32 AS Concept</ns1:omop_cdm_name>
  </rdf:Description>
  <rdf:Description rdf:about="https://w3id.org/omop/ontology/has_place_of_service">
    <rdf:type rdf:resource="http://www.w3.org/2002/07/owl#FunctionalProperty"/>
    <rdf:type rdf:resource="http://www.w3.org/2002/07/owl#ObjectProperty"/>
    <ns2:python_name rdf:datatype="http://www.w3.org/2001/XMLSchema#string">place_of_service</ns2:python_name>
    <rdfs:comment xml:lang="en">(for CareSite:) This is a high-level way of characterizing a Care Site. Typically, however, Care Sites can provide care in multiple settings (inpatient, outpatient, etc.) and this granularity should be reflected in the visit.
Choose the concept in the visit domain that best represents the setting in which healthcare is provided in the Care Site. If most visits in a Care Site are Inpatient, then the place_of_service_concept_id should represent Inpatient. If information is present about a unique Care Site (e.g. Pharmacy) then a Care Site record should be created. If this information is not available then set to 0. [Accepted Concepts](https://athena.ohdsi.org/search-terms/terms?domain=Visit&amp;standardConcept=Standard&amp;page=2&amp;pageSize=15&amp;query=).</rdfs:comment>
    <rdfs:domain rdf:resource="https://w3id.org/omop/ontology/CareSite"/>
    <rdfs:range rdf:resource="https://w3id.org/omop/ontology/Concept"/>
    <ns1:omop_cdm_name rdf:datatype="http://www.w3.org/2001/XMLSchema#string">care_site.place_of_service_concept_id#269 AS Concept</ns1:omop_cdm_name>
  </rdf:Description>
  <rdf:Description rdf:nodeID="nde7e53d44aa94269b5c0c83d6d8798ccb690">
    <rdf:type rdf:resource="http://www.w3.org/2002/07/owl#Restriction"/>
    <owl:allValuesFrom rdf:resource="http://www.w3.org/2001/XMLSchema#string"/>
    <owl:onProperty rdf:resource="https://w3id.org/omop/ontology/standard"/>
  </rdf:Description>
  <rdf:Description rdf:nodeID="nde7e53d44aa94269b5c0c83d6d8798ccb276">
    <rdf:type rdf:resource="http://www.w3.org/2002/07/owl#Restriction"/>
    <owl:allValuesFrom rdf:resource="http://www.w3.org/2001/XMLSchema#string"/>
    <owl:onProperty rdf:resource="https://w3id.org/omop/ontology/name"/>
  </rdf:Description>
  <rdf:Description rdf:nodeID="nde7e53d44aa94269b5c0c83d6d8798ccb365">
    <rdf:first rdf:resource="https://w3id.org/omop/ontology/ProcedureOccurrence"/>
    <rdf:rest rdf:nodeID="nde7e53d44aa94269b5c0c83d6d8798ccb366"/>
  </rdf:Description>
  <rdf:Description rdf:nodeID="nde7e53d44aa94269b5c0c83d6d8798ccb92">
    <rdf:type rdf:resource="http://www.w3.org/2002/07/owl#Restriction"/>
    <owl:allValuesFrom rdf:resource="http://www.w3.org/2001/XMLSchema#decimal"/>
    <owl:onProperty rdf:resource="https://w3id.org/omop/ontology/value"/>
  </rdf:Description>
  <rdf:Description rdf:nodeID="nde7e53d44aa94269b5c0c83d6d8798ccb434">
    <rdf:type rdf:resource="http://www.w3.org/2002/07/owl#Restriction"/>
    <owl:allValuesFrom rdf:resource="https://w3id.org/omop/ontology/Observation"/>
    <owl:onProperty rdf:resource="https://w3id.org/omop/ontology/has_observation"/>
  </rdf:Description>
  <rdf:Description rdf:nodeID="nde7e53d44aa94269b5c0c83d6d8798ccb270">
    <rdf:first rdf:resource="https://w3id.org/omop/ontology/BaseVisit"/>
    <rdf:rest rdf:nodeID="nde7e53d44aa94269b5c0c83d6d8798ccb271"/>
  </rdf:Description>
  <rdf:Description rdf:about="https://w3id.org/omop/ontology/occurrence_count">
    <rdf:type rdf:resource="http://www.w3.org/2002/07/owl#DatatypeProperty"/>
    <rdf:type rdf:resource="http://www.w3.org/2002/07/owl#FunctionalProperty"/>
    <rdfs:comment xml:lang="en">(for ConditionEra:) The number of individual Condition
Occurrences used to construct the
condition era.</rdfs:comment>
    <rdfs:domain rdf:resource="https://w3id.org/omop/ontology/ConditionEra"/>
    <rdfs:range rdf:resource="http://www.w3.org/2001/XMLSchema#integer"/>
    <ns1:omop_cdm_name rdf:datatype="http://www.w3.org/2001/XMLSchema#string">condition_era.condition_occurrence_count#344 AS int</ns1:omop_cdm_name>
  </rdf:Description>
  <rdf:Description rdf:nodeID="nde7e53d44aa94269b5c0c83d6d8798ccb88">
    <rdf:type rdf:resource="http://www.w3.org/2002/07/owl#Restriction"/>
    <owl:allValuesFrom rdf:resource="http://www.w3.org/2001/XMLSchema#string"/>
    <owl:onProperty rdf:resource="https://w3id.org/omop/ontology/name"/>
  </rdf:Description>
  <rdf:Description rdf:nodeID="nde7e53d44aa94269b5c0c83d6d8798ccb424">
    <rdf:type rdf:resource="http://www.w3.org/2002/07/owl#Restriction"/>
    <owl:onProperty rdf:resource="https://w3id.org/omop/ontology/has_class"/>
    <owl:someValuesFrom rdf:resource="https://w3id.org/omop/ontology/Concept"/>
  </rdf:Description>
  <rdf:Description rdf:nodeID="nde7e53d44aa94269b5c0c83d6d8798ccb465">
    <rdf:type rdf:resource="http://www.w3.org/2002/07/owl#Restriction"/>
    <owl:allValuesFrom rdf:resource="https://w3id.org/omop/ontology/Concept"/>
    <owl:onProperty rdf:resource="https://w3id.org/omop/ontology/has_operator"/>
  </rdf:Description>
  <rdf:Description rdf:nodeID="nde7e53d44aa94269b5c0c83d6d8798ccb679">
    <rdf:type rdf:resource="http://www.w3.org/2002/07/owl#Restriction"/>
    <owl:onProperty rdf:resource="https://w3id.org/omop/ontology/valid_end_date"/>
    <owl:someValuesFrom rdf:resource="http://www.w3.org/2001/XMLSchema#date"/>
  </rdf:Description>
  <rdf:Description rdf:nodeID="nde7e53d44aa94269b5c0c83d6d8798ccb244">
    <rdf:type rdf:resource="http://www.w3.org/2002/07/owl#Restriction"/>
    <owl:onProperty rdf:resource="https://w3id.org/omop/ontology/name"/>
    <owl:someValuesFrom rdf:resource="http://www.w3.org/2001/XMLSchema#string"/>
  </rdf:Description>
  <rdf:Description rdf:nodeID="nde7e53d44aa94269b5c0c83d6d8798ccb396">
    <rdf:type rdf:resource="http://www.w3.org/2002/07/owl#Restriction"/>
    <owl:allValuesFrom rdf:resource="http://www.w3.org/2001/XMLSchema#string"/>
    <owl:onProperty rdf:resource="https://w3id.org/omop/ontology/anatomic_site_source_value"/>
  </rdf:Description>
  <rdf:Description rdf:about="https://w3id.org/omop/ontology/has_specialty_source">
    <rdf:type rdf:resource="http://www.w3.org/2002/07/owl#FunctionalProperty"/>
    <rdf:type rdf:resource="http://www.w3.org/2002/07/owl#ObjectProperty"/>
    <ns2:python_name rdf:datatype="http://www.w3.org/2001/XMLSchema#string">specialty_source</ns2:python_name>
    <rdfs:comment xml:lang="en">(for Provider:) This is often zero as many sites use proprietary codes to store physician speciality.
If the source data codes provider specialty in an OMOP supported vocabulary store the concept_id here. If not available, set to 0.</rdfs:comment>
    <rdfs:domain rdf:resource="https://w3id.org/omop/ontology/Provider"/>
    <rdfs:range rdf:resource="https://w3id.org/omop/ontology/Concept"/>
    <ns1:omop_cdm_name rdf:datatype="http://www.w3.org/2001/XMLSchema#string">provider.specialty_source_concept_id#283 AS Concept</ns1:omop_cdm_name>
  </rdf:Description>
  <rdf:Description rdf:about="https://w3id.org/omop/ontology/survey_end_date">
    <rdf:type rdf:resource="http://www.w3.org/2002/07/owl#DatatypeProperty"/>
    <rdf:type rdf:resource="http://www.w3.org/2002/07/owl#FunctionalProperty"/>
    <rdfs:comment xml:lang="en">(for SurveyConduct:) Date on which the survey was completed.</rdfs:comment>
    <rdfs:domain rdf:resource="https://w3id.org/omop/ontology/SurveyConduct"/>
    <rdfs:range rdf:resource="http://www.w3.org/2001/XMLSchema#date"/>
    <ns1:omop_cdm_name rdf:datatype="http://www.w3.org/2001/XMLSchema#string">survey_conduct.survey_end_date#232 AS date</ns1:omop_cdm_name>
  </rdf:Description>
  <rdf:Description rdf:nodeID="nde7e53d44aa94269b5c0c83d6d8798ccb486">
    <rdf:first rdf:resource="https://w3id.org/omop/ontology/Specimen"/>
    <rdf:rest rdf:nodeID="nde7e53d44aa94269b5c0c83d6d8798ccb487"/>
  </rdf:Description>
  <rdf:Description rdf:about="https://w3id.org/omop/ontology/has_preceding_visit_occurrence">
    <rdf:type rdf:resource="http://www.w3.org/2002/07/owl#FunctionalProperty"/>
    <rdf:type rdf:resource="http://www.w3.org/2002/07/owl#ObjectProperty"/>
    <ns2:python_name rdf:datatype="http://www.w3.org/2001/XMLSchema#string">preceding_visit_occurrence</ns2:python_name>
    <rdfs:comment xml:lang="en">(for VisitOccurrence:) Use this field to find the visit that occurred for the person prior to the given visit. There could be a few days or a few years in between.
The preceding_visit_id can be used to link a visit immediately preceding the current visit. Note this is not symmetrical, and there is no such thing as a "following_visit_id".</rdfs:comment>
    <rdfs:domain rdf:resource="https://w3id.org/omop/ontology/VisitOccurrence"/>
    <rdfs:range rdf:resource="https://w3id.org/omop/ontology/VisitOccurrence"/>
    <ns1:omop_cdm_name rdf:datatype="http://www.w3.org/2001/XMLSchema#string">visit_occurrence.preceding_visit_occurrence_id#41 AS VisitOccurrence</ns1:omop_cdm_name>
  </rdf:Description>
  <rdf:Description rdf:nodeID="nde7e53d44aa94269b5c0c83d6d8798ccb475">
    <rdf:type rdf:resource="http://www.w3.org/2002/07/owl#Restriction"/>
    <owl:allValuesFrom rdf:resource="http://www.w3.org/2001/XMLSchema#string"/>
    <owl:onProperty rdf:resource="https://w3id.org/omop/ontology/dea"/>
  </rdf:Description>
  <rdf:Description rdf:about="https://w3id.org/omop/ontology/disease_status_source_value">
    <rdf:type rdf:resource="http://www.w3.org/2002/07/owl#DatatypeProperty"/>
    <rdf:type rdf:resource="http://www.w3.org/2002/07/owl#FunctionalProperty"/>
    <rdfs:domain rdf:resource="https://w3id.org/omop/ontology/Specimen"/>
    <rdfs:range rdf:resource="http://www.w3.org/2001/XMLSchema#string"/>
    <ns1:omop_cdm_name rdf:datatype="http://www.w3.org/2001/XMLSchema#string">specimen.disease_status_source_value#221 AS str</ns1:omop_cdm_name>
  </rdf:Description>
  <rdf:Description rdf:about="https://w3id.org/omop/ontology/valid_start_date">
    <rdf:type rdf:resource="http://www.w3.org/2002/07/owl#DatatypeProperty"/>
    <rdf:type rdf:resource="http://www.w3.org/2002/07/owl#FunctionalProperty"/>
    <rdfs:comment xml:lang="en">(for Concept:) The date when the Concept was first
recorded. The default value is
1-Jan-1970, meaning, the Concept has no
(known) date of inception.</rdfs:comment>
    <rdfs:comment xml:lang="en">(for ConceptRelationship:) The date when the relationship is first recorded.</rdfs:comment>
    <rdfs:comment xml:lang="en">(for DrugStrength:) The date when the Concept was first
recorded. The default value is
1-Jan-1970.</rdfs:comment>
    <rdfs:comment xml:lang="en">(for SourceToConceptMap:) The date when the mapping
instance was first recorded.</rdfs:comment>
    <rdfs:domain rdf:nodeID="nde7e53d44aa94269b5c0c83d6d8798ccb232"/>
    <rdfs:range rdf:resource="http://www.w3.org/2001/XMLSchema#date"/>
    <ns1:omop_cdm_name rdf:datatype="http://www.w3.org/2001/XMLSchema#string">concept.valid_start_date#369 AS date</ns1:omop_cdm_name>
    <ns1:omop_cdm_name rdf:datatype="http://www.w3.org/2001/XMLSchema#string">concept_relationship.valid_start_date#386 AS date</ns1:omop_cdm_name>
    <ns1:omop_cdm_name rdf:datatype="http://www.w3.org/2001/XMLSchema#string">drug_strength.valid_start_date#420 AS date</ns1:omop_cdm_name>
    <ns1:omop_cdm_name rdf:datatype="http://www.w3.org/2001/XMLSchema#string">source_to_concept_map.valid_start_date#408 AS date</ns1:omop_cdm_name>
  </rdf:Description>
  <rdf:Description rdf:about="https://w3id.org/omop/ontology/address_2">
    <rdf:type rdf:resource="http://www.w3.org/2002/07/owl#DatatypeProperty"/>
    <rdf:type rdf:resource="http://www.w3.org/2002/07/owl#FunctionalProperty"/>
    <rdfs:comment xml:lang="en">(for Location:) This is the second line of the address</rdfs:comment>
    <rdfs:domain rdf:resource="https://w3id.org/omop/ontology/Location"/>
    <rdfs:range rdf:resource="http://www.w3.org/2001/XMLSchema#string"/>
    <ns1:omop_cdm_name rdf:datatype="http://www.w3.org/2001/XMLSchema#string">location.address_2#253 AS str</ns1:omop_cdm_name>
  </rdf:Description>
  <rdf:Description rdf:nodeID="nde7e53d44aa94269b5c0c83d6d8798ccb534">
    <rdf:type rdf:resource="http://www.w3.org/2002/07/owl#Restriction"/>
    <owl:allValuesFrom rdf:resource="https://w3id.org/omop/ontology/Concept"/>
    <owl:onProperty rdf:resource="https://w3id.org/omop/ontology/has_contract"/>
  </rdf:Description>
  <rdf:Description rdf:nodeID="nde7e53d44aa94269b5c0c83d6d8798ccb409">
    <rdf:type rdf:resource="http://www.w3.org/2002/07/owl#Restriction"/>
    <owl:allValuesFrom rdf:resource="http://www.w3.org/2001/XMLSchema#string"/>
    <owl:onProperty rdf:resource="https://w3id.org/omop/ontology/address_2"/>
  </rdf:Description>
  <rdf:Description rdf:about="https://w3id.org/omop/ontology/birth_datetime">
    <rdf:type rdf:resource="http://www.w3.org/2002/07/owl#DatatypeProperty"/>
    <rdf:type rdf:resource="http://www.w3.org/2002/07/owl#FunctionalProperty"/>
    <rdfs:comment xml:lang="en">(for Person:) This field is not required but highly encouraged. For data sources that provide the precise datetime of birth, that value should be stored in this field. If birth_datetime is not provided in the source, use the following logic to infer the date: If day_of_birth is null and month_of_birth is not null then use the first of the month in that year. If month_of_birth is null or if day_of_birth AND month_of_birth are both null and the person has records during their year of birth then use the date of the earliest record, otherwise use the 15th of June of that year. If time of birth is not given use midnight (00:00:0000).</rdfs:comment>
    <rdfs:domain rdf:resource="https://w3id.org/omop/ontology/Person"/>
    <rdfs:range rdf:resource="http://www.w3.org/2001/XMLSchema#dateTime"/>
    <ns1:omop_cdm_name rdf:datatype="http://www.w3.org/2001/XMLSchema#string">person.birth_datetime#6 AS datetime</ns1:omop_cdm_name>
  </rdf:Description>
  <rdf:Description rdf:about="https://w3id.org/omop/ontology/modifier_source_value">
    <rdf:type rdf:resource="http://www.w3.org/2002/07/owl#DatatypeProperty"/>
    <rdf:type rdf:resource="http://www.w3.org/2002/07/owl#FunctionalProperty"/>
    <rdfs:comment xml:lang="en">(for ProcedureOccurrence:) The original modifier code from the source is stored here for reference.</rdfs:comment>
    <rdfs:domain rdf:resource="https://w3id.org/omop/ontology/ProcedureOccurrence"/>
    <rdfs:range rdf:resource="http://www.w3.org/2001/XMLSchema#string"/>
    <ns1:omop_cdm_name rdf:datatype="http://www.w3.org/2001/XMLSchema#string">procedure_occurrence.modifier_source_value#113 AS str</ns1:omop_cdm_name>
  </rdf:Description>
  <rdf:Description rdf:nodeID="nde7e53d44aa94269b5c0c83d6d8798ccb652">
    <rdf:type rdf:resource="http://www.w3.org/2002/07/owl#Restriction"/>
    <owl:allValuesFrom rdf:resource="https://w3id.org/omop/ontology/ProcedureOccurrence"/>
    <owl:onProperty rdf:resource="https://w3id.org/omop/ontology/has_procedure_occurrence"/>
  </rdf:Description>
  <rdf:Description rdf:about="https://w3id.org/omop/ontology/syntax">
    <rdf:type rdf:resource="http://www.w3.org/2002/07/owl#DatatypeProperty"/>
    <rdf:type rdf:resource="http://www.w3.org/2002/07/owl#FunctionalProperty"/>
    <rdfs:comment xml:lang="en">(for CohortDefinition:) Syntax or code to operationalize the Cohort Definition.</rdfs:comment>
    <rdfs:domain rdf:resource="https://w3id.org/omop/ontology/CohortDefinition"/>
    <rdfs:range rdf:resource="http://www.w3.org/2001/XMLSchema#string"/>
    <ns1:omop_cdm_name rdf:datatype="http://www.w3.org/2001/XMLSchema#string">cohort_definition.cohort_definition_syntax#431 AS str</ns1:omop_cdm_name>
  </rdf:Description>
  <rdf:Description rdf:nodeID="nde7e53d44aa94269b5c0c83d6d8798ccb654">
    <rdf:type rdf:resource="http://www.w3.org/2002/07/owl#Restriction"/>
    <owl:allValuesFrom rdf:resource="http://www.w3.org/2001/XMLSchema#integer"/>
    <owl:onProperty rdf:resource="https://w3id.org/omop/ontology/day_of_birth"/>
  </rdf:Description>
  <rdf:Description rdf:nodeID="nde7e53d44aa94269b5c0c83d6d8798ccb665">
    <rdf:type rdf:resource="http://www.w3.org/2002/07/owl#Restriction"/>
    <owl:allValuesFrom rdf:resource="https://w3id.org/omop/ontology/Cost"/>
    <owl:onProperty rdf:resource="https://w3id.org/omop/ontology/has_cost"/>
  </rdf:Description>
  <rdf:Description rdf:nodeID="nde7e53d44aa94269b5c0c83d6d8798ccb407">
    <rdf:type rdf:resource="http://www.w3.org/2002/07/owl#Restriction"/>
    <owl:allValuesFrom rdf:resource="http://www.w3.org/2001/XMLSchema#decimal"/>
    <owl:onProperty rdf:resource="https://w3id.org/omop/ontology/longitude"/>
  </rdf:Description>
  <rdf:Description rdf:nodeID="nde7e53d44aa94269b5c0c83d6d8798ccb688">
    <rdf:type rdf:resource="http://www.w3.org/2002/07/owl#Restriction"/>
    <owl:allValuesFrom rdf:resource="https://w3id.org/omop/ontology/Domain"/>
    <owl:onProperty rdf:resource="https://w3id.org/omop/ontology/has_domain"/>
  </rdf:Description>
  <rdf:Description rdf:about="https://w3id.org/omop/ontology/gap_days">
    <rdf:type rdf:resource="http://www.w3.org/2002/07/owl#DatatypeProperty"/>
    <rdf:type rdf:resource="http://www.w3.org/2002/07/owl#FunctionalProperty"/>
    <rdfs:comment xml:lang="en">(for DrugEra:) The Gap Days determine how many total drug-free days are observed between all Drug Exposure events that contribute to a DRUG_ERA record. It is assumed that the drugs are "not stockpiled" by the patient, i.e. that if a new drug prescription or refill is observed (a new DRUG_EXPOSURE record is written), the remaining supply from the previous events is abandoned.   The difference between Persistence Window and Gap Days is that the former is the maximum drug-free time allowed between two subsequent DRUG_EXPOSURE records, while the latter is the sum of actual drug-free days for the given Drug Era under the above assumption of non-stockpiling.</rdfs:comment>
    <rdfs:domain rdf:resource="https://w3id.org/omop/ontology/DrugEra"/>
    <rdfs:range rdf:resource="http://www.w3.org/2001/XMLSchema#integer"/>
    <ns1:omop_cdm_name rdf:datatype="http://www.w3.org/2001/XMLSchema#string">drug_era.gap_days#331 AS int</ns1:omop_cdm_name>
  </rdf:Description>
  <rdf:Description rdf:nodeID="nde7e53d44aa94269b5c0c83d6d8798ccb61">
    <rdf:first rdf:resource="https://w3id.org/omop/ontology/Cost"/>
    <rdf:rest rdf:nodeID="nde7e53d44aa94269b5c0c83d6d8798ccb62"/>
  </rdf:Description>
  <rdf:Description rdf:about="https://w3id.org/omop/ontology/source_code">
    <rdf:type rdf:resource="http://www.w3.org/2002/07/owl#DatatypeProperty"/>
    <rdf:type rdf:resource="http://www.w3.org/2002/07/owl#FunctionalProperty"/>
    <rdfs:comment xml:lang="en">(for SourceToConceptMap:) The source code being translated
into a Standard Concept.</rdfs:comment>
    <rdfs:domain rdf:resource="https://w3id.org/omop/ontology/SourceToConceptMap"/>
    <rdfs:range rdf:resource="http://www.w3.org/2001/XMLSchema#string"/>
    <ns1:omop_cdm_name rdf:datatype="http://www.w3.org/2001/XMLSchema#string">source_to_concept_map.source_code#402 AS str</ns1:omop_cdm_name>
  </rdf:Description>
  <rdf:Description rdf:nodeID="nde7e53d44aa94269b5c0c83d6d8798ccb200">
    <rdf:type rdf:resource="http://www.w3.org/2002/07/owl#Restriction"/>
    <owl:allValuesFrom rdf:resource="http://www.w3.org/2001/XMLSchema#string"/>
    <owl:onProperty rdf:resource="https://w3id.org/omop/ontology/name"/>
  </rdf:Description>
  <rdf:Description rdf:nodeID="nde7e53d44aa94269b5c0c83d6d8798ccb533">
    <rdf:type rdf:resource="http://www.w3.org/2002/07/owl#Restriction"/>
    <owl:onProperty rdf:resource="https://w3id.org/omop/ontology/has_contract_source"/>
    <owl:someValuesFrom rdf:resource="https://w3id.org/omop/ontology/Concept"/>
  </rdf:Description>
  <rdf:Description rdf:nodeID="nde7e53d44aa94269b5c0c83d6d8798ccb215">
    <rdf:type rdf:resource="http://www.w3.org/2002/07/owl#Restriction"/>
    <owl:onProperty rdf:resource="https://w3id.org/omop/ontology/defines_ancestry"/>
    <owl:someValuesFrom rdf:resource="http://www.w3.org/2001/XMLSchema#string"/>
  </rdf:Description>
  <rdf:Description rdf:nodeID="nde7e53d44aa94269b5c0c83d6d8798ccb615">
    <rdf:type rdf:resource="http://www.w3.org/2002/07/owl#Restriction"/>
    <owl:onProperty rdf:resource="https://w3id.org/omop/ontology/has_respondent_type"/>
    <owl:someValuesFrom rdf:resource="https://w3id.org/omop/ontology/Concept"/>
  </rdf:Description>
  <rdf:Description rdf:nodeID="nde7e53d44aa94269b5c0c83d6d8798ccb558">
    <rdf:type rdf:resource="http://www.w3.org/2002/07/owl#Restriction"/>
    <owl:allValuesFrom rdf:resource="http://www.w3.org/2001/XMLSchema#string"/>
    <owl:onProperty rdf:resource="https://w3id.org/omop/ontology/family_source_value"/>
  </rdf:Description>
  <rdf:Description rdf:nodeID="nde7e53d44aa94269b5c0c83d6d8798ccb340">
    <rdf:type rdf:resource="http://www.w3.org/2002/07/owl#Restriction"/>
    <owl:allValuesFrom rdf:resource="https://w3id.org/omop/ontology/Concept"/>
    <owl:onProperty rdf:resource="https://w3id.org/omop/ontology/has_source"/>
  </rdf:Description>
  <rdf:Description rdf:nodeID="nde7e53d44aa94269b5c0c83d6d8798ccb564">
    <rdf:first rdf:resource="https://w3id.org/omop/ontology/ProcedureOccurrence"/>
    <rdf:rest rdf:nodeID="nde7e53d44aa94269b5c0c83d6d8798ccb565"/>
  </rdf:Description>
  <rdf:Description rdf:nodeID="nde7e53d44aa94269b5c0c83d6d8798ccb160">
    <rdf:type rdf:resource="http://www.w3.org/2002/07/owl#Restriction"/>
    <owl:onProperty rdf:resource="https://w3id.org/omop/ontology/domain_concept_id_1"/>
    <owl:someValuesFrom rdf:resource="http://www.w3.org/2001/XMLSchema#integer"/>
  </rdf:Description>
  <rdf:Description rdf:nodeID="nde7e53d44aa94269b5c0c83d6d8798ccb324">
    <rdf:type rdf:resource="http://www.w3.org/2002/07/owl#Restriction"/>
    <owl:allValuesFrom rdf:resource="https://w3id.org/omop/ontology/Concept"/>
    <owl:onProperty rdf:resource="https://w3id.org/omop/ontology/has_numerator_unit"/>
  </rdf:Description>
  <rdf:Description rdf:about="https://w3id.org/omop/ontology/start_date">
    <rdf:type rdf:resource="http://www.w3.org/2002/07/owl#DatatypeProperty"/>
    <rdf:type rdf:resource="http://www.w3.org/2002/07/owl#FunctionalProperty"/>
    <rdfs:comment xml:lang="en">(for ConditionOccurrence:) Use this date to determine the start date of the condition
Most often data sources do not have the idea of a start date for a condition. Rather, if a source only has one date associated with a condition record it is acceptable to use that date for both the CONDITION_START_DATE and the CONDITION_END_DATE.</rdfs:comment>
    <rdfs:comment xml:lang="en">(for DeviceExposure:) Use this date to determine the start date of the device record.
Valid entries include a start date of a procedure to implant a device, the date of a prescription for a device, or the date of device administration.</rdfs:comment>
    <rdfs:comment xml:lang="en">(for DrugExposure:) Use this date to determine the start date of the drug record.
Valid entries include a start date of a prescription, the date a prescription was filled, or the date on which a Drug administration was recorded. It is a valid ETL choice to use the date the drug was ordered as the DRUG_EXPOSURE_START_DATE.</rdfs:comment>
    <rdfs:comment xml:lang="en">(for LocationHistory:) The date the relationship started</rdfs:comment>
    <rdfs:comment xml:lang="en">(for ObservationPeriod:) Use this date to determine the start date of the Observation Period
It is often the case that the idea of Observation Periods does not exist in source data. In those cases, the observation_period_start_date can be inferred as the earliest Event date available for the Person. In insurance claim data, the Observation Period can be considered as the time period the Person is enrolled with a payer. If a Person switches plans but stays with the same payer, and therefore capturing of data continues, that change would be captured in [PAYER_PLAN_PERIOD](https://ohdsi.github.io/CommonDataModel/cdm60.html#payer_plan_period).</rdfs:comment>
    <rdfs:comment xml:lang="en">(for PayerPlanPeriod:) Start date of Plan coverage.</rdfs:comment>
    <rdfs:comment xml:lang="en">(for VisitDetail:) This is the date of the start of the encounter. This may or may not be equal to the date of the Visit the Visit Detail is associated with.
When populating visit_start_date, you should think about the patient experience to make decisions on how to define visits. Most likely this should be the date of the patient-provider interaction.</rdfs:comment>
    <rdfs:comment xml:lang="en">(for VisitOccurrence:) For inpatient visits, the start date is typically the admission date. For outpatient visits the start date and end date will be the same.
When populating visit_start_date, you should think about the patient experience to make decisions on how to define visits. In the case of an inpatient visit this should be the date the patient was admitted to the hospital or institution. In all other cases this should be the date of the patient-provider interaction.</rdfs:comment>
    <rdfs:domain rdf:resource="https://w3id.org/omop/ontology/DateDuration"/>
    <rdfs:range rdf:resource="http://www.w3.org/2001/XMLSchema#date"/>
    <ns1:omop_cdm_name rdf:datatype="http://www.w3.org/2001/XMLSchema#string">cohort.cohort_start_date#425 AS date</ns1:omop_cdm_name>
    <ns1:omop_cdm_name rdf:datatype="http://www.w3.org/2001/XMLSchema#string">condition_occurrence.condition_start_date#64 AS date</ns1:omop_cdm_name>
    <ns1:omop_cdm_name rdf:datatype="http://www.w3.org/2001/XMLSchema#string">device_exposure.device_exposure_start_date#117 AS date</ns1:omop_cdm_name>
    <ns1:omop_cdm_name rdf:datatype="http://www.w3.org/2001/XMLSchema#string">drug_exposure.drug_exposure_start_date#80 AS date</ns1:omop_cdm_name>
    <ns1:omop_cdm_name rdf:datatype="http://www.w3.org/2001/XMLSchema#string">location_history.start_date#265 AS date</ns1:omop_cdm_name>
    <ns1:omop_cdm_name rdf:datatype="http://www.w3.org/2001/XMLSchema#string">observation_period.observation_period_start_date#22 AS date</ns1:omop_cdm_name>
    <ns1:omop_cdm_name rdf:datatype="http://www.w3.org/2001/XMLSchema#string">payer_plan_period.payer_plan_period_start_date#289 AS date</ns1:omop_cdm_name>
    <ns1:omop_cdm_name rdf:datatype="http://www.w3.org/2001/XMLSchema#string">visit_detail.visit_detail_start_date#45 AS date</ns1:omop_cdm_name>
    <ns1:omop_cdm_name rdf:datatype="http://www.w3.org/2001/XMLSchema#string">visit_occurrence.visit_start_date#28 AS date</ns1:omop_cdm_name>
  </rdf:Description>
  <rdf:Description rdf:about="https://w3id.org/omop/ontology/death_datetime">
    <rdf:type rdf:resource="http://www.w3.org/2002/07/owl#DatatypeProperty"/>
    <rdf:type rdf:resource="http://www.w3.org/2002/07/owl#FunctionalProperty"/>
    <rdfs:comment xml:lang="en">(for Person:) This field is the death date to be used in analysis, as determined by the ETL logic. Any additional information about a Person's death is stored in the [OBSERVATION](https://ohdsi.github.io/CommonDataModel/cdm60.html#observation) table with the concept_id [4306655](https://athena.ohdsi.org/search-terms/terms/4306655) or in the CONDITION_OCCURRENCE .
If there are multiple dates of death given for a Person, choose the one that is deemed most reliable. This may be a discharge from the hospital where the Person is listed as deceased or it could be latest death date provided. If a patient has clinical activity more than 60 days after the death date given in the source, it is a viable option to drop the death record as it may have been falsely reported. Similarly, if the death record is from a reputable source (e.g. government provided information) it is also a viable option to remove event records that occur in the data &gt; 60 days after death.</rdfs:comment>
    <rdfs:domain rdf:resource="https://w3id.org/omop/ontology/Person"/>
    <rdfs:range rdf:resource="http://www.w3.org/2001/XMLSchema#dateTime"/>
    <ns1:omop_cdm_name rdf:datatype="http://www.w3.org/2001/XMLSchema#string">person.death_datetime#7 AS datetime</ns1:omop_cdm_name>
  </rdf:Description>
  <rdf:Description rdf:nodeID="nde7e53d44aa94269b5c0c83d6d8798ccb165">
    <rdf:type rdf:resource="http://www.w3.org/2002/07/owl#Restriction"/>
    <owl:allValuesFrom rdf:resource="https://w3id.org/omop/ontology/Concept"/>
    <owl:onProperty rdf:resource="https://w3id.org/omop/ontology/has_type"/>
  </rdf:Description>
  <rdf:Description rdf:nodeID="nde7e53d44aa94269b5c0c83d6d8798ccb601">
    <rdf:type rdf:resource="http://www.w3.org/2002/07/owl#Restriction"/>
    <owl:onProperty rdf:resource="https://w3id.org/omop/ontology/has_validated_survey"/>
    <owl:someValuesFrom rdf:resource="https://w3id.org/omop/ontology/Concept"/>
  </rdf:Description>
  <rdf:Description rdf:nodeID="nde7e53d44aa94269b5c0c83d6d8798ccb528">
    <rdf:type rdf:resource="http://www.w3.org/2002/07/owl#Restriction"/>
    <owl:onProperty rdf:resource="https://w3id.org/omop/ontology/has_type"/>
    <owl:someValuesFrom rdf:resource="https://w3id.org/omop/ontology/Concept"/>
  </rdf:Description>
  <rdf:Description rdf:nodeID="nde7e53d44aa94269b5c0c83d6d8798ccb114">
    <rdf:first rdf:resource="https://w3id.org/omop/ontology/Note"/>
    <rdf:rest rdf:resource="http://www.w3.org/1999/02/22-rdf-syntax-ns#nil"/>
  </rdf:Description>
  <rdf:Description rdf:about="https://w3id.org/omop/ontology/address_1">
    <rdf:type rdf:resource="http://www.w3.org/2002/07/owl#DatatypeProperty"/>
    <rdf:type rdf:resource="http://www.w3.org/2002/07/owl#FunctionalProperty"/>
    <rdfs:comment xml:lang="en">(for Location:) This is the first line of the address.</rdfs:comment>
    <rdfs:domain rdf:resource="https://w3id.org/omop/ontology/Location"/>
    <rdfs:range rdf:resource="http://www.w3.org/2001/XMLSchema#string"/>
    <ns1:omop_cdm_name rdf:datatype="http://www.w3.org/2001/XMLSchema#string">location.address_1#252 AS str</ns1:omop_cdm_name>
  </rdf:Description>
  <rdf:Description rdf:nodeID="nde7e53d44aa94269b5c0c83d6d8798ccb158">
    <rdf:type rdf:resource="http://www.w3.org/2002/07/owl#Restriction"/>
    <owl:allValuesFrom rdf:resource="http://www.w3.org/2001/XMLSchema#integer"/>
    <owl:onProperty rdf:resource="https://w3id.org/omop/ontology/domain_concept_id_1"/>
  </rdf:Description>
  <rdf:Description rdf:about="https://w3id.org/omop/ontology/Location">
    <rdf:type rdf:resource="http://www.w3.org/2002/07/owl#Class"/>
    <rdfs:subClassOf rdf:nodeID="nde7e53d44aa94269b5c0c83d6d8798ccb407"/>
    <rdfs:subClassOf rdf:nodeID="nde7e53d44aa94269b5c0c83d6d8798ccb408"/>
    <rdfs:subClassOf rdf:nodeID="nde7e53d44aa94269b5c0c83d6d8798ccb409"/>
    <rdfs:subClassOf rdf:nodeID="nde7e53d44aa94269b5c0c83d6d8798ccb410"/>
    <rdfs:subClassOf rdf:nodeID="nde7e53d44aa94269b5c0c83d6d8798ccb411"/>
    <rdfs:subClassOf rdf:nodeID="nde7e53d44aa94269b5c0c83d6d8798ccb412"/>
    <rdfs:subClassOf rdf:nodeID="nde7e53d44aa94269b5c0c83d6d8798ccb413"/>
    <rdfs:subClassOf rdf:nodeID="nde7e53d44aa94269b5c0c83d6d8798ccb414"/>
    <rdfs:subClassOf rdf:nodeID="nde7e53d44aa94269b5c0c83d6d8798ccb415"/>
    <rdfs:subClassOf rdf:resource="https://w3id.org/omop/ontology/OmopCDMThing"/>
    <ns1:omop_cdm_name rdf:datatype="http://www.w3.org/2001/XMLSchema#string">location</ns1:omop_cdm_name>
  </rdf:Description>
  <rdf:Description rdf:about="https://w3id.org/omop/ontology/has_qualifier">
    <rdf:type rdf:resource="http://www.w3.org/2002/07/owl#FunctionalProperty"/>
    <rdf:type rdf:resource="http://www.w3.org/2002/07/owl#ObjectProperty"/>
    <ns2:python_name rdf:datatype="http://www.w3.org/2001/XMLSchema#string">qualifier</ns2:python_name>
    <rdfs:comment xml:lang="en">(for Observation:) This field contains all attributes specifying the clinical fact further, such as as degrees, severities, drug-drug interaction alerts etc.
Use your best judgement as to what Concepts to use here and if they are necessary to accurately represent the clinical record. There is no restriction on the domain of these Concepts, they just need to be Standard.</rdfs:comment>
    <rdfs:domain rdf:resource="https://w3id.org/omop/ontology/Observation"/>
    <rdfs:range rdf:resource="https://w3id.org/omop/ontology/Concept"/>
    <ns1:omop_cdm_name rdf:datatype="http://www.w3.org/2001/XMLSchema#string">observation.qualifier_concept_id#158 AS Concept</ns1:omop_cdm_name>
  </rdf:Description>
  <rdf:Description rdf:about="https://w3id.org/omop/ontology/has_domain">
    <rdf:type rdf:resource="http://www.w3.org/2002/07/owl#FunctionalProperty"/>
    <rdf:type rdf:resource="http://www.w3.org/2002/07/owl#ObjectProperty"/>
    <ns2:python_name rdf:datatype="http://www.w3.org/2001/XMLSchema#string">domain</ns2:python_name>
    <rdfs:comment xml:lang="en">(for Concept:) A foreign key to the [DOMAIN](https://ohdsi.github.io/CommonDataModel/cdm531.html#domain) table the Concept belongs to.</rdfs:comment>
    <rdfs:comment xml:lang="en">(for LocationHistory:) The domain of the entity that is related to the location. Either PERSON, PROVIDER, or CARE_SITE.</rdfs:comment>
    <rdfs:domain rdf:nodeID="nde7e53d44aa94269b5c0c83d6d8798ccb115"/>
    <rdfs:range rdf:resource="https://w3id.org/omop/ontology/Domain"/>
    <ns1:omop_cdm_name rdf:datatype="http://www.w3.org/2001/XMLSchema#string">concept.domain_id#364 AS Domain</ns1:omop_cdm_name>
    <ns1:omop_cdm_name rdf:datatype="http://www.w3.org/2001/XMLSchema#string">location_history.domain_id#263 AS Domain</ns1:omop_cdm_name>
  </rdf:Description>
  <rdf:Description rdf:about="https://w3id.org/omop/ontology/invalid_reason">
    <rdf:type rdf:resource="http://www.w3.org/2002/07/owl#DatatypeProperty"/>
    <rdf:type rdf:resource="http://www.w3.org/2002/07/owl#FunctionalProperty"/>
    <rdfs:comment xml:lang="en">(for Concept:) Reason the Concept was invalidated.
Possible values are D (deleted), U
(replaced with an update) or NULL when
valid_end_date has the default value.</rdfs:comment>
    <rdfs:comment xml:lang="en">(for ConceptRelationship:) Reason the relationship was invalidated. Possible values are 'D' (deleted), 'U' (updated) or NULL.</rdfs:comment>
    <rdfs:comment xml:lang="en">(for DrugStrength:) Reason the concept was invalidated. Possible values are D (deleted), U (replaced with an update) or NULL when valid_end_date has the default value.</rdfs:comment>
    <rdfs:comment xml:lang="en">(for SourceToConceptMap:) Reason the mapping instance was
invalidated. Possible values are D
(deleted), U (replaced with an
update) or NULL when
valid_end_date has the default
value.</rdfs:comment>
    <rdfs:domain rdf:nodeID="nde7e53d44aa94269b5c0c83d6d8798ccb138"/>
    <rdfs:range rdf:resource="http://www.w3.org/2001/XMLSchema#string"/>
    <ns1:omop_cdm_name rdf:datatype="http://www.w3.org/2001/XMLSchema#string">concept.invalid_reason#371 AS str</ns1:omop_cdm_name>
    <ns1:omop_cdm_name rdf:datatype="http://www.w3.org/2001/XMLSchema#string">concept_relationship.invalid_reason#388 AS str</ns1:omop_cdm_name>
    <ns1:omop_cdm_name rdf:datatype="http://www.w3.org/2001/XMLSchema#string">drug_strength.invalid_reason#422 AS str</ns1:omop_cdm_name>
    <ns1:omop_cdm_name rdf:datatype="http://www.w3.org/2001/XMLSchema#string">source_to_concept_map.invalid_reason#410 AS str</ns1:omop_cdm_name>
  </rdf:Description>
  <rdf:Description rdf:nodeID="nde7e53d44aa94269b5c0c83d6d8798ccb123">
    <rdf:first rdf:resource="https://w3id.org/omop/ontology/ConceptSynonym"/>
    <rdf:rest rdf:nodeID="nde7e53d44aa94269b5c0c83d6d8798ccb124"/>
  </rdf:Description>
  <rdf:Description rdf:about="https://w3id.org/omop/ontology/description">
    <rdf:type rdf:resource="http://www.w3.org/2002/07/owl#DatatypeProperty"/>
    <rdf:type rdf:resource="http://www.w3.org/2002/07/owl#FunctionalProperty"/>
    <rdfs:comment xml:lang="en">(for CohortDefinition:) A complete description of the cohort.</rdfs:comment>
    <rdfs:domain rdf:resource="https://w3id.org/omop/ontology/CohortDefinition"/>
    <rdfs:range rdf:resource="http://www.w3.org/2001/XMLSchema#string"/>
    <ns1:omop_cdm_name rdf:datatype="http://www.w3.org/2001/XMLSchema#string">cohort_definition.cohort_definition_description#429 AS str</ns1:omop_cdm_name>
  </rdf:Description>
  <rdf:Description rdf:nodeID="nde7e53d44aa94269b5c0c83d6d8798ccb334">
    <rdf:type rdf:resource="http://www.w3.org/2002/07/owl#Restriction"/>
    <owl:allValuesFrom rdf:resource="http://www.w3.org/2001/XMLSchema#date"/>
    <owl:onProperty rdf:resource="https://w3id.org/omop/ontology/valid_end_date"/>
  </rdf:Description>
  <rdf:Description rdf:nodeID="nde7e53d44aa94269b5c0c83d6d8798ccb539">
    <rdf:type rdf:resource="http://www.w3.org/2002/07/owl#Restriction"/>
    <owl:allValuesFrom rdf:resource="https://w3id.org/omop/ontology/Concept"/>
    <owl:onProperty rdf:resource="https://w3id.org/omop/ontology/has_contract_source"/>
  </rdf:Description>
  <rdf:Description rdf:nodeID="nde7e53d44aa94269b5c0c83d6d8798ccb441">
    <rdf:type rdf:resource="http://www.w3.org/2002/07/owl#Restriction"/>
    <owl:allValuesFrom rdf:resource="https://w3id.org/omop/ontology/CareSite"/>
    <owl:onProperty rdf:resource="https://w3id.org/omop/ontology/has_care_site"/>
  </rdf:Description>
  <rdf:Description rdf:nodeID="nde7e53d44aa94269b5c0c83d6d8798ccb314">
    <rdf:type rdf:resource="http://www.w3.org/2002/07/owl#Restriction"/>
    <owl:onProperty rdf:nodeID="nde7e53d44aa94269b5c0c83d6d8798ccb315"/>
    <owl:someValuesFrom rdf:resource="https://w3id.org/omop/ontology/VisitOccurrence"/>
  </rdf:Description>
  <rdf:Description rdf:nodeID="nde7e53d44aa94269b5c0c83d6d8798ccb612">
    <rdf:type rdf:resource="http://www.w3.org/2002/07/owl#Restriction"/>
    <owl:allValuesFrom rdf:resource="https://w3id.org/omop/ontology/Concept"/>
    <owl:onProperty rdf:resource="https://w3id.org/omop/ontology/has_timing"/>
  </rdf:Description>
  <rdf:Description rdf:nodeID="nde7e53d44aa94269b5c0c83d6d8798ccb316">
    <rdf:type rdf:resource="http://www.w3.org/2002/07/owl#Restriction"/>
    <owl:allValuesFrom rdf:resource="https://w3id.org/omop/ontology/VisitDetail"/>
    <owl:onProperty rdf:resource="https://w3id.org/omop/ontology/has_preceding_visit_detail"/>
  </rdf:Description>
  <rdf:Description rdf:about="https://w3id.org/omop/ontology/has_provider">
    <rdf:type rdf:resource="http://www.w3.org/2002/07/owl#FunctionalProperty"/>
    <rdf:type rdf:resource="http://www.w3.org/2002/07/owl#ObjectProperty"/>
    <ns2:python_name rdf:datatype="http://www.w3.org/2001/XMLSchema#string">provider</ns2:python_name>
    <rdfs:comment xml:lang="en">(for ConditionOccurrence:) The provider associated with condition record, e.g. the provider who made the diagnosis or the provider who recorded the symptom.
The ETL may need to make a choice as to which PROVIDER_ID to put here. Based on what is available this may or may not be different than the provider associated with the overall VISIT_OCCURRENCE record, for example the admitting vs attending physician on an EHR record.</rdfs:comment>
    <rdfs:comment xml:lang="en">(for DeviceExposure:) The Provider associated with device record, e.g. the provider who wrote the prescription or the provider who implanted the device.
The ETL may need to make a choice as to which PROVIDER_ID to put here. Based on what is available this may or may not be different than the provider associated with the overall VISIT_OCCURRENCE record.</rdfs:comment>
    <rdfs:comment xml:lang="en">(for DrugExposure:) The Provider associated with drug record, e.g. the provider who wrote the prescription or the provider who administered the drug.
The ETL may need to make a choice as to which PROVIDER_ID to put here. Based on what is available this may or may not be different than the provider associated with the overall VISIT_OCCURRENCE record, for example the ordering vs administering physician on an EHR record.</rdfs:comment>
    <rdfs:comment xml:lang="en">(for Measurement:) The provider associated with measurement record, e.g. the provider who ordered the test or the provider who recorded the result.
The ETL may need to make a choice as to which PROVIDER_ID to put here. Based on what is available this may or may not be different than the provider associated with the overall VISIT_OCCURRENCE record. For example the admitting vs attending physician on an EHR record.</rdfs:comment>
    <rdfs:comment xml:lang="en">(for Note:) The Provider who wrote the note.
The ETL may need to make a determination on which provider to put here.</rdfs:comment>
    <rdfs:comment xml:lang="en">(for Observation:) The provider associated with the observation record, e.g. the provider who ordered the test or the provider who recorded the result.
The ETL may need to make a choice as to which PROVIDER_ID to put here. Based on what is available this may or may not be different than the provider associated with the overall VISIT_OCCURRENCE record. For example the admitting vs attending physician on an EHR record.</rdfs:comment>
    <rdfs:comment xml:lang="en">(for Person:) The Provider refers to the last known primary care provider (General Practitioner).
Put the provider_id from the PROVIDER table of the last known general practitioner of the person. If there are multiple providers, it is up to the ETL to decide which to put here.</rdfs:comment>
    <rdfs:comment xml:lang="en">(for ProcedureOccurrence:) The provider associated with the procedure record, e.g. the provider who performed the Procedure.
The ETL may need to make a choice as to which PROVIDER_ID to put here. Based on what is available this may or may not be different than the provider associated with the overall VISIT_OCCURRENCE record, for example the admitting vs attending physician on an EHR record.</rdfs:comment>
    <rdfs:comment xml:lang="en">(for SurveyConduct:) This is the Provider associated with the survey completion.
The ETL may need to make a choice as to which Provider to put here. This could either be the provider that ordered the survey or the provider who observed the completion of the survey.</rdfs:comment>
    <rdfs:comment xml:lang="en">(for VisitDetail:) There will only be one provider per  **visit** record and the ETL document should clearly state how they were chosen (attending, admitting, etc.). This is a typical reason for leveraging the VISIT_DETAIL table as even though each VISIT_DETAIL record can only have one provider, there is no limit to the number of VISIT_DETAIL records that can be associated to a VISIT_OCCURRENCE record.
The additional providers associated to a Visit can be stored in this table where each VISIT_DETAIL record represents a different provider.</rdfs:comment>
    <rdfs:comment xml:lang="en">(for VisitOccurrence:) There will only be one provider per visit record and the ETL document should clearly state how they were chosen (attending, admitting, etc.). If there are multiple providers associated with a visit in the source, this can be reflected in the event tables (CONDITION_OCCURRENCE, PROCEDURE_OCCURRENCE, etc.) or in the VISIT_DETAIL table.
If there are multiple providers associated with a visit, you will need to choose which one to put here. The additional providers can be stored in the visit_detail table.</rdfs:comment>
    <rdfs:domain rdf:nodeID="nde7e53d44aa94269b5c0c83d6d8798ccb264"/>
    <rdfs:range rdf:resource="https://w3id.org/omop/ontology/Provider"/>
    <ns1:omop_cdm_name rdf:datatype="http://www.w3.org/2001/XMLSchema#string">condition_occurrence.provider_id#71 AS Provider</ns1:omop_cdm_name>
    <ns1:omop_cdm_name rdf:datatype="http://www.w3.org/2001/XMLSchema#string">device_exposure.provider_id#124 AS Provider</ns1:omop_cdm_name>
    <ns1:omop_cdm_name rdf:datatype="http://www.w3.org/2001/XMLSchema#string">drug_exposure.provider_id#93 AS Provider</ns1:omop_cdm_name>
    <ns1:omop_cdm_name rdf:datatype="http://www.w3.org/2001/XMLSchema#string">measurement.provider_id#142 AS Provider</ns1:omop_cdm_name>
    <ns1:omop_cdm_name rdf:datatype="http://www.w3.org/2001/XMLSchema#string">note.provider_id#189 AS Provider</ns1:omop_cdm_name>
    <ns1:omop_cdm_name rdf:datatype="http://www.w3.org/2001/XMLSchema#string">observation.provider_id#160 AS Provider</ns1:omop_cdm_name>
    <ns1:omop_cdm_name rdf:datatype="http://www.w3.org/2001/XMLSchema#string">person.provider_id#11 AS Provider</ns1:omop_cdm_name>
    <ns1:omop_cdm_name rdf:datatype="http://www.w3.org/2001/XMLSchema#string">procedure_occurrence.provider_id#108 AS Provider</ns1:omop_cdm_name>
    <ns1:omop_cdm_name rdf:datatype="http://www.w3.org/2001/XMLSchema#string">survey_conduct.provider_id#234 AS Provider</ns1:omop_cdm_name>
    <ns1:omop_cdm_name rdf:datatype="http://www.w3.org/2001/XMLSchema#string">visit_detail.provider_id#50 AS Provider</ns1:omop_cdm_name>
    <ns1:omop_cdm_name rdf:datatype="http://www.w3.org/2001/XMLSchema#string">visit_occurrence.provider_id#33 AS Provider</ns1:omop_cdm_name>
  </rdf:Description>
  <rdf:Description rdf:nodeID="nde7e53d44aa94269b5c0c83d6d8798ccb286">
    <rdf:type rdf:resource="http://www.w3.org/2002/07/owl#Restriction"/>
    <owl:allValuesFrom rdf:resource="http://www.w3.org/2001/XMLSchema#dateTime"/>
    <owl:onProperty rdf:resource="https://w3id.org/omop/ontology/datetime"/>
  </rdf:Description>
  <rdf:Description rdf:about="https://w3id.org/omop/ontology/value_as_number">
    <rdf:type rdf:resource="http://www.w3.org/2002/07/owl#DatatypeProperty"/>
    <rdf:type rdf:resource="http://www.w3.org/2002/07/owl#FunctionalProperty"/>
    <rdfs:comment xml:lang="en">(for Measurement:) This is the numerical value of the Result of the Measurement, if available. Note that measurements such as blood pressures will be split into their component parts i.e. one record for systolic, one record for diastolic.
If there is a negative value coming from the source, set the VALUE_AS_NUMBER to NULL, with the exception of the following Measurements (listed as LOINC codes):&lt;br&gt;-  [1925-7](https://athena.ohdsi.org/search-terms/terms/3003396) Base excess in Arterial blood by calculation - [1927-3](https://athena.ohdsi.org/search-terms/terms/3002032) Base excess in Venous blood by calculation - [8632-2](https://athena.ohdsi.org/search-terms/terms/3006277) QRS-Axis - [11555-0](https://athena.ohdsi.org/search-terms/terms/3012501) Base excess in Blood by calculation - [1926-5](https://athena.ohdsi.org/search-terms/terms/3003129) Base excess in Capillary blood by calculation - [28638-5](https://athena.ohdsi.org/search-terms/terms/3004959) Base excess in Arterial cord blood by calculation [28639-3](https://athena.ohdsi.org/search-terms/terms/3007435) Base excess in Venous cord blood by calculation</rdfs:comment>
    <rdfs:comment xml:lang="en">(for Observation:) This is the numerical value of the Result of the Observation, if applicable and available. It is not expected that all Observations will have numeric results, rather, this field is here to house values should they exist.</rdfs:comment>
    <rdfs:domain rdf:nodeID="nde7e53d44aa94269b5c0c83d6d8798ccb14"/>
    <rdfs:range rdf:resource="http://www.w3.org/2001/XMLSchema#decimal"/>
    <ns1:omop_cdm_name rdf:datatype="http://www.w3.org/2001/XMLSchema#string">measurement.value_as_number#137 AS float</ns1:omop_cdm_name>
    <ns1:omop_cdm_name rdf:datatype="http://www.w3.org/2001/XMLSchema#string">observation.value_as_number#155 AS float</ns1:omop_cdm_name>
  </rdf:Description>
  <rdf:Description rdf:about="https://w3id.org/omop/ontology/has_source_vocabulary">
    <rdf:type rdf:resource="http://www.w3.org/2002/07/owl#FunctionalProperty"/>
    <rdf:type rdf:resource="http://www.w3.org/2002/07/owl#ObjectProperty"/>
    <ns2:python_name rdf:datatype="http://www.w3.org/2001/XMLSchema#string">source_vocabulary</ns2:python_name>
    <rdfs:comment xml:lang="en">(for SourceToConceptMap:) A foreign key to the
VOCABULARY table defining the
vocabulary of the source code that
is being translated to a Standard
Concept.</rdfs:comment>
    <rdfs:domain rdf:resource="https://w3id.org/omop/ontology/SourceToConceptMap"/>
    <rdfs:range rdf:resource="https://w3id.org/omop/ontology/Vocabulary"/>
    <ns1:omop_cdm_name rdf:datatype="http://www.w3.org/2001/XMLSchema#string">source_to_concept_map.source_vocabulary_id#404 AS Vocabulary</ns1:omop_cdm_name>
  </rdf:Description>
  <rdf:Description rdf:nodeID="nde7e53d44aa94269b5c0c83d6d8798ccb239">
    <rdf:type rdf:resource="http://www.w3.org/2002/07/owl#Restriction"/>
    <owl:onProperty rdf:resource="https://w3id.org/omop/ontology/has_subject"/>
    <owl:someValuesFrom rdf:resource="https://w3id.org/omop/ontology/Concept"/>
  </rdf:Description>
  <rdf:Description rdf:about="https://w3id.org/omop/ontology/has_disease_status">
    <rdf:type rdf:resource="http://www.w3.org/2002/07/owl#FunctionalProperty"/>
    <rdf:type rdf:resource="http://www.w3.org/2002/07/owl#ObjectProperty"/>
    <ns2:python_name rdf:datatype="http://www.w3.org/2001/XMLSchema#string">disease_status</ns2:python_name>
    <rdfs:domain rdf:resource="https://w3id.org/omop/ontology/Specimen"/>
    <rdfs:range rdf:resource="https://w3id.org/omop/ontology/Concept"/>
    <ns1:omop_cdm_name rdf:datatype="http://www.w3.org/2001/XMLSchema#string">specimen.disease_status_concept_id#216 AS Concept</ns1:omop_cdm_name>
  </rdf:Description>
  <rdf:Description rdf:nodeID="nde7e53d44aa94269b5c0c83d6d8798ccb116">
    <rdf:first rdf:resource="https://w3id.org/omop/ontology/Concept"/>
    <rdf:rest rdf:nodeID="nde7e53d44aa94269b5c0c83d6d8798ccb117"/>
  </rdf:Description>
  <rdf:Description rdf:about="https://w3id.org/omop/ontology/has_cause_source">
    <rdf:type rdf:resource="http://www.w3.org/2002/07/owl#FunctionalProperty"/>
    <rdf:type rdf:resource="http://www.w3.org/2002/07/owl#ObjectProperty"/>
    <ns2:python_name rdf:datatype="http://www.w3.org/2001/XMLSchema#string">cause_source</ns2:python_name>
    <rdfs:domain rdf:resource="https://w3id.org/omop/ontology/Death"/>
    <rdfs:range rdf:resource="https://w3id.org/omop/ontology/Concept"/>
    <ns1:omop_cdm_name rdf:datatype="http://www.w3.org/2001/XMLSchema#string">death.cause_source_concept_id#176 AS Concept</ns1:omop_cdm_name>
  </rdf:Description>
  <rdf:Description rdf:about="https://w3id.org/omop/ontology/has_visit_detail">
    <rdf:type rdf:resource="http://www.w3.org/2002/07/owl#ObjectProperty"/>
    <ns2:python_name rdf:datatype="http://www.w3.org/2001/XMLSchema#string">visit_details</ns2:python_name>
    <rdfs:comment xml:lang="en">(reversed relation, for VisitDetail:) Use this field to link the VISIT_DETAIL record to its VISIT_OCCURRENCE.
Put the VISIT_OCCURRENCE_ID that subsumes the VISIT_DETAIL record here.</rdfs:comment>
    <rdfs:domain rdf:nodeID="nde7e53d44aa94269b5c0c83d6d8798ccb135"/>
    <rdfs:range rdf:resource="https://w3id.org/omop/ontology/VisitDetail"/>
    <ns1:omop_cdm_name rdf:datatype="http://www.w3.org/2001/XMLSchema#string">visit_detail.person_id#43 AS Person</ns1:omop_cdm_name>
    <ns1:omop_cdm_name rdf:datatype="http://www.w3.org/2001/XMLSchema#string">visit_detail.visit_occurrence_id#60 AS VisitOccurrence</ns1:omop_cdm_name>
  </rdf:Description>
  <rdf:Description rdf:nodeID="nde7e53d44aa94269b5c0c83d6d8798ccb307">
    <rdf:type rdf:resource="http://www.w3.org/2002/07/owl#Restriction"/>
    <owl:allValuesFrom rdf:resource="http://www.w3.org/2001/XMLSchema#integer"/>
    <owl:onProperty rdf:resource="https://w3id.org/omop/ontology/quantity"/>
  </rdf:Description>
  <rdf:Description rdf:nodeID="nde7e53d44aa94269b5c0c83d6d8798ccb153">
    <rdf:type rdf:resource="http://www.w3.org/2002/07/owl#Restriction"/>
    <owl:allValuesFrom rdf:resource="http://www.w3.org/2001/XMLSchema#integer"/>
    <owl:onProperty rdf:resource="https://w3id.org/omop/ontology/fact_id_1"/>
  </rdf:Description>
  <rdf:Description rdf:about="https://w3id.org/omop/ontology/term_modifiers">
    <rdf:type rdf:resource="http://www.w3.org/2002/07/owl#DatatypeProperty"/>
    <rdf:type rdf:resource="http://www.w3.org/2002/07/owl#FunctionalProperty"/>
    <rdfs:comment xml:lang="en">(for NoteNlp:) For the modifiers that are there, they would have to have these values:&lt;br&gt;&lt;br&gt;
- Negation = false
- Subject = patient
- Conditional = false
- Rule_out = false
- Uncertain = true or high or moderate or even low (could argue about low). Term_modifiers will concatenate all modifiers for different types of entities (conditions, drugs, labs etc) into one string. Lab values will be saved as one of the modifiers.</rdfs:comment>
    <rdfs:domain rdf:resource="https://w3id.org/omop/ontology/NoteNlp"/>
    <rdfs:range rdf:resource="http://www.w3.org/2001/XMLSchema#string"/>
    <ns1:omop_cdm_name rdf:datatype="http://www.w3.org/2001/XMLSchema#string">note_nlp.term_modifiers#206 AS str</ns1:omop_cdm_name>
  </rdf:Description>
  <rdf:Description rdf:nodeID="nde7e53d44aa94269b5c0c83d6d8798ccb186">
    <rdf:type rdf:resource="http://www.w3.org/2002/07/owl#Restriction"/>
    <owl:allValuesFrom rdf:resource="http://www.w3.org/2001/XMLSchema#dateTime"/>
    <owl:onProperty rdf:resource="https://w3id.org/omop/ontology/end_datetime"/>
  </rdf:Description>
  <rdf:Description rdf:about="https://w3id.org/omop/ontology/has_survey_source">
    <rdf:type rdf:resource="http://www.w3.org/2002/07/owl#FunctionalProperty"/>
    <rdf:type rdf:resource="http://www.w3.org/2002/07/owl#ObjectProperty"/>
    <ns2:python_name rdf:datatype="http://www.w3.org/2001/XMLSchema#string">survey_source</ns2:python_name>
    <rdfs:comment xml:lang="en">(for SurveyConduct:) If unavailable, set to 0.</rdfs:comment>
    <rdfs:domain rdf:resource="https://w3id.org/omop/ontology/SurveyConduct"/>
    <rdfs:range rdf:resource="https://w3id.org/omop/ontology/Concept"/>
    <ns1:omop_cdm_name rdf:datatype="http://www.w3.org/2001/XMLSchema#string">survey_conduct.survey_source_concept_id#244 AS Concept</ns1:omop_cdm_name>
  </rdf:Description>
  <rdf:Description rdf:nodeID="nde7e53d44aa94269b5c0c83d6d8798ccb502">
    <rdf:type rdf:resource="http://www.w3.org/2002/07/owl#Restriction"/>
    <owl:allValuesFrom rdf:resource="https://w3id.org/omop/ontology/Concept"/>
    <owl:onProperty rdf:resource="https://w3id.org/omop/ontology/has_drg"/>
  </rdf:Description>
  <rdf:Description rdf:about="https://w3id.org/omop/ontology/has_death">
    <rdf:type rdf:resource="http://www.w3.org/2002/07/owl#ObjectProperty"/>
    <ns2:python_name rdf:datatype="http://www.w3.org/2001/XMLSchema#string">deaths</ns2:python_name>
    <rdfs:domain rdf:resource="https://w3id.org/omop/ontology/Person"/>
    <rdfs:range rdf:resource="https://w3id.org/omop/ontology/Death"/>
    <ns1:omop_cdm_name rdf:datatype="http://www.w3.org/2001/XMLSchema#string">death.person_id#170 AS Person</ns1:omop_cdm_name>
  </rdf:Description>
  <rdf:Description rdf:about="https://w3id.org/omop/ontology/incurred_date">
    <rdf:type rdf:resource="http://www.w3.org/2002/07/owl#DatatypeProperty"/>
    <rdf:type rdf:resource="http://www.w3.org/2002/07/owl#FunctionalProperty"/>
    <rdfs:comment xml:lang="en">(for Cost:) The first date of service of the clinical event corresponding to the cost as in table capturing the information (e.g. date of visit, date of procedure, date of condition, date of drug etc).</rdfs:comment>
    <rdfs:domain rdf:resource="https://w3id.org/omop/ontology/Cost"/>
    <rdfs:range rdf:resource="http://www.w3.org/2001/XMLSchema#date"/>
    <ns1:omop_cdm_name rdf:datatype="http://www.w3.org/2001/XMLSchema#string">cost.incurred_date#317 AS date</ns1:omop_cdm_name>
  </rdf:Description>
  <rdf:Description rdf:nodeID="nde7e53d44aa94269b5c0c83d6d8798ccb145">
    <rdf:first rdf:resource="https://w3id.org/omop/ontology/DeviceExposure"/>
    <rdf:rest rdf:nodeID="nde7e53d44aa94269b5c0c83d6d8798ccb146"/>
  </rdf:Description>
  <rdf:Description rdf:nodeID="nde7e53d44aa94269b5c0c83d6d8798ccb485">
    <rdf:first rdf:resource="https://w3id.org/omop/ontology/ProcedureOccurrence"/>
    <rdf:rest rdf:nodeID="nde7e53d44aa94269b5c0c83d6d8798ccb486"/>
  </rdf:Description>
  <rdf:Description rdf:about="https://w3id.org/omop/ontology/cdm_etl_reference">
    <rdf:type rdf:resource="http://www.w3.org/2002/07/owl#DatatypeProperty"/>
    <rdf:type rdf:resource="http://www.w3.org/2002/07/owl#FunctionalProperty"/>
    <rdfs:comment xml:lang="en">(for CdmSource:) Put the link to the CDM version used.</rdfs:comment>
    <rdfs:domain rdf:resource="https://w3id.org/omop/ontology/CdmSource"/>
    <rdfs:range rdf:resource="http://www.w3.org/2001/XMLSchema#string"/>
    <ns1:omop_cdm_name rdf:datatype="http://www.w3.org/2001/XMLSchema#string">cdm_source.cdm_etl_reference#357 AS str</ns1:omop_cdm_name>
  </rdf:Description>
  <rdf:Description rdf:nodeID="nde7e53d44aa94269b5c0c83d6d8798ccb121">
    <rdf:first rdf:resource="https://w3id.org/omop/ontology/Cost"/>
    <rdf:rest rdf:resource="http://www.w3.org/1999/02/22-rdf-syntax-ns#nil"/>
  </rdf:Description>
  <rdf:Description rdf:nodeID="nde7e53d44aa94269b5c0c83d6d8798ccb368">
    <rdf:first rdf:resource="https://w3id.org/omop/ontology/Cost"/>
    <rdf:rest rdf:nodeID="nde7e53d44aa94269b5c0c83d6d8798ccb369"/>
  </rdf:Description>
  <rdf:Description rdf:nodeID="nde7e53d44aa94269b5c0c83d6d8798ccb96">
    <rdf:type rdf:resource="http://www.w3.org/2002/07/owl#Restriction"/>
    <owl:onProperty rdf:resource="https://w3id.org/omop/ontology/value"/>
    <owl:someValuesFrom rdf:resource="http://www.w3.org/2001/XMLSchema#decimal"/>
  </rdf:Description>
  <rdf:Description rdf:nodeID="nde7e53d44aa94269b5c0c83d6d8798ccb138">
    <rdf:type rdf:resource="http://www.w3.org/2002/07/owl#Class"/>
    <owl:unionOf rdf:nodeID="nde7e53d44aa94269b5c0c83d6d8798ccb139"/>
  </rdf:Description>
  <rdf:Description rdf:nodeID="nde7e53d44aa94269b5c0c83d6d8798ccb338">
    <rdf:type rdf:resource="http://www.w3.org/2002/07/owl#Restriction"/>
    <owl:allValuesFrom rdf:resource="http://www.w3.org/2001/XMLSchema#decimal"/>
    <owl:onProperty rdf:resource="https://w3id.org/omop/ontology/numerator_value"/>
  </rdf:Description>
  <rdf:Description rdf:nodeID="nde7e53d44aa94269b5c0c83d6d8798ccb144">
    <rdf:first rdf:resource="https://w3id.org/omop/ontology/ProcedureOccurrence"/>
    <rdf:rest rdf:nodeID="nde7e53d44aa94269b5c0c83d6d8798ccb145"/>
  </rdf:Description>
  <rdf:Description rdf:nodeID="nde7e53d44aa94269b5c0c83d6d8798ccb367">
    <rdf:first rdf:resource="https://w3id.org/omop/ontology/Observation"/>
    <rdf:rest rdf:nodeID="nde7e53d44aa94269b5c0c83d6d8798ccb368"/>
  </rdf:Description>
  <rdf:Description rdf:nodeID="nde7e53d44aa94269b5c0c83d6d8798ccb682">
    <rdf:type rdf:resource="http://www.w3.org/2002/07/owl#Restriction"/>
    <owl:allValuesFrom rdf:resource="http://www.w3.org/2001/XMLSchema#date"/>
    <owl:onProperty rdf:resource="https://w3id.org/omop/ontology/valid_start_date"/>
  </rdf:Description>
  <rdf:Description rdf:nodeID="nde7e53d44aa94269b5c0c83d6d8798ccb89">
    <rdf:type rdf:resource="http://www.w3.org/2002/07/owl#Restriction"/>
    <owl:allValuesFrom rdf:resource="https://w3id.org/omop/ontology/Concept"/>
    <owl:onProperty rdf:resource="https://w3id.org/omop/ontology/has_concept"/>
  </rdf:Description>
  <rdf:Description rdf:nodeID="nde7e53d44aa94269b5c0c83d6d8798ccb432">
    <rdf:type rdf:resource="http://www.w3.org/2002/07/owl#Restriction"/>
    <owl:allValuesFrom rdf:resource="https://w3id.org/omop/ontology/Concept"/>
    <owl:onProperty rdf:resource="https://w3id.org/omop/ontology/has_class"/>
  </rdf:Description>
  <rdf:Description rdf:about="https://w3id.org/omop/ontology/has_route">
    <rdf:type rdf:resource="http://www.w3.org/2002/07/owl#FunctionalProperty"/>
    <rdf:type rdf:resource="http://www.w3.org/2002/07/owl#ObjectProperty"/>
    <ns2:python_name rdf:datatype="http://www.w3.org/2001/XMLSchema#string">route</ns2:python_name>
    <rdfs:comment xml:lang="en">(for DrugExposure:) The standard CONCEPT_ID that the ROUTE_SOURCE_VALUE maps to in the route domain.</rdfs:comment>
    <rdfs:domain rdf:resource="https://w3id.org/omop/ontology/DrugExposure"/>
    <rdfs:range rdf:resource="https://w3id.org/omop/ontology/Concept"/>
    <ns1:omop_cdm_name rdf:datatype="http://www.w3.org/2001/XMLSchema#string">drug_exposure.route_concept_id#91 AS Concept</ns1:omop_cdm_name>
  </rdf:Description>
  <rdf:Description rdf:about="https://w3id.org/omop/ontology/has_subject">
    <rdf:type rdf:resource="http://www.w3.org/2002/07/owl#FunctionalProperty"/>
    <rdf:type rdf:resource="http://www.w3.org/2002/07/owl#ObjectProperty"/>
    <ns2:python_name rdf:datatype="http://www.w3.org/2001/XMLSchema#string">subject</ns2:python_name>
    <rdfs:comment xml:lang="en">(for CohortDefinition:) This field contains a Concept that represents the domain of the subjects that are members of the cohort (e.g., Person, Provider, Visit).</rdfs:comment>
    <rdfs:domain rdf:nodeID="nde7e53d44aa94269b5c0c83d6d8798ccb132"/>
    <ns1:omop_cdm_name rdf:datatype="http://www.w3.org/2001/XMLSchema#string">cohort.subject_id#424 AS Thing</ns1:omop_cdm_name>
    <ns1:omop_cdm_name rdf:datatype="http://www.w3.org/2001/XMLSchema#string">cohort_definition.subject_concept_id#432 AS Concept</ns1:omop_cdm_name>
  </rdf:Description>
  <rdf:Description rdf:nodeID="nde7e53d44aa94269b5c0c83d6d8798ccb569">
    <rdf:first rdf:resource="https://w3id.org/omop/ontology/Metadata"/>
    <rdf:rest rdf:nodeID="nde7e53d44aa94269b5c0c83d6d8798ccb570"/>
  </rdf:Description>
  <rdf:Description rdf:about="https://w3id.org/omop/ontology/has_descendant">
    <rdf:type rdf:resource="http://www.w3.org/2002/07/owl#FunctionalProperty"/>
    <rdf:type rdf:resource="http://www.w3.org/2002/07/owl#ObjectProperty"/>
    <ns2:python_name rdf:datatype="http://www.w3.org/2001/XMLSchema#string">descendant</ns2:python_name>
    <rdfs:comment xml:lang="en">(for ConceptAncestor:) The Concept Id for the lower-level concept
that forms the descendant in the
relationship.</rdfs:comment>
    <rdfs:domain rdf:resource="https://w3id.org/omop/ontology/ConceptAncestor"/>
    <rdfs:range rdf:resource="https://w3id.org/omop/ontology/Concept"/>
    <ns1:omop_cdm_name rdf:datatype="http://www.w3.org/2001/XMLSchema#string">concept_ancestor.descendant_concept_id#399 AS Concept</ns1:omop_cdm_name>
  </rdf:Description>
  <rdf:Description rdf:about="https://w3id.org/omop/ontology/has_measurement">
    <rdf:type rdf:resource="http://www.w3.org/2002/07/owl#ObjectProperty"/>
    <ns2:python_name rdf:datatype="http://www.w3.org/2001/XMLSchema#string">measurements</ns2:python_name>
    <rdfs:comment xml:lang="en">(reversed relation, for Measurement:) The PERSON_ID of the PERSON for whom the measurement is recorded. This may be a system generated code.</rdfs:comment>
    <rdfs:comment xml:lang="en">(reversed relation, for Measurement:) The VISIT_DETAIL record during which the Measurement occurred. For example, if the Person was in the ICU at the time the VISIT_OCCURRENCE record would reflect the overall hospital stay and the VISIT_DETAIL record would reflect the ICU stay during the hospital visit.
Same rules apply as for the VISIT_OCCURRENCE_ID.</rdfs:comment>
    <rdfs:comment xml:lang="en">(reversed relation, for Measurement:) The visit during which the Measurement occurred.
Depending on the structure of the source data, this may have to be determined based on dates. If a MEASUREMENT_DATE occurs within the start and end date of a Visit it is a valid ETL choice to choose the VISIT_OCCURRENCE_ID from the visit that subsumes it, even if not explicitly stated in the data. While not required, an attempt should be made to locate the VISIT_OCCURRENCE_ID of the measurement record. If a measurement is related to a visit explicitly in the source data, it is possible that the result date of the Measurement falls outside of the bounds of the Visit dates.</rdfs:comment>
    <rdfs:domain rdf:nodeID="nde7e53d44aa94269b5c0c83d6d8798ccb51"/>
    <rdfs:range rdf:resource="https://w3id.org/omop/ontology/Measurement"/>
    <ns1:omop_cdm_name rdf:datatype="http://www.w3.org/2001/XMLSchema#string">measurement.person_id#130 AS Person</ns1:omop_cdm_name>
    <ns1:omop_cdm_name rdf:datatype="http://www.w3.org/2001/XMLSchema#string">measurement.visit_detail_id#144 AS VisitDetail</ns1:omop_cdm_name>
    <ns1:omop_cdm_name rdf:datatype="http://www.w3.org/2001/XMLSchema#string">measurement.visit_occurrence_id#143 AS VisitOccurrence</ns1:omop_cdm_name>
  </rdf:Description>
  <rdf:Description rdf:nodeID="nde7e53d44aa94269b5c0c83d6d8798ccb509">
    <rdf:type rdf:resource="http://www.w3.org/2002/07/owl#Restriction"/>
    <owl:allValuesFrom rdf:resource="http://www.w3.org/2001/XMLSchema#string"/>
    <owl:onProperty rdf:resource="https://w3id.org/omop/ontology/source_value"/>
  </rdf:Description>
  <rdf:Description rdf:about="https://w3id.org/omop/ontology/time">
    <rdf:type rdf:resource="http://www.w3.org/2002/07/owl#DatatypeProperty"/>
    <rdf:type rdf:resource="http://www.w3.org/2002/07/owl#FunctionalProperty"/>
    <rdfs:comment xml:lang="en">(for Measurement:) This is present for backwards compatibility and will be deprecated in an upcoming version.</rdfs:comment>
    <rdfs:domain rdf:resource="https://w3id.org/omop/ontology/Measurement"/>
    <rdfs:range rdf:resource="http://www.w3.org/2001/XMLSchema#string"/>
    <ns1:omop_cdm_name rdf:datatype="http://www.w3.org/2001/XMLSchema#string">measurement.measurement_time#134 AS str</ns1:omop_cdm_name>
  </rdf:Description>
  <rdf:Description rdf:nodeID="nde7e53d44aa94269b5c0c83d6d8798ccb97">
    <rdf:type rdf:resource="http://www.w3.org/2002/07/owl#Restriction"/>
    <owl:onProperty rdf:resource="https://w3id.org/omop/ontology/has_unit"/>
    <owl:someValuesFrom rdf:resource="https://w3id.org/omop/ontology/Concept"/>
  </rdf:Description>
  <rdf:Description rdf:nodeID="nde7e53d44aa94269b5c0c83d6d8798ccb487">
    <rdf:first rdf:resource="https://w3id.org/omop/ontology/Observation"/>
    <rdf:rest rdf:nodeID="nde7e53d44aa94269b5c0c83d6d8798ccb488"/>
  </rdf:Description>
  <rdf:Description rdf:nodeID="nde7e53d44aa94269b5c0c83d6d8798ccb646">
    <rdf:type rdf:resource="http://www.w3.org/2002/07/owl#Restriction"/>
    <owl:allValuesFrom rdf:resource="https://w3id.org/omop/ontology/Provider"/>
    <owl:onProperty rdf:resource="https://w3id.org/omop/ontology/has_provider"/>
  </rdf:Description>
  <rdf:Description rdf:about="https://w3id.org/omop/ontology/ClinicalElement">
    <rdf:type rdf:resource="http://www.w3.org/2002/07/owl#Class"/>
    <rdfs:subClassOf rdf:resource="https://w3id.org/omop/ontology/OmopCDMThing"/>
  </rdf:Description>
  <rdf:Description rdf:nodeID="nde7e53d44aa94269b5c0c83d6d8798ccb437">
    <rdf:type rdf:resource="http://www.w3.org/2002/07/owl#Restriction"/>
    <owl:allValuesFrom rdf:resource="https://w3id.org/omop/ontology/Concept"/>
    <owl:onProperty rdf:resource="https://w3id.org/omop/ontology/has_concept"/>
  </rdf:Description>
  <rdf:Description rdf:nodeID="nde7e53d44aa94269b5c0c83d6d8798ccb38">
    <rdf:first rdf:resource="https://w3id.org/omop/ontology/VisitDetail"/>
    <rdf:rest rdf:resource="http://www.w3.org/1999/02/22-rdf-syntax-ns#nil"/>
  </rdf:Description>
  <rdf:Description rdf:about="https://w3id.org/omop/ontology/system">
    <rdf:type rdf:resource="http://www.w3.org/2002/07/owl#DatatypeProperty"/>
    <rdf:type rdf:resource="http://www.w3.org/2002/07/owl#FunctionalProperty"/>
    <rdfs:comment xml:lang="en">(for NoteNlp:) Name and version of the NLP system that extracted the term. Useful for data provenance.</rdfs:comment>
    <rdfs:domain rdf:resource="https://w3id.org/omop/ontology/NoteNlp"/>
    <rdfs:range rdf:resource="http://www.w3.org/2001/XMLSchema#string"/>
    <ns1:omop_cdm_name rdf:datatype="http://www.w3.org/2001/XMLSchema#string">note_nlp.nlp_system#201 AS str</ns1:omop_cdm_name>
  </rdf:Description>
  <rdf:Description rdf:nodeID="nde7e53d44aa94269b5c0c83d6d8798ccb513">
    <rdf:type rdf:resource="http://www.w3.org/2002/07/owl#Restriction"/>
    <owl:allValuesFrom rdf:resource="https://w3id.org/omop/ontology/Concept"/>
    <owl:onProperty rdf:resource="https://w3id.org/omop/ontology/has_type"/>
  </rdf:Description>
  <rdf:Description rdf:about="https://w3id.org/omop/ontology/term_exists">
    <rdf:type rdf:resource="http://www.w3.org/2002/07/owl#DatatypeProperty"/>
    <rdf:type rdf:resource="http://www.w3.org/2002/07/owl#FunctionalProperty"/>
    <rdfs:comment xml:lang="en">(for NoteNlp:) Term_exists is defined as a flag that indicates if the patient actually has or had the condition. Any of the following modifiers would make Term_exists false:
Negation = true
Subject = [anything other than the patient]
Conditional = true/li&gt;
Rule_out = true
Uncertain = very low certainty or any lower certainties
A complete lack of modifiers would make Term_exists true.
</rdfs:comment>
    <rdfs:domain rdf:resource="https://w3id.org/omop/ontology/NoteNlp"/>
    <rdfs:range rdf:resource="http://www.w3.org/2001/XMLSchema#string"/>
    <ns1:omop_cdm_name rdf:datatype="http://www.w3.org/2001/XMLSchema#string">note_nlp.term_exists#204 AS str</ns1:omop_cdm_name>
  </rdf:Description>
  <rdf:Description rdf:nodeID="nde7e53d44aa94269b5c0c83d6d8798ccb597">
    <rdf:type rdf:resource="http://www.w3.org/2002/07/owl#Restriction"/>
    <owl:allValuesFrom rdf:resource="http://www.w3.org/2001/XMLSchema#string"/>
    <owl:onProperty rdf:resource="https://w3id.org/omop/ontology/collection_method_source_value"/>
  </rdf:Description>
  <rdf:Description rdf:nodeID="nde7e53d44aa94269b5c0c83d6d8798ccb592">
    <rdf:type rdf:resource="http://www.w3.org/2002/07/owl#Restriction"/>
    <owl:allValuesFrom rdf:resource="http://www.w3.org/2001/XMLSchema#string"/>
    <owl:onProperty rdf:resource="https://w3id.org/omop/ontology/timing_source_value"/>
  </rdf:Description>
  <rdf:Description rdf:about="https://w3id.org/omop/ontology/source_value">
    <rdf:type rdf:resource="http://www.w3.org/2002/07/owl#DatatypeProperty"/>
    <rdf:type rdf:resource="http://www.w3.org/2002/07/owl#FunctionalProperty"/>
    <rdfs:comment xml:lang="en">(for CareSite:) The identifier of the care_site as it appears in the source data. This could be an identifier separate from the name of the care_site.</rdfs:comment>
    <rdfs:comment xml:lang="en">(for ConditionOccurrence:) This field houses the verbatim value from the source data representing the condition that occurred. For example, this could be an ICD10 or Read code.
This code is mapped to a Standard Condition Concept in the Standardized Vocabularies and the original code is stored here for reference.</rdfs:comment>
    <rdfs:comment xml:lang="en">(for Cost:) The source value for the cost as it appears in the source data</rdfs:comment>
    <rdfs:comment xml:lang="en">(for DeviceExposure:) This field houses the verbatim value from the source data representing the device exposure that occurred. For example, this could be an NDC or Gemscript code.
This code is mapped to a Standard Device Concept in the Standardized Vocabularies and the original code is stored here for reference.</rdfs:comment>
    <rdfs:comment xml:lang="en">(for DrugExposure:) This field houses the verbatim value from the source data representing the drug exposure that occurred. For example, this could be an NDC or Gemscript code.
This code is mapped to a Standard Drug Concept in the Standardized Vocabularies and the original code is stored here for reference.</rdfs:comment>
    <rdfs:comment xml:lang="en">(for Location:) Put the verbatim value for the location here, as it shows up in the source.</rdfs:comment>
    <rdfs:comment xml:lang="en">(for Measurement:) This field houses the verbatim value from the source data representing the Measurement that occurred. For example, this could be an ICD10 or Read code.
This code is mapped to a Standard Measurement Concept in the Standardized Vocabularies and the original code is stored here for reference.</rdfs:comment>
    <rdfs:comment xml:lang="en">(for Note:) The source value mapped to the NOTE_CLASS_CONCEPT_ID.</rdfs:comment>
    <rdfs:comment xml:lang="en">(for Observation:) This field houses the verbatim value from the source data representing the Observation that occurred. For example, this could be an ICD10 or Read code.
This code is mapped to a Standard Concept in the Standardized Vocabularies and the original code is stored here for reference.</rdfs:comment>
    <rdfs:comment xml:lang="en">(for Person:) Use this field to link back to persons in the source data. This is typically used for error checking of ETL logic.
Some use cases require the ability to link back to persons in the source data. This field allows for the storing of the person value as it appears in the source. This field is not required but strongly recommended.</rdfs:comment>
    <rdfs:comment xml:lang="en">(for ProcedureOccurrence:) This field houses the verbatim value from the source data representing the procedure that occurred. For example, this could be an CPT4 or OPCS4 code.
Use this value to look up the source concept id and then map the source concept id to a standard concept id.</rdfs:comment>
    <rdfs:comment xml:lang="en">(for Provider:) Use this field to link back to providers in the source data. This is typically used for error checking of ETL logic.
Some use cases require the ability to link back to providers in the source data. This field allows for the storing of the provider identifier as it appears in the source.</rdfs:comment>
    <rdfs:comment xml:lang="en">(for VisitDetail:) This field houses the verbatim value from the source data representing the kind of visit detail that took place (inpatient, outpatient, emergency, etc.)
If there is information about the kind of visit detail in the source data that value should be stored here. If a visit is an amalgamation of visits from the source then use a hierarchy to choose the VISIT_DETAIL_SOURCE_VALUE, such as IP -&gt; ER-&gt; OP. This should line up with the logic chosen to determine how visits are created.</rdfs:comment>
    <rdfs:comment xml:lang="en">(for VisitOccurrence:) This field houses the verbatim value from the source data representing the kind of visit that took place (inpatient, outpatient, emergency, etc.)
If there is information about the kind of visit in the source data that value should be stored here. If a visit is an amalgamation of visits from the source then use a hierarchy to choose the visit source value, such as IP -&gt; ER-&gt; OP. This should line up with the logic chosen to determine how visits are created.</rdfs:comment>
    <rdfs:domain rdf:nodeID="nde7e53d44aa94269b5c0c83d6d8798ccb360"/>
    <rdfs:range rdf:resource="http://www.w3.org/2001/XMLSchema#string"/>
    <ns1:omop_cdm_name rdf:datatype="http://www.w3.org/2001/XMLSchema#string">care_site.care_site_source_value#271 AS str</ns1:omop_cdm_name>
    <ns1:omop_cdm_name rdf:datatype="http://www.w3.org/2001/XMLSchema#string">condition_occurrence.condition_source_value#74 AS str</ns1:omop_cdm_name>
    <ns1:omop_cdm_name rdf:datatype="http://www.w3.org/2001/XMLSchema#string">cost.cost_source_value#314 AS str</ns1:omop_cdm_name>
    <ns1:omop_cdm_name rdf:datatype="http://www.w3.org/2001/XMLSchema#string">device_exposure.device_source_value#127 AS str</ns1:omop_cdm_name>
    <ns1:omop_cdm_name rdf:datatype="http://www.w3.org/2001/XMLSchema#string">drug_exposure.drug_source_value#96 AS str</ns1:omop_cdm_name>
    <ns1:omop_cdm_name rdf:datatype="http://www.w3.org/2001/XMLSchema#string">location.location_source_value#258 AS str</ns1:omop_cdm_name>
    <ns1:omop_cdm_name rdf:datatype="http://www.w3.org/2001/XMLSchema#string">measurement.measurement_source_value#145 AS str</ns1:omop_cdm_name>
    <ns1:omop_cdm_name rdf:datatype="http://www.w3.org/2001/XMLSchema#string">note.note_source_value#192 AS str</ns1:omop_cdm_name>
    <ns1:omop_cdm_name rdf:datatype="http://www.w3.org/2001/XMLSchema#string">observation.observation_source_value#163 AS str</ns1:omop_cdm_name>
    <ns1:omop_cdm_name rdf:datatype="http://www.w3.org/2001/XMLSchema#string">person.person_source_value#13 AS str</ns1:omop_cdm_name>
    <ns1:omop_cdm_name rdf:datatype="http://www.w3.org/2001/XMLSchema#string">procedure_occurrence.procedure_source_value#111 AS str</ns1:omop_cdm_name>
    <ns1:omop_cdm_name rdf:datatype="http://www.w3.org/2001/XMLSchema#string">provider.provider_source_value#281 AS str</ns1:omop_cdm_name>
    <ns1:omop_cdm_name rdf:datatype="http://www.w3.org/2001/XMLSchema#string">specimen.specimen_source_value#218 AS str</ns1:omop_cdm_name>
    <ns1:omop_cdm_name rdf:datatype="http://www.w3.org/2001/XMLSchema#string">visit_detail.visit_detail_source_value#52 AS str</ns1:omop_cdm_name>
    <ns1:omop_cdm_name rdf:datatype="http://www.w3.org/2001/XMLSchema#string">visit_occurrence.visit_source_value#35 AS str</ns1:omop_cdm_name>
  </rdf:Description>
  <rdf:Description rdf:nodeID="nde7e53d44aa94269b5c0c83d6d8798ccb27">
    <rdf:type rdf:resource="http://www.w3.org/2002/07/owl#Restriction"/>
    <owl:onProperty rdf:nodeID="nde7e53d44aa94269b5c0c83d6d8798ccb28"/>
    <owl:someValuesFrom rdf:resource="https://w3id.org/omop/ontology/Person"/>
  </rdf:Description>
  <rdf:Description rdf:nodeID="nde7e53d44aa94269b5c0c83d6d8798ccb532">
    <rdf:type rdf:resource="http://www.w3.org/2002/07/owl#Restriction"/>
    <owl:onProperty rdf:resource="https://w3id.org/omop/ontology/has_payer_source"/>
    <owl:someValuesFrom rdf:resource="https://w3id.org/omop/ontology/Concept"/>
  </rdf:Description>
  <rdf:Description rdf:nodeID="nde7e53d44aa94269b5c0c83d6d8798ccb22">
    <rdf:type rdf:resource="http://www.w3.org/2002/07/owl#Restriction"/>
    <owl:allValuesFrom rdf:resource="http://www.w3.org/2001/XMLSchema#string"/>
    <owl:onProperty rdf:resource="https://w3id.org/omop/ontology/name"/>
  </rdf:Description>
  <rdf:Description rdf:nodeID="nde7e53d44aa94269b5c0c83d6d8798ccb237">
    <rdf:type rdf:resource="http://www.w3.org/2002/07/owl#Restriction"/>
    <owl:allValuesFrom rdf:resource="http://www.w3.org/2001/XMLSchema#string"/>
    <owl:onProperty rdf:resource="https://w3id.org/omop/ontology/name"/>
  </rdf:Description>
  <rdf:Description rdf:about="https://w3id.org/omop/ontology/has_note">
    <rdf:type rdf:resource="http://www.w3.org/2002/07/owl#ObjectProperty"/>
    <ns2:python_name rdf:datatype="http://www.w3.org/2001/XMLSchema#string">notes</ns2:python_name>
    <rdfs:comment xml:lang="en">(reversed relation, for Note:) The Visit Detail during which the note was written.</rdfs:comment>
    <rdfs:comment xml:lang="en">(reversed relation, for Note:) The Visit during which the note was written.</rdfs:comment>
    <rdfs:domain rdf:nodeID="nde7e53d44aa94269b5c0c83d6d8798ccb54"/>
    <rdfs:range rdf:resource="https://w3id.org/omop/ontology/Note"/>
    <ns1:omop_cdm_name rdf:datatype="http://www.w3.org/2001/XMLSchema#string">note.person_id#178 AS Person</ns1:omop_cdm_name>
    <ns1:omop_cdm_name rdf:datatype="http://www.w3.org/2001/XMLSchema#string">note.visit_detail_id#191 AS VisitDetail</ns1:omop_cdm_name>
    <ns1:omop_cdm_name rdf:datatype="http://www.w3.org/2001/XMLSchema#string">note.visit_occurrence_id#190 AS VisitOccurrence</ns1:omop_cdm_name>
  </rdf:Description>
  <rdf:Description rdf:nodeID="nde7e53d44aa94269b5c0c83d6d8798ccb260">
    <rdf:type rdf:resource="http://www.w3.org/2002/07/owl#Restriction"/>
    <owl:allValuesFrom rdf:resource="https://w3id.org/omop/ontology/Vocabulary"/>
    <owl:onProperty rdf:resource="https://w3id.org/omop/ontology/has_target_vocabulary"/>
  </rdf:Description>
  <rdf:Description rdf:nodeID="nde7e53d44aa94269b5c0c83d6d8798ccb525">
    <owl:inverseOf rdf:resource="https://w3id.org/omop/ontology/has_observation"/>
  </rdf:Description>
  <rdf:Description rdf:about="https://w3id.org/omop/ontology/end_date">
    <rdf:type rdf:resource="http://www.w3.org/2002/07/owl#DatatypeProperty"/>
    <rdf:type rdf:resource="http://www.w3.org/2002/07/owl#FunctionalProperty"/>
    <rdfs:comment xml:lang="en">(for ConditionOccurrence:) Use this date to determine the end date of the condition
Most often data sources do not have the idea of a start date for a condition. Rather, if a source only has one date associated with a condition record it is acceptable to use that date for both the CONDITION_START_DATE and the CONDITION_END_DATE.</rdfs:comment>
    <rdfs:comment xml:lang="en">(for DeviceExposure:) The DEVICE_EXPOSURE_END_DATE denotes the day the device exposure ended for the patient, if given.
Put the end date or discontinuation date as it appears from the source data or leave blank if unavailable.</rdfs:comment>
    <rdfs:comment xml:lang="en">(for DrugExposure:) The DRUG_EXPOSURE_END_DATE denotes the day the drug exposure ended for the patient.
If this information is not explicitly available in the data, infer the end date using the following methods:/n/n 1. Start first with duration or days supply using the calculation drug start date + days supply -1 day. 2. Use quantity divided by daily dose that you may obtain from the sig or a source field (or assumed daily dose of 1) for solid, indivisibile, drug products. If quantity represents ingredient amount, quantity divided by daily dose * concentration (from drug_strength) drug concept id tells you the dose form. 3. If it is an administration record, set drug end date equal to drug start date. If the record is a written prescription then set end date to start date + 29. If the record is a mail-order prescription set end date to start date + 89. The end date must be equal to or greater than the start date. Ibuprofen 20mg/mL oral solution concept tells us this is oral solution. Calculate duration as quantity (200 example) * daily dose (5mL) /concentration (20mg/mL) 200*5/20 = 50 days. [Examples by dose form](https://ohdsi.github.io/CommonDataModel/drug_dose.html)</rdfs:comment>
    <rdfs:comment xml:lang="en">(for LocationHistory:) The date the relationship ended</rdfs:comment>
    <rdfs:comment xml:lang="en">(for ObservationPeriod:) Use this date to determine the end date of the period for which we can assume that all events for a Person are recorded.
It is often the case that the idea of Observation Periods does not exist in source data. In those cases, the observation_period_end_date can be inferred as the last Event date available for the Person. In insurance claim data, the Observation Period can be considered as the time period the Person is enrolled with a payer.</rdfs:comment>
    <rdfs:comment xml:lang="en">(for PayerPlanPeriod:) End date of Plan coverage.</rdfs:comment>
    <rdfs:comment xml:lang="en">(for VisitDetail:) This the end date of the patient-provider interaction.
Visit Detail end dates are mandatory. If end dates are not provided in the source there are three ways in which to derive them:&lt;br&gt;
- Outpatient Visit Detail: visit_detail_end_datetime = visit_detail_start_datetime
- Emergency Room Visit Detail: visit_detail_end_datetime = visit_detail_start_datetime
- Inpatient Visit Detail: Usually there is information about discharge. If not, you should be able to derive the end date from the sudden decline of activity or from the absence of inpatient procedures/drugs.
- Non-hospital institution Visit Details: Particularly for claims data, if end dates are not provided assume the visit is for the duration of month that it occurs.&lt;br&gt;
For Inpatient Visit Details ongoing at the date of ETL, put date of processing the data into visit_detai_end_datetime and visit_detail_type_concept_id with 32220 "Still patient" to identify the visit as incomplete.
All other Visits Details: visit_detail_end_datetime = visit_detail_start_datetime.</rdfs:comment>
    <rdfs:comment xml:lang="en">(for VisitOccurrence:) For inpatient visits the end date is typically the discharge date.
Visit end dates are mandatory. If end dates are not provided in the source there are three ways in which to derive them:
Outpatient Visit: visit_end_datetime = visit_start_datetime
Emergency Room Visit: visit_end_datetime = visit_start_datetime
Inpatient Visit: Usually there is information about discharge. If not, you should be able to derive the end date from the sudden decline of activity or from the absence of inpatient procedures/drugs.
Non-hospital institution Visits: Particularly for claims data, if end dates are not provided assume the visit is for the duration of month that it occurs.
For Inpatient Visits ongoing at the date of ETL, put date of processing the data into visit_end_datetime and visit_type_concept_id with 32220 "Still patient" to identify the visit as incomplete.
All other Visits: visit_end_datetime = visit_start_datetime. If this is a one-day visit the end date should match the start date.</rdfs:comment>
    <rdfs:domain rdf:resource="https://w3id.org/omop/ontology/DateDuration"/>
    <rdfs:range rdf:resource="http://www.w3.org/2001/XMLSchema#date"/>
    <ns1:omop_cdm_name rdf:datatype="http://www.w3.org/2001/XMLSchema#string">cohort.cohort_end_date#426 AS date</ns1:omop_cdm_name>
    <ns1:omop_cdm_name rdf:datatype="http://www.w3.org/2001/XMLSchema#string">condition_occurrence.condition_end_date#66 AS date</ns1:omop_cdm_name>
    <ns1:omop_cdm_name rdf:datatype="http://www.w3.org/2001/XMLSchema#string">device_exposure.device_exposure_end_date#119 AS date</ns1:omop_cdm_name>
    <ns1:omop_cdm_name rdf:datatype="http://www.w3.org/2001/XMLSchema#string">drug_exposure.drug_exposure_end_date#82 AS date</ns1:omop_cdm_name>
    <ns1:omop_cdm_name rdf:datatype="http://www.w3.org/2001/XMLSchema#string">location_history.end_date#266 AS date</ns1:omop_cdm_name>
    <ns1:omop_cdm_name rdf:datatype="http://www.w3.org/2001/XMLSchema#string">observation_period.observation_period_end_date#23 AS date</ns1:omop_cdm_name>
    <ns1:omop_cdm_name rdf:datatype="http://www.w3.org/2001/XMLSchema#string">payer_plan_period.payer_plan_period_end_date#290 AS date</ns1:omop_cdm_name>
    <ns1:omop_cdm_name rdf:datatype="http://www.w3.org/2001/XMLSchema#string">visit_detail.visit_detail_end_date#47 AS date</ns1:omop_cdm_name>
    <ns1:omop_cdm_name rdf:datatype="http://www.w3.org/2001/XMLSchema#string">visit_occurrence.visit_end_date#30 AS date</ns1:omop_cdm_name>
  </rdf:Description>
  <rdf:Description rdf:nodeID="nde7e53d44aa94269b5c0c83d6d8798ccb141">
    <rdf:first rdf:resource="https://w3id.org/omop/ontology/SourceToConceptMap"/>
    <rdf:rest rdf:nodeID="nde7e53d44aa94269b5c0c83d6d8798ccb142"/>
  </rdf:Description>
  <rdf:Description rdf:nodeID="nde7e53d44aa94269b5c0c83d6d8798ccb250">
    <rdf:type rdf:resource="http://www.w3.org/2002/07/owl#Restriction"/>
    <owl:onProperty rdf:resource="https://w3id.org/omop/ontology/has_source_vocabulary"/>
    <owl:someValuesFrom rdf:resource="https://w3id.org/omop/ontology/Vocabulary"/>
  </rdf:Description>
  <rdf:Description rdf:about="https://w3id.org/omop/ontology/has_validated_survey">
    <rdf:type rdf:resource="http://www.w3.org/2002/07/owl#FunctionalProperty"/>
    <rdf:type rdf:resource="http://www.w3.org/2002/07/owl#ObjectProperty"/>
    <ns2:python_name rdf:datatype="http://www.w3.org/2001/XMLSchema#string">validated_survey</ns2:python_name>
    <rdfs:comment xml:lang="en">(for SurveyConduct:) If unavailable, set to 0.</rdfs:comment>
    <rdfs:domain rdf:resource="https://w3id.org/omop/ontology/SurveyConduct"/>
    <rdfs:range rdf:resource="https://w3id.org/omop/ontology/Concept"/>
    <ns1:omop_cdm_name rdf:datatype="http://www.w3.org/2001/XMLSchema#string">survey_conduct.validated_survey_concept_id#246 AS Concept</ns1:omop_cdm_name>
  </rdf:Description>
  <rdf:Description rdf:nodeID="nde7e53d44aa94269b5c0c83d6d8798ccb657">
    <rdf:type rdf:resource="http://www.w3.org/2002/07/owl#Restriction"/>
    <owl:allValuesFrom rdf:resource="https://w3id.org/omop/ontology/SurveyConduct"/>
    <owl:onProperty rdf:resource="https://w3id.org/omop/ontology/has_survey_conduct"/>
  </rdf:Description>
  <rdf:Description rdf:nodeID="nde7e53d44aa94269b5c0c83d6d8798ccb546">
    <rdf:type rdf:resource="http://www.w3.org/2002/07/owl#Restriction"/>
    <owl:allValuesFrom rdf:resource="https://w3id.org/omop/ontology/Concept"/>
    <owl:onProperty rdf:resource="https://w3id.org/omop/ontology/has_sponsor"/>
  </rdf:Description>
  <rdf:Description rdf:nodeID="nde7e53d44aa94269b5c0c83d6d8798ccb395">
    <rdf:type rdf:resource="http://www.w3.org/2002/07/owl#Restriction"/>
    <owl:onProperty rdf:resource="https://w3id.org/omop/ontology/has_concept"/>
    <owl:someValuesFrom rdf:resource="https://w3id.org/omop/ontology/Concept"/>
  </rdf:Description>
  <rdf:Description rdf:nodeID="nde7e53d44aa94269b5c0c83d6d8798ccb521">
    <rdf:type rdf:resource="http://www.w3.org/2002/07/owl#Restriction"/>
    <owl:allValuesFrom rdf:resource="https://w3id.org/omop/ontology/Concept"/>
    <owl:onProperty rdf:resource="https://w3id.org/omop/ontology/has_qualifier"/>
  </rdf:Description>
  <rdf:Description rdf:nodeID="nde7e53d44aa94269b5c0c83d6d8798ccb180">
    <rdf:type rdf:resource="http://www.w3.org/2002/07/owl#Restriction"/>
    <owl:allValuesFrom rdf:resource="http://www.w3.org/2001/XMLSchema#string"/>
    <owl:onProperty rdf:resource="https://w3id.org/omop/ontology/invalid_reason"/>
  </rdf:Description>
  <rdf:Description rdf:nodeID="nde7e53d44aa94269b5c0c83d6d8798ccb183">
    <rdf:type rdf:resource="http://www.w3.org/2002/07/owl#Restriction"/>
    <owl:allValuesFrom rdf:resource="http://www.w3.org/2001/XMLSchema#date"/>
    <owl:onProperty rdf:resource="https://w3id.org/omop/ontology/valid_end_date"/>
  </rdf:Description>
  <rdf:Description rdf:nodeID="nde7e53d44aa94269b5c0c83d6d8798ccb32">
    <rdf:type rdf:resource="http://www.w3.org/2002/07/owl#Restriction"/>
    <owl:allValuesFrom rdf:resource="https://w3id.org/omop/ontology/Concept"/>
    <owl:onProperty rdf:resource="https://w3id.org/omop/ontology/has_period_type"/>
  </rdf:Description>
  <rdf:Description rdf:nodeID="nde7e53d44aa94269b5c0c83d6d8798ccb162">
    <rdf:type rdf:resource="http://www.w3.org/2002/07/owl#Restriction"/>
    <owl:onProperty rdf:resource="https://w3id.org/omop/ontology/name"/>
    <owl:someValuesFrom rdf:resource="http://www.w3.org/2001/XMLSchema#string"/>
  </rdf:Description>
  <rdf:Description rdf:nodeID="nde7e53d44aa94269b5c0c83d6d8798ccb420">
    <rdf:type rdf:resource="http://www.w3.org/2002/07/owl#Restriction"/>
    <owl:allValuesFrom rdf:resource="http://www.w3.org/2002/07/owl#Thing"/>
    <owl:onProperty rdf:resource="https://w3id.org/omop/ontology/has_event"/>
  </rdf:Description>
  <rdf:Description rdf:nodeID="nde7e53d44aa94269b5c0c83d6d8798ccb518">
    <rdf:type rdf:resource="http://www.w3.org/2002/07/owl#Restriction"/>
    <owl:allValuesFrom rdf:resource="https://w3id.org/omop/ontology/Concept"/>
    <owl:onProperty rdf:resource="https://w3id.org/omop/ontology/has_obs_event_field"/>
  </rdf:Description>
  <rdf:Description rdf:nodeID="nde7e53d44aa94269b5c0c83d6d8798ccb442">
    <rdf:type rdf:resource="http://www.w3.org/2002/07/owl#Restriction"/>
    <owl:onProperty rdf:resource="https://w3id.org/omop/ontology/has_type"/>
    <owl:someValuesFrom rdf:resource="https://w3id.org/omop/ontology/Concept"/>
  </rdf:Description>
  <rdf:Description rdf:nodeID="nde7e53d44aa94269b5c0c83d6d8798ccb107">
    <rdf:type rdf:resource="http://www.w3.org/2002/07/owl#Restriction"/>
    <owl:allValuesFrom rdf:resource="https://w3id.org/omop/ontology/Concept"/>
    <owl:onProperty rdf:resource="https://w3id.org/omop/ontology/has_relationship_type"/>
  </rdf:Description>
  <rdf:Description rdf:nodeID="nde7e53d44aa94269b5c0c83d6d8798ccb11">
    <rdf:type rdf:resource="http://www.w3.org/2002/07/owl#Class"/>
    <owl:unionOf rdf:nodeID="nde7e53d44aa94269b5c0c83d6d8798ccb12"/>
  </rdf:Description>
  <rdf:Description rdf:about="https://w3id.org/omop/ontology/source_code_description">
    <rdf:type rdf:resource="http://www.w3.org/2002/07/owl#DatatypeProperty"/>
    <rdf:type rdf:resource="http://www.w3.org/2002/07/owl#FunctionalProperty"/>
    <rdfs:comment xml:lang="en">(for SourceToConceptMap:) An optional description for the
source code. This is included as a
convenience to compare the
description of the source code to
the name of the concept.</rdfs:comment>
    <rdfs:domain rdf:resource="https://w3id.org/omop/ontology/SourceToConceptMap"/>
    <rdfs:range rdf:resource="http://www.w3.org/2001/XMLSchema#string"/>
    <ns1:omop_cdm_name rdf:datatype="http://www.w3.org/2001/XMLSchema#string">source_to_concept_map.source_code_description#405 AS str</ns1:omop_cdm_name>
  </rdf:Description>
  <rdf:Description rdf:nodeID="nde7e53d44aa94269b5c0c83d6d8798ccb453">
    <rdf:type rdf:resource="http://www.w3.org/2002/07/owl#Restriction"/>
    <owl:allValuesFrom rdf:resource="https://w3id.org/omop/ontology/Concept"/>
    <owl:onProperty rdf:resource="https://w3id.org/omop/ontology/has_source"/>
  </rdf:Description>
  <rdf:Description rdf:nodeID="nde7e53d44aa94269b5c0c83d6d8798ccb457">
    <rdf:type rdf:resource="http://www.w3.org/2002/07/owl#Restriction"/>
    <owl:allValuesFrom rdf:resource="http://www.w3.org/2001/XMLSchema#decimal"/>
    <owl:onProperty rdf:resource="https://w3id.org/omop/ontology/value_as_number"/>
  </rdf:Description>
  <rdf:Description rdf:nodeID="nde7e53d44aa94269b5c0c83d6d8798ccb326">
    <rdf:type rdf:resource="http://www.w3.org/2002/07/owl#Restriction"/>
    <owl:allValuesFrom rdf:resource="http://www.w3.org/2001/XMLSchema#date"/>
    <owl:onProperty rdf:resource="https://w3id.org/omop/ontology/valid_start_date"/>
  </rdf:Description>
  <rdf:Description rdf:nodeID="nde7e53d44aa94269b5c0c83d6d8798ccb673">
    <rdf:type rdf:resource="http://www.w3.org/2002/07/owl#Restriction"/>
    <owl:allValuesFrom rdf:resource="https://w3id.org/omop/ontology/Concept"/>
    <owl:onProperty rdf:resource="https://w3id.org/omop/ontology/has_ethnicity"/>
  </rdf:Description>
  <rdf:Description rdf:nodeID="nde7e53d44aa94269b5c0c83d6d8798ccb279">
    <rdf:type rdf:resource="http://www.w3.org/2002/07/owl#Restriction"/>
    <owl:allValuesFrom rdf:resource="http://www.w3.org/2001/XMLSchema#string"/>
    <owl:onProperty rdf:resource="https://w3id.org/omop/ontology/cdm_version"/>
  </rdf:Description>
  <rdf:Description rdf:about="https://w3id.org/omop/ontology/DateDuration">
    <rdf:type rdf:resource="http://www.w3.org/2002/07/owl#Class"/>
    <rdfs:subClassOf rdf:nodeID="nde7e53d44aa94269b5c0c83d6d8798ccb246"/>
    <rdfs:subClassOf rdf:nodeID="nde7e53d44aa94269b5c0c83d6d8798ccb247"/>
    <rdfs:subClassOf rdf:resource="https://w3id.org/omop/ontology/Duration"/>
  </rdf:Description>
  <rdf:Description rdf:nodeID="nde7e53d44aa94269b5c0c83d6d8798ccb318">
    <rdf:type rdf:resource="http://www.w3.org/2002/07/owl#Restriction"/>
    <owl:allValuesFrom rdf:resource="http://www.w3.org/2001/XMLSchema#integer"/>
    <owl:onProperty rdf:resource="https://w3id.org/omop/ontology/admitted_from_source_value"/>
  </rdf:Description>
  <rdf:Description rdf:about="https://w3id.org/omop/ontology/snippet">
    <rdf:type rdf:resource="http://www.w3.org/2002/07/owl#DatatypeProperty"/>
    <rdf:type rdf:resource="http://www.w3.org/2002/07/owl#FunctionalProperty"/>
    <rdfs:comment xml:lang="en">(for NoteNlp:) A small window of text surrounding the term</rdfs:comment>
    <rdfs:domain rdf:resource="https://w3id.org/omop/ontology/NoteNlp"/>
    <rdfs:range rdf:resource="http://www.w3.org/2001/XMLSchema#string"/>
    <ns1:omop_cdm_name rdf:datatype="http://www.w3.org/2001/XMLSchema#string">note_nlp.snippet#196 AS str</ns1:omop_cdm_name>
  </rdf:Description>
  <rdf:Description rdf:nodeID="nde7e53d44aa94269b5c0c83d6d8798ccb274">
    <rdf:type rdf:resource="http://www.w3.org/2002/07/owl#Restriction"/>
    <owl:allValuesFrom rdf:resource="http://www.w3.org/2001/XMLSchema#string"/>
    <owl:onProperty rdf:resource="https://w3id.org/omop/ontology/cdm_etl_reference"/>
  </rdf:Description>
  <rdf:Description rdf:nodeID="nde7e53d44aa94269b5c0c83d6d8798ccb570">
    <rdf:first rdf:resource="https://w3id.org/omop/ontology/Measurement"/>
    <rdf:rest rdf:resource="http://www.w3.org/1999/02/22-rdf-syntax-ns#nil"/>
  </rdf:Description>
  <rdf:Description rdf:nodeID="nde7e53d44aa94269b5c0c83d6d8798ccb498">
    <rdf:type rdf:resource="http://www.w3.org/2002/07/owl#Restriction"/>
    <owl:allValuesFrom rdf:resource="http://www.w3.org/2001/XMLSchema#string"/>
    <owl:onProperty rdf:resource="https://w3id.org/omop/ontology/drg_source_value"/>
  </rdf:Description>
  <rdf:Description rdf:nodeID="nde7e53d44aa94269b5c0c83d6d8798ccb216">
    <rdf:type rdf:resource="http://www.w3.org/2002/07/owl#Restriction"/>
    <owl:onProperty rdf:resource="https://w3id.org/omop/ontology/has_reverse_relationship"/>
    <owl:someValuesFrom rdf:resource="http://www.w3.org/2002/07/owl#Thing"/>
  </rdf:Description>
  <rdf:Description rdf:nodeID="nde7e53d44aa94269b5c0c83d6d8798ccb110">
    <rdf:type rdf:resource="http://www.w3.org/2002/07/owl#Restriction"/>
    <owl:allValuesFrom rdf:resource="https://w3id.org/omop/ontology/Domain"/>
    <owl:onProperty rdf:resource="https://w3id.org/omop/ontology/has_domain"/>
  </rdf:Description>
  <rdf:Description rdf:about="https://w3id.org/omop/ontology/has_event_field">
    <rdf:type rdf:resource="http://www.w3.org/2002/07/owl#FunctionalProperty"/>
    <rdf:type rdf:resource="http://www.w3.org/2002/07/owl#ObjectProperty"/>
    <ns2:python_name rdf:datatype="http://www.w3.org/2001/XMLSchema#string">event_field</ns2:python_name>
    <rdfs:comment xml:lang="en">(for Cost:) If the Cost record is related to another record in the database, this field is the CONCEPT_ID that identifies which table the primary key of the linked record came from.
Put the CONCEPT_ID that identifies which table and field the COST_EVENT_ID came from.</rdfs:comment>
    <rdfs:domain rdf:nodeID="nde7e53d44aa94269b5c0c83d6d8798ccb48"/>
    <rdfs:range rdf:resource="https://w3id.org/omop/ontology/Concept"/>
    <ns1:omop_cdm_name rdf:datatype="http://www.w3.org/2001/XMLSchema#string">cost.cost_event_field_concept_id#310 AS Concept</ns1:omop_cdm_name>
    <ns1:omop_cdm_name rdf:datatype="http://www.w3.org/2001/XMLSchema#string">note.note_event_field_concept_id#180 AS Concept</ns1:omop_cdm_name>
  </rdf:Description>
  <rdf:Description rdf:nodeID="nde7e53d44aa94269b5c0c83d6d8798ccb261">
    <rdf:type rdf:resource="http://www.w3.org/2002/07/owl#Restriction"/>
    <owl:allValuesFrom rdf:resource="http://www.w3.org/2001/XMLSchema#date"/>
    <owl:onProperty rdf:resource="https://w3id.org/omop/ontology/valid_start_date"/>
  </rdf:Description>
  <rdf:Description rdf:about="https://w3id.org/omop/ontology/ethnicity_source_value">
    <rdf:type rdf:resource="http://www.w3.org/2002/07/owl#DatatypeProperty"/>
    <rdf:type rdf:resource="http://www.w3.org/2002/07/owl#FunctionalProperty"/>
    <rdfs:comment xml:lang="en">(for Person:) This field is used to store the ethnicity of the person from the source data. It is not intended for use in standard analytics but for reference only.
If the person has an ethnicity other than the OMB standard of "Hispanic" or "Not Hispanic" store that value from the source data here.</rdfs:comment>
    <rdfs:domain rdf:resource="https://w3id.org/omop/ontology/Person"/>
    <rdfs:range rdf:resource="http://www.w3.org/2001/XMLSchema#string"/>
    <ns1:omop_cdm_name rdf:datatype="http://www.w3.org/2001/XMLSchema#string">person.ethnicity_source_value#18 AS str</ns1:omop_cdm_name>
  </rdf:Description>
  <rdf:Description rdf:nodeID="nde7e53d44aa94269b5c0c83d6d8798ccb310">
    <rdf:type rdf:resource="http://www.w3.org/2002/07/owl#Restriction"/>
    <owl:onProperty rdf:nodeID="nde7e53d44aa94269b5c0c83d6d8798ccb311"/>
    <owl:someValuesFrom rdf:resource="https://w3id.org/omop/ontology/Person"/>
  </rdf:Description>
  <rdf:Description rdf:nodeID="nde7e53d44aa94269b5c0c83d6d8798ccb82">
    <rdf:type rdf:resource="http://www.w3.org/2002/07/owl#Restriction"/>
    <owl:allValuesFrom rdf:resource="http://www.w3.org/2001/XMLSchema#integer"/>
    <owl:onProperty rdf:resource="https://w3id.org/omop/ontology/max_levels_of_separation"/>
  </rdf:Description>
  <rdf:Description rdf:nodeID="nde7e53d44aa94269b5c0c83d6d8798ccb672">
    <rdf:type rdf:resource="http://www.w3.org/2002/07/owl#Restriction"/>
    <owl:allValuesFrom rdf:resource="http://www.w3.org/2001/XMLSchema#integer"/>
    <owl:onProperty rdf:resource="https://w3id.org/omop/ontology/year_of_birth"/>
  </rdf:Description>
  <rdf:Description rdf:about="https://w3id.org/omop/ontology/has_denominator_unit">
    <rdf:type rdf:resource="http://www.w3.org/2002/07/owl#FunctionalProperty"/>
    <rdf:type rdf:resource="http://www.w3.org/2002/07/owl#ObjectProperty"/>
    <ns2:python_name rdf:datatype="http://www.w3.org/2001/XMLSchema#string">denominator_unit</ns2:python_name>
    <rdfs:comment xml:lang="en">(for DrugStrength:) The Concept representing the denominator unit for the concentration of active ingredient.</rdfs:comment>
    <rdfs:domain rdf:resource="https://w3id.org/omop/ontology/DrugStrength"/>
    <rdfs:range rdf:resource="https://w3id.org/omop/ontology/Concept"/>
    <ns1:omop_cdm_name rdf:datatype="http://www.w3.org/2001/XMLSchema#string">drug_strength.denominator_unit_concept_id#418 AS Concept</ns1:omop_cdm_name>
  </rdf:Description>
  <rdf:Description rdf:about="https://w3id.org/omop/ontology/has_drg">
    <rdf:type rdf:resource="http://www.w3.org/2002/07/owl#FunctionalProperty"/>
    <rdf:type rdf:resource="http://www.w3.org/2002/07/owl#ObjectProperty"/>
    <ns2:python_name rdf:datatype="http://www.w3.org/2001/XMLSchema#string">drg</ns2:python_name>
    <rdfs:comment xml:lang="en">(for Cost:) A foreign key referring to a Standard Concept ID in the Standardized Vocabularies for DRG codes belonging to the 'DRG' vocabulary.</rdfs:comment>
    <rdfs:domain rdf:resource="https://w3id.org/omop/ontology/Cost"/>
    <rdfs:range rdf:resource="https://w3id.org/omop/ontology/Concept"/>
    <ns1:omop_cdm_name rdf:datatype="http://www.w3.org/2001/XMLSchema#string">cost.drg_concept_id#321 AS Concept</ns1:omop_cdm_name>
  </rdf:Description>
  <rdf:Description rdf:nodeID="nde7e53d44aa94269b5c0c83d6d8798ccb333">
    <rdf:type rdf:resource="http://www.w3.org/2002/07/owl#Restriction"/>
    <owl:allValuesFrom rdf:resource="http://www.w3.org/2001/XMLSchema#decimal"/>
    <owl:onProperty rdf:resource="https://w3id.org/omop/ontology/denominator_value"/>
  </rdf:Description>
  <rdf:Description rdf:about="https://w3id.org/omop/ontology/has_discharge_to">
    <rdf:type rdf:resource="http://www.w3.org/2002/07/owl#FunctionalProperty"/>
    <rdf:type rdf:resource="http://www.w3.org/2002/07/owl#ObjectProperty"/>
    <ns2:python_name rdf:datatype="http://www.w3.org/2001/XMLSchema#string">discharge_to</ns2:python_name>
    <rdfs:comment xml:lang="en">(for VisitDetail:) Use this field to determine where the patient was discharged to after a visit detail record. This concept is part of the visit domain and can indicate if a patient was discharged to home or sent to a long-term care facility, for example.
If available, map the DISCHARGE_TO_SOURCE_VALUE to a Standard Concept in the Visit domain. If not available, set to 0. [Accepted Concepts](https://athena.ohdsi.org/search-terms/terms?domain=Visit&amp;standardConcept=Standard&amp;page=1&amp;pageSize=15&amp;query=).</rdfs:comment>
    <rdfs:comment xml:lang="en">(for VisitOccurrence:) Use this field to determine where the patient was discharged to after a visit. This concept is part of the visit domain and can indicate if a patient was discharged to home or sent to a long-term care facility, for example.
If available, map the discharge_to_source_value to a standard concept in the visit domain. If not available set to 0.</rdfs:comment>
    <rdfs:domain rdf:resource="https://w3id.org/omop/ontology/BaseVisit"/>
    <rdfs:range rdf:resource="https://w3id.org/omop/ontology/Concept"/>
    <ns1:omop_cdm_name rdf:datatype="http://www.w3.org/2001/XMLSchema#string">visit_detail.discharge_to_concept_id#57 AS Concept</ns1:omop_cdm_name>
    <ns1:omop_cdm_name rdf:datatype="http://www.w3.org/2001/XMLSchema#string">visit_occurrence.discharge_to_concept_id#39 AS Concept</ns1:omop_cdm_name>
  </rdf:Description>
  <rdf:Description rdf:nodeID="nde7e53d44aa94269b5c0c83d6d8798ccb278">
    <rdf:type rdf:resource="http://www.w3.org/2002/07/owl#Restriction"/>
    <owl:allValuesFrom rdf:resource="http://www.w3.org/2001/XMLSchema#string"/>
    <owl:onProperty rdf:resource="https://w3id.org/omop/ontology/abbreviation"/>
  </rdf:Description>
  <rdf:Description rdf:about="https://w3id.org/omop/ontology/has_unique_device">
    <rdf:type rdf:resource="http://www.w3.org/2002/07/owl#FunctionalProperty"/>
    <rdf:type rdf:resource="http://www.w3.org/2002/07/owl#ObjectProperty"/>
    <ns2:python_name rdf:datatype="http://www.w3.org/2001/XMLSchema#string">unique_device</ns2:python_name>
    <rdfs:comment xml:lang="en">(for DeviceExposure:) This is the Unique Device Identification number for devices regulated by the FDA, if given.
For medical devices that are regulated by the FDA, a Unique Device Identification (UDI) is provided if available in the data source and is recorded in the UNIQUE_DEVICE_ID field.</rdfs:comment>
    <rdfs:domain rdf:resource="https://w3id.org/omop/ontology/DeviceExposure"/>
    <ns1:omop_cdm_name rdf:datatype="http://www.w3.org/2001/XMLSchema#string">device_exposure.unique_device_id#122 AS Thing</ns1:omop_cdm_name>
  </rdf:Description>
  <rdf:Description rdf:about="https://w3id.org/omop/ontology/has_collection_method">
    <rdf:type rdf:resource="http://www.w3.org/2002/07/owl#FunctionalProperty"/>
    <rdf:type rdf:resource="http://www.w3.org/2002/07/owl#ObjectProperty"/>
    <ns2:python_name rdf:datatype="http://www.w3.org/2001/XMLSchema#string">collection_method</ns2:python_name>
    <rdfs:comment xml:lang="en">(for SurveyConduct:) This Concept represents how the responses were collected.
Use the concepts that have the relationship 'Has Answer' with the CONCEPT_ID [42529316](https://athena.ohdsi.org/search-terms/terms/42529316).</rdfs:comment>
    <rdfs:domain rdf:resource="https://w3id.org/omop/ontology/SurveyConduct"/>
    <rdfs:range rdf:resource="https://w3id.org/omop/ontology/Concept"/>
    <ns1:omop_cdm_name rdf:datatype="http://www.w3.org/2001/XMLSchema#string">survey_conduct.collection_method_concept_id#238 AS Concept</ns1:omop_cdm_name>
  </rdf:Description>
  <rdf:Description rdf:about="https://w3id.org/omop/ontology/cdm_holder">
    <rdf:type rdf:resource="http://www.w3.org/2002/07/owl#DatatypeProperty"/>
    <rdf:type rdf:resource="http://www.w3.org/2002/07/owl#FunctionalProperty"/>
    <rdfs:comment xml:lang="en">(for CdmSource:) The holder of the CDM instance.</rdfs:comment>
    <rdfs:domain rdf:resource="https://w3id.org/omop/ontology/CdmSource"/>
    <rdfs:range rdf:resource="http://www.w3.org/2001/XMLSchema#string"/>
    <ns1:omop_cdm_name rdf:datatype="http://www.w3.org/2001/XMLSchema#string">cdm_source.cdm_holder#354 AS str</ns1:omop_cdm_name>
  </rdf:Description>
  <rdf:Description rdf:nodeID="nde7e53d44aa94269b5c0c83d6d8798ccb630">
    <rdf:first rdf:resource="https://w3id.org/omop/ontology/Vocabulary"/>
    <rdf:rest rdf:nodeID="nde7e53d44aa94269b5c0c83d6d8798ccb631"/>
  </rdf:Description>
  <rdf:Description rdf:nodeID="nde7e53d44aa94269b5c0c83d6d8798ccb206">
    <rdf:type rdf:resource="http://www.w3.org/2002/07/owl#Restriction"/>
    <owl:allValuesFrom rdf:resource="https://w3id.org/omop/ontology/Concept"/>
    <owl:onProperty rdf:resource="https://w3id.org/omop/ontology/has_concept"/>
  </rdf:Description>
  <rdf:Description rdf:about="https://w3id.org/omop/ontology/ObservationPeriod">
    <rdf:type rdf:resource="http://www.w3.org/2002/07/owl#Class"/>
    <rdfs:subClassOf rdf:nodeID="nde7e53d44aa94269b5c0c83d6d8798ccb29"/>
    <rdfs:subClassOf rdf:nodeID="nde7e53d44aa94269b5c0c83d6d8798ccb31"/>
    <rdfs:subClassOf rdf:nodeID="nde7e53d44aa94269b5c0c83d6d8798ccb32"/>
    <rdfs:subClassOf rdf:resource="https://w3id.org/omop/ontology/ClinicalElement"/>
    <rdfs:subClassOf rdf:resource="https://w3id.org/omop/ontology/DateDuration"/>
    <ns1:omop_cdm_name rdf:datatype="http://www.w3.org/2001/XMLSchema#string">observation_period</ns1:omop_cdm_name>
  </rdf:Description>
  <rdf:Description rdf:about="https://w3id.org/omop/ontology/has_encoding">
    <rdf:type rdf:resource="http://www.w3.org/2002/07/owl#FunctionalProperty"/>
    <rdf:type rdf:resource="http://www.w3.org/2002/07/owl#ObjectProperty"/>
    <ns2:python_name rdf:datatype="http://www.w3.org/2001/XMLSchema#string">encoding</ns2:python_name>
    <rdfs:comment xml:lang="en">(for Note:) This is the Concept representing the character encoding type.
Put the Concept Id that represents the encoding character type here. Currently the only option is UTF-8 ([32678](https://athena.ohdsi.org/search-terms/terms/32678)). It the note is encoded in any other type, like ASCII then put 0.</rdfs:comment>
    <rdfs:domain rdf:resource="https://w3id.org/omop/ontology/Note"/>
    <rdfs:range rdf:resource="https://w3id.org/omop/ontology/Concept"/>
    <ns1:omop_cdm_name rdf:datatype="http://www.w3.org/2001/XMLSchema#string">note.encoding_concept_id#187 AS Concept</ns1:omop_cdm_name>
  </rdf:Description>
  <rdf:Description rdf:nodeID="nde7e53d44aa94269b5c0c83d6d8798ccb164">
    <rdf:type rdf:resource="http://www.w3.org/2002/07/owl#Restriction"/>
    <owl:allValuesFrom rdf:resource="http://www.w3.org/2001/XMLSchema#string"/>
    <owl:onProperty rdf:resource="https://w3id.org/omop/ontology/value_as_string"/>
  </rdf:Description>
  <rdf:Description rdf:about="https://w3id.org/omop/ontology/day_of_birth">
    <rdf:type rdf:resource="http://www.w3.org/2002/07/owl#DatatypeProperty"/>
    <rdf:type rdf:resource="http://www.w3.org/2002/07/owl#FunctionalProperty"/>
    <rdfs:comment xml:lang="en">(for Person:) For data sources that provide the precise date of birth, the day should be extracted and stored in this field.</rdfs:comment>
    <rdfs:domain rdf:resource="https://w3id.org/omop/ontology/Person"/>
    <rdfs:range rdf:resource="http://www.w3.org/2001/XMLSchema#integer"/>
    <ns1:omop_cdm_name rdf:datatype="http://www.w3.org/2001/XMLSchema#string">person.day_of_birth#5 AS int</ns1:omop_cdm_name>
  </rdf:Description>
  <rdf:Description rdf:about="https://w3id.org/omop/ontology/OmopCDMThing">
    <rdf:type rdf:resource="http://www.w3.org/2002/07/owl#Class"/>
    <rdfs:subClassOf rdf:nodeID="nde7e53d44aa94269b5c0c83d6d8798ccb583"/>
    <rdfs:subClassOf rdf:nodeID="nde7e53d44aa94269b5c0c83d6d8798ccb587"/>
    <rdfs:subClassOf rdf:resource="http://www.w3.org/2002/07/owl#Thing"/>
  </rdf:Description>
  <rdf:Description rdf:nodeID="nde7e53d44aa94269b5c0c83d6d8798ccb628">
    <rdf:first rdf:resource="https://w3id.org/omop/ontology/Cost"/>
    <rdf:rest rdf:nodeID="nde7e53d44aa94269b5c0c83d6d8798ccb629"/>
  </rdf:Description>
  <rdf:Description rdf:nodeID="nde7e53d44aa94269b5c0c83d6d8798ccb686">
    <rdf:type rdf:resource="http://www.w3.org/2002/07/owl#Restriction"/>
    <owl:allValuesFrom rdf:resource="https://w3id.org/omop/ontology/Vocabulary"/>
    <owl:onProperty rdf:resource="https://w3id.org/omop/ontology/has_vocabulary"/>
  </rdf:Description>
  <rdf:Description rdf:nodeID="nde7e53d44aa94269b5c0c83d6d8798ccb492">
    <rdf:type rdf:resource="http://www.w3.org/2002/07/owl#Restriction"/>
    <owl:allValuesFrom rdf:resource="https://w3id.org/omop/ontology/PayerPlanPeriod"/>
    <owl:onProperty rdf:resource="https://w3id.org/omop/ontology/has_payer_plan_period"/>
  </rdf:Description>
  <rdf:Description rdf:nodeID="nde7e53d44aa94269b5c0c83d6d8798ccb204">
    <rdf:type rdf:resource="http://www.w3.org/2002/07/owl#Restriction"/>
    <owl:onProperty rdf:resource="https://w3id.org/omop/ontology/has_source"/>
    <owl:someValuesFrom rdf:resource="https://w3id.org/omop/ontology/Concept"/>
  </rdf:Description>
  <rdf:Description rdf:nodeID="nde7e53d44aa94269b5c0c83d6d8798ccb398">
    <rdf:type rdf:resource="http://www.w3.org/2002/07/owl#Restriction"/>
    <owl:allValuesFrom rdf:resource="http://www.w3.org/2001/XMLSchema#decimal"/>
    <owl:onProperty rdf:resource="https://w3id.org/omop/ontology/quantity"/>
  </rdf:Description>
  <rdf:Description rdf:nodeID="nde7e53d44aa94269b5c0c83d6d8798ccb347">
    <rdf:type rdf:resource="http://www.w3.org/2002/07/owl#Restriction"/>
    <owl:onProperty rdf:resource="https://w3id.org/omop/ontology/lexical_variant"/>
    <owl:someValuesFrom rdf:resource="http://www.w3.org/2001/XMLSchema#string"/>
  </rdf:Description>
  <rdf:Description rdf:about="https://w3id.org/omop/ontology/name">
    <rdf:type rdf:resource="http://www.w3.org/2002/07/owl#DatatypeProperty"/>
    <rdf:type rdf:resource="http://www.w3.org/2002/07/owl#FunctionalProperty"/>
    <rdfs:comment xml:lang="en">(for CareSite:) The name of the care_site as it appears in the source data</rdfs:comment>
    <rdfs:comment xml:lang="en">(for CdmSource:) The name of the CDM instance.</rdfs:comment>
    <rdfs:comment xml:lang="en">(for CohortDefinition:) A short description of the cohort</rdfs:comment>
    <rdfs:comment xml:lang="en">(for Concept:) An unambiguous, meaningful and descriptive name for the Concept.</rdfs:comment>
    <rdfs:comment xml:lang="en">(for ConceptClass:) The name describing the Concept Class, e.g.
Clinical Finding, Ingredient, etc.</rdfs:comment>
    <rdfs:comment xml:lang="en">(for Domain:) The name describing the Domain, e.g.
Condition, Procedure, Measurement
etc.</rdfs:comment>
    <rdfs:comment xml:lang="en">(for Provider:) This field is not necessary as it is not necessary to have the actual identity of the Provider. Rather, the idea is to uniquely and anonymously identify providers of care across the database.</rdfs:comment>
    <rdfs:comment xml:lang="en">(for Vocabulary:) The name describing the vocabulary, for
example International Classification of
Diseases, Ninth Revision, Clinical
Modification, Volume 1 and 2 (NCHS) etc.</rdfs:comment>
    <rdfs:domain rdf:nodeID="nde7e53d44aa94269b5c0c83d6d8798ccb571"/>
    <rdfs:range rdf:resource="http://www.w3.org/2001/XMLSchema#string"/>
    <ns1:omop_cdm_name rdf:datatype="http://www.w3.org/2001/XMLSchema#string">care_site.care_site_name#268 AS str</ns1:omop_cdm_name>
    <ns1:omop_cdm_name rdf:datatype="http://www.w3.org/2001/XMLSchema#string">cdm_source.cdm_source_name#352 AS str</ns1:omop_cdm_name>
    <ns1:omop_cdm_name rdf:datatype="http://www.w3.org/2001/XMLSchema#string">cohort_definition.cohort_definition_name#428 AS str</ns1:omop_cdm_name>
    <ns1:omop_cdm_name rdf:datatype="http://www.w3.org/2001/XMLSchema#string">concept.concept_name#363 AS str</ns1:omop_cdm_name>
    <ns1:omop_cdm_name rdf:datatype="http://www.w3.org/2001/XMLSchema#string">concept_class.concept_class_name#381 AS str</ns1:omop_cdm_name>
    <ns1:omop_cdm_name rdf:datatype="http://www.w3.org/2001/XMLSchema#string">concept_synonym.concept_synonym_name#396 AS str</ns1:omop_cdm_name>
    <ns1:omop_cdm_name rdf:datatype="http://www.w3.org/2001/XMLSchema#string">domain.domain_name#378 AS str</ns1:omop_cdm_name>
    <ns1:omop_cdm_name rdf:datatype="http://www.w3.org/2001/XMLSchema#string">metadata.name#347 AS str</ns1:omop_cdm_name>
    <ns1:omop_cdm_name rdf:datatype="http://www.w3.org/2001/XMLSchema#string">provider.provider_name#274 AS str</ns1:omop_cdm_name>
    <ns1:omop_cdm_name rdf:datatype="http://www.w3.org/2001/XMLSchema#string">relationship.relationship_name#390 AS str</ns1:omop_cdm_name>
    <ns1:omop_cdm_name rdf:datatype="http://www.w3.org/2001/XMLSchema#string">vocabulary.vocabulary_name#373 AS str</ns1:omop_cdm_name>
  </rdf:Description>
  <rdf:Description rdf:nodeID="nde7e53d44aa94269b5c0c83d6d8798ccb428">
    <rdf:type rdf:resource="http://www.w3.org/2002/07/owl#Restriction"/>
    <owl:allValuesFrom rdf:resource="https://w3id.org/omop/ontology/Provider"/>
    <owl:onProperty rdf:resource="https://w3id.org/omop/ontology/has_provider"/>
  </rdf:Description>
  <rdf:Description rdf:nodeID="nde7e53d44aa94269b5c0c83d6d8798ccb575">
    <rdf:first rdf:resource="https://w3id.org/omop/ontology/ConceptClass"/>
    <rdf:rest rdf:nodeID="nde7e53d44aa94269b5c0c83d6d8798ccb576"/>
  </rdf:Description>
  <rdf:Description rdf:about="https://w3id.org/omop/ontology/has_period_type">
    <rdf:type rdf:resource="http://www.w3.org/2002/07/owl#FunctionalProperty"/>
    <rdf:type rdf:resource="http://www.w3.org/2002/07/owl#ObjectProperty"/>
    <ns2:python_name rdf:datatype="http://www.w3.org/2001/XMLSchema#string">period_type</ns2:python_name>
    <rdfs:comment xml:lang="en">(for ObservationPeriod:) This field can be used to determine the provenance of the Observation Period as in whether the period was determined from an insurance enrollment file, EHR healthcare encounters, or other sources.
Choose the observation_period_type_concept_id that best represents how the period was determined. [Accepted Concepts](https://athena.ohdsi.org/search-terms/terms?domain=Type+Concept&amp;standardConcept=Standard&amp;page=1&amp;pageSize=15&amp;query=).</rdfs:comment>
    <rdfs:domain rdf:resource="https://w3id.org/omop/ontology/ObservationPeriod"/>
    <rdfs:range rdf:resource="https://w3id.org/omop/ontology/Concept"/>
    <ns1:omop_cdm_name rdf:datatype="http://www.w3.org/2001/XMLSchema#string">observation_period.period_type_concept_id#24 AS Concept</ns1:omop_cdm_name>
  </rdf:Description>
  <rdf:Description rdf:nodeID="nde7e53d44aa94269b5c0c83d6d8798ccb283">
    <rdf:type rdf:resource="http://www.w3.org/2002/07/owl#Restriction"/>
    <owl:allValuesFrom rdf:resource="http://www.w3.org/2001/XMLSchema#string"/>
    <owl:onProperty rdf:resource="https://w3id.org/omop/ontology/source_description"/>
  </rdf:Description>
  <rdf:Description rdf:nodeID="nde7e53d44aa94269b5c0c83d6d8798ccb220">
    <rdf:type rdf:resource="http://www.w3.org/2002/07/owl#Restriction"/>
    <owl:allValuesFrom rdf:resource="https://w3id.org/omop/ontology/Concept"/>
    <owl:onProperty rdf:resource="https://w3id.org/omop/ontology/has_concept"/>
  </rdf:Description>
  <rdf:Description rdf:about="https://w3id.org/omop/ontology/CareSite">
    <rdf:type rdf:resource="http://www.w3.org/2002/07/owl#Class"/>
    <rdfs:subClassOf rdf:nodeID="nde7e53d44aa94269b5c0c83d6d8798ccb221"/>
    <rdfs:subClassOf rdf:nodeID="nde7e53d44aa94269b5c0c83d6d8798ccb222"/>
    <rdfs:subClassOf rdf:nodeID="nde7e53d44aa94269b5c0c83d6d8798ccb223"/>
    <rdfs:subClassOf rdf:nodeID="nde7e53d44aa94269b5c0c83d6d8798ccb224"/>
    <rdfs:subClassOf rdf:nodeID="nde7e53d44aa94269b5c0c83d6d8798ccb225"/>
    <rdfs:subClassOf rdf:nodeID="nde7e53d44aa94269b5c0c83d6d8798ccb226"/>
    <rdfs:subClassOf rdf:resource="https://w3id.org/omop/ontology/OmopCDMThing"/>
    <ns1:omop_cdm_name rdf:datatype="http://www.w3.org/2001/XMLSchema#string">care_site</ns1:omop_cdm_name>
  </rdf:Description>
  <rdf:Description rdf:about="https://w3id.org/omop/ontology/validated_survey_source_value">
    <rdf:type rdf:resource="http://www.w3.org/2002/07/owl#DatatypeProperty"/>
    <rdf:type rdf:resource="http://www.w3.org/2002/07/owl#FunctionalProperty"/>
    <rdfs:comment xml:lang="en">(for SurveyConduct:) Source value representing the validation status of the survey.</rdfs:comment>
    <rdfs:domain rdf:resource="https://w3id.org/omop/ontology/SurveyConduct"/>
    <rdfs:range rdf:resource="http://www.w3.org/2001/XMLSchema#integer"/>
    <ns1:omop_cdm_name rdf:datatype="http://www.w3.org/2001/XMLSchema#string">survey_conduct.validated_survey_source_value#247 AS int</ns1:omop_cdm_name>
  </rdf:Description>
  <rdf:Description rdf:nodeID="nde7e53d44aa94269b5c0c83d6d8798ccb671">
    <rdf:type rdf:resource="http://www.w3.org/2002/07/owl#Restriction"/>
    <owl:allValuesFrom rdf:resource="https://w3id.org/omop/ontology/DoseEra"/>
    <owl:onProperty rdf:resource="https://w3id.org/omop/ontology/has_dose_era"/>
  </rdf:Description>
  <rdf:Description rdf:nodeID="nde7e53d44aa94269b5c0c83d6d8798ccb268">
    <rdf:first rdf:resource="https://w3id.org/omop/ontology/ProcedureOccurrence"/>
    <rdf:rest rdf:nodeID="nde7e53d44aa94269b5c0c83d6d8798ccb269"/>
  </rdf:Description>
  <rdf:Description rdf:about="https://w3id.org/omop/ontology/source_documentation_reference">
    <rdf:type rdf:resource="http://www.w3.org/2002/07/owl#DatatypeProperty"/>
    <rdf:type rdf:resource="http://www.w3.org/2002/07/owl#FunctionalProperty"/>
    <rdfs:domain rdf:resource="https://w3id.org/omop/ontology/CdmSource"/>
    <rdfs:range rdf:resource="http://www.w3.org/2001/XMLSchema#string"/>
    <ns1:omop_cdm_name rdf:datatype="http://www.w3.org/2001/XMLSchema#string">cdm_source.source_documentation_reference#356 AS str</ns1:omop_cdm_name>
  </rdf:Description>
  <rdf:Description rdf:nodeID="nde7e53d44aa94269b5c0c83d6d8798ccb118">
    <rdf:type rdf:resource="http://www.w3.org/2002/07/owl#Class"/>
    <owl:unionOf rdf:nodeID="nde7e53d44aa94269b5c0c83d6d8798ccb119"/>
  </rdf:Description>
  <rdf:Description rdf:nodeID="nde7e53d44aa94269b5c0c83d6d8798ccb108">
    <rdf:type rdf:resource="http://www.w3.org/2002/07/owl#Restriction"/>
    <owl:onProperty rdf:resource="https://w3id.org/omop/ontology/has_relationship_type"/>
    <owl:someValuesFrom rdf:resource="https://w3id.org/omop/ontology/Concept"/>
  </rdf:Description>
  <rdf:Description rdf:nodeID="nde7e53d44aa94269b5c0c83d6d8798ccb354">
    <rdf:type rdf:resource="http://www.w3.org/2002/07/owl#Restriction"/>
    <owl:allValuesFrom rdf:resource="https://w3id.org/omop/ontology/SurveyConduct"/>
    <owl:onProperty rdf:resource="https://w3id.org/omop/ontology/has_survey_conduct"/>
  </rdf:Description>
  <rdf:Description rdf:about="https://w3id.org/omop/ontology/contract_source_value">
    <rdf:type rdf:resource="http://www.w3.org/2002/07/owl#DatatypeProperty"/>
    <rdf:type rdf:resource="http://www.w3.org/2002/07/owl#FunctionalProperty"/>
    <rdfs:comment xml:lang="en">(for PayerPlanPeriod:) This is the relationship of the PERSON_ID to CONTRACT_PERSON_ID as it appears in the source data.</rdfs:comment>
    <rdfs:domain rdf:resource="https://w3id.org/omop/ontology/PayerPlanPeriod"/>
    <rdfs:range rdf:resource="http://www.w3.org/2001/XMLSchema#string"/>
    <ns1:omop_cdm_name rdf:datatype="http://www.w3.org/2001/XMLSchema#string">payer_plan_period.contract_source_value#298 AS str</ns1:omop_cdm_name>
  </rdf:Description>
  <rdf:Description rdf:nodeID="nde7e53d44aa94269b5c0c83d6d8798ccb425">
    <rdf:type rdf:resource="http://www.w3.org/2002/07/owl#Restriction"/>
    <owl:allValuesFrom rdf:resource="https://w3id.org/omop/ontology/Concept"/>
    <owl:onProperty rdf:resource="https://w3id.org/omop/ontology/has_type"/>
  </rdf:Description>
  <rdf:Description rdf:nodeID="nde7e53d44aa94269b5c0c83d6d8798ccb450">
    <rdf:type rdf:resource="http://www.w3.org/2002/07/owl#Restriction"/>
    <owl:allValuesFrom rdf:resource="https://w3id.org/omop/ontology/Concept"/>
    <owl:onProperty rdf:resource="https://w3id.org/omop/ontology/has_type"/>
  </rdf:Description>
  <rdf:Description rdf:about="https://w3id.org/omop/ontology/has_target_vocabulary">
    <rdf:type rdf:resource="http://www.w3.org/2002/07/owl#FunctionalProperty"/>
    <rdf:type rdf:resource="http://www.w3.org/2002/07/owl#ObjectProperty"/>
    <ns2:python_name rdf:datatype="http://www.w3.org/2001/XMLSchema#string">target_vocabulary</ns2:python_name>
    <rdfs:comment xml:lang="en">(for SourceToConceptMap:) The Vocabulary of the target Concept.</rdfs:comment>
    <rdfs:domain rdf:resource="https://w3id.org/omop/ontology/SourceToConceptMap"/>
    <rdfs:range rdf:resource="https://w3id.org/omop/ontology/Vocabulary"/>
    <ns1:omop_cdm_name rdf:datatype="http://www.w3.org/2001/XMLSchema#string">source_to_concept_map.target_vocabulary_id#407 AS Vocabulary</ns1:omop_cdm_name>
  </rdf:Description>
  <rdf:Description rdf:nodeID="nde7e53d44aa94269b5c0c83d6d8798ccb209">
    <rdf:type rdf:resource="http://www.w3.org/2002/07/owl#Restriction"/>
    <owl:allValuesFrom rdf:resource="https://w3id.org/omop/ontology/Provider"/>
    <owl:onProperty rdf:resource="https://w3id.org/omop/ontology/has_provider"/>
  </rdf:Description>
  <rdf:Description rdf:nodeID="nde7e53d44aa94269b5c0c83d6d8798ccb435">
    <rdf:type rdf:resource="http://www.w3.org/2002/07/owl#Restriction"/>
    <owl:allValuesFrom rdf:resource="https://w3id.org/omop/ontology/ProcedureOccurrence"/>
    <owl:onProperty rdf:resource="https://w3id.org/omop/ontology/has_procedure_occurrence"/>
  </rdf:Description>
  <rdf:Description rdf:about="https://w3id.org/omop/ontology/dose_unit_source_value">
    <rdf:type rdf:resource="http://www.w3.org/2002/07/owl#DatatypeProperty"/>
    <rdf:type rdf:resource="http://www.w3.org/2002/07/owl#FunctionalProperty"/>
    <rdfs:comment xml:lang="en">(for DrugExposure:) This field houses the verbatim value from the source data representing the dose unit of the drug given.
This information may be called something different in the source data but the field is meant to contain a value indicating the unit of dosage of drug given to the patient. This is an older column and will be deprecated in an upcoming version.</rdfs:comment>
    <rdfs:domain rdf:resource="https://w3id.org/omop/ontology/DrugExposure"/>
    <rdfs:range rdf:resource="http://www.w3.org/2001/XMLSchema#string"/>
    <ns1:omop_cdm_name rdf:datatype="http://www.w3.org/2001/XMLSchema#string">drug_exposure.dose_unit_source_value#99 AS str</ns1:omop_cdm_name>
  </rdf:Description>
  <rdf:Description rdf:nodeID="nde7e53d44aa94269b5c0c83d6d8798ccb446">
    <rdf:type rdf:resource="http://www.w3.org/2002/07/owl#Restriction"/>
    <owl:allValuesFrom rdf:resource="https://w3id.org/omop/ontology/Concept"/>
    <owl:onProperty rdf:resource="https://w3id.org/omop/ontology/has_discharge_to"/>
  </rdf:Description>
  <rdf:Description rdf:nodeID="nde7e53d44aa94269b5c0c83d6d8798ccb517">
    <rdf:type rdf:resource="http://www.w3.org/2002/07/owl#Restriction"/>
    <owl:allValuesFrom rdf:resource="https://w3id.org/omop/ontology/Concept"/>
    <owl:onProperty rdf:resource="https://w3id.org/omop/ontology/has_unit"/>
  </rdf:Description>
  <rdf:Description rdf:about="https://w3id.org/omop/ontology/DatetimeDuration">
    <rdf:type rdf:resource="http://www.w3.org/2002/07/owl#Class"/>
    <rdfs:subClassOf rdf:nodeID="nde7e53d44aa94269b5c0c83d6d8798ccb186"/>
    <rdfs:subClassOf rdf:nodeID="nde7e53d44aa94269b5c0c83d6d8798ccb187"/>
    <rdfs:subClassOf rdf:resource="https://w3id.org/omop/ontology/Duration"/>
  </rdf:Description>
  <rdf:Description rdf:nodeID="nde7e53d44aa94269b5c0c83d6d8798ccb72">
    <rdf:first rdf:resource="https://w3id.org/omop/ontology/Metadata"/>
    <rdf:rest rdf:resource="http://www.w3.org/1999/02/22-rdf-syntax-ns#nil"/>
  </rdf:Description>
  <rdf:Description rdf:nodeID="nde7e53d44aa94269b5c0c83d6d8798ccb169">
    <rdf:type rdf:resource="http://www.w3.org/2002/07/owl#Restriction"/>
    <owl:allValuesFrom rdf:resource="https://w3id.org/omop/ontology/Concept"/>
    <owl:onProperty rdf:resource="https://w3id.org/omop/ontology/has_concept"/>
  </rdf:Description>
  <rdf:Description rdf:nodeID="nde7e53d44aa94269b5c0c83d6d8798ccb343">
    <rdf:type rdf:resource="http://www.w3.org/2002/07/owl#Restriction"/>
    <owl:allValuesFrom rdf:resource="http://www.w3.org/2001/XMLSchema#string"/>
    <owl:onProperty rdf:resource="https://w3id.org/omop/ontology/term_temporal"/>
  </rdf:Description>
  <rdf:Description rdf:nodeID="nde7e53d44aa94269b5c0c83d6d8798ccb322">
    <rdf:type rdf:resource="http://www.w3.org/2002/07/owl#Restriction"/>
    <owl:allValuesFrom rdf:resource="https://w3id.org/omop/ontology/Concept"/>
    <owl:onProperty rdf:resource="https://w3id.org/omop/ontology/has_admitted_from"/>
  </rdf:Description>
  <rdf:Description rdf:nodeID="nde7e53d44aa94269b5c0c83d6d8798ccb370">
    <rdf:first rdf:resource="https://w3id.org/omop/ontology/Exposure"/>
    <rdf:rest rdf:nodeID="nde7e53d44aa94269b5c0c83d6d8798ccb371"/>
  </rdf:Description>
  <rdf:Description rdf:nodeID="nde7e53d44aa94269b5c0c83d6d8798ccb454">
    <rdf:type rdf:resource="http://www.w3.org/2002/07/owl#Restriction"/>
    <owl:onProperty rdf:resource="https://w3id.org/omop/ontology/has_type"/>
    <owl:someValuesFrom rdf:resource="https://w3id.org/omop/ontology/Concept"/>
  </rdf:Description>
  <rdf:Description rdf:about="https://w3id.org/omop/ontology/box_size">
    <rdf:type rdf:resource="http://www.w3.org/2002/07/owl#DatatypeProperty"/>
    <rdf:type rdf:resource="http://www.w3.org/2002/07/owl#FunctionalProperty"/>
    <rdfs:comment xml:lang="en">(for DrugStrength:) The number of units of Clinical Branded Drug or Quantified Clinical or Branded Drug contained in a box as dispensed to the patient.</rdfs:comment>
    <rdfs:domain rdf:resource="https://w3id.org/omop/ontology/DrugStrength"/>
    <rdfs:range rdf:resource="http://www.w3.org/2001/XMLSchema#integer"/>
    <ns1:omop_cdm_name rdf:datatype="http://www.w3.org/2001/XMLSchema#string">drug_strength.box_size#419 AS int</ns1:omop_cdm_name>
  </rdf:Description>
  <rdf:Description rdf:nodeID="nde7e53d44aa94269b5c0c83d6d8798ccb356">
    <rdf:type rdf:resource="http://www.w3.org/2002/07/owl#Restriction"/>
    <owl:allValuesFrom rdf:resource="http://www.w3.org/2001/XMLSchema#string"/>
    <owl:onProperty rdf:resource="https://w3id.org/omop/ontology/admitted_from_source_value"/>
  </rdf:Description>
  <rdf:Description rdf:nodeID="nde7e53d44aa94269b5c0c83d6d8798ccb303">
    <rdf:type rdf:resource="http://www.w3.org/2002/07/owl#Restriction"/>
    <owl:onProperty rdf:resource="https://w3id.org/omop/ontology/has_type"/>
    <owl:someValuesFrom rdf:resource="https://w3id.org/omop/ontology/Concept"/>
  </rdf:Description>
  <rdf:Description rdf:about="https://w3id.org/omop/ontology/domain_concept_id_2">
    <rdf:type rdf:resource="http://www.w3.org/2002/07/owl#DatatypeProperty"/>
    <rdf:type rdf:resource="http://www.w3.org/2002/07/owl#FunctionalProperty"/>
    <rdfs:domain rdf:resource="https://w3id.org/omop/ontology/FactRelationship"/>
    <rdfs:range rdf:resource="http://www.w3.org/2001/XMLSchema#integer"/>
    <ns1:omop_cdm_name rdf:datatype="http://www.w3.org/2001/XMLSchema#string">fact_relationship.domain_concept_id_2#224 AS int</ns1:omop_cdm_name>
  </rdf:Description>
  <rdf:Description rdf:nodeID="nde7e53d44aa94269b5c0c83d6d8798ccb594">
    <rdf:type rdf:resource="http://www.w3.org/2002/07/owl#Restriction"/>
    <owl:allValuesFrom rdf:resource="http://www.w3.org/2001/XMLSchema#dateTime"/>
    <owl:onProperty rdf:resource="https://w3id.org/omop/ontology/survey_end_datetime"/>
  </rdf:Description>
  <rdf:Description rdf:nodeID="nde7e53d44aa94269b5c0c83d6d8798ccb265">
    <rdf:first rdf:resource="https://w3id.org/omop/ontology/Note"/>
    <rdf:rest rdf:nodeID="nde7e53d44aa94269b5c0c83d6d8798ccb266"/>
  </rdf:Description>
  <rdf:Description rdf:about="https://w3id.org/omop/ontology/code">
    <rdf:type rdf:resource="http://www.w3.org/2002/07/owl#DatatypeProperty"/>
    <rdf:type rdf:resource="http://www.w3.org/2002/07/owl#FunctionalProperty"/>
    <rdfs:comment xml:lang="en">(for Concept:) The concept code represents the identifier
of the Concept in the source vocabulary,
such as SNOMED-CT concept IDs,
RxNorm RXCUIs etc. Note that concept
codes are not unique across vocabularies.</rdfs:comment>
    <rdfs:domain rdf:resource="https://w3id.org/omop/ontology/Concept"/>
    <rdfs:range rdf:resource="http://www.w3.org/2001/XMLSchema#string"/>
    <ns1:omop_cdm_name rdf:datatype="http://www.w3.org/2001/XMLSchema#string">concept.concept_code#368 AS str</ns1:omop_cdm_name>
  </rdf:Description>
  <rdf:Description rdf:nodeID="nde7e53d44aa94269b5c0c83d6d8798ccb84">
    <rdf:type rdf:resource="http://www.w3.org/2002/07/owl#Restriction"/>
    <owl:allValuesFrom rdf:resource="http://www.w3.org/2001/XMLSchema#integer"/>
    <owl:onProperty rdf:resource="https://w3id.org/omop/ontology/min_levels_of_separation"/>
  </rdf:Description>
  <rdf:Description rdf:nodeID="nde7e53d44aa94269b5c0c83d6d8798ccb24">
    <rdf:type rdf:resource="http://www.w3.org/2002/07/owl#Restriction"/>
    <owl:allValuesFrom rdf:resource="https://w3id.org/omop/ontology/Concept"/>
    <owl:onProperty rdf:resource="https://w3id.org/omop/ontology/has_concept"/>
  </rdf:Description>
  <rdf:Description rdf:about="https://w3id.org/omop/ontology/status_source_value">
    <rdf:type rdf:resource="http://www.w3.org/2002/07/owl#DatatypeProperty"/>
    <rdf:type rdf:resource="http://www.w3.org/2002/07/owl#FunctionalProperty"/>
    <rdfs:comment xml:lang="en">(for ConditionOccurrence:) This field houses the verbatim value from the source data representing the condition status.
This information may be called something different in the source data but the field is meant to contain a value indicating when and how a diagnosis was given to a patient. This source value is mapped to a standard concept which is stored in the CONDITION_STATUS_CONCEPT_ID field.</rdfs:comment>
    <rdfs:domain rdf:resource="https://w3id.org/omop/ontology/ConditionOccurrence"/>
    <rdfs:range rdf:resource="http://www.w3.org/2001/XMLSchema#string"/>
    <ns1:omop_cdm_name rdf:datatype="http://www.w3.org/2001/XMLSchema#string">condition_occurrence.condition_status_source_value#76 AS str</ns1:omop_cdm_name>
  </rdf:Description>
  <rdf:Description rdf:nodeID="nde7e53d44aa94269b5c0c83d6d8798ccb120">
    <rdf:first rdf:resource="https://w3id.org/omop/ontology/Observation"/>
    <rdf:rest rdf:nodeID="nde7e53d44aa94269b5c0c83d6d8798ccb121"/>
  </rdf:Description>
  <rdf:Description rdf:nodeID="nde7e53d44aa94269b5c0c83d6d8798ccb429">
    <rdf:type rdf:resource="http://www.w3.org/2002/07/owl#Restriction"/>
    <owl:onProperty rdf:resource="https://w3id.org/omop/ontology/text"/>
    <owl:someValuesFrom rdf:resource="http://www.w3.org/2001/XMLSchema#string"/>
  </rdf:Description>
  <rdf:Description rdf:nodeID="nde7e53d44aa94269b5c0c83d6d8798ccb587">
    <rdf:type rdf:resource="http://www.w3.org/2002/07/owl#Restriction"/>
    <owl:onProperty rdf:resource="https://w3id.org/omop/ontology/id"/>
    <owl:someValuesFrom rdf:nodeID="nde7e53d44aa94269b5c0c83d6d8798ccb588"/>
  </rdf:Description>
  <rdf:Description rdf:nodeID="nde7e53d44aa94269b5c0c83d6d8798ccb416">
    <rdf:type rdf:resource="http://www.w3.org/2002/07/owl#Restriction"/>
    <owl:allValuesFrom rdf:resource="http://www.w3.org/2001/XMLSchema#string"/>
    <owl:onProperty rdf:resource="https://w3id.org/omop/ontology/title"/>
  </rdf:Description>
  <rdf:Description rdf:nodeID="nde7e53d44aa94269b5c0c83d6d8798ccb464">
    <rdf:type rdf:resource="http://www.w3.org/2002/07/owl#Restriction"/>
    <owl:onProperty rdf:resource="https://w3id.org/omop/ontology/has_source"/>
    <owl:someValuesFrom rdf:resource="https://w3id.org/omop/ontology/Concept"/>
  </rdf:Description>
  <rdf:Description rdf:about="https://w3id.org/omop/ontology/has_response_visit_occurrence">
    <rdf:type rdf:resource="http://www.w3.org/2002/07/owl#FunctionalProperty"/>
    <rdf:type rdf:resource="http://www.w3.org/2002/07/owl#ObjectProperty"/>
    <ns2:python_name rdf:datatype="http://www.w3.org/2001/XMLSchema#string">response_visit_occurrence</ns2:python_name>
    <rdfs:comment xml:lang="en">(for SurveyConduct:) The Visit during which any treatment related to the Survey was carried out.</rdfs:comment>
    <rdfs:domain rdf:resource="https://w3id.org/omop/ontology/SurveyConduct"/>
    <rdfs:range rdf:resource="https://w3id.org/omop/ontology/VisitOccurrence"/>
    <ns1:omop_cdm_name rdf:datatype="http://www.w3.org/2001/XMLSchema#string">survey_conduct.response_visit_occurrence_id#250 AS VisitOccurrence</ns1:omop_cdm_name>
  </rdf:Description>
  <rdf:Description rdf:about="https://w3id.org/omop/ontology/month_of_birth">
    <rdf:type rdf:resource="http://www.w3.org/2002/07/owl#DatatypeProperty"/>
    <rdf:type rdf:resource="http://www.w3.org/2002/07/owl#FunctionalProperty"/>
    <rdfs:comment xml:lang="en">(for Person:) For data sources that provide the precise date of birth, the month should be extracted and stored in this field.</rdfs:comment>
    <rdfs:domain rdf:resource="https://w3id.org/omop/ontology/Person"/>
    <rdfs:range rdf:resource="http://www.w3.org/2001/XMLSchema#integer"/>
    <ns1:omop_cdm_name rdf:datatype="http://www.w3.org/2001/XMLSchema#string">person.month_of_birth#4 AS int</ns1:omop_cdm_name>
  </rdf:Description>
  <rdf:Description rdf:about="https://w3id.org/omop/ontology/has_relationship_type">
    <rdf:type rdf:resource="http://www.w3.org/2002/07/owl#FunctionalProperty"/>
    <rdf:type rdf:resource="http://www.w3.org/2002/07/owl#ObjectProperty"/>
    <ns2:python_name rdf:datatype="http://www.w3.org/2001/XMLSchema#string">relationship_type</ns2:python_name>
    <rdfs:comment xml:lang="en">(for LocationHistory:) This is the relationship between the location and the entity (PERSON, PROVIDER, or CARE_SITE)
Concepts in this field must be in the Location class. [Accepted Concepts](https://athena.ohdsi.org/search-terms/terms?standardConcept=Standard&amp;conceptClass=Location&amp;page=1&amp;pageSize=15&amp;query=&amp;boosts). If the DOMAIN_ID is CARE_SITE this should be 0 and when the domain is PROVIDER the value is [Office](https://athena.ohdsi.org/search-terms/terms/4121722).</rdfs:comment>
    <rdfs:domain rdf:resource="https://w3id.org/omop/ontology/LocationHistory"/>
    <rdfs:range rdf:resource="https://w3id.org/omop/ontology/Concept"/>
    <ns1:omop_cdm_name rdf:datatype="http://www.w3.org/2001/XMLSchema#string">location_history.relationship_type_concept_id#262 AS Concept</ns1:omop_cdm_name>
  </rdf:Description>
  <rdf:Description rdf:nodeID="nde7e53d44aa94269b5c0c83d6d8798ccb461">
    <rdf:type rdf:resource="http://www.w3.org/2002/07/owl#Restriction"/>
    <owl:allValuesFrom rdf:resource="https://w3id.org/omop/ontology/Concept"/>
    <owl:onProperty rdf:resource="https://w3id.org/omop/ontology/has_value_as_concept"/>
  </rdf:Description>
  <rdf:Description rdf:nodeID="nde7e53d44aa94269b5c0c83d6d8798ccb399">
    <rdf:type rdf:resource="http://www.w3.org/2002/07/owl#Restriction"/>
    <owl:onProperty rdf:resource="https://w3id.org/omop/ontology/has_type"/>
    <owl:someValuesFrom rdf:resource="https://w3id.org/omop/ontology/Concept"/>
  </rdf:Description>
  <rdf:Description rdf:nodeID="nde7e53d44aa94269b5c0c83d6d8798ccb63">
    <rdf:type rdf:resource="http://www.w3.org/2002/07/owl#Class"/>
    <owl:unionOf rdf:nodeID="nde7e53d44aa94269b5c0c83d6d8798ccb64"/>
  </rdf:Description>
  <rdf:Description rdf:about="https://w3id.org/omop/ontology/has_contract">
    <rdf:type rdf:resource="http://www.w3.org/2002/07/owl#FunctionalProperty"/>
    <rdf:type rdf:resource="http://www.w3.org/2002/07/owl#ObjectProperty"/>
    <ns2:python_name rdf:datatype="http://www.w3.org/2001/XMLSchema#string">contract</ns2:python_name>
    <rdfs:comment xml:lang="en">(for PayerPlanPeriod:) This field represents the relationship between the PERSON_ID and CONTRACT_PERSON_ID. It should be read as PERSON_ID is the *CONTRACT_CONCEPT_ID* of the CONTRACT_PERSON_ID. So if CONTRACT_CONCEPT_ID represents the relationship 'Stepdaughter' then the Person for whom PAYER_PLAN_PERIOD record was recorded is the stepdaughter of the CONTRACT_PERSON_ID.
If available, use this field to represent the relationship between the PERSON_ID and the CONTRACT_PERSON_ID. If the Person for whom the PAYER_PLAN_PERIOD record was recorded is the stepdaughter of the CONTRACT_PERSON_ID then CONTRACT_CONCEPT_ID would be [4330864](https://athena.ohdsi.org/search-terms/terms/4330864). If not available, set to 0. [Accepted Concepts](https://athena.ohdsi.org/search-terms/terms?standardConcept=Standard&amp;domain=Relationship&amp;page=12&amp;pageSize=15&amp;query=).</rdfs:comment>
    <rdfs:domain rdf:resource="https://w3id.org/omop/ontology/PayerPlanPeriod"/>
    <rdfs:range rdf:resource="https://w3id.org/omop/ontology/Concept"/>
    <ns1:omop_cdm_name rdf:datatype="http://www.w3.org/2001/XMLSchema#string">payer_plan_period.contract_concept_id#297 AS Concept</ns1:omop_cdm_name>
  </rdf:Description>
  <rdf:Description rdf:about="https://w3id.org/omop/ontology/ProcedureOccurrence">
    <rdf:type rdf:resource="http://www.w3.org/2002/07/owl#Class"/>
    <rdfs:subClassOf rdf:nodeID="nde7e53d44aa94269b5c0c83d6d8798ccb301"/>
    <rdfs:subClassOf rdf:nodeID="nde7e53d44aa94269b5c0c83d6d8798ccb302"/>
    <rdfs:subClassOf rdf:nodeID="nde7e53d44aa94269b5c0c83d6d8798ccb303"/>
    <rdfs:subClassOf rdf:nodeID="nde7e53d44aa94269b5c0c83d6d8798ccb304"/>
    <rdfs:subClassOf rdf:nodeID="nde7e53d44aa94269b5c0c83d6d8798ccb305"/>
    <rdfs:subClassOf rdf:nodeID="nde7e53d44aa94269b5c0c83d6d8798ccb306"/>
    <rdfs:subClassOf rdf:nodeID="nde7e53d44aa94269b5c0c83d6d8798ccb307"/>
    <rdfs:subClassOf rdf:nodeID="nde7e53d44aa94269b5c0c83d6d8798ccb308"/>
    <rdfs:subClassOf rdf:nodeID="nde7e53d44aa94269b5c0c83d6d8798ccb309"/>
    <rdfs:subClassOf rdf:nodeID="nde7e53d44aa94269b5c0c83d6d8798ccb310"/>
    <rdfs:subClassOf rdf:nodeID="nde7e53d44aa94269b5c0c83d6d8798ccb312"/>
    <rdfs:subClassOf rdf:nodeID="nde7e53d44aa94269b5c0c83d6d8798ccb313"/>
    <rdfs:subClassOf rdf:resource="https://w3id.org/omop/ontology/Event"/>
    <rdfs:subClassOf rdf:resource="https://w3id.org/omop/ontology/Occurrence"/>
    <ns1:omop_cdm_name rdf:datatype="http://www.w3.org/2001/XMLSchema#string">procedure_occurrence</ns1:omop_cdm_name>
  </rdf:Description>
  <rdf:Description rdf:nodeID="nde7e53d44aa94269b5c0c83d6d8798ccb289">
    <rdf:type rdf:resource="http://www.w3.org/2002/07/owl#Restriction"/>
    <owl:onProperty rdf:resource="https://w3id.org/omop/ontology/has_concept"/>
    <owl:someValuesFrom rdf:resource="https://w3id.org/omop/ontology/Concept"/>
  </rdf:Description>
  <rdf:Description rdf:nodeID="nde7e53d44aa94269b5c0c83d6d8798ccb391">
    <rdf:type rdf:resource="http://www.w3.org/2002/07/owl#Restriction"/>
    <owl:allValuesFrom rdf:resource="http://www.w3.org/2001/XMLSchema#string"/>
    <owl:onProperty rdf:resource="https://w3id.org/omop/ontology/disease_status_source_value"/>
  </rdf:Description>
  <rdf:Description rdf:nodeID="nde7e53d44aa94269b5c0c83d6d8798ccb482">
    <rdf:first rdf:resource="https://w3id.org/omop/ontology/SourceToConceptMap"/>
    <rdf:rest rdf:nodeID="nde7e53d44aa94269b5c0c83d6d8798ccb483"/>
  </rdf:Description>
  <rdf:Description rdf:nodeID="nde7e53d44aa94269b5c0c83d6d8798ccb514">
    <rdf:type rdf:resource="http://www.w3.org/2002/07/owl#Restriction"/>
    <owl:allValuesFrom rdf:resource="http://www.w3.org/2001/XMLSchema#string"/>
    <owl:onProperty rdf:resource="https://w3id.org/omop/ontology/unit_source_value"/>
  </rdf:Description>
  <rdf:Description rdf:about="https://w3id.org/omop/ontology/has_preceding_visit_detail">
    <rdf:type rdf:resource="http://www.w3.org/2002/07/owl#FunctionalProperty"/>
    <rdf:type rdf:resource="http://www.w3.org/2002/07/owl#ObjectProperty"/>
    <ns2:python_name rdf:datatype="http://www.w3.org/2001/XMLSchema#string">preceding_visit_detail</ns2:python_name>
    <rdfs:comment xml:lang="en">(for VisitDetail:) Use this field to find the visit detail that occurred for the person prior to the given visit detail record. There could be a few days or a few years in between.
The PRECEDING_VISIT_DETAIL_ID can be used to link a visit immediately preceding the current Visit Detail. Note this is not symmetrical, and there is no such thing as a "following_visit_id".</rdfs:comment>
    <rdfs:domain rdf:resource="https://w3id.org/omop/ontology/VisitDetail"/>
    <rdfs:range rdf:resource="https://w3id.org/omop/ontology/VisitDetail"/>
    <ns1:omop_cdm_name rdf:datatype="http://www.w3.org/2001/XMLSchema#string">visit_detail.preceding_visit_detail_id#58 AS VisitDetail</ns1:omop_cdm_name>
  </rdf:Description>
  <rdf:Description rdf:nodeID="nde7e53d44aa94269b5c0c83d6d8798ccb19">
    <rdf:first rdf:resource="https://w3id.org/omop/ontology/Metadata"/>
    <rdf:rest rdf:resource="http://www.w3.org/1999/02/22-rdf-syntax-ns#nil"/>
  </rdf:Description>
  <rdf:Description rdf:nodeID="nde7e53d44aa94269b5c0c83d6d8798ccb691">
    <rdf:type rdf:resource="http://www.w3.org/2002/07/owl#Restriction"/>
    <owl:allValuesFrom rdf:resource="http://www.w3.org/2001/XMLSchema#string"/>
    <owl:onProperty rdf:resource="https://w3id.org/omop/ontology/code"/>
  </rdf:Description>
  <rdf:Description rdf:nodeID="nde7e53d44aa94269b5c0c83d6d8798ccb680">
    <rdf:type rdf:resource="http://www.w3.org/2002/07/owl#Restriction"/>
    <owl:onProperty rdf:resource="https://w3id.org/omop/ontology/valid_start_date"/>
    <owl:someValuesFrom rdf:resource="http://www.w3.org/2001/XMLSchema#date"/>
  </rdf:Description>
  <rdf:Description rdf:about="https://w3id.org/omop/ontology/payer_source_value">
    <rdf:type rdf:resource="http://www.w3.org/2002/07/owl#DatatypeProperty"/>
    <rdf:type rdf:resource="http://www.w3.org/2002/07/owl#FunctionalProperty"/>
    <rdfs:comment xml:lang="en">(for PayerPlanPeriod:) This is the Payer as it appears in the source data.</rdfs:comment>
    <rdfs:domain rdf:resource="https://w3id.org/omop/ontology/PayerPlanPeriod"/>
    <rdfs:range rdf:resource="http://www.w3.org/2001/XMLSchema#string"/>
    <ns1:omop_cdm_name rdf:datatype="http://www.w3.org/2001/XMLSchema#string">payer_plan_period.payer_source_value#292 AS str</ns1:omop_cdm_name>
  </rdf:Description>
  <rdf:Description rdf:about="https://w3id.org/omop/ontology/has_language">
    <rdf:type rdf:resource="http://www.w3.org/2002/07/owl#FunctionalProperty"/>
    <rdf:type rdf:resource="http://www.w3.org/2002/07/owl#ObjectProperty"/>
    <ns2:python_name rdf:datatype="http://www.w3.org/2001/XMLSchema#string">language</ns2:python_name>
    <rdfs:comment xml:lang="en">(for Note:) The language of the note.
Use Concepts that are descendants of the concept [4182347](https://athena.ohdsi.org/search-terms/terms/4182347) (World Languages).</rdfs:comment>
    <rdfs:domain rdf:nodeID="nde7e53d44aa94269b5c0c83d6d8798ccb122"/>
    <rdfs:range rdf:resource="https://w3id.org/omop/ontology/Concept"/>
    <ns1:omop_cdm_name rdf:datatype="http://www.w3.org/2001/XMLSchema#string">concept_synonym.language_concept_id#397 AS Concept</ns1:omop_cdm_name>
    <ns1:omop_cdm_name rdf:datatype="http://www.w3.org/2001/XMLSchema#string">note.language_concept_id#188 AS Concept</ns1:omop_cdm_name>
  </rdf:Description>
  <rdf:Description rdf:nodeID="nde7e53d44aa94269b5c0c83d6d8798ccb351">
    <rdf:type rdf:resource="http://www.w3.org/2002/07/owl#Restriction"/>
    <owl:allValuesFrom rdf:resource="https://w3id.org/omop/ontology/Concept"/>
    <owl:onProperty rdf:resource="https://w3id.org/omop/ontology/has_section"/>
  </rdf:Description>
  <rdf:Description rdf:nodeID="nde7e53d44aa94269b5c0c83d6d8798ccb647">
    <rdf:type rdf:resource="http://www.w3.org/2002/07/owl#Restriction"/>
    <owl:onProperty rdf:resource="https://w3id.org/omop/ontology/has_ethnicity"/>
    <owl:someValuesFrom rdf:resource="https://w3id.org/omop/ontology/Concept"/>
  </rdf:Description>
  <rdf:Description rdf:about="https://w3id.org/omop/ontology/has_observation">
    <rdf:type rdf:resource="http://www.w3.org/2002/07/owl#ObjectProperty"/>
    <ns2:python_name rdf:datatype="http://www.w3.org/2001/XMLSchema#string">observations</ns2:python_name>
    <rdfs:comment xml:lang="en">(reversed relation, for Observation:) The PERSON_ID of the Person for whom the Observation is recorded. This may be a system generated code.</rdfs:comment>
    <rdfs:comment xml:lang="en">(reversed relation, for Observation:) The VISIT_DETAIL record during which the Observation occurred. For example, if the Person was in the ICU at the time the VISIT_OCCURRENCE record would reflect the overall hospital stay and the VISIT_DETAIL record would reflect the ICU stay during the hospital visit.
Same rules apply as for the VISIT_OCCURRENCE_ID.</rdfs:comment>
    <rdfs:comment xml:lang="en">(reversed relation, for Observation:) The visit during which the Observation occurred.
Depending on the structure of the source data, this may have to be determined based on dates. If an OBSERVATION_DATE occurs within the start and end date of a Visit it is a valid ETL choice to choose the VISIT_OCCURRENCE_ID from the visit that subsumes it, even if not explicitly stated in the data. While not required, an attempt should be made to locate the VISIT_OCCURRENCE_ID of the observation record. If an observation is related to a visit explicitly in the source data, it is possible that the result date of the Observation falls outside of the bounds of the Visit dates.</rdfs:comment>
    <rdfs:domain rdf:nodeID="nde7e53d44aa94269b5c0c83d6d8798ccb57"/>
    <rdfs:range rdf:resource="https://w3id.org/omop/ontology/Observation"/>
    <ns1:omop_cdm_name rdf:datatype="http://www.w3.org/2001/XMLSchema#string">observation.person_id#150 AS Person</ns1:omop_cdm_name>
    <ns1:omop_cdm_name rdf:datatype="http://www.w3.org/2001/XMLSchema#string">observation.visit_detail_id#162 AS VisitDetail</ns1:omop_cdm_name>
    <ns1:omop_cdm_name rdf:datatype="http://www.w3.org/2001/XMLSchema#string">observation.visit_occurrence_id#161 AS VisitOccurrence</ns1:omop_cdm_name>
  </rdf:Description>
  <rdf:Description rdf:about="https://w3id.org/omop/ontology/city">
    <rdf:type rdf:resource="http://www.w3.org/2002/07/owl#DatatypeProperty"/>
    <rdf:type rdf:resource="http://www.w3.org/2002/07/owl#FunctionalProperty"/>
    <rdfs:domain rdf:resource="https://w3id.org/omop/ontology/Location"/>
    <rdfs:range rdf:resource="http://www.w3.org/2001/XMLSchema#string"/>
    <ns1:omop_cdm_name rdf:datatype="http://www.w3.org/2001/XMLSchema#string">location.city#254 AS str</ns1:omop_cdm_name>
  </rdf:Description>
  <rdf:Description rdf:nodeID="nde7e53d44aa94269b5c0c83d6d8798ccb46">
    <rdf:first rdf:resource="https://w3id.org/omop/ontology/BaseVisit"/>
    <rdf:rest rdf:nodeID="nde7e53d44aa94269b5c0c83d6d8798ccb47"/>
  </rdf:Description>
  <rdf:Description rdf:nodeID="nde7e53d44aa94269b5c0c83d6d8798ccb472">
    <rdf:type rdf:resource="http://www.w3.org/2002/07/owl#Restriction"/>
    <owl:allValuesFrom rdf:resource="https://w3id.org/omop/ontology/Concept"/>
    <owl:onProperty rdf:resource="https://w3id.org/omop/ontology/has_specialty_source"/>
  </rdf:Description>
  <rdf:Description rdf:nodeID="nde7e53d44aa94269b5c0c83d6d8798ccb131">
    <rdf:first rdf:resource="https://w3id.org/omop/ontology/ConceptRelationship"/>
    <rdf:rest rdf:resource="http://www.w3.org/1999/02/22-rdf-syntax-ns#nil"/>
  </rdf:Description>
  <rdf:Description rdf:about="https://w3id.org/omop/ontology/exposure_count">
    <rdf:type rdf:resource="http://www.w3.org/2002/07/owl#DatatypeProperty"/>
    <rdf:type rdf:resource="http://www.w3.org/2002/07/owl#FunctionalProperty"/>
    <rdfs:domain rdf:resource="https://w3id.org/omop/ontology/DrugEra"/>
    <rdfs:range rdf:resource="http://www.w3.org/2001/XMLSchema#integer"/>
    <ns1:omop_cdm_name rdf:datatype="http://www.w3.org/2001/XMLSchema#string">drug_era.drug_exposure_count#330 AS int</ns1:omop_cdm_name>
  </rdf:Description>
  <rdf:Description rdf:about="https://w3id.org/omop/ontology/route_source_value">
    <rdf:type rdf:resource="http://www.w3.org/2002/07/owl#DatatypeProperty"/>
    <rdf:type rdf:resource="http://www.w3.org/2002/07/owl#FunctionalProperty"/>
    <rdfs:comment xml:lang="en">(for DrugExposure:) This field houses the verbatim value from the source data representing the drug route.
This information may be called something different in the source data but the field is meant to contain a value indicating when and how a drug was given to a patient. This source value is mapped to a standard concept which is stored in the ROUTE_CONCEPT_ID field.</rdfs:comment>
    <rdfs:domain rdf:resource="https://w3id.org/omop/ontology/DrugExposure"/>
    <rdfs:range rdf:resource="http://www.w3.org/2001/XMLSchema#string"/>
    <ns1:omop_cdm_name rdf:datatype="http://www.w3.org/2001/XMLSchema#string">drug_exposure.route_source_value#98 AS str</ns1:omop_cdm_name>
  </rdf:Description>
  <rdf:Description rdf:nodeID="nde7e53d44aa94269b5c0c83d6d8798ccb302">
    <rdf:type rdf:resource="http://www.w3.org/2002/07/owl#Restriction"/>
    <owl:allValuesFrom rdf:resource="https://w3id.org/omop/ontology/Concept"/>
    <owl:onProperty rdf:resource="https://w3id.org/omop/ontology/has_type"/>
  </rdf:Description>
  <rdf:Description rdf:nodeID="nde7e53d44aa94269b5c0c83d6d8798ccb193">
    <rdf:type rdf:resource="http://www.w3.org/2002/07/owl#Restriction"/>
    <owl:onProperty rdf:resource="https://w3id.org/omop/ontology/has_gender_source"/>
    <owl:someValuesFrom rdf:resource="https://w3id.org/omop/ontology/Concept"/>
  </rdf:Description>
  <rdf:Description rdf:about="https://w3id.org/omop/ontology/title">
    <rdf:type rdf:resource="http://www.w3.org/2002/07/owl#DatatypeProperty"/>
    <rdf:type rdf:resource="http://www.w3.org/2002/07/owl#FunctionalProperty"/>
    <rdfs:comment xml:lang="en">(for Note:) The title of the note.</rdfs:comment>
    <rdfs:domain rdf:resource="https://w3id.org/omop/ontology/Note"/>
    <rdfs:range rdf:resource="http://www.w3.org/2001/XMLSchema#string"/>
    <ns1:omop_cdm_name rdf:datatype="http://www.w3.org/2001/XMLSchema#string">note.note_title#185 AS str</ns1:omop_cdm_name>
  </rdf:Description>
  <rdf:Description rdf:about="https://w3id.org/omop/ontology/state">
    <rdf:type rdf:resource="http://www.w3.org/2002/07/owl#DatatypeProperty"/>
    <rdf:type rdf:resource="http://www.w3.org/2002/07/owl#FunctionalProperty"/>
    <rdfs:domain rdf:resource="https://w3id.org/omop/ontology/Location"/>
    <rdfs:range rdf:resource="http://www.w3.org/2001/XMLSchema#string"/>
    <ns1:omop_cdm_name rdf:datatype="http://www.w3.org/2001/XMLSchema#string">location.state#255 AS str</ns1:omop_cdm_name>
  </rdf:Description>
  <rdf:Description rdf:nodeID="nde7e53d44aa94269b5c0c83d6d8798ccb249">
    <rdf:type rdf:resource="http://www.w3.org/2002/07/owl#Restriction"/>
    <owl:onProperty rdf:resource="https://w3id.org/omop/ontology/has_source"/>
    <owl:someValuesFrom rdf:resource="https://w3id.org/omop/ontology/Concept"/>
  </rdf:Description>
  <rdf:Description rdf:nodeID="nde7e53d44aa94269b5c0c83d6d8798ccb163">
    <rdf:type rdf:resource="http://www.w3.org/2002/07/owl#Restriction"/>
    <owl:allValuesFrom rdf:resource="https://w3id.org/omop/ontology/Concept"/>
    <owl:onProperty rdf:resource="https://w3id.org/omop/ontology/has_value_as_concept"/>
  </rdf:Description>
  <rdf:Description rdf:nodeID="nde7e53d44aa94269b5c0c83d6d8798ccb376">
    <rdf:type rdf:resource="http://www.w3.org/2002/07/owl#Restriction"/>
    <owl:onProperty rdf:nodeID="nde7e53d44aa94269b5c0c83d6d8798ccb377"/>
    <owl:someValuesFrom rdf:resource="https://w3id.org/omop/ontology/Person"/>
  </rdf:Description>
  <rdf:Description rdf:nodeID="nde7e53d44aa94269b5c0c83d6d8798ccb488">
    <rdf:first rdf:resource="https://w3id.org/omop/ontology/Cost"/>
    <rdf:rest rdf:nodeID="nde7e53d44aa94269b5c0c83d6d8798ccb489"/>
  </rdf:Description>
  <rdf:Description rdf:nodeID="nde7e53d44aa94269b5c0c83d6d8798ccb176">
    <rdf:type rdf:resource="http://www.w3.org/2002/07/owl#Restriction"/>
    <owl:onProperty rdf:resource="https://w3id.org/omop/ontology/concept_id_1"/>
    <owl:someValuesFrom rdf:resource="http://www.w3.org/2001/XMLSchema#integer"/>
  </rdf:Description>
  <rdf:Description rdf:nodeID="nde7e53d44aa94269b5c0c83d6d8798ccb649">
    <rdf:type rdf:resource="http://www.w3.org/2002/07/owl#Restriction"/>
    <owl:onProperty rdf:resource="https://w3id.org/omop/ontology/has_race_source"/>
    <owl:someValuesFrom rdf:resource="https://w3id.org/omop/ontology/Concept"/>
  </rdf:Description>
  <rdf:Description rdf:nodeID="nde7e53d44aa94269b5c0c83d6d8798ccb557">
    <rdf:type rdf:resource="http://www.w3.org/2002/07/owl#Restriction"/>
    <owl:allValuesFrom rdf:resource="http://www.w3.org/2001/XMLSchema#string"/>
    <owl:onProperty rdf:resource="https://w3id.org/omop/ontology/sponsor_source_value"/>
  </rdf:Description>
  <rdf:Description rdf:nodeID="nde7e53d44aa94269b5c0c83d6d8798ccb600">
    <rdf:type rdf:resource="http://www.w3.org/2002/07/owl#Restriction"/>
    <owl:allValuesFrom rdf:resource="http://www.w3.org/2001/XMLSchema#string"/>
    <owl:onProperty rdf:resource="https://w3id.org/omop/ontology/survey_source_identifier"/>
  </rdf:Description>
  <rdf:Description rdf:nodeID="nde7e53d44aa94269b5c0c83d6d8798ccb74">
    <rdf:first rdf:resource="https://w3id.org/omop/ontology/Measurement"/>
    <rdf:rest rdf:nodeID="nde7e53d44aa94269b5c0c83d6d8798ccb75"/>
  </rdf:Description>
  <rdf:Description rdf:nodeID="nde7e53d44aa94269b5c0c83d6d8798ccb222">
    <rdf:type rdf:resource="http://www.w3.org/2002/07/owl#Restriction"/>
    <owl:onProperty rdf:resource="https://w3id.org/omop/ontology/has_place_of_service"/>
    <owl:someValuesFrom rdf:resource="https://w3id.org/omop/ontology/Concept"/>
  </rdf:Description>
  <rdf:Description rdf:nodeID="nde7e53d44aa94269b5c0c83d6d8798ccb20">
    <rdf:type rdf:resource="http://www.w3.org/2002/07/owl#Restriction"/>
    <owl:onProperty rdf:resource="https://w3id.org/omop/ontology/name"/>
    <owl:someValuesFrom rdf:resource="http://www.w3.org/2001/XMLSchema#string"/>
  </rdf:Description>
  <rdf:Description rdf:nodeID="nde7e53d44aa94269b5c0c83d6d8798ccb352">
    <rdf:type rdf:resource="http://www.w3.org/2002/07/owl#Restriction"/>
    <owl:allValuesFrom rdf:resource="https://w3id.org/omop/ontology/Concept"/>
    <owl:onProperty rdf:resource="https://w3id.org/omop/ontology/has_admitted_from"/>
  </rdf:Description>
  <rdf:Description rdf:nodeID="nde7e53d44aa94269b5c0c83d6d8798ccb93">
    <rdf:type rdf:resource="http://www.w3.org/2002/07/owl#Restriction"/>
    <owl:onProperty rdf:nodeID="nde7e53d44aa94269b5c0c83d6d8798ccb94"/>
    <owl:someValuesFrom rdf:resource="https://w3id.org/omop/ontology/Person"/>
  </rdf:Description>
  <rdf:Description rdf:nodeID="nde7e53d44aa94269b5c0c83d6d8798ccb636">
    <rdf:first rdf:resource="https://w3id.org/omop/ontology/Relationship"/>
    <rdf:rest rdf:nodeID="nde7e53d44aa94269b5c0c83d6d8798ccb637"/>
  </rdf:Description>
  <rdf:Description rdf:about="https://w3id.org/omop/ontology/has_contract_source">
    <rdf:type rdf:resource="http://www.w3.org/2002/07/owl#FunctionalProperty"/>
    <rdf:type rdf:resource="http://www.w3.org/2002/07/owl#ObjectProperty"/>
    <ns2:python_name rdf:datatype="http://www.w3.org/2001/XMLSchema#string">contract_source</ns2:python_name>
    <rdfs:comment xml:lang="en">(for PayerPlanPeriod:) If the source data codes the relationship between the PERSON_ID and CONTRACT_PERSON_ID in an OMOP supported vocabulary store the concept_id here. If not available, set to 0.</rdfs:comment>
    <rdfs:domain rdf:resource="https://w3id.org/omop/ontology/PayerPlanPeriod"/>
    <rdfs:range rdf:resource="https://w3id.org/omop/ontology/Concept"/>
    <ns1:omop_cdm_name rdf:datatype="http://www.w3.org/2001/XMLSchema#string">payer_plan_period.contract_source_concept_id#299 AS Concept</ns1:omop_cdm_name>
  </rdf:Description>
  <rdf:Description rdf:nodeID="nde7e53d44aa94269b5c0c83d6d8798ccb117">
    <rdf:first rdf:resource="https://w3id.org/omop/ontology/LocationHistory"/>
    <rdf:rest rdf:resource="http://www.w3.org/1999/02/22-rdf-syntax-ns#nil"/>
  </rdf:Description>
  <rdf:Description rdf:nodeID="nde7e53d44aa94269b5c0c83d6d8798ccb31">
    <rdf:type rdf:resource="http://www.w3.org/2002/07/owl#Restriction"/>
    <owl:onProperty rdf:resource="https://w3id.org/omop/ontology/has_period_type"/>
    <owl:someValuesFrom rdf:resource="https://w3id.org/omop/ontology/Concept"/>
  </rdf:Description>
  <rdf:Description rdf:about="https://w3id.org/omop/ontology/has_survey">
    <rdf:type rdf:resource="http://www.w3.org/2002/07/owl#FunctionalProperty"/>
    <rdf:type rdf:resource="http://www.w3.org/2002/07/owl#ObjectProperty"/>
    <ns2:python_name rdf:datatype="http://www.w3.org/2001/XMLSchema#string">survey</ns2:python_name>
    <rdfs:comment xml:lang="en">(for SurveyConduct:) This is the Concept that represents the survey that was completed.
Put the CONCEPT_ID that identifies the survey that the Person completed. There is no specified domain for this table but the concept class 'staging/scales' contains many common surveys. [Accepted Concepts](https://athena.ohdsi.org/search-terms/terms?standardConcept=Standard&amp;conceptClass=Staging+%2F+Scales&amp;page=5&amp;pageSize=15&amp;query=).</rdfs:comment>
    <rdfs:domain rdf:resource="https://w3id.org/omop/ontology/SurveyConduct"/>
    <rdfs:range rdf:resource="https://w3id.org/omop/ontology/Concept"/>
    <ns1:omop_cdm_name rdf:datatype="http://www.w3.org/2001/XMLSchema#string">survey_conduct.survey_concept_id#229 AS Concept</ns1:omop_cdm_name>
  </rdf:Description>
  <rdf:Description rdf:about="https://w3id.org/omop/ontology/has_cost">
    <rdf:type rdf:resource="http://www.w3.org/2002/07/owl#ObjectProperty"/>
    <ns2:python_name rdf:datatype="http://www.w3.org/2001/XMLSchema#string">costs</ns2:python_name>
    <rdfs:domain rdf:resource="https://w3id.org/omop/ontology/Person"/>
    <rdfs:range rdf:resource="https://w3id.org/omop/ontology/Cost"/>
    <ns1:omop_cdm_name rdf:datatype="http://www.w3.org/2001/XMLSchema#string">cost.person_id#308 AS Person</ns1:omop_cdm_name>
  </rdf:Description>
  <rdf:Description rdf:nodeID="nde7e53d44aa94269b5c0c83d6d8798ccb455">
    <rdf:type rdf:resource="http://www.w3.org/2002/07/owl#Restriction"/>
    <owl:allValuesFrom rdf:resource="http://www.w3.org/2001/XMLSchema#string"/>
    <owl:onProperty rdf:resource="https://w3id.org/omop/ontology/time"/>
  </rdf:Description>
  <rdf:Description rdf:about="https://w3id.org/omop/ontology/verbatim_end_date">
    <rdf:type rdf:resource="http://www.w3.org/2002/07/owl#DatatypeProperty"/>
    <rdf:type rdf:resource="http://www.w3.org/2002/07/owl#FunctionalProperty"/>
    <rdfs:comment xml:lang="en">(for DrugExposure:) This is the end date of the drug exposure as it appears in the source data, if it is given
Put the end date or discontinuation date as it appears from the source data or leave blank if unavailable.</rdfs:comment>
    <rdfs:domain rdf:resource="https://w3id.org/omop/ontology/DrugExposure"/>
    <rdfs:range rdf:resource="http://www.w3.org/2001/XMLSchema#date"/>
    <ns1:omop_cdm_name rdf:datatype="http://www.w3.org/2001/XMLSchema#string">drug_exposure.verbatim_end_date#84 AS date</ns1:omop_cdm_name>
  </rdf:Description>
  <rdf:Description rdf:nodeID="nde7e53d44aa94269b5c0c83d6d8798ccb584">
    <rdf:type rdf:resource="http://www.w3.org/2000/01/rdf-schema#Datatype"/>
    <owl:unionOf rdf:nodeID="nde7e53d44aa94269b5c0c83d6d8798ccb585"/>
  </rdf:Description>
  <rdf:Description rdf:nodeID="nde7e53d44aa94269b5c0c83d6d8798ccb168">
    <rdf:type rdf:resource="http://www.w3.org/2002/07/owl#Restriction"/>
    <owl:onProperty rdf:resource="https://w3id.org/omop/ontology/has_concept"/>
    <owl:someValuesFrom rdf:resource="https://w3id.org/omop/ontology/Concept"/>
  </rdf:Description>
  <rdf:Description rdf:about="https://w3id.org/omop/ontology/Occurrence">
    <rdf:type rdf:resource="http://www.w3.org/2002/07/owl#Class"/>
    <rdfs:subClassOf rdf:resource="https://w3id.org/omop/ontology/ClinicalElement"/>
  </rdf:Description>
  <rdf:Description rdf:nodeID="nde7e53d44aa94269b5c0c83d6d8798ccb500">
    <rdf:type rdf:resource="http://www.w3.org/2002/07/owl#Restriction"/>
    <owl:allValuesFrom rdf:resource="https://w3id.org/omop/ontology/Concept"/>
    <owl:onProperty rdf:resource="https://w3id.org/omop/ontology/has_type"/>
  </rdf:Description>
  <rdf:Description rdf:nodeID="nde7e53d44aa94269b5c0c83d6d8798ccb540">
    <rdf:type rdf:resource="http://www.w3.org/2002/07/owl#Restriction"/>
    <owl:onProperty rdf:resource="https://w3id.org/omop/ontology/has_plan_source"/>
    <owl:someValuesFrom rdf:resource="https://w3id.org/omop/ontology/Concept"/>
  </rdf:Description>
  <rdf:Description rdf:nodeID="nde7e53d44aa94269b5c0c83d6d8798ccb591">
    <rdf:type rdf:resource="http://www.w3.org/2002/07/owl#Restriction"/>
    <owl:allValuesFrom rdf:resource="https://w3id.org/omop/ontology/VisitOccurrence"/>
    <owl:onProperty rdf:resource="https://w3id.org/omop/ontology/has_response_visit_occurrence"/>
  </rdf:Description>
  <rdf:Description rdf:nodeID="nde7e53d44aa94269b5c0c83d6d8798ccb375">
    <rdf:type rdf:resource="http://www.w3.org/2002/07/owl#Restriction"/>
    <owl:allValuesFrom rdf:resource="http://www.w3.org/2001/XMLSchema#string"/>
    <owl:onProperty rdf:resource="https://w3id.org/omop/ontology/dose_unit_source_value"/>
  </rdf:Description>
  <rdf:Description rdf:nodeID="nde7e53d44aa94269b5c0c83d6d8798ccb436">
    <rdf:type rdf:resource="http://www.w3.org/2002/07/owl#Restriction"/>
    <owl:allValuesFrom rdf:resource="https://w3id.org/omop/ontology/Note"/>
    <owl:onProperty rdf:resource="https://w3id.org/omop/ontology/has_note"/>
  </rdf:Description>
  <rdf:Description rdf:nodeID="nde7e53d44aa94269b5c0c83d6d8798ccb263">
    <rdf:type rdf:resource="http://www.w3.org/2002/07/owl#Restriction"/>
    <owl:onProperty rdf:resource="https://w3id.org/omop/ontology/has_target"/>
    <owl:someValuesFrom rdf:resource="https://w3id.org/omop/ontology/Concept"/>
  </rdf:Description>
  <rdf:Description rdf:about="https://w3id.org/omop/ontology/has_drug_exposure">
    <rdf:type rdf:resource="http://www.w3.org/2002/07/owl#ObjectProperty"/>
    <ns2:python_name rdf:datatype="http://www.w3.org/2001/XMLSchema#string">drug_exposures</ns2:python_name>
    <rdfs:comment xml:lang="en">(reversed relation, for DrugExposure:) The PERSON_ID of the PERSON for whom the drug dispensing or administration is recorded. This may be a system generated code.</rdfs:comment>
    <rdfs:comment xml:lang="en">(reversed relation, for DrugExposure:) The VISIT_DETAIL record during which the drug exposure occurred. For example, if the person was in the ICU at the time of the drug administration the VISIT_OCCURRENCE record would reflect the overall hospital stay and the VISIT_DETAIL record would reflect the ICU stay during the hospital visit.
Same rules apply as for the VISIT_OCCURRENCE_ID.</rdfs:comment>
    <rdfs:comment xml:lang="en">(reversed relation, for DrugExposure:) The Visit during which the drug was prescribed, administered or dispensed.
To populate this field drug exposures must be explicitly initiated in the visit.</rdfs:comment>
    <rdfs:domain rdf:nodeID="nde7e53d44aa94269b5c0c83d6d8798ccb45"/>
    <rdfs:range rdf:resource="https://w3id.org/omop/ontology/DrugExposure"/>
    <ns1:omop_cdm_name rdf:datatype="http://www.w3.org/2001/XMLSchema#string">drug_exposure.person_id#78 AS Person</ns1:omop_cdm_name>
    <ns1:omop_cdm_name rdf:datatype="http://www.w3.org/2001/XMLSchema#string">drug_exposure.visit_detail_id#95 AS VisitDetail</ns1:omop_cdm_name>
    <ns1:omop_cdm_name rdf:datatype="http://www.w3.org/2001/XMLSchema#string">drug_exposure.visit_occurrence_id#94 AS VisitOccurrence</ns1:omop_cdm_name>
  </rdf:Description>
  <rdf:Description rdf:nodeID="nde7e53d44aa94269b5c0c83d6d8798ccb43">
    <rdf:first rdf:resource="https://w3id.org/omop/ontology/BaseVisit"/>
    <rdf:rest rdf:nodeID="nde7e53d44aa94269b5c0c83d6d8798ccb44"/>
  </rdf:Description>
  <rdf:Description rdf:nodeID="nde7e53d44aa94269b5c0c83d6d8798ccb644">
    <rdf:type rdf:resource="http://www.w3.org/2002/07/owl#Restriction"/>
    <owl:allValuesFrom rdf:resource="https://w3id.org/omop/ontology/Note"/>
    <owl:onProperty rdf:resource="https://w3id.org/omop/ontology/has_note"/>
  </rdf:Description>
  <rdf:Description rdf:nodeID="nde7e53d44aa94269b5c0c83d6d8798ccb666">
    <rdf:type rdf:resource="http://www.w3.org/2002/07/owl#Restriction"/>
    <owl:allValuesFrom rdf:resource="https://w3id.org/omop/ontology/Concept"/>
    <owl:onProperty rdf:resource="https://w3id.org/omop/ontology/has_ethnicity_source"/>
  </rdf:Description>
  <rdf:Description rdf:about="https://w3id.org/omop/ontology/has_modifier">
    <rdf:type rdf:resource="http://www.w3.org/2002/07/owl#FunctionalProperty"/>
    <rdf:type rdf:resource="http://www.w3.org/2002/07/owl#ObjectProperty"/>
    <ns2:python_name rdf:datatype="http://www.w3.org/2001/XMLSchema#string">modifier</ns2:python_name>
    <rdfs:comment xml:lang="en">(for ProcedureOccurrence:) The modifiers are intended to give additional information about the procedure but as of now the vocabulary is under review.
It is up to the ETL to choose how to map modifiers if they exist in source data. These concepts are typically distinguished by 'Modifier' concept classes (e.g., 'CPT4 Modifier' as part of the 'CPT4' vocabulary). If there is more than one modifier on a record, one should be chosen that pertains to the procedure rather than provider. If not available, set to 0. [Accepted Concepts](https://athena.ohdsi.org/search-terms/terms?conceptClass=CPT4+Modifier&amp;conceptClass=HCPCS+Modifier&amp;vocabulary=CPT4&amp;vocabulary=HCPCS&amp;standardConcept=Standard&amp;page=1&amp;pageSize=15&amp;query=).</rdfs:comment>
    <rdfs:domain rdf:resource="https://w3id.org/omop/ontology/ProcedureOccurrence"/>
    <rdfs:range rdf:resource="https://w3id.org/omop/ontology/Concept"/>
    <ns1:omop_cdm_name rdf:datatype="http://www.w3.org/2001/XMLSchema#string">procedure_occurrence.modifier_concept_id#106 AS Concept</ns1:omop_cdm_name>
  </rdf:Description>
  <rdf:Description rdf:about="https://w3id.org/omop/ontology/concept_id_1">
    <rdf:type rdf:resource="http://www.w3.org/2002/07/owl#DatatypeProperty"/>
    <rdf:type rdf:resource="http://www.w3.org/2002/07/owl#FunctionalProperty"/>
    <rdfs:domain rdf:resource="https://w3id.org/omop/ontology/ConceptRelationship"/>
    <rdfs:range rdf:resource="http://www.w3.org/2001/XMLSchema#integer"/>
    <ns1:omop_cdm_name rdf:datatype="http://www.w3.org/2001/XMLSchema#string">concept_relationship.concept_id_1#383 AS int</ns1:omop_cdm_name>
  </rdf:Description>
  <rdf:Description rdf:nodeID="nde7e53d44aa94269b5c0c83d6d8798ccb304">
    <rdf:type rdf:resource="http://www.w3.org/2002/07/owl#Restriction"/>
    <owl:allValuesFrom rdf:resource="http://www.w3.org/2001/XMLSchema#string"/>
    <owl:onProperty rdf:resource="https://w3id.org/omop/ontology/modifier_source_value"/>
  </rdf:Description>
  <rdf:Description rdf:nodeID="nde7e53d44aa94269b5c0c83d6d8798ccb65">
    <rdf:first rdf:resource="https://w3id.org/omop/ontology/Person"/>
    <rdf:rest rdf:resource="http://www.w3.org/1999/02/22-rdf-syntax-ns#nil"/>
  </rdf:Description>
  <rdf:Description rdf:nodeID="nde7e53d44aa94269b5c0c83d6d8798ccb346">
    <rdf:type rdf:resource="http://www.w3.org/2002/07/owl#Restriction"/>
    <owl:allValuesFrom rdf:resource="https://w3id.org/omop/ontology/Concept"/>
    <owl:onProperty rdf:resource="https://w3id.org/omop/ontology/has_concept"/>
  </rdf:Description>
  <rdf:Description rdf:nodeID="nde7e53d44aa94269b5c0c83d6d8798ccb388">
    <rdf:type rdf:resource="http://www.w3.org/2002/07/owl#Restriction"/>
    <owl:allValuesFrom rdf:resource="https://w3id.org/omop/ontology/Concept"/>
    <owl:onProperty rdf:resource="https://w3id.org/omop/ontology/has_type"/>
  </rdf:Description>
  <rdf:Description rdf:nodeID="nde7e53d44aa94269b5c0c83d6d8798ccb555">
    <rdf:type rdf:resource="http://www.w3.org/2002/07/owl#Restriction"/>
    <owl:allValuesFrom rdf:resource="http://www.w3.org/2001/XMLSchema#string"/>
    <owl:onProperty rdf:resource="https://w3id.org/omop/ontology/contract_source_value"/>
  </rdf:Description>
  <rdf:Description rdf:nodeID="nde7e53d44aa94269b5c0c83d6d8798ccb259">
    <rdf:type rdf:resource="http://www.w3.org/2002/07/owl#Restriction"/>
    <owl:allValuesFrom rdf:resource="http://www.w3.org/2001/XMLSchema#string"/>
    <owl:onProperty rdf:resource="https://w3id.org/omop/ontology/invalid_reason"/>
  </rdf:Description>
  <rdf:Description rdf:nodeID="nde7e53d44aa94269b5c0c83d6d8798ccb1">
    <rdf:type rdf:resource="http://www.w3.org/2002/07/owl#Restriction"/>
    <owl:allValuesFrom rdf:resource="http://www.w3.org/2002/07/owl#Thing"/>
    <owl:onProperty rdf:resource="https://w3id.org/omop/ontology/has_subject"/>
  </rdf:Description>
  <rdf:Description rdf:about="https://w3id.org/omop/ontology/range_high">
    <rdf:type rdf:resource="http://www.w3.org/2002/07/owl#DatatypeProperty"/>
    <rdf:type rdf:resource="http://www.w3.org/2002/07/owl#FunctionalProperty"/>
    <rdfs:comment xml:lang="en">(for Measurement:) Ranges have the same unit as the VALUE_AS_NUMBER. These ranges are provided by the source and should remain NULL if not given.
If reference ranges for upper and lower limit of normal as provided (typically by a laboratory) these are stored in the RANGE_HIGH and RANGE_LOW fields. This should be set to NULL if not provided.</rdfs:comment>
    <rdfs:domain rdf:resource="https://w3id.org/omop/ontology/Measurement"/>
    <rdfs:range rdf:resource="http://www.w3.org/2001/XMLSchema#decimal"/>
    <ns1:omop_cdm_name rdf:datatype="http://www.w3.org/2001/XMLSchema#string">measurement.range_high#141 AS float</ns1:omop_cdm_name>
  </rdf:Description>
  <rdf:Description rdf:about="https://w3id.org/omop/ontology/has_plan">
    <rdf:type rdf:resource="http://www.w3.org/2002/07/owl#FunctionalProperty"/>
    <rdf:type rdf:resource="http://www.w3.org/2002/07/owl#ObjectProperty"/>
    <ns2:python_name rdf:datatype="http://www.w3.org/2001/XMLSchema#string">plan</ns2:python_name>
    <rdfs:comment xml:lang="en">(for PayerPlanPeriod:) This field represents the specific health benefit Plan the Person is enrolled in.
Map the Plan directly to a standard CONCEPT_ID. If one does not exists please contact the vocabulary team. There is no global controlled vocabulary available for this information. The point is to stratify on this information and identify if Persons have the same health benefit Plan though the name of the Plan is not necessary. If not available, set to 0. [Accepted Concepts](http://athena.ohdsi.org/search-terms/terms?domain=Plan&amp;standardConcept=Standard&amp;page=1&amp;pageSize=15&amp;query=).</rdfs:comment>
    <rdfs:domain rdf:resource="https://w3id.org/omop/ontology/PayerPlanPeriod"/>
    <rdfs:range rdf:resource="https://w3id.org/omop/ontology/Concept"/>
    <ns1:omop_cdm_name rdf:datatype="http://www.w3.org/2001/XMLSchema#string">payer_plan_period.plan_concept_id#294 AS Concept</ns1:omop_cdm_name>
  </rdf:Description>
  <rdf:Description rdf:nodeID="nde7e53d44aa94269b5c0c83d6d8798ccb309">
    <rdf:type rdf:resource="http://www.w3.org/2002/07/owl#Restriction"/>
    <owl:onProperty rdf:resource="https://w3id.org/omop/ontology/has_source"/>
    <owl:someValuesFrom rdf:resource="https://w3id.org/omop/ontology/Concept"/>
  </rdf:Description>
  <rdf:Description rdf:nodeID="nde7e53d44aa94269b5c0c83d6d8798ccb552">
    <rdf:type rdf:resource="http://www.w3.org/2002/07/owl#Restriction"/>
    <owl:allValuesFrom rdf:resource="https://w3id.org/omop/ontology/Concept"/>
    <owl:onProperty rdf:resource="https://w3id.org/omop/ontology/has_plan_source"/>
  </rdf:Description>
  <rdf:Description rdf:nodeID="nde7e53d44aa94269b5c0c83d6d8798ccb621">
    <rdf:type rdf:resource="http://www.w3.org/2002/07/owl#Restriction"/>
    <owl:allValuesFrom rdf:resource="http://www.w3.org/2001/XMLSchema#string"/>
    <owl:onProperty rdf:resource="https://w3id.org/omop/ontology/survey_source_value"/>
  </rdf:Description>
  <rdf:Description rdf:nodeID="nde7e53d44aa94269b5c0c83d6d8798ccb14">
    <rdf:type rdf:resource="http://www.w3.org/2002/07/owl#Class"/>
    <owl:unionOf rdf:nodeID="nde7e53d44aa94269b5c0c83d6d8798ccb15"/>
  </rdf:Description>
  <rdf:Description rdf:nodeID="nde7e53d44aa94269b5c0c83d6d8798ccb252">
    <rdf:type rdf:resource="http://www.w3.org/2002/07/owl#Restriction"/>
    <owl:allValuesFrom rdf:resource="https://w3id.org/omop/ontology/Concept"/>
    <owl:onProperty rdf:resource="https://w3id.org/omop/ontology/has_target"/>
  </rdf:Description>
  <rdf:Description rdf:about="https://w3id.org/omop/ontology/has_currency">
    <rdf:type rdf:resource="http://www.w3.org/2002/07/owl#FunctionalProperty"/>
    <rdf:type rdf:resource="http://www.w3.org/2002/07/owl#ObjectProperty"/>
    <ns2:python_name rdf:datatype="http://www.w3.org/2001/XMLSchema#string">currency</ns2:python_name>
    <rdfs:comment xml:lang="en">(for Cost:) A foreign key identifier to the concept representing the 3-letter code used to delineate international currencies, such as USD for US Dollar. These belong to the 'Currency' vocabulary</rdfs:comment>
    <rdfs:domain rdf:resource="https://w3id.org/omop/ontology/Cost"/>
    <rdfs:range rdf:resource="https://w3id.org/omop/ontology/Concept"/>
    <ns1:omop_cdm_name rdf:datatype="http://www.w3.org/2001/XMLSchema#string">cost.currency_concept_id#315 AS Concept</ns1:omop_cdm_name>
  </rdf:Description>
  <rdf:Description rdf:about="https://w3id.org/omop/ontology/zip">
    <rdf:type rdf:resource="http://www.w3.org/2002/07/owl#DatatypeProperty"/>
    <rdf:type rdf:resource="http://www.w3.org/2002/07/owl#FunctionalProperty"/>
    <rdfs:comment xml:lang="en">(for Location:) Zip codes are handled as strings of up to 9 characters length. For US addresses, these represent either a 3-digit abbreviated Zip code as provided by many sources for patient protection reasons, the full 5-digit Zip or the 9-digit (ZIP + 4) codes. Unless for specific reasons analytical methods should expect and utilize only the first 3 digits. For international addresses, different rules apply.</rdfs:comment>
    <rdfs:domain rdf:resource="https://w3id.org/omop/ontology/Location"/>
    <rdfs:range rdf:resource="http://www.w3.org/2001/XMLSchema#string"/>
    <ns1:omop_cdm_name rdf:datatype="http://www.w3.org/2001/XMLSchema#string">location.zip#256 AS str</ns1:omop_cdm_name>
  </rdf:Description>
  <rdf:Description rdf:about="https://w3id.org/omop/ontology/standard">
    <rdf:type rdf:resource="http://www.w3.org/2002/07/owl#DatatypeProperty"/>
    <rdf:type rdf:resource="http://www.w3.org/2002/07/owl#FunctionalProperty"/>
    <rdfs:comment xml:lang="en">(for Concept:) This flag determines where a Concept is
a Standard Concept, i.e. is used in the
data, a Classification Concept, or a
non-standard Source Concept. The
allowable values are 'S' (Standard
Concept) and 'C' (Classification
Concept), otherwise the content is NULL.</rdfs:comment>
    <rdfs:domain rdf:resource="https://w3id.org/omop/ontology/Concept"/>
    <rdfs:range rdf:resource="http://www.w3.org/2001/XMLSchema#string"/>
    <ns1:omop_cdm_name rdf:datatype="http://www.w3.org/2001/XMLSchema#string">concept.standard_concept#367 AS str</ns1:omop_cdm_name>
  </rdf:Description>
  <rdf:Description rdf:nodeID="nde7e53d44aa94269b5c0c83d6d8798ccb49">
    <rdf:first rdf:resource="https://w3id.org/omop/ontology/Note"/>
    <rdf:rest rdf:nodeID="nde7e53d44aa94269b5c0c83d6d8798ccb50"/>
  </rdf:Description>
  <rdf:Description rdf:nodeID="nde7e53d44aa94269b5c0c83d6d8798ccb480">
    <rdf:type rdf:resource="http://www.w3.org/2002/07/owl#Restriction"/>
    <owl:allValuesFrom rdf:resource="http://www.w3.org/2001/XMLSchema#integer"/>
    <owl:onProperty rdf:resource="https://w3id.org/omop/ontology/year_of_birth"/>
  </rdf:Description>
  <rdf:Description rdf:nodeID="nde7e53d44aa94269b5c0c83d6d8798ccb101">
    <rdf:type rdf:resource="http://www.w3.org/2002/07/owl#Restriction"/>
    <owl:allValuesFrom rdf:resource="http://www.w3.org/2001/XMLSchema#integer"/>
    <owl:onProperty rdf:resource="https://w3id.org/omop/ontology/gap_days"/>
  </rdf:Description>
  <rdf:Description rdf:about="https://w3id.org/omop/ontology/survey_start_datetime">
    <rdf:type rdf:resource="http://www.w3.org/2002/07/owl#DatatypeProperty"/>
    <rdf:type rdf:resource="http://www.w3.org/2002/07/owl#FunctionalProperty"/>
    <rdfs:comment xml:lang="en">(for SurveyConduct:) If no time given, set to midnight.</rdfs:comment>
    <rdfs:domain rdf:resource="https://w3id.org/omop/ontology/SurveyConduct"/>
    <rdfs:range rdf:resource="http://www.w3.org/2001/XMLSchema#dateTime"/>
    <ns1:omop_cdm_name rdf:datatype="http://www.w3.org/2001/XMLSchema#string">survey_conduct.survey_start_datetime#231 AS datetime</ns1:omop_cdm_name>
  </rdf:Description>
  <rdf:Description rdf:nodeID="nde7e53d44aa94269b5c0c83d6d8798ccb507">
    <rdf:type rdf:resource="http://www.w3.org/2002/07/owl#Restriction"/>
    <owl:allValuesFrom rdf:resource="http://www.w3.org/2001/XMLSchema#decimal"/>
    <owl:onProperty rdf:resource="https://w3id.org/omop/ontology/cost"/>
  </rdf:Description>
  <rdf:Description rdf:nodeID="nde7e53d44aa94269b5c0c83d6d8798ccb358">
    <rdf:type rdf:resource="http://www.w3.org/2002/07/owl#Restriction"/>
    <owl:onProperty rdf:nodeID="nde7e53d44aa94269b5c0c83d6d8798ccb359"/>
    <owl:someValuesFrom rdf:resource="https://w3id.org/omop/ontology/Person"/>
  </rdf:Description>
  <rdf:Description rdf:nodeID="nde7e53d44aa94269b5c0c83d6d8798ccb44">
    <rdf:first rdf:resource="https://w3id.org/omop/ontology/Person"/>
    <rdf:rest rdf:resource="http://www.w3.org/1999/02/22-rdf-syntax-ns#nil"/>
  </rdf:Description>
  <rdf:Description rdf:nodeID="nde7e53d44aa94269b5c0c83d6d8798ccb95">
    <rdf:type rdf:resource="http://www.w3.org/2002/07/owl#Restriction"/>
    <owl:allValuesFrom rdf:resource="https://w3id.org/omop/ontology/Concept"/>
    <owl:onProperty rdf:resource="https://w3id.org/omop/ontology/has_unit"/>
  </rdf:Description>
  <rdf:Description rdf:nodeID="nde7e53d44aa94269b5c0c83d6d8798ccb233">
    <rdf:first rdf:resource="https://w3id.org/omop/ontology/DrugStrength"/>
    <rdf:rest rdf:nodeID="nde7e53d44aa94269b5c0c83d6d8798ccb234"/>
  </rdf:Description>
  <rdf:Description rdf:about="https://w3id.org/omop/ontology/has_revenue_code">
    <rdf:type rdf:resource="http://www.w3.org/2002/07/owl#FunctionalProperty"/>
    <rdf:type rdf:resource="http://www.w3.org/2002/07/owl#ObjectProperty"/>
    <ns2:python_name rdf:datatype="http://www.w3.org/2001/XMLSchema#string">revenue_code</ns2:python_name>
    <rdfs:comment xml:lang="en">(for Cost:) A foreign key referring to a Standard Concept ID in the Standardized Vocabularies for Revenue codes belonging to the 'Revenue Code' vocabulary.</rdfs:comment>
    <rdfs:domain rdf:resource="https://w3id.org/omop/ontology/Cost"/>
    <rdfs:range rdf:resource="https://w3id.org/omop/ontology/Concept"/>
    <ns1:omop_cdm_name rdf:datatype="http://www.w3.org/2001/XMLSchema#string">cost.revenue_code_concept_id#320 AS Concept</ns1:omop_cdm_name>
  </rdf:Description>
  <rdf:Description rdf:nodeID="nde7e53d44aa94269b5c0c83d6d8798ccb251">
    <rdf:type rdf:resource="http://www.w3.org/2002/07/owl#Restriction"/>
    <owl:onProperty rdf:resource="https://w3id.org/omop/ontology/valid_start_date"/>
    <owl:someValuesFrom rdf:resource="http://www.w3.org/2001/XMLSchema#date"/>
  </rdf:Description>
  <rdf:Description rdf:nodeID="nde7e53d44aa94269b5c0c83d6d8798ccb325">
    <rdf:type rdf:resource="http://www.w3.org/2002/07/owl#Restriction"/>
    <owl:allValuesFrom rdf:resource="https://w3id.org/omop/ontology/Concept"/>
    <owl:onProperty rdf:resource="https://w3id.org/omop/ontology/has_amount_unit"/>
  </rdf:Description>
  <rdf:Description rdf:nodeID="nde7e53d44aa94269b5c0c83d6d8798ccb526">
    <rdf:type rdf:resource="http://www.w3.org/2002/07/owl#Restriction"/>
    <owl:allValuesFrom rdf:resource="http://www.w3.org/2001/XMLSchema#string"/>
    <owl:onProperty rdf:resource="https://w3id.org/omop/ontology/qualifier_source_value"/>
  </rdf:Description>
  <rdf:Description rdf:nodeID="nde7e53d44aa94269b5c0c83d6d8798ccb355">
    <rdf:type rdf:resource="http://www.w3.org/2002/07/owl#Restriction"/>
    <owl:allValuesFrom rdf:resource="https://w3id.org/omop/ontology/VisitDetail"/>
    <owl:onProperty rdf:resource="https://w3id.org/omop/ontology/has_visit_detail"/>
  </rdf:Description>
  <rdf:Description rdf:nodeID="nde7e53d44aa94269b5c0c83d6d8798ccb148">
    <rdf:type rdf:resource="http://www.w3.org/2002/07/owl#Restriction"/>
    <owl:onProperty rdf:nodeID="nde7e53d44aa94269b5c0c83d6d8798ccb149"/>
    <owl:someValuesFrom rdf:resource="https://w3id.org/omop/ontology/Person"/>
  </rdf:Description>
  <rdf:Description rdf:about="https://w3id.org/omop/ontology/lexical_variant">
    <rdf:type rdf:resource="http://www.w3.org/2002/07/owl#DatatypeProperty"/>
    <rdf:type rdf:resource="http://www.w3.org/2002/07/owl#FunctionalProperty"/>
    <rdfs:comment xml:lang="en">(for NoteNlp:) Raw text extracted from the NLP tool.</rdfs:comment>
    <rdfs:domain rdf:resource="https://w3id.org/omop/ontology/NoteNlp"/>
    <rdfs:range rdf:resource="http://www.w3.org/2001/XMLSchema#string"/>
    <ns1:omop_cdm_name rdf:datatype="http://www.w3.org/2001/XMLSchema#string">note_nlp.lexical_variant#198 AS str</ns1:omop_cdm_name>
  </rdf:Description>
  <rdf:Description rdf:about="https://w3id.org/omop/ontology/cohort_initiation_date">
    <rdf:type rdf:resource="http://www.w3.org/2002/07/owl#DatatypeProperty"/>
    <rdf:type rdf:resource="http://www.w3.org/2002/07/owl#FunctionalProperty"/>
    <rdfs:comment xml:lang="en">(for CohortDefinition:) A date to indicate when the Cohort was initiated in the COHORT table.</rdfs:comment>
    <rdfs:domain rdf:resource="https://w3id.org/omop/ontology/CohortDefinition"/>
    <rdfs:range rdf:resource="http://www.w3.org/2001/XMLSchema#date"/>
    <ns1:omop_cdm_name rdf:datatype="http://www.w3.org/2001/XMLSchema#string">cohort_definition.cohort_initiation_date#433 AS date</ns1:omop_cdm_name>
  </rdf:Description>
  <rdf:Description rdf:about="https://w3id.org/omop/ontology/ConceptClass">
    <rdf:type rdf:resource="http://www.w3.org/2002/07/owl#Class"/>
    <rdfs:subClassOf rdf:nodeID="nde7e53d44aa94269b5c0c83d6d8798ccb88"/>
    <rdfs:subClassOf rdf:nodeID="nde7e53d44aa94269b5c0c83d6d8798ccb89"/>
    <rdfs:subClassOf rdf:nodeID="nde7e53d44aa94269b5c0c83d6d8798ccb90"/>
    <rdfs:subClassOf rdf:nodeID="nde7e53d44aa94269b5c0c83d6d8798ccb91"/>
    <rdfs:subClassOf rdf:resource="https://w3id.org/omop/ontology/OmopCDMThing"/>
    <ns1:omop_cdm_name rdf:datatype="http://www.w3.org/2001/XMLSchema#string">concept_class</ns1:omop_cdm_name>
  </rdf:Description>
  <rdf:Description rdf:nodeID="nde7e53d44aa94269b5c0c83d6d8798ccb676">
    <rdf:type rdf:resource="http://www.w3.org/2002/07/owl#Restriction"/>
    <owl:allValuesFrom rdf:resource="http://www.w3.org/2001/XMLSchema#string"/>
    <owl:onProperty rdf:resource="https://w3id.org/omop/ontology/invalid_reason"/>
  </rdf:Description>
  <rdf:Description rdf:nodeID="nde7e53d44aa94269b5c0c83d6d8798ccb320">
    <owl:inverseOf rdf:resource="https://w3id.org/omop/ontology/has_visit_detail"/>
  </rdf:Description>
  <rdf:Description rdf:about="https://w3id.org/omop/ontology/has_target">
    <rdf:type rdf:resource="http://www.w3.org/2002/07/owl#FunctionalProperty"/>
    <rdf:type rdf:resource="http://www.w3.org/2002/07/owl#ObjectProperty"/>
    <ns2:python_name rdf:datatype="http://www.w3.org/2001/XMLSchema#string">target</ns2:python_name>
    <rdfs:comment xml:lang="en">(for SourceToConceptMap:) The target Concept
to which the source code is being
mapped.</rdfs:comment>
    <rdfs:domain rdf:resource="https://w3id.org/omop/ontology/SourceToConceptMap"/>
    <rdfs:range rdf:resource="https://w3id.org/omop/ontology/Concept"/>
    <ns1:omop_cdm_name rdf:datatype="http://www.w3.org/2001/XMLSchema#string">source_to_concept_map.target_concept_id#406 AS Concept</ns1:omop_cdm_name>
  </rdf:Description>
  <rdf:Description rdf:nodeID="nde7e53d44aa94269b5c0c83d6d8798ccb103">
    <rdf:type rdf:resource="http://www.w3.org/2002/07/owl#Restriction"/>
    <owl:onProperty rdf:resource="https://w3id.org/omop/ontology/has_concept"/>
    <owl:someValuesFrom rdf:resource="https://w3id.org/omop/ontology/Concept"/>
  </rdf:Description>
  <rdf:Description rdf:nodeID="nde7e53d44aa94269b5c0c83d6d8798ccb329">
    <rdf:type rdf:resource="http://www.w3.org/2002/07/owl#Restriction"/>
    <owl:allValuesFrom rdf:resource="http://www.w3.org/2001/XMLSchema#decimal"/>
    <owl:onProperty rdf:resource="https://w3id.org/omop/ontology/amount_value"/>
  </rdf:Description>
  <rdf:Description rdf:about="https://w3id.org/omop/ontology/survey_source_value">
    <rdf:type rdf:resource="http://www.w3.org/2002/07/owl#DatatypeProperty"/>
    <rdf:type rdf:resource="http://www.w3.org/2002/07/owl#FunctionalProperty"/>
    <rdfs:comment xml:lang="en">(for SurveyConduct:) The survey name as it appears in the source data.</rdfs:comment>
    <rdfs:domain rdf:resource="https://w3id.org/omop/ontology/SurveyConduct"/>
    <rdfs:range rdf:resource="http://www.w3.org/2001/XMLSchema#string"/>
    <ns1:omop_cdm_name rdf:datatype="http://www.w3.org/2001/XMLSchema#string">survey_conduct.survey_source_value#243 AS str</ns1:omop_cdm_name>
  </rdf:Description>
  <rdf:Description rdf:about="https://w3id.org/omop/ontology/has_assisted">
    <rdf:type rdf:resource="http://www.w3.org/2002/07/owl#FunctionalProperty"/>
    <rdf:type rdf:resource="http://www.w3.org/2002/07/owl#ObjectProperty"/>
    <ns2:python_name rdf:datatype="http://www.w3.org/2001/XMLSchema#string">assisted</ns2:python_name>
    <rdfs:comment xml:lang="en">(for SurveyConduct:) This is a Concept that represents whether the survey was completed with assistance or independently.
There is no specific domain or class for this field, just choose the one that best represents the value given in the source.</rdfs:comment>
    <rdfs:domain rdf:resource="https://w3id.org/omop/ontology/SurveyConduct"/>
    <rdfs:range rdf:resource="https://w3id.org/omop/ontology/Concept"/>
    <ns1:omop_cdm_name rdf:datatype="http://www.w3.org/2001/XMLSchema#string">survey_conduct.assisted_concept_id#235 AS Concept</ns1:omop_cdm_name>
  </rdf:Description>
  <rdf:Description rdf:nodeID="nde7e53d44aa94269b5c0c83d6d8798ccb205">
    <rdf:type rdf:resource="http://www.w3.org/2002/07/owl#Restriction"/>
    <owl:allValuesFrom rdf:resource="https://w3id.org/omop/ontology/Concept"/>
    <owl:onProperty rdf:resource="https://w3id.org/omop/ontology/has_source"/>
  </rdf:Description>
  <rdf:Description rdf:nodeID="nde7e53d44aa94269b5c0c83d6d8798ccb669">
    <rdf:type rdf:resource="http://www.w3.org/2002/07/owl#Restriction"/>
    <owl:allValuesFrom rdf:resource="https://w3id.org/omop/ontology/ObservationPeriod"/>
    <owl:onProperty rdf:resource="https://w3id.org/omop/ontology/has_observation_period"/>
  </rdf:Description>
  <rdf:Description rdf:nodeID="nde7e53d44aa94269b5c0c83d6d8798ccb150">
    <rdf:type rdf:resource="http://www.w3.org/2002/07/owl#Restriction"/>
    <owl:allValuesFrom rdf:resource="http://www.w3.org/2001/XMLSchema#integer"/>
    <owl:onProperty rdf:resource="https://w3id.org/omop/ontology/quantity"/>
  </rdf:Description>
  <rdf:Description rdf:nodeID="nde7e53d44aa94269b5c0c83d6d8798ccb47">
    <rdf:first rdf:resource="https://w3id.org/omop/ontology/Person"/>
    <rdf:rest rdf:resource="http://www.w3.org/1999/02/22-rdf-syntax-ns#nil"/>
  </rdf:Description>
  <rdf:Description rdf:about="https://w3id.org/omop/ontology/concept_id_2">
    <rdf:type rdf:resource="http://www.w3.org/2002/07/owl#DatatypeProperty"/>
    <rdf:type rdf:resource="http://www.w3.org/2002/07/owl#FunctionalProperty"/>
    <rdfs:domain rdf:resource="https://w3id.org/omop/ontology/ConceptRelationship"/>
    <rdfs:range rdf:resource="http://www.w3.org/2001/XMLSchema#integer"/>
    <ns1:omop_cdm_name rdf:datatype="http://www.w3.org/2001/XMLSchema#string">concept_relationship.concept_id_2#384 AS int</ns1:omop_cdm_name>
  </rdf:Description>
  <rdf:Description rdf:nodeID="nde7e53d44aa94269b5c0c83d6d8798ccb80">
    <rdf:type rdf:resource="http://www.w3.org/2002/07/owl#Restriction"/>
    <owl:onProperty rdf:resource="https://w3id.org/omop/ontology/max_levels_of_separation"/>
    <owl:someValuesFrom rdf:resource="http://www.w3.org/2001/XMLSchema#integer"/>
  </rdf:Description>
  <rdf:Description rdf:nodeID="nde7e53d44aa94269b5c0c83d6d8798ccb219">
    <rdf:type rdf:resource="http://www.w3.org/2002/07/owl#Restriction"/>
    <owl:onProperty rdf:resource="https://w3id.org/omop/ontology/is_hierarchical"/>
    <owl:someValuesFrom rdf:resource="http://www.w3.org/2001/XMLSchema#string"/>
  </rdf:Description>
  <rdf:Description rdf:about="https://w3id.org/omop/ontology/has_condition_era">
    <rdf:type rdf:resource="http://www.w3.org/2002/07/owl#ObjectProperty"/>
    <ns2:python_name rdf:datatype="http://www.w3.org/2001/XMLSchema#string">condition_eras</ns2:python_name>
    <rdfs:domain rdf:resource="https://w3id.org/omop/ontology/Person"/>
    <rdfs:range rdf:resource="https://w3id.org/omop/ontology/ConditionEra"/>
    <ns1:omop_cdm_name rdf:datatype="http://www.w3.org/2001/XMLSchema#string">condition_era.person_id#340 AS Person</ns1:omop_cdm_name>
  </rdf:Description>
  <rdf:Description rdf:nodeID="nde7e53d44aa94269b5c0c83d6d8798ccb317">
    <rdf:type rdf:resource="http://www.w3.org/2002/07/owl#Restriction"/>
    <owl:allValuesFrom rdf:resource="https://w3id.org/omop/ontology/VisitDetail"/>
    <owl:onProperty rdf:resource="https://w3id.org/omop/ontology/has_parent"/>
  </rdf:Description>
  <rdf:Description rdf:nodeID="nde7e53d44aa94269b5c0c83d6d8798ccb397">
    <rdf:type rdf:resource="http://www.w3.org/2002/07/owl#Restriction"/>
    <owl:allValuesFrom rdf:resource="https://w3id.org/omop/ontology/Concept"/>
    <owl:onProperty rdf:resource="https://w3id.org/omop/ontology/has_concept"/>
  </rdf:Description>
  <rdf:Description rdf:nodeID="nde7e53d44aa94269b5c0c83d6d8798ccb369">
    <rdf:first rdf:resource="https://w3id.org/omop/ontology/BaseVisit"/>
    <rdf:rest rdf:nodeID="nde7e53d44aa94269b5c0c83d6d8798ccb370"/>
  </rdf:Description>
  <rdf:Description rdf:nodeID="nde7e53d44aa94269b5c0c83d6d8798ccb412">
    <rdf:type rdf:resource="http://www.w3.org/2002/07/owl#Restriction"/>
    <owl:allValuesFrom rdf:resource="http://www.w3.org/2001/XMLSchema#string"/>
    <owl:onProperty rdf:resource="https://w3id.org/omop/ontology/zip"/>
  </rdf:Description>
  <rdf:Description rdf:nodeID="nde7e53d44aa94269b5c0c83d6d8798ccb560">
    <rdf:first rdf:resource="https://w3id.org/omop/ontology/Note"/>
    <rdf:rest rdf:nodeID="nde7e53d44aa94269b5c0c83d6d8798ccb561"/>
  </rdf:Description>
  <rdf:Description rdf:nodeID="nde7e53d44aa94269b5c0c83d6d8798ccb447">
    <rdf:type rdf:resource="http://www.w3.org/2002/07/owl#Restriction"/>
    <owl:allValuesFrom rdf:resource="https://w3id.org/omop/ontology/Measurement"/>
    <owl:onProperty rdf:resource="https://w3id.org/omop/ontology/has_measurement"/>
  </rdf:Description>
  <rdf:Description rdf:nodeID="nde7e53d44aa94269b5c0c83d6d8798ccb297">
    <rdf:type rdf:resource="http://www.w3.org/2002/07/owl#Restriction"/>
    <owl:onProperty rdf:resource="https://w3id.org/omop/ontology/has_status"/>
    <owl:someValuesFrom rdf:resource="https://w3id.org/omop/ontology/Concept"/>
  </rdf:Description>
  <rdf:Description rdf:nodeID="nde7e53d44aa94269b5c0c83d6d8798ccb159">
    <rdf:type rdf:resource="http://www.w3.org/2002/07/owl#Restriction"/>
    <owl:allValuesFrom rdf:resource="http://www.w3.org/2001/XMLSchema#integer"/>
    <owl:onProperty rdf:resource="https://w3id.org/omop/ontology/domain_concept_id_2"/>
  </rdf:Description>
  <rdf:Description rdf:nodeID="nde7e53d44aa94269b5c0c83d6d8798ccb622">
    <rdf:type rdf:resource="http://www.w3.org/2002/07/owl#Class"/>
    <owl:unionOf rdf:nodeID="nde7e53d44aa94269b5c0c83d6d8798ccb623"/>
  </rdf:Description>
  <rdf:Description rdf:nodeID="nde7e53d44aa94269b5c0c83d6d8798ccb305">
    <rdf:type rdf:resource="http://www.w3.org/2002/07/owl#Restriction"/>
    <owl:allValuesFrom rdf:resource="https://w3id.org/omop/ontology/Provider"/>
    <owl:onProperty rdf:resource="https://w3id.org/omop/ontology/has_provider"/>
  </rdf:Description>
  <rdf:Description rdf:nodeID="nde7e53d44aa94269b5c0c83d6d8798ccb91">
    <rdf:type rdf:resource="http://www.w3.org/2002/07/owl#Restriction"/>
    <owl:onProperty rdf:resource="https://w3id.org/omop/ontology/has_concept"/>
    <owl:someValuesFrom rdf:resource="https://w3id.org/omop/ontology/Concept"/>
  </rdf:Description>
  <rdf:Description rdf:nodeID="nde7e53d44aa94269b5c0c83d6d8798ccb378">
    <rdf:type rdf:resource="http://www.w3.org/2002/07/owl#Restriction"/>
    <owl:allValuesFrom rdf:resource="http://www.w3.org/2001/XMLSchema#string"/>
    <owl:onProperty rdf:resource="https://w3id.org/omop/ontology/lot_number"/>
  </rdf:Description>
  <rdf:Description rdf:nodeID="nde7e53d44aa94269b5c0c83d6d8798ccb293">
    <rdf:type rdf:resource="http://www.w3.org/2002/07/owl#Restriction"/>
    <owl:onProperty rdf:resource="https://w3id.org/omop/ontology/has_source"/>
    <owl:someValuesFrom rdf:resource="https://w3id.org/omop/ontology/Concept"/>
  </rdf:Description>
  <rdf:Description rdf:nodeID="nde7e53d44aa94269b5c0c83d6d8798ccb87">
    <rdf:type rdf:resource="http://www.w3.org/2002/07/owl#Restriction"/>
    <owl:allValuesFrom rdf:resource="https://w3id.org/omop/ontology/Concept"/>
    <owl:onProperty rdf:resource="https://w3id.org/omop/ontology/has_ancestor"/>
  </rdf:Description>
  <rdf:Description rdf:nodeID="nde7e53d44aa94269b5c0c83d6d8798ccb499">
    <rdf:type rdf:resource="http://www.w3.org/2002/07/owl#Restriction"/>
    <owl:onProperty rdf:resource="https://w3id.org/omop/ontology/has_event"/>
    <owl:someValuesFrom rdf:resource="http://www.w3.org/2002/07/owl#Thing"/>
  </rdf:Description>
  <rdf:Description rdf:nodeID="nde7e53d44aa94269b5c0c83d6d8798ccb178">
    <rdf:type rdf:resource="http://www.w3.org/2002/07/owl#Restriction"/>
    <owl:allValuesFrom rdf:resource="http://www.w3.org/2001/XMLSchema#integer"/>
    <owl:onProperty rdf:resource="https://w3id.org/omop/ontology/concept_id_2"/>
  </rdf:Description>
  <rdf:Description rdf:nodeID="nde7e53d44aa94269b5c0c83d6d8798ccb253">
    <rdf:type rdf:resource="http://www.w3.org/2002/07/owl#Restriction"/>
    <owl:allValuesFrom rdf:resource="https://w3id.org/omop/ontology/Vocabulary"/>
    <owl:onProperty rdf:resource="https://w3id.org/omop/ontology/has_source_vocabulary"/>
  </rdf:Description>
  <rdf:Description rdf:nodeID="nde7e53d44aa94269b5c0c83d6d8798ccb403">
    <rdf:type rdf:resource="http://www.w3.org/2002/07/owl#Restriction"/>
    <owl:allValuesFrom rdf:resource="http://www.w3.org/2001/XMLSchema#string"/>
    <owl:onProperty rdf:resource="https://w3id.org/omop/ontology/reference"/>
  </rdf:Description>
  <rdf:Description rdf:nodeID="nde7e53d44aa94269b5c0c83d6d8798ccb12">
    <rdf:first rdf:resource="https://w3id.org/omop/ontology/DrugExposure"/>
    <rdf:rest rdf:nodeID="nde7e53d44aa94269b5c0c83d6d8798ccb13"/>
  </rdf:Description>
  <rdf:Description rdf:about="https://w3id.org/omop/ontology/ConditionEra">
    <rdf:type rdf:resource="http://www.w3.org/2002/07/owl#Class"/>
    <rdfs:subClassOf rdf:nodeID="nde7e53d44aa94269b5c0c83d6d8798ccb26"/>
    <rdfs:subClassOf rdf:nodeID="nde7e53d44aa94269b5c0c83d6d8798ccb27"/>
    <rdfs:subClassOf rdf:resource="https://w3id.org/omop/ontology/Era"/>
    <ns1:omop_cdm_name rdf:datatype="http://www.w3.org/2001/XMLSchema#string">condition_era</ns1:omop_cdm_name>
  </rdf:Description>
  <rdf:Description rdf:about="https://w3id.org/omop/ontology/offset">
    <rdf:type rdf:resource="http://www.w3.org/2002/07/owl#DatatypeProperty"/>
    <rdf:type rdf:resource="http://www.w3.org/2002/07/owl#FunctionalProperty"/>
    <rdfs:comment xml:lang="en">(for NoteNlp:) Character offset of the extracted term in the input note</rdfs:comment>
    <rdfs:domain rdf:resource="https://w3id.org/omop/ontology/NoteNlp"/>
    <rdfs:range rdf:resource="http://www.w3.org/2001/XMLSchema#string"/>
    <ns1:omop_cdm_name rdf:datatype="http://www.w3.org/2001/XMLSchema#string">note_nlp.offset#197 AS str</ns1:omop_cdm_name>
  </rdf:Description>
  <rdf:Description rdf:about="https://w3id.org/omop/ontology">
    <rdf:type rdf:resource="http://www.w3.org/2002/07/owl#Ontology"/>
  </rdf:Description>
  <rdf:Description rdf:about="https://w3id.org/omop/ontology/has_observation_period">
    <rdf:type rdf:resource="http://www.w3.org/2002/07/owl#ObjectProperty"/>
    <ns2:python_name rdf:datatype="http://www.w3.org/2001/XMLSchema#string">observation_periods</ns2:python_name>
    <rdfs:comment xml:lang="en">(reversed relation, for ObservationPeriod:) The Person ID of the PERSON record for which the Observation Period is recorded.</rdfs:comment>
    <rdfs:domain rdf:resource="https://w3id.org/omop/ontology/Person"/>
    <rdfs:range rdf:resource="https://w3id.org/omop/ontology/ObservationPeriod"/>
    <ns1:omop_cdm_name rdf:datatype="http://www.w3.org/2001/XMLSchema#string">observation_period.person_id#21 AS Person</ns1:omop_cdm_name>
  </rdf:Description>
  <rdf:Description rdf:nodeID="nde7e53d44aa94269b5c0c83d6d8798ccb471">
    <rdf:type rdf:resource="http://www.w3.org/2002/07/owl#Restriction"/>
    <owl:allValuesFrom rdf:resource="https://w3id.org/omop/ontology/Concept"/>
    <owl:onProperty rdf:resource="https://w3id.org/omop/ontology/has_type"/>
  </rdf:Description>
  <rdf:Description rdf:nodeID="nde7e53d44aa94269b5c0c83d6d8798ccb681">
    <rdf:type rdf:resource="http://www.w3.org/2002/07/owl#Restriction"/>
    <owl:allValuesFrom rdf:resource="http://www.w3.org/2001/XMLSchema#date"/>
    <owl:onProperty rdf:resource="https://w3id.org/omop/ontology/valid_end_date"/>
  </rdf:Description>
  <rdf:Description rdf:nodeID="nde7e53d44aa94269b5c0c83d6d8798ccb179">
    <rdf:type rdf:resource="http://www.w3.org/2002/07/owl#Restriction"/>
    <owl:allValuesFrom rdf:resource="http://www.w3.org/2001/XMLSchema#date"/>
    <owl:onProperty rdf:resource="https://w3id.org/omop/ontology/valid_start_date"/>
  </rdf:Description>
  <rdf:Description rdf:nodeID="nde7e53d44aa94269b5c0c83d6d8798ccb547">
    <rdf:type rdf:resource="http://www.w3.org/2002/07/owl#Restriction"/>
    <owl:onProperty rdf:resource="https://w3id.org/omop/ontology/has_sponsor"/>
    <owl:someValuesFrom rdf:resource="https://w3id.org/omop/ontology/Concept"/>
  </rdf:Description>
  <rdf:Description rdf:nodeID="nde7e53d44aa94269b5c0c83d6d8798ccb635">
    <rdf:first rdf:resource="https://w3id.org/omop/ontology/Metadata"/>
    <rdf:rest rdf:nodeID="nde7e53d44aa94269b5c0c83d6d8798ccb636"/>
  </rdf:Description>
  <rdf:Description rdf:nodeID="nde7e53d44aa94269b5c0c83d6d8798ccb638">
    <rdf:first rdf:resource="https://w3id.org/omop/ontology/BaseVisit"/>
    <rdf:rest rdf:nodeID="nde7e53d44aa94269b5c0c83d6d8798ccb639"/>
  </rdf:Description>
  <rdf:Description rdf:about="https://w3id.org/omop/ontology/has_parent">
    <rdf:type rdf:resource="http://www.w3.org/2002/07/owl#FunctionalProperty"/>
    <rdf:type rdf:resource="http://www.w3.org/2002/07/owl#ObjectProperty"/>
    <ns2:python_name rdf:datatype="http://www.w3.org/2001/XMLSchema#string">parent</ns2:python_name>
    <rdfs:comment xml:lang="en">(for VisitDetail:) Use this field to find the visit detail that subsumes the given visit detail record. This is used in the case that a visit detail record needs to be nested beyond the VISIT_OCCURRENCE/VISIT_DETAIL relationship.
If there are multiple nested levels to how Visits are represented in the source, the VISIT_DETAIL_PARENT_ID can be used to record this relationship.</rdfs:comment>
    <rdfs:domain rdf:resource="https://w3id.org/omop/ontology/VisitDetail"/>
    <rdfs:range rdf:resource="https://w3id.org/omop/ontology/VisitDetail"/>
    <ns1:omop_cdm_name rdf:datatype="http://www.w3.org/2001/XMLSchema#string">visit_detail.visit_detail_parent_id#59 AS VisitDetail</ns1:omop_cdm_name>
  </rdf:Description>
  <rdf:Description rdf:nodeID="nde7e53d44aa94269b5c0c83d6d8798ccb549">
    <rdf:type rdf:resource="http://www.w3.org/2002/07/owl#Restriction"/>
    <owl:allValuesFrom rdf:resource="https://w3id.org/omop/ontology/Concept"/>
    <owl:onProperty rdf:resource="https://w3id.org/omop/ontology/has_plan"/>
  </rdf:Description>
  <rdf:Description rdf:nodeID="nde7e53d44aa94269b5c0c83d6d8798ccb234">
    <rdf:first rdf:resource="https://w3id.org/omop/ontology/Concept"/>
    <rdf:rest rdf:nodeID="nde7e53d44aa94269b5c0c83d6d8798ccb235"/>
  </rdf:Description>
  <rdf:Description rdf:nodeID="nde7e53d44aa94269b5c0c83d6d8798ccb468">
    <rdf:type rdf:resource="http://www.w3.org/2002/07/owl#Restriction"/>
    <owl:allValuesFrom rdf:resource="http://www.w3.org/2001/XMLSchema#decimal"/>
    <owl:onProperty rdf:resource="https://w3id.org/omop/ontology/range_low"/>
  </rdf:Description>
  <rdf:Description rdf:about="https://w3id.org/omop/ontology/has_specialty">
    <rdf:type rdf:resource="http://www.w3.org/2002/07/owl#FunctionalProperty"/>
    <rdf:type rdf:resource="http://www.w3.org/2002/07/owl#ObjectProperty"/>
    <ns2:python_name rdf:datatype="http://www.w3.org/2001/XMLSchema#string">specialty</ns2:python_name>
    <rdfs:comment xml:lang="en">(for Provider:) This field either represents the most common specialty that occurs in the data or the most specific concept that represents all specialties listed, should the provider have more than one. This includes physician specialties such as internal medicine, emergency medicine, etc. and allied health professionals such as nurses, midwives, and pharmacists.
If a Provider has more than one Specialty, there are two options: 1. Choose a concept_id which is a common ancestor to the multiple specialties, or, 2. Choose the specialty that occurs most often for the provider. Concepts in this field should be Standard with a domain of Provider. If not available, set to 0. [Accepted Concepts](http://athena.ohdsi.org/search-terms/terms?domain=Provider&amp;standardConcept=Standard&amp;page=1&amp;pageSize=15&amp;query=).</rdfs:comment>
    <rdfs:domain rdf:resource="https://w3id.org/omop/ontology/Provider"/>
    <rdfs:range rdf:resource="https://w3id.org/omop/ontology/Concept"/>
    <ns1:omop_cdm_name rdf:datatype="http://www.w3.org/2001/XMLSchema#string">provider.specialty_concept_id#277 AS Concept</ns1:omop_cdm_name>
  </rdf:Description>
  <rdf:Description rdf:nodeID="nde7e53d44aa94269b5c0c83d6d8798ccb445">
    <rdf:type rdf:resource="http://www.w3.org/2002/07/owl#Restriction"/>
    <owl:onProperty rdf:resource="https://w3id.org/omop/ontology/has_concept"/>
    <owl:someValuesFrom rdf:resource="https://w3id.org/omop/ontology/Concept"/>
  </rdf:Description>
  <rdf:Description rdf:about="https://w3id.org/omop/ontology/has_definition">
    <rdf:type rdf:resource="http://www.w3.org/2002/07/owl#FunctionalProperty"/>
    <rdf:type rdf:resource="http://www.w3.org/2002/07/owl#ObjectProperty"/>
    <ns2:python_name rdf:datatype="http://www.w3.org/2001/XMLSchema#string">definition</ns2:python_name>
    <rdfs:domain rdf:resource="https://w3id.org/omop/ontology/Cohort"/>
    <rdfs:range rdf:resource="https://w3id.org/omop/ontology/CohortDefinition"/>
    <ns1:omop_cdm_name rdf:datatype="http://www.w3.org/2001/XMLSchema#string">cohort.cohort_definition_id#423 AS CohortDefinition</ns1:omop_cdm_name>
  </rdf:Description>
  <rdf:Description rdf:nodeID="nde7e53d44aa94269b5c0c83d6d8798ccb37">
    <rdf:first rdf:resource="https://w3id.org/omop/ontology/VisitOccurrence"/>
    <rdf:rest rdf:nodeID="nde7e53d44aa94269b5c0c83d6d8798ccb38"/>
  </rdf:Description>
  <rdf:Description rdf:about="https://w3id.org/omop/ontology/has_obs_event_field">
    <rdf:type rdf:resource="http://www.w3.org/2002/07/owl#FunctionalProperty"/>
    <rdf:type rdf:resource="http://www.w3.org/2002/07/owl#ObjectProperty"/>
    <ns2:python_name rdf:datatype="http://www.w3.org/2001/XMLSchema#string">obs_event_field</ns2:python_name>
    <rdfs:comment xml:lang="en">(for Observation:) If the Observation record is related to another record in the database, this field is the CONCEPT_ID that identifies which table the primary key of the linked record came from.
Put the CONCEPT_ID that identifies which table and field the OBSERVATION_EVENT_ID came from.</rdfs:comment>
    <rdfs:domain rdf:resource="https://w3id.org/omop/ontology/Observation"/>
    <rdfs:range rdf:resource="https://w3id.org/omop/ontology/Concept"/>
    <ns1:omop_cdm_name rdf:datatype="http://www.w3.org/2001/XMLSchema#string">observation.obs_event_field_concept_id#168 AS Concept</ns1:omop_cdm_name>
  </rdf:Description>
  <rdf:Description rdf:nodeID="nde7e53d44aa94269b5c0c83d6d8798ccb26">
    <rdf:type rdf:resource="http://www.w3.org/2002/07/owl#Restriction"/>
    <owl:allValuesFrom rdf:resource="http://www.w3.org/2001/XMLSchema#integer"/>
    <owl:onProperty rdf:resource="https://w3id.org/omop/ontology/occurrence_count"/>
  </rdf:Description>
  <rdf:Description rdf:about="https://w3id.org/omop/ontology/abbreviation">
    <rdf:type rdf:resource="http://www.w3.org/2002/07/owl#DatatypeProperty"/>
    <rdf:type rdf:resource="http://www.w3.org/2002/07/owl#FunctionalProperty"/>
    <rdfs:comment xml:lang="en">(for CdmSource:) The abbreviation of the CDM instance.</rdfs:comment>
    <rdfs:domain rdf:resource="https://w3id.org/omop/ontology/CdmSource"/>
    <rdfs:range rdf:resource="http://www.w3.org/2001/XMLSchema#string"/>
    <ns1:omop_cdm_name rdf:datatype="http://www.w3.org/2001/XMLSchema#string">cdm_source.cdm_source_abbreviation#353 AS str</ns1:omop_cdm_name>
  </rdf:Description>
  <rdf:Description rdf:about="https://w3id.org/omop/ontology/quantity">
    <rdf:type rdf:resource="http://www.w3.org/2002/07/owl#DatatypeProperty"/>
    <rdf:type rdf:resource="http://www.w3.org/2002/07/owl#FunctionalProperty"/>
    <rdfs:comment xml:lang="en">(for DrugExposure:) To find the dose form of a drug the RELATIONSHIP table can be used where the relationship_id is 'Has dose form'. If liquid, quantity stands for the total amount dispensed or ordered of ingredient in the units given by the drug_strength table. If the unit from the source data does not align with the unit in the DRUG_STRENGTH table the quantity should be converted to the correct unit given in DRUG_STRENGTH. For clinical drugs with fixed dose forms (tablets etc.) the quantity is the number of units/tablets/capsules prescribed or dispensed (can be partial, but then only 1/2 or 1/3, not 0.01). Clinical drugs with divisible dose forms (injections) the quantity is the amount of ingredient the patient got. For example, if the injection is 2mg/mL but the patient got 80mL then quantity is reported as 160.
Quantified clinical drugs with divisible dose forms (prefilled syringes), the quantity is the amount of ingredient similar to clinical drugs. Please see [how to calculate drug dose](https://ohdsi.github.io/CommonDataModel/drug_dose.html) for more information.
</rdfs:comment>
    <rdfs:comment xml:lang="en">(for ProcedureOccurrence:) If the quantity value is omitted, a single procedure is assumed.
If a Procedure has a quantity of '0' in the source, this should default to '1' in the ETL. If there is a record in the source it can be assumed the exposure occurred at least once</rdfs:comment>
    <rdfs:comment xml:lang="en">(for Specimen:) The amount of specimen collected from the person.</rdfs:comment>
    <rdfs:domain rdf:nodeID="nde7e53d44aa94269b5c0c83d6d8798ccb143"/>
    <ns1:omop_cdm_name rdf:datatype="http://www.w3.org/2001/XMLSchema#string">device_exposure.quantity#123 AS int</ns1:omop_cdm_name>
    <ns1:omop_cdm_name rdf:datatype="http://www.w3.org/2001/XMLSchema#string">drug_exposure.quantity#88 AS float</ns1:omop_cdm_name>
    <ns1:omop_cdm_name rdf:datatype="http://www.w3.org/2001/XMLSchema#string">procedure_occurrence.quantity#107 AS int</ns1:omop_cdm_name>
    <ns1:omop_cdm_name rdf:datatype="http://www.w3.org/2001/XMLSchema#string">specimen.quantity#213 AS float</ns1:omop_cdm_name>
  </rdf:Description>
  <rdf:Description rdf:about="https://w3id.org/omop/ontology/survey_end_datetime">
    <rdf:type rdf:resource="http://www.w3.org/2002/07/owl#DatatypeProperty"/>
    <rdf:type rdf:resource="http://www.w3.org/2002/07/owl#FunctionalProperty"/>
    <rdfs:comment xml:lang="en">(for SurveyConduct:) If no time given, set to midnight.</rdfs:comment>
    <rdfs:domain rdf:resource="https://w3id.org/omop/ontology/SurveyConduct"/>
    <rdfs:range rdf:resource="http://www.w3.org/2001/XMLSchema#dateTime"/>
    <ns1:omop_cdm_name rdf:datatype="http://www.w3.org/2001/XMLSchema#string">survey_conduct.survey_end_datetime#233 AS datetime</ns1:omop_cdm_name>
  </rdf:Description>
  <rdf:Description rdf:nodeID="nde7e53d44aa94269b5c0c83d6d8798ccb496">
    <rdf:type rdf:resource="http://www.w3.org/2002/07/owl#Restriction"/>
    <owl:allValuesFrom rdf:resource="http://www.w3.org/2001/XMLSchema#date"/>
    <owl:onProperty rdf:resource="https://w3id.org/omop/ontology/incurred_date"/>
  </rdf:Description>
  <rdf:Description rdf:nodeID="nde7e53d44aa94269b5c0c83d6d8798ccb444">
    <rdf:type rdf:resource="http://www.w3.org/2002/07/owl#Restriction"/>
    <owl:allValuesFrom rdf:resource="https://w3id.org/omop/ontology/DrugExposure"/>
    <owl:onProperty rdf:resource="https://w3id.org/omop/ontology/has_drug_exposure"/>
  </rdf:Description>
  <rdf:Description rdf:nodeID="nde7e53d44aa94269b5c0c83d6d8798ccb199">
    <rdf:type rdf:resource="http://www.w3.org/2002/07/owl#Restriction"/>
    <owl:onProperty rdf:resource="https://w3id.org/omop/ontology/has_concept"/>
    <owl:someValuesFrom rdf:resource="https://w3id.org/omop/ontology/Concept"/>
  </rdf:Description>
  <rdf:Description rdf:nodeID="nde7e53d44aa94269b5c0c83d6d8798ccb207">
    <rdf:type rdf:resource="http://www.w3.org/2002/07/owl#Restriction"/>
    <owl:onProperty rdf:resource="https://w3id.org/omop/ontology/has_type"/>
    <owl:someValuesFrom rdf:resource="https://w3id.org/omop/ontology/Concept"/>
  </rdf:Description>
  <rdf:Description rdf:about="https://w3id.org/omop/ontology/has_specimen">
    <rdf:type rdf:resource="http://www.w3.org/2002/07/owl#ObjectProperty"/>
    <ns2:python_name rdf:datatype="http://www.w3.org/2001/XMLSchema#string">specimens</ns2:python_name>
    <rdfs:comment xml:lang="en">(reversed relation, for Specimen:) The person from whom the specimen is collected.</rdfs:comment>
    <rdfs:domain rdf:resource="https://w3id.org/omop/ontology/Person"/>
    <rdfs:range rdf:resource="https://w3id.org/omop/ontology/Specimen"/>
    <ns1:omop_cdm_name rdf:datatype="http://www.w3.org/2001/XMLSchema#string">specimen.person_id#208 AS Person</ns1:omop_cdm_name>
  </rdf:Description>
  <rdf:Description rdf:nodeID="nde7e53d44aa94269b5c0c83d6d8798ccb474">
    <rdf:type rdf:resource="http://www.w3.org/2002/07/owl#Restriction"/>
    <owl:allValuesFrom rdf:resource="http://www.w3.org/2001/XMLSchema#string"/>
    <owl:onProperty rdf:resource="https://w3id.org/omop/ontology/specialty_source_value"/>
  </rdf:Description>
  <rdf:Description rdf:about="https://w3id.org/omop/ontology/Relationship">
    <rdf:type rdf:resource="http://www.w3.org/2002/07/owl#Class"/>
    <rdfs:subClassOf rdf:nodeID="nde7e53d44aa94269b5c0c83d6d8798ccb211"/>
    <rdfs:subClassOf rdf:nodeID="nde7e53d44aa94269b5c0c83d6d8798ccb212"/>
    <rdfs:subClassOf rdf:nodeID="nde7e53d44aa94269b5c0c83d6d8798ccb213"/>
    <rdfs:subClassOf rdf:nodeID="nde7e53d44aa94269b5c0c83d6d8798ccb214"/>
    <rdfs:subClassOf rdf:nodeID="nde7e53d44aa94269b5c0c83d6d8798ccb215"/>
    <rdfs:subClassOf rdf:nodeID="nde7e53d44aa94269b5c0c83d6d8798ccb216"/>
    <rdfs:subClassOf rdf:nodeID="nde7e53d44aa94269b5c0c83d6d8798ccb217"/>
    <rdfs:subClassOf rdf:nodeID="nde7e53d44aa94269b5c0c83d6d8798ccb218"/>
    <rdfs:subClassOf rdf:nodeID="nde7e53d44aa94269b5c0c83d6d8798ccb219"/>
    <rdfs:subClassOf rdf:nodeID="nde7e53d44aa94269b5c0c83d6d8798ccb220"/>
    <rdfs:subClassOf rdf:resource="https://w3id.org/omop/ontology/OmopCDMThing"/>
    <ns1:omop_cdm_name rdf:datatype="http://www.w3.org/2001/XMLSchema#string">relationship</ns1:omop_cdm_name>
  </rdf:Description>
  <rdf:Description rdf:nodeID="nde7e53d44aa94269b5c0c83d6d8798ccb548">
    <rdf:type rdf:resource="http://www.w3.org/2002/07/owl#Restriction"/>
    <owl:allValuesFrom rdf:resource="http://www.w3.org/2001/XMLSchema#string"/>
    <owl:onProperty rdf:resource="https://w3id.org/omop/ontology/payer_source_value"/>
  </rdf:Description>
  <rdf:Description rdf:nodeID="nde7e53d44aa94269b5c0c83d6d8798ccb275">
    <rdf:type rdf:resource="http://www.w3.org/2002/07/owl#Restriction"/>
    <owl:allValuesFrom rdf:resource="http://www.w3.org/2001/XMLSchema#string"/>
    <owl:onProperty rdf:resource="https://w3id.org/omop/ontology/vocabulary_version"/>
  </rdf:Description>
  <rdf:Description rdf:about="https://w3id.org/omop/ontology/has_amount_unit">
    <rdf:type rdf:resource="http://www.w3.org/2002/07/owl#FunctionalProperty"/>
    <rdf:type rdf:resource="http://www.w3.org/2002/07/owl#ObjectProperty"/>
    <ns2:python_name rdf:datatype="http://www.w3.org/2001/XMLSchema#string">amount_unit</ns2:python_name>
    <rdfs:comment xml:lang="en">(for DrugStrength:) The Concept representing the Unit of measure for the amount of active ingredient contained within the drug product.</rdfs:comment>
    <rdfs:domain rdf:resource="https://w3id.org/omop/ontology/DrugStrength"/>
    <rdfs:range rdf:resource="https://w3id.org/omop/ontology/Concept"/>
    <ns1:omop_cdm_name rdf:datatype="http://www.w3.org/2001/XMLSchema#string">drug_strength.amount_unit_concept_id#414 AS Concept</ns1:omop_cdm_name>
  </rdf:Description>
  <rdf:Description rdf:nodeID="nde7e53d44aa94269b5c0c83d6d8798ccb535">
    <rdf:type rdf:resource="http://www.w3.org/2002/07/owl#Restriction"/>
    <owl:allValuesFrom rdf:resource="https://w3id.org/omop/ontology/Person"/>
    <owl:onProperty rdf:resource="https://w3id.org/omop/ontology/has_contract_person"/>
  </rdf:Description>
  <rdf:Description rdf:nodeID="nde7e53d44aa94269b5c0c83d6d8798ccb531">
    <rdf:type rdf:resource="http://www.w3.org/2002/07/owl#Restriction"/>
    <owl:onProperty rdf:resource="https://w3id.org/omop/ontology/has_concept"/>
    <owl:someValuesFrom rdf:resource="https://w3id.org/omop/ontology/Concept"/>
  </rdf:Description>
  <rdf:Description rdf:nodeID="nde7e53d44aa94269b5c0c83d6d8798ccb550">
    <rdf:type rdf:resource="http://www.w3.org/2002/07/owl#Restriction"/>
    <owl:allValuesFrom rdf:resource="https://w3id.org/omop/ontology/Concept"/>
    <owl:onProperty rdf:resource="https://w3id.org/omop/ontology/has_payer_source"/>
  </rdf:Description>
  <rdf:Description rdf:nodeID="nde7e53d44aa94269b5c0c83d6d8798ccb660">
    <rdf:type rdf:resource="http://www.w3.org/2002/07/owl#Restriction"/>
    <owl:allValuesFrom rdf:resource="https://w3id.org/omop/ontology/DrugExposure"/>
    <owl:onProperty rdf:resource="https://w3id.org/omop/ontology/has_drug_exposure"/>
  </rdf:Description>
  <rdf:Description rdf:about="https://w3id.org/omop/ontology/text">
    <rdf:type rdf:resource="http://www.w3.org/2002/07/owl#DatatypeProperty"/>
    <rdf:type rdf:resource="http://www.w3.org/2002/07/owl#FunctionalProperty"/>
    <rdfs:comment xml:lang="en">(for Note:) The content of the note.</rdfs:comment>
    <rdfs:domain rdf:resource="https://w3id.org/omop/ontology/Note"/>
    <rdfs:range rdf:resource="http://www.w3.org/2001/XMLSchema#string"/>
    <ns1:omop_cdm_name rdf:datatype="http://www.w3.org/2001/XMLSchema#string">note.note_text#186 AS str</ns1:omop_cdm_name>
  </rdf:Description>
  <rdf:Description rdf:nodeID="nde7e53d44aa94269b5c0c83d6d8798ccb668">
    <rdf:type rdf:resource="http://www.w3.org/2002/07/owl#Restriction"/>
    <owl:allValuesFrom rdf:resource="https://w3id.org/omop/ontology/Specimen"/>
    <owl:onProperty rdf:resource="https://w3id.org/omop/ontology/has_specimen"/>
  </rdf:Description>
  <rdf:Description rdf:nodeID="nde7e53d44aa94269b5c0c83d6d8798ccb156">
    <rdf:type rdf:resource="http://www.w3.org/2002/07/owl#Restriction"/>
    <owl:allValuesFrom rdf:resource="http://www.w3.org/2001/XMLSchema#integer"/>
    <owl:onProperty rdf:resource="https://w3id.org/omop/ontology/fact_id_2"/>
  </rdf:Description>
  <rdf:Description rdf:nodeID="nde7e53d44aa94269b5c0c83d6d8798ccb656">
    <rdf:type rdf:resource="http://www.w3.org/2002/07/owl#Restriction"/>
    <owl:allValuesFrom rdf:resource="https://w3id.org/omop/ontology/Concept"/>
    <owl:onProperty rdf:resource="https://w3id.org/omop/ontology/has_race"/>
  </rdf:Description>
  <rdf:Description rdf:nodeID="nde7e53d44aa94269b5c0c83d6d8798ccb458">
    <rdf:type rdf:resource="http://www.w3.org/2002/07/owl#Restriction"/>
    <owl:allValuesFrom rdf:resource="https://w3id.org/omop/ontology/Concept"/>
    <owl:onProperty rdf:resource="https://w3id.org/omop/ontology/has_concept"/>
  </rdf:Description>
  <rdf:Description rdf:nodeID="nde7e53d44aa94269b5c0c83d6d8798ccb175">
    <rdf:type rdf:resource="http://www.w3.org/2002/07/owl#Restriction"/>
    <owl:allValuesFrom rdf:resource="https://w3id.org/omop/ontology/Relationship"/>
    <owl:onProperty rdf:resource="https://w3id.org/omop/ontology/has_relationship"/>
  </rdf:Description>
  <rdf:Description rdf:nodeID="nde7e53d44aa94269b5c0c83d6d8798ccb596">
    <rdf:type rdf:resource="http://www.w3.org/2002/07/owl#Restriction"/>
    <owl:allValuesFrom rdf:resource="http://www.w3.org/2001/XMLSchema#date"/>
    <owl:onProperty rdf:resource="https://w3id.org/omop/ontology/survey_start_date"/>
  </rdf:Description>
  <rdf:Description rdf:nodeID="nde7e53d44aa94269b5c0c83d6d8798ccb18">
    <rdf:first rdf:resource="https://w3id.org/omop/ontology/Observation"/>
    <rdf:rest rdf:nodeID="nde7e53d44aa94269b5c0c83d6d8798ccb19"/>
  </rdf:Description>
  <rdf:Description rdf:nodeID="nde7e53d44aa94269b5c0c83d6d8798ccb357">
    <rdf:type rdf:resource="http://www.w3.org/2002/07/owl#Restriction"/>
    <owl:allValuesFrom rdf:resource="https://w3id.org/omop/ontology/VisitOccurrence"/>
    <owl:onProperty rdf:resource="https://w3id.org/omop/ontology/has_preceding_visit_occurrence"/>
  </rdf:Description>
  <rdf:Description rdf:nodeID="nde7e53d44aa94269b5c0c83d6d8798ccb678">
    <rdf:type rdf:resource="http://www.w3.org/2002/07/owl#Restriction"/>
    <owl:onProperty rdf:resource="https://w3id.org/omop/ontology/has_domain"/>
    <owl:someValuesFrom rdf:resource="https://w3id.org/omop/ontology/Domain"/>
  </rdf:Description>
  <rdf:Description rdf:nodeID="nde7e53d44aa94269b5c0c83d6d8798ccb287">
    <rdf:type rdf:resource="http://www.w3.org/2002/07/owl#Restriction"/>
    <owl:allValuesFrom rdf:resource="https://w3id.org/omop/ontology/Concept"/>
    <owl:onProperty rdf:resource="https://w3id.org/omop/ontology/has_status"/>
  </rdf:Description>
  <rdf:Description rdf:nodeID="nde7e53d44aa94269b5c0c83d6d8798ccb392">
    <rdf:type rdf:resource="http://www.w3.org/2002/07/owl#Restriction"/>
    <owl:allValuesFrom rdf:resource="http://www.w3.org/2001/XMLSchema#string"/>
    <owl:onProperty rdf:resource="https://w3id.org/omop/ontology/unit_source_value"/>
  </rdf:Description>
  <rdf:Description rdf:about="https://w3id.org/omop/ontology/timing_source_value">
    <rdf:type rdf:resource="http://www.w3.org/2002/07/owl#DatatypeProperty"/>
    <rdf:type rdf:resource="http://www.w3.org/2002/07/owl#FunctionalProperty"/>
    <rdfs:comment xml:lang="en">(for SurveyConduct:) Text string representing the timing of the survey. Example: Baseline, 6-month follow-up.</rdfs:comment>
    <rdfs:domain rdf:resource="https://w3id.org/omop/ontology/SurveyConduct"/>
    <rdfs:range rdf:resource="http://www.w3.org/2001/XMLSchema#string"/>
    <ns1:omop_cdm_name rdf:datatype="http://www.w3.org/2001/XMLSchema#string">survey_conduct.timing_source_value#241 AS str</ns1:omop_cdm_name>
  </rdf:Description>
  <rdf:Description rdf:nodeID="nde7e53d44aa94269b5c0c83d6d8798ccb264">
    <rdf:type rdf:resource="http://www.w3.org/2002/07/owl#Class"/>
    <owl:unionOf rdf:nodeID="nde7e53d44aa94269b5c0c83d6d8798ccb265"/>
  </rdf:Description>
  <rdf:Description rdf:about="https://w3id.org/omop/ontology/Domain">
    <rdf:type rdf:resource="http://www.w3.org/2002/07/owl#Class"/>
    <rdfs:subClassOf rdf:nodeID="nde7e53d44aa94269b5c0c83d6d8798ccb199"/>
    <rdfs:subClassOf rdf:nodeID="nde7e53d44aa94269b5c0c83d6d8798ccb200"/>
    <rdfs:subClassOf rdf:nodeID="nde7e53d44aa94269b5c0c83d6d8798ccb201"/>
    <rdfs:subClassOf rdf:nodeID="nde7e53d44aa94269b5c0c83d6d8798ccb202"/>
    <rdfs:subClassOf rdf:resource="https://w3id.org/omop/ontology/OmopCDMThing"/>
    <ns1:omop_cdm_name rdf:datatype="http://www.w3.org/2001/XMLSchema#string">domain</ns1:omop_cdm_name>
  </rdf:Description>
  <rdf:Description rdf:nodeID="nde7e53d44aa94269b5c0c83d6d8798ccb328">
    <rdf:type rdf:resource="http://www.w3.org/2002/07/owl#Restriction"/>
    <owl:allValuesFrom rdf:resource="https://w3id.org/omop/ontology/Concept"/>
    <owl:onProperty rdf:resource="https://w3id.org/omop/ontology/has_denominator_unit"/>
  </rdf:Description>
  <rdf:Description rdf:about="https://w3id.org/omop/ontology/cdm_version">
    <rdf:type rdf:resource="http://www.w3.org/2002/07/owl#DatatypeProperty"/>
    <rdf:type rdf:resource="http://www.w3.org/2002/07/owl#FunctionalProperty"/>
    <rdfs:domain rdf:resource="https://w3id.org/omop/ontology/CdmSource"/>
    <rdfs:range rdf:resource="http://www.w3.org/2001/XMLSchema#string"/>
    <ns1:omop_cdm_name rdf:datatype="http://www.w3.org/2001/XMLSchema#string">cdm_source.cdm_version#360 AS str</ns1:omop_cdm_name>
  </rdf:Description>
  <rdf:Description rdf:nodeID="nde7e53d44aa94269b5c0c83d6d8798ccb556">
    <rdf:type rdf:resource="http://www.w3.org/2002/07/owl#Restriction"/>
    <owl:onProperty rdf:resource="https://w3id.org/omop/ontology/contract_source_value"/>
    <owl:someValuesFrom rdf:resource="http://www.w3.org/2001/XMLSchema#string"/>
  </rdf:Description>
  <rdf:Description rdf:nodeID="nde7e53d44aa94269b5c0c83d6d8798ccb319">
    <rdf:type rdf:resource="http://www.w3.org/2002/07/owl#Restriction"/>
    <owl:onProperty rdf:nodeID="nde7e53d44aa94269b5c0c83d6d8798ccb320"/>
    <owl:someValuesFrom rdf:resource="https://w3id.org/omop/ontology/Person"/>
  </rdf:Description>
  <rdf:Description rdf:nodeID="nde7e53d44aa94269b5c0c83d6d8798ccb603">
    <rdf:type rdf:resource="http://www.w3.org/2002/07/owl#Restriction"/>
    <owl:allValuesFrom rdf:resource="https://w3id.org/omop/ontology/Concept"/>
    <owl:onProperty rdf:resource="https://w3id.org/omop/ontology/has_validated_survey"/>
  </rdf:Description>
  <rdf:Description rdf:nodeID="nde7e53d44aa94269b5c0c83d6d8798ccb332">
    <rdf:type rdf:resource="http://www.w3.org/2002/07/owl#Restriction"/>
    <owl:onProperty rdf:resource="https://w3id.org/omop/ontology/valid_start_date"/>
    <owl:someValuesFrom rdf:resource="http://www.w3.org/2001/XMLSchema#date"/>
  </rdf:Description>
  <rdf:Description rdf:nodeID="nde7e53d44aa94269b5c0c83d6d8798ccb111">
    <rdf:type rdf:resource="http://www.w3.org/2002/07/owl#Restriction"/>
    <owl:onProperty rdf:resource="https://w3id.org/omop/ontology/has_entity"/>
    <owl:someValuesFrom rdf:resource="http://www.w3.org/2002/07/owl#Thing"/>
  </rdf:Description>
  <rdf:Description rdf:nodeID="nde7e53d44aa94269b5c0c83d6d8798ccb617">
    <rdf:type rdf:resource="http://www.w3.org/2002/07/owl#Restriction"/>
    <owl:allValuesFrom rdf:resource="http://www.w3.org/2001/XMLSchema#string"/>
    <owl:onProperty rdf:resource="https://w3id.org/omop/ontology/respondent_type_source_value"/>
  </rdf:Description>
  <rdf:Description rdf:about="https://w3id.org/omop/ontology/term_temporal">
    <rdf:type rdf:resource="http://www.w3.org/2002/07/owl#DatatypeProperty"/>
    <rdf:type rdf:resource="http://www.w3.org/2002/07/owl#FunctionalProperty"/>
    <rdfs:comment xml:lang="en">(for NoteNlp:) Term_temporal is to indicate if a condition is present or just in the past. The following would be past:&lt;br&gt;&lt;br&gt;
- History = true
- Concept_date = anything before the time of the report</rdfs:comment>
    <rdfs:domain rdf:resource="https://w3id.org/omop/ontology/NoteNlp"/>
    <rdfs:range rdf:resource="http://www.w3.org/2001/XMLSchema#string"/>
    <ns1:omop_cdm_name rdf:datatype="http://www.w3.org/2001/XMLSchema#string">note_nlp.term_temporal#205 AS str</ns1:omop_cdm_name>
  </rdf:Description>
  <rdf:Description rdf:nodeID="nde7e53d44aa94269b5c0c83d6d8798ccb2">
    <rdf:type rdf:resource="http://www.w3.org/2002/07/owl#Restriction"/>
    <owl:allValuesFrom rdf:resource="https://w3id.org/omop/ontology/CohortDefinition"/>
    <owl:onProperty rdf:resource="https://w3id.org/omop/ontology/has_definition"/>
  </rdf:Description>
  <rdf:Description rdf:about="https://w3id.org/omop/ontology/reference">
    <rdf:type rdf:resource="http://www.w3.org/2002/07/owl#DatatypeProperty"/>
    <rdf:type rdf:resource="http://www.w3.org/2002/07/owl#FunctionalProperty"/>
    <rdfs:comment xml:lang="en">(for Vocabulary:) External reference to documentation or
available download of the about the
vocabulary.</rdfs:comment>
    <rdfs:domain rdf:resource="https://w3id.org/omop/ontology/Vocabulary"/>
    <rdfs:range rdf:resource="http://www.w3.org/2001/XMLSchema#string"/>
    <ns1:omop_cdm_name rdf:datatype="http://www.w3.org/2001/XMLSchema#string">vocabulary.vocabulary_reference#374 AS str</ns1:omop_cdm_name>
  </rdf:Description>
  <rdf:Description rdf:nodeID="nde7e53d44aa94269b5c0c83d6d8798ccb410">
    <rdf:type rdf:resource="http://www.w3.org/2002/07/owl#Restriction"/>
    <owl:allValuesFrom rdf:resource="http://www.w3.org/2001/XMLSchema#string"/>
    <owl:onProperty rdf:resource="https://w3id.org/omop/ontology/address_1"/>
  </rdf:Description>
  <rdf:Description rdf:nodeID="nde7e53d44aa94269b5c0c83d6d8798ccb146">
    <rdf:first rdf:resource="https://w3id.org/omop/ontology/DrugExposure"/>
    <rdf:rest rdf:nodeID="nde7e53d44aa94269b5c0c83d6d8798ccb147"/>
  </rdf:Description>
  <rdf:Description rdf:nodeID="nde7e53d44aa94269b5c0c83d6d8798ccb227">
    <rdf:type rdf:resource="http://www.w3.org/2002/07/owl#Class"/>
    <owl:unionOf rdf:nodeID="nde7e53d44aa94269b5c0c83d6d8798ccb228"/>
  </rdf:Description>
  <rdf:Description rdf:nodeID="nde7e53d44aa94269b5c0c83d6d8798ccb586">
    <rdf:first rdf:resource="http://www.w3.org/2001/XMLSchema#string"/>
    <rdf:rest rdf:resource="http://www.w3.org/1999/02/22-rdf-syntax-ns#nil"/>
  </rdf:Description>
  <rdf:Description rdf:nodeID="nde7e53d44aa94269b5c0c83d6d8798ccb224">
    <rdf:type rdf:resource="http://www.w3.org/2002/07/owl#Restriction"/>
    <owl:allValuesFrom rdf:resource="https://w3id.org/omop/ontology/Concept"/>
    <owl:onProperty rdf:resource="https://w3id.org/omop/ontology/has_place_of_service"/>
  </rdf:Description>
  <rdf:Description rdf:nodeID="nde7e53d44aa94269b5c0c83d6d8798ccb642">
    <rdf:type rdf:resource="http://www.w3.org/2002/07/owl#Restriction"/>
    <owl:allValuesFrom rdf:resource="http://www.w3.org/2001/XMLSchema#integer"/>
    <owl:onProperty rdf:resource="https://w3id.org/omop/ontology/month_of_birth"/>
  </rdf:Description>
  <rdf:Description rdf:nodeID="nde7e53d44aa94269b5c0c83d6d8798ccb50">
    <rdf:first rdf:resource="https://w3id.org/omop/ontology/Cost"/>
    <rdf:rest rdf:resource="http://www.w3.org/1999/02/22-rdf-syntax-ns#nil"/>
  </rdf:Description>
  <rdf:Description rdf:about="https://w3id.org/omop/ontology/has_sponsor_source">
    <rdf:type rdf:resource="http://www.w3.org/2002/07/owl#FunctionalProperty"/>
    <rdf:type rdf:resource="http://www.w3.org/2002/07/owl#ObjectProperty"/>
    <ns2:python_name rdf:datatype="http://www.w3.org/2001/XMLSchema#string">sponsor_source</ns2:python_name>
    <rdfs:comment xml:lang="en">(for PayerPlanPeriod:) If the source data codes the sponsor in an OMOP supported vocabulary store the concept_id here.</rdfs:comment>
    <rdfs:domain rdf:resource="https://w3id.org/omop/ontology/PayerPlanPeriod"/>
    <rdfs:range rdf:resource="https://w3id.org/omop/ontology/Concept"/>
    <ns1:omop_cdm_name rdf:datatype="http://www.w3.org/2001/XMLSchema#string">payer_plan_period.sponsor_source_concept_id#302 AS Concept</ns1:omop_cdm_name>
  </rdf:Description>
  <rdf:Description rdf:nodeID="nde7e53d44aa94269b5c0c83d6d8798ccb383">
    <rdf:type rdf:resource="http://www.w3.org/2002/07/owl#Restriction"/>
    <owl:allValuesFrom rdf:resource="https://w3id.org/omop/ontology/Concept"/>
    <owl:onProperty rdf:resource="https://w3id.org/omop/ontology/has_route"/>
  </rdf:Description>
  <rdf:Description rdf:nodeID="nde7e53d44aa94269b5c0c83d6d8798ccb633">
    <rdf:first rdf:resource="https://w3id.org/omop/ontology/Specimen"/>
    <rdf:rest rdf:nodeID="nde7e53d44aa94269b5c0c83d6d8798ccb634"/>
  </rdf:Description>
  <rdf:Description rdf:about="https://w3id.org/omop/ontology/year_of_birth">
    <rdf:type rdf:resource="http://www.w3.org/2002/07/owl#DatatypeProperty"/>
    <rdf:type rdf:resource="http://www.w3.org/2002/07/owl#FunctionalProperty"/>
    <rdfs:comment xml:lang="en">(for Person:) Compute age using year_of_birth.
For data sources with date of birth, the year should be extracted. For data sources where the year of birth is not available, the approximate year of birth could be derived based on age group categorization, if available.</rdfs:comment>
    <rdfs:domain rdf:nodeID="nde7e53d44aa94269b5c0c83d6d8798ccb77"/>
    <rdfs:range rdf:resource="http://www.w3.org/2001/XMLSchema#integer"/>
    <ns1:omop_cdm_name rdf:datatype="http://www.w3.org/2001/XMLSchema#string">person.year_of_birth#3 AS int</ns1:omop_cdm_name>
    <ns1:omop_cdm_name rdf:datatype="http://www.w3.org/2001/XMLSchema#string">provider.year_of_birth#279 AS int</ns1:omop_cdm_name>
  </rdf:Description>
  <rdf:Description rdf:nodeID="nde7e53d44aa94269b5c0c83d6d8798ccb505">
    <rdf:type rdf:resource="http://www.w3.org/2002/07/owl#Restriction"/>
    <owl:onProperty rdf:resource="https://w3id.org/omop/ontology/has_event_field"/>
    <owl:someValuesFrom rdf:resource="https://w3id.org/omop/ontology/Concept"/>
  </rdf:Description>
  <rdf:Description rdf:nodeID="nde7e53d44aa94269b5c0c83d6d8798ccb515">
    <rdf:type rdf:resource="http://www.w3.org/2002/07/owl#Restriction"/>
    <owl:allValuesFrom rdf:resource="http://www.w3.org/2001/XMLSchema#string"/>
    <owl:onProperty rdf:resource="https://w3id.org/omop/ontology/value_as_string"/>
  </rdf:Description>
  <rdf:Description rdf:nodeID="nde7e53d44aa94269b5c0c83d6d8798ccb664">
    <rdf:type rdf:resource="http://www.w3.org/2002/07/owl#Restriction"/>
    <owl:allValuesFrom rdf:resource="https://w3id.org/omop/ontology/Measurement"/>
    <owl:onProperty rdf:resource="https://w3id.org/omop/ontology/has_measurement"/>
  </rdf:Description>
  <rdf:Description rdf:about="https://w3id.org/omop/ontology/cost">
    <rdf:type rdf:resource="http://www.w3.org/2002/07/owl#DatatypeProperty"/>
    <rdf:type rdf:resource="http://www.w3.org/2002/07/owl#FunctionalProperty"/>
    <rdfs:comment xml:lang="en">(for Cost:) The actual financial cost amount</rdfs:comment>
    <rdfs:domain rdf:resource="https://w3id.org/omop/ontology/Cost"/>
    <rdfs:range rdf:resource="http://www.w3.org/2001/XMLSchema#decimal"/>
    <ns1:omop_cdm_name rdf:datatype="http://www.w3.org/2001/XMLSchema#string">cost.cost#316 AS float</ns1:omop_cdm_name>
  </rdf:Description>
  <rdf:Description rdf:nodeID="nde7e53d44aa94269b5c0c83d6d8798ccb404">
    <rdf:type rdf:resource="http://www.w3.org/2002/07/owl#Restriction"/>
    <owl:allValuesFrom rdf:resource="http://www.w3.org/2001/XMLSchema#string"/>
    <owl:onProperty rdf:resource="https://w3id.org/omop/ontology/name"/>
  </rdf:Description>
  <rdf:Description rdf:nodeID="nde7e53d44aa94269b5c0c83d6d8798ccb372">
    <rdf:first rdf:resource="https://w3id.org/omop/ontology/Measurement"/>
    <rdf:rest rdf:resource="http://www.w3.org/1999/02/22-rdf-syntax-ns#nil"/>
  </rdf:Description>
  <rdf:Description rdf:nodeID="nde7e53d44aa94269b5c0c83d6d8798ccb473">
    <rdf:type rdf:resource="http://www.w3.org/2002/07/owl#Restriction"/>
    <owl:onProperty rdf:resource="https://w3id.org/omop/ontology/has_specialty_source"/>
    <owl:someValuesFrom rdf:resource="https://w3id.org/omop/ontology/Concept"/>
  </rdf:Description>
  <rdf:Description rdf:about="https://w3id.org/omop/ontology/has_contract_person">
    <rdf:type rdf:resource="http://www.w3.org/2002/07/owl#FunctionalProperty"/>
    <rdf:type rdf:resource="http://www.w3.org/2002/07/owl#ObjectProperty"/>
    <ns2:python_name rdf:datatype="http://www.w3.org/2001/XMLSchema#string">contract_person</ns2:python_name>
    <rdfs:comment xml:lang="en">(for PayerPlanPeriod:) The Person who is the primary subscriber/contract owner for Plan.
This may or may not be the same as the PERSON_ID. For example, if a mother has her son on her plan and the PAYER_PLAN_PERIOD record is the for son, the sons's PERSON_ID would go in PAYER_PLAN_PERIOD.PERSON_ID and the mother's PERSON_ID would go in PAYER_PLAN_PERIOD.CONTRACT_PERSON_ID.</rdfs:comment>
    <rdfs:domain rdf:resource="https://w3id.org/omop/ontology/PayerPlanPeriod"/>
    <rdfs:range rdf:resource="https://w3id.org/omop/ontology/Person"/>
    <ns1:omop_cdm_name rdf:datatype="http://www.w3.org/2001/XMLSchema#string">payer_plan_period.contract_person_id#288 AS Person</ns1:omop_cdm_name>
  </rdf:Description>
  <rdf:Description rdf:nodeID="nde7e53d44aa94269b5c0c83d6d8798ccb214">
    <rdf:type rdf:resource="http://www.w3.org/2002/07/owl#Restriction"/>
    <owl:allValuesFrom rdf:resource="http://www.w3.org/2001/XMLSchema#string"/>
    <owl:onProperty rdf:resource="https://w3id.org/omop/ontology/name"/>
  </rdf:Description>
  <rdf:Description rdf:nodeID="nde7e53d44aa94269b5c0c83d6d8798ccb56">
    <rdf:first rdf:resource="https://w3id.org/omop/ontology/Person"/>
    <rdf:rest rdf:resource="http://www.w3.org/1999/02/22-rdf-syntax-ns#nil"/>
  </rdf:Description>
  <rdf:Description rdf:nodeID="nde7e53d44aa94269b5c0c83d6d8798ccb663">
    <rdf:type rdf:resource="http://www.w3.org/2002/07/owl#Restriction"/>
    <owl:allValuesFrom rdf:resource="https://w3id.org/omop/ontology/VisitOccurrence"/>
    <owl:onProperty rdf:resource="https://w3id.org/omop/ontology/has_visit_occurrence"/>
  </rdf:Description>
  <rdf:Description rdf:about="https://w3id.org/omop/ontology/qualifier_source_value">
    <rdf:type rdf:resource="http://www.w3.org/2002/07/owl#DatatypeProperty"/>
    <rdf:type rdf:resource="http://www.w3.org/2002/07/owl#FunctionalProperty"/>
    <rdfs:comment xml:lang="en">(for Observation:) This field houses the verbatim value from the source data representing the qualifier of the Observation that occurred.
This code is mapped to a Standard Condition Concept in the Standardized Vocabularies and the original code is stored here for reference.</rdfs:comment>
    <rdfs:domain rdf:resource="https://w3id.org/omop/ontology/Observation"/>
    <rdfs:range rdf:resource="http://www.w3.org/2001/XMLSchema#string"/>
    <ns1:omop_cdm_name rdf:datatype="http://www.w3.org/2001/XMLSchema#string">observation.qualifier_source_value#166 AS str</ns1:omop_cdm_name>
  </rdf:Description>
  <rdf:Description rdf:nodeID="nde7e53d44aa94269b5c0c83d6d8798ccb167">
    <rdf:type rdf:resource="http://www.w3.org/2002/07/owl#Restriction"/>
    <owl:onProperty rdf:resource="https://w3id.org/omop/ontology/has_type"/>
    <owl:someValuesFrom rdf:resource="https://w3id.org/omop/ontology/Concept"/>
  </rdf:Description>
  <rdf:Description rdf:nodeID="nde7e53d44aa94269b5c0c83d6d8798ccb573">
    <rdf:first rdf:resource="https://w3id.org/omop/ontology/Concept"/>
    <rdf:rest rdf:nodeID="nde7e53d44aa94269b5c0c83d6d8798ccb574"/>
  </rdf:Description>
  <rdf:Description rdf:nodeID="nde7e53d44aa94269b5c0c83d6d8798ccb593">
    <rdf:type rdf:resource="http://www.w3.org/2002/07/owl#Restriction"/>
    <owl:allValuesFrom rdf:resource="http://www.w3.org/2001/XMLSchema#dateTime"/>
    <owl:onProperty rdf:resource="https://w3id.org/omop/ontology/survey_start_datetime"/>
  </rdf:Description>
  <rdf:Description rdf:nodeID="nde7e53d44aa94269b5c0c83d6d8798ccb609">
    <rdf:type rdf:resource="http://www.w3.org/2002/07/owl#Restriction"/>
    <owl:onProperty rdf:resource="https://w3id.org/omop/ontology/has_collection_method"/>
    <owl:someValuesFrom rdf:resource="https://w3id.org/omop/ontology/Concept"/>
  </rdf:Description>
  <rdf:Description rdf:nodeID="nde7e53d44aa94269b5c0c83d6d8798ccb269">
    <rdf:first rdf:resource="https://w3id.org/omop/ontology/Observation"/>
    <rdf:rest rdf:nodeID="nde7e53d44aa94269b5c0c83d6d8798ccb270"/>
  </rdf:Description>
  <rdf:Description rdf:nodeID="nde7e53d44aa94269b5c0c83d6d8798ccb157">
    <rdf:type rdf:resource="http://www.w3.org/2002/07/owl#Restriction"/>
    <owl:onProperty rdf:resource="https://w3id.org/omop/ontology/fact_id_2"/>
    <owl:someValuesFrom rdf:resource="http://www.w3.org/2001/XMLSchema#integer"/>
  </rdf:Description>
  <rdf:Description rdf:nodeID="nde7e53d44aa94269b5c0c83d6d8798ccb187">
    <rdf:type rdf:resource="http://www.w3.org/2002/07/owl#Restriction"/>
    <owl:allValuesFrom rdf:resource="http://www.w3.org/2001/XMLSchema#dateTime"/>
    <owl:onProperty rdf:resource="https://w3id.org/omop/ontology/start_datetime"/>
  </rdf:Description>
  <rdf:Description rdf:nodeID="nde7e53d44aa94269b5c0c83d6d8798ccb519">
    <rdf:type rdf:resource="http://www.w3.org/2002/07/owl#Restriction"/>
    <owl:allValuesFrom rdf:resource="https://w3id.org/omop/ontology/Concept"/>
    <owl:onProperty rdf:resource="https://w3id.org/omop/ontology/has_value_as_concept"/>
  </rdf:Description>
  <rdf:Description rdf:nodeID="nde7e53d44aa94269b5c0c83d6d8798ccb506">
    <rdf:type rdf:resource="http://www.w3.org/2002/07/owl#Restriction"/>
    <owl:allValuesFrom rdf:resource="http://www.w3.org/2001/XMLSchema#date"/>
    <owl:onProperty rdf:resource="https://w3id.org/omop/ontology/paid_date"/>
  </rdf:Description>
  <rdf:Description rdf:nodeID="nde7e53d44aa94269b5c0c83d6d8798ccb323">
    <rdf:type rdf:resource="http://www.w3.org/2002/07/owl#Restriction"/>
    <owl:onProperty rdf:resource="https://w3id.org/omop/ontology/has_ingredient"/>
    <owl:someValuesFrom rdf:resource="https://w3id.org/omop/ontology/Concept"/>
  </rdf:Description>
  <rdf:Description rdf:nodeID="nde7e53d44aa94269b5c0c83d6d8798ccb374">
    <rdf:type rdf:resource="http://www.w3.org/2002/07/owl#Restriction"/>
    <owl:allValuesFrom rdf:resource="http://www.w3.org/2001/XMLSchema#decimal"/>
    <owl:onProperty rdf:resource="https://w3id.org/omop/ontology/quantity"/>
  </rdf:Description>
  <rdf:Description rdf:nodeID="nde7e53d44aa94269b5c0c83d6d8798ccb537">
    <rdf:type rdf:resource="http://www.w3.org/2002/07/owl#Restriction"/>
    <owl:allValuesFrom rdf:resource="https://w3id.org/omop/ontology/Concept"/>
    <owl:onProperty rdf:resource="https://w3id.org/omop/ontology/has_payer"/>
  </rdf:Description>
  <rdf:Description rdf:nodeID="nde7e53d44aa94269b5c0c83d6d8798ccb308">
    <rdf:type rdf:resource="http://www.w3.org/2002/07/owl#Restriction"/>
    <owl:onProperty rdf:resource="https://w3id.org/omop/ontology/has_concept"/>
    <owl:someValuesFrom rdf:resource="https://w3id.org/omop/ontology/Concept"/>
  </rdf:Description>
  <rdf:Description rdf:nodeID="nde7e53d44aa94269b5c0c83d6d8798ccb5">
    <rdf:type rdf:resource="http://www.w3.org/2002/07/owl#Class"/>
    <owl:unionOf rdf:nodeID="nde7e53d44aa94269b5c0c83d6d8798ccb6"/>
  </rdf:Description>
  <rdf:Description rdf:about="https://w3id.org/omop/ontology/has_survey_conduct">
    <rdf:type rdf:resource="http://www.w3.org/2002/07/owl#ObjectProperty"/>
    <ns2:python_name rdf:datatype="http://www.w3.org/2001/XMLSchema#string">survey_conducts</ns2:python_name>
    <rdfs:comment xml:lang="en">(reversed relation, for SurveyConduct:) The Visit during which the Survey occurred.</rdfs:comment>
    <rdfs:domain rdf:nodeID="nde7e53d44aa94269b5c0c83d6d8798ccb66"/>
    <rdfs:range rdf:resource="https://w3id.org/omop/ontology/SurveyConduct"/>
    <ns1:omop_cdm_name rdf:datatype="http://www.w3.org/2001/XMLSchema#string">survey_conduct.person_id#228 AS Person</ns1:omop_cdm_name>
    <ns1:omop_cdm_name rdf:datatype="http://www.w3.org/2001/XMLSchema#string">survey_conduct.visit_occurrence_id#249 AS VisitOccurrence</ns1:omop_cdm_name>
  </rdf:Description>
  <rdf:Description rdf:nodeID="nde7e53d44aa94269b5c0c83d6d8798ccb112">
    <rdf:type rdf:resource="http://www.w3.org/2002/07/owl#Class"/>
    <owl:unionOf rdf:nodeID="nde7e53d44aa94269b5c0c83d6d8798ccb113"/>
  </rdf:Description>
  <rdf:Description rdf:nodeID="nde7e53d44aa94269b5c0c83d6d8798ccb607">
    <rdf:type rdf:resource="http://www.w3.org/2002/07/owl#Restriction"/>
    <owl:onProperty rdf:nodeID="nde7e53d44aa94269b5c0c83d6d8798ccb608"/>
    <owl:someValuesFrom rdf:resource="https://w3id.org/omop/ontology/Person"/>
  </rdf:Description>
  <rdf:Description rdf:nodeID="nde7e53d44aa94269b5c0c83d6d8798ccb248">
    <rdf:type rdf:resource="http://www.w3.org/2002/07/owl#Restriction"/>
    <owl:allValuesFrom rdf:resource="http://www.w3.org/2001/XMLSchema#string"/>
    <owl:onProperty rdf:resource="https://w3id.org/omop/ontology/source_code"/>
  </rdf:Description>
  <rdf:Description rdf:nodeID="nde7e53d44aa94269b5c0c83d6d8798ccb245">
    <rdf:type rdf:resource="http://www.w3.org/2002/07/owl#Restriction"/>
    <owl:allValuesFrom rdf:resource="https://w3id.org/omop/ontology/Concept"/>
    <owl:onProperty rdf:resource="https://w3id.org/omop/ontology/has_definition_type"/>
  </rdf:Description>
  <rdf:Description rdf:nodeID="nde7e53d44aa94269b5c0c83d6d8798ccb257">
    <rdf:type rdf:resource="http://www.w3.org/2002/07/owl#Restriction"/>
    <owl:allValuesFrom rdf:resource="http://www.w3.org/2001/XMLSchema#date"/>
    <owl:onProperty rdf:resource="https://w3id.org/omop/ontology/valid_end_date"/>
  </rdf:Description>
  <rdf:Description rdf:nodeID="nde7e53d44aa94269b5c0c83d6d8798ccb348">
    <rdf:type rdf:resource="http://www.w3.org/2002/07/owl#Restriction"/>
    <owl:allValuesFrom rdf:resource="http://www.w3.org/2001/XMLSchema#string"/>
    <owl:onProperty rdf:resource="https://w3id.org/omop/ontology/term_modifiers"/>
  </rdf:Description>
  <rdf:Description rdf:nodeID="nde7e53d44aa94269b5c0c83d6d8798ccb198">
    <rdf:type rdf:resource="http://www.w3.org/2002/07/owl#Restriction"/>
    <owl:allValuesFrom rdf:resource="https://w3id.org/omop/ontology/Concept"/>
    <owl:onProperty rdf:resource="https://w3id.org/omop/ontology/has_gender"/>
  </rdf:Description>
  <rdf:Description rdf:nodeID="nde7e53d44aa94269b5c0c83d6d8798ccb33">
    <rdf:type rdf:resource="http://www.w3.org/2002/07/owl#Class"/>
    <owl:unionOf rdf:nodeID="nde7e53d44aa94269b5c0c83d6d8798ccb34"/>
  </rdf:Description>
  <rdf:Description rdf:nodeID="nde7e53d44aa94269b5c0c83d6d8798ccb466">
    <rdf:type rdf:resource="http://www.w3.org/2002/07/owl#Restriction"/>
    <owl:onProperty rdf:resource="https://w3id.org/omop/ontology/has_concept"/>
    <owl:someValuesFrom rdf:resource="https://w3id.org/omop/ontology/Concept"/>
  </rdf:Description>
  <rdf:Description rdf:nodeID="nde7e53d44aa94269b5c0c83d6d8798ccb438">
    <rdf:type rdf:resource="http://www.w3.org/2002/07/owl#Restriction"/>
    <owl:onProperty rdf:resource="https://w3id.org/omop/ontology/has_discharge_to"/>
    <owl:someValuesFrom rdf:resource="https://w3id.org/omop/ontology/Concept"/>
  </rdf:Description>
  <rdf:Description rdf:about="https://w3id.org/omop/ontology/place_of_service_source_value">
    <rdf:type rdf:resource="http://www.w3.org/2002/07/owl#DatatypeProperty"/>
    <rdf:type rdf:resource="http://www.w3.org/2002/07/owl#FunctionalProperty"/>
    <rdfs:comment xml:lang="en">(for CareSite:) Put the place of service of the care_site as it appears in the source data.</rdfs:comment>
    <rdfs:domain rdf:resource="https://w3id.org/omop/ontology/CareSite"/>
    <rdfs:range rdf:resource="http://www.w3.org/2001/XMLSchema#string"/>
    <ns1:omop_cdm_name rdf:datatype="http://www.w3.org/2001/XMLSchema#string">care_site.place_of_service_source_value#272 AS str</ns1:omop_cdm_name>
  </rdf:Description>
  <rdf:Description rdf:about="https://w3id.org/omop/ontology/has_note_nlp">
    <rdf:type rdf:resource="http://www.w3.org/2002/07/owl#ObjectProperty"/>
    <ns2:python_name rdf:datatype="http://www.w3.org/2001/XMLSchema#string">note_nlps</ns2:python_name>
    <rdfs:comment xml:lang="en">(reversed relation, for NoteNlp:) This is the NOTE_ID for the NOTE record the NLP record is associated to.</rdfs:comment>
    <rdfs:domain rdf:resource="https://w3id.org/omop/ontology/Note"/>
    <rdfs:range rdf:resource="https://w3id.org/omop/ontology/NoteNlp"/>
    <ns1:omop_cdm_name rdf:datatype="http://www.w3.org/2001/XMLSchema#string">note_nlp.note_id#194 AS Note</ns1:omop_cdm_name>
  </rdf:Description>
  <rdf:Description rdf:nodeID="nde7e53d44aa94269b5c0c83d6d8798ccb541">
    <rdf:type rdf:resource="http://www.w3.org/2002/07/owl#Restriction"/>
    <owl:allValuesFrom rdf:resource="http://www.w3.org/2001/XMLSchema#string"/>
    <owl:onProperty rdf:resource="https://w3id.org/omop/ontology/stop_reason_source_value"/>
  </rdf:Description>
  <rdf:Description rdf:nodeID="nde7e53d44aa94269b5c0c83d6d8798ccb551">
    <rdf:type rdf:resource="http://www.w3.org/2002/07/owl#Restriction"/>
    <owl:allValuesFrom rdf:resource="http://www.w3.org/2001/XMLSchema#string"/>
    <owl:onProperty rdf:resource="https://w3id.org/omop/ontology/plan_source_value"/>
  </rdf:Description>
  <rdf:Description rdf:nodeID="nde7e53d44aa94269b5c0c83d6d8798ccb170">
    <rdf:type rdf:resource="http://www.w3.org/2002/07/owl#Class"/>
    <owl:unionOf rdf:nodeID="nde7e53d44aa94269b5c0c83d6d8798ccb171"/>
  </rdf:Description>
  <rdf:Description rdf:nodeID="nde7e53d44aa94269b5c0c83d6d8798ccb106">
    <rdf:type rdf:resource="http://www.w3.org/2002/07/owl#Restriction"/>
    <owl:allValuesFrom rdf:resource="https://w3id.org/omop/ontology/Location"/>
    <owl:onProperty rdf:resource="https://w3id.org/omop/ontology/has_location"/>
  </rdf:Description>
  <rdf:Description rdf:nodeID="nde7e53d44aa94269b5c0c83d6d8798ccb190">
    <rdf:type rdf:resource="http://www.w3.org/2002/07/owl#Restriction"/>
    <owl:allValuesFrom rdf:resource="https://w3id.org/omop/ontology/Concept"/>
    <owl:onProperty rdf:resource="https://w3id.org/omop/ontology/has_cause_source"/>
  </rdf:Description>
  <rdf:Description rdf:nodeID="nde7e53d44aa94269b5c0c83d6d8798ccb582">
    <rdf:first rdf:resource="https://w3id.org/omop/ontology/Vocabulary"/>
    <rdf:rest rdf:resource="http://www.w3.org/1999/02/22-rdf-syntax-ns#nil"/>
  </rdf:Description>
  <rdf:Description rdf:nodeID="nde7e53d44aa94269b5c0c83d6d8798ccb568">
    <rdf:first rdf:resource="https://w3id.org/omop/ontology/Exposure"/>
    <rdf:rest rdf:nodeID="nde7e53d44aa94269b5c0c83d6d8798ccb569"/>
  </rdf:Description>
  <rdf:Description rdf:nodeID="nde7e53d44aa94269b5c0c83d6d8798ccb79">
    <rdf:first rdf:resource="https://w3id.org/omop/ontology/Person"/>
    <rdf:rest rdf:resource="http://www.w3.org/1999/02/22-rdf-syntax-ns#nil"/>
  </rdf:Description>
  <rdf:Description rdf:nodeID="nde7e53d44aa94269b5c0c83d6d8798ccb196">
    <rdf:type rdf:resource="http://www.w3.org/2002/07/owl#Restriction"/>
    <owl:allValuesFrom rdf:resource="http://www.w3.org/2001/XMLSchema#string"/>
    <owl:onProperty rdf:resource="https://w3id.org/omop/ontology/source_value"/>
  </rdf:Description>
  <rdf:Description rdf:nodeID="nde7e53d44aa94269b5c0c83d6d8798ccb149">
    <owl:inverseOf rdf:resource="https://w3id.org/omop/ontology/has_device_exposure"/>
  </rdf:Description>
  <rdf:Description rdf:nodeID="nde7e53d44aa94269b5c0c83d6d8798ccb13">
    <rdf:first rdf:resource="https://w3id.org/omop/ontology/ConditionOccurrence"/>
    <rdf:rest rdf:resource="http://www.w3.org/1999/02/22-rdf-syntax-ns#nil"/>
  </rdf:Description>
  <rdf:Description rdf:nodeID="nde7e53d44aa94269b5c0c83d6d8798ccb543">
    <rdf:type rdf:resource="http://www.w3.org/2002/07/owl#Restriction"/>
    <owl:onProperty rdf:resource="https://w3id.org/omop/ontology/has_payer"/>
    <owl:someValuesFrom rdf:resource="https://w3id.org/omop/ontology/Concept"/>
  </rdf:Description>
  <rdf:Description rdf:nodeID="nde7e53d44aa94269b5c0c83d6d8798ccb511">
    <rdf:type rdf:resource="http://www.w3.org/2002/07/owl#Restriction"/>
    <owl:allValuesFrom rdf:resource="https://w3id.org/omop/ontology/Concept"/>
    <owl:onProperty rdf:resource="https://w3id.org/omop/ontology/has_source"/>
  </rdf:Description>
  <rdf:Description rdf:nodeID="nde7e53d44aa94269b5c0c83d6d8798ccb618">
    <rdf:type rdf:resource="http://www.w3.org/2002/07/owl#Restriction"/>
    <owl:allValuesFrom rdf:resource="http://www.w3.org/2001/XMLSchema#date"/>
    <owl:onProperty rdf:resource="https://w3id.org/omop/ontology/survey_end_date"/>
  </rdf:Description>
  <rdf:Description rdf:nodeID="nde7e53d44aa94269b5c0c83d6d8798ccb235">
    <rdf:first rdf:resource="https://w3id.org/omop/ontology/SourceToConceptMap"/>
    <rdf:rest rdf:nodeID="nde7e53d44aa94269b5c0c83d6d8798ccb236"/>
  </rdf:Description>
  <rdf:Description rdf:about="https://w3id.org/omop/ontology/Cohort">
    <rdf:type rdf:resource="http://www.w3.org/2002/07/owl#Class"/>
    <rdfs:subClassOf rdf:nodeID="nde7e53d44aa94269b5c0c83d6d8798ccb1"/>
    <rdfs:subClassOf rdf:nodeID="nde7e53d44aa94269b5c0c83d6d8798ccb2"/>
    <rdfs:subClassOf rdf:nodeID="nde7e53d44aa94269b5c0c83d6d8798ccb3"/>
    <rdfs:subClassOf rdf:nodeID="nde7e53d44aa94269b5c0c83d6d8798ccb4"/>
    <rdfs:subClassOf rdf:resource="https://w3id.org/omop/ontology/DateDuration"/>
    <ns1:omop_cdm_name rdf:datatype="http://www.w3.org/2001/XMLSchema#string">cohort</ns1:omop_cdm_name>
  </rdf:Description>
  <rdf:Description rdf:about="https://w3id.org/omop/ontology/survey_version_number">
    <rdf:type rdf:resource="http://www.w3.org/2002/07/owl#DatatypeProperty"/>
    <rdf:type rdf:resource="http://www.w3.org/2002/07/owl#FunctionalProperty"/>
    <rdfs:comment xml:lang="en">(for SurveyConduct:) Version number of the questionnaire or survey used.</rdfs:comment>
    <rdfs:domain rdf:resource="https://w3id.org/omop/ontology/SurveyConduct"/>
    <rdfs:range rdf:resource="http://www.w3.org/2001/XMLSchema#string"/>
    <ns1:omop_cdm_name rdf:datatype="http://www.w3.org/2001/XMLSchema#string">survey_conduct.survey_version_number#248 AS str</ns1:omop_cdm_name>
  </rdf:Description>
  <rdf:Description rdf:nodeID="nde7e53d44aa94269b5c0c83d6d8798ccb7">
    <rdf:first rdf:resource="https://w3id.org/omop/ontology/BasePerson"/>
    <rdf:rest rdf:resource="http://www.w3.org/1999/02/22-rdf-syntax-ns#nil"/>
  </rdf:Description>
  <rdf:Description rdf:nodeID="nde7e53d44aa94269b5c0c83d6d8798ccb83">
    <rdf:type rdf:resource="http://www.w3.org/2002/07/owl#Restriction"/>
    <owl:onProperty rdf:resource="https://w3id.org/omop/ontology/has_ancestor"/>
    <owl:someValuesFrom rdf:resource="https://w3id.org/omop/ontology/Concept"/>
  </rdf:Description>
  <rdf:Description rdf:nodeID="nde7e53d44aa94269b5c0c83d6d8798ccb241">
    <rdf:type rdf:resource="http://www.w3.org/2002/07/owl#Restriction"/>
    <owl:onProperty rdf:resource="https://w3id.org/omop/ontology/has_definition_type"/>
    <owl:someValuesFrom rdf:resource="https://w3id.org/omop/ontology/Concept"/>
  </rdf:Description>
  <rdf:Description rdf:nodeID="nde7e53d44aa94269b5c0c83d6d8798ccb185">
    <rdf:type rdf:resource="http://www.w3.org/2002/07/owl#Restriction"/>
    <owl:onProperty rdf:resource="https://w3id.org/omop/ontology/has_relationship"/>
    <owl:someValuesFrom rdf:resource="https://w3id.org/omop/ontology/Relationship"/>
  </rdf:Description>
  <rdf:Description rdf:nodeID="nde7e53d44aa94269b5c0c83d6d8798ccb290">
    <rdf:type rdf:resource="http://www.w3.org/2002/07/owl#Restriction"/>
    <owl:onProperty rdf:nodeID="nde7e53d44aa94269b5c0c83d6d8798ccb291"/>
    <owl:someValuesFrom rdf:resource="https://w3id.org/omop/ontology/Person"/>
  </rdf:Description>
  <rdf:Description rdf:nodeID="nde7e53d44aa94269b5c0c83d6d8798ccb58">
    <rdf:first rdf:resource="https://w3id.org/omop/ontology/BaseVisit"/>
    <rdf:rest rdf:nodeID="nde7e53d44aa94269b5c0c83d6d8798ccb59"/>
  </rdf:Description>
  <rdf:Description rdf:nodeID="nde7e53d44aa94269b5c0c83d6d8798ccb203">
    <rdf:type rdf:resource="http://www.w3.org/2002/07/owl#Restriction"/>
    <owl:allValuesFrom rdf:resource="https://w3id.org/omop/ontology/Concept"/>
    <owl:onProperty rdf:resource="https://w3id.org/omop/ontology/has_type"/>
  </rdf:Description>
  <rdf:Description rdf:nodeID="nde7e53d44aa94269b5c0c83d6d8798ccb559">
    <rdf:type rdf:resource="http://www.w3.org/2002/07/owl#Class"/>
    <owl:unionOf rdf:nodeID="nde7e53d44aa94269b5c0c83d6d8798ccb560"/>
  </rdf:Description>
  <rdf:Description rdf:nodeID="nde7e53d44aa94269b5c0c83d6d8798ccb522">
    <rdf:type rdf:resource="http://www.w3.org/2002/07/owl#Restriction"/>
    <owl:allValuesFrom rdf:resource="https://w3id.org/omop/ontology/Concept"/>
    <owl:onProperty rdf:resource="https://w3id.org/omop/ontology/has_source"/>
  </rdf:Description>
  <rdf:Description rdf:nodeID="nde7e53d44aa94269b5c0c83d6d8798ccb563">
    <rdf:first rdf:resource="https://w3id.org/omop/ontology/Specimen"/>
    <rdf:rest rdf:nodeID="nde7e53d44aa94269b5c0c83d6d8798ccb564"/>
  </rdf:Description>
  <rdf:Description rdf:nodeID="nde7e53d44aa94269b5c0c83d6d8798ccb344">
    <rdf:type rdf:resource="http://www.w3.org/2002/07/owl#Restriction"/>
    <owl:onProperty rdf:nodeID="nde7e53d44aa94269b5c0c83d6d8798ccb345"/>
    <owl:someValuesFrom rdf:resource="https://w3id.org/omop/ontology/Note"/>
  </rdf:Description>
  <rdf:Description rdf:nodeID="nde7e53d44aa94269b5c0c83d6d8798ccb595">
    <rdf:type rdf:resource="http://www.w3.org/2002/07/owl#Restriction"/>
    <owl:onProperty rdf:resource="https://w3id.org/omop/ontology/has_timing"/>
    <owl:someValuesFrom rdf:resource="https://w3id.org/omop/ontology/Concept"/>
  </rdf:Description>
  <rdf:Description rdf:nodeID="nde7e53d44aa94269b5c0c83d6d8798ccb387">
    <rdf:type rdf:resource="http://www.w3.org/2002/07/owl#Restriction"/>
    <owl:allValuesFrom rdf:resource="http://www.w3.org/2002/07/owl#Thing"/>
    <owl:onProperty rdf:resource="https://w3id.org/omop/ontology/has_source"/>
  </rdf:Description>
  <rdf:Description rdf:nodeID="nde7e53d44aa94269b5c0c83d6d8798ccb508">
    <rdf:type rdf:resource="http://www.w3.org/2002/07/owl#Restriction"/>
    <owl:allValuesFrom rdf:resource="https://w3id.org/omop/ontology/Concept"/>
    <owl:onProperty rdf:resource="https://w3id.org/omop/ontology/has_concept"/>
  </rdf:Description>
  <rdf:Description rdf:about="https://w3id.org/omop/ontology/value_source_value">
    <rdf:type rdf:resource="http://www.w3.org/2002/07/owl#DatatypeProperty"/>
    <rdf:type rdf:resource="http://www.w3.org/2002/07/owl#FunctionalProperty"/>
    <rdfs:comment xml:lang="en">(for Measurement:) This field houses the verbatim result value of the Measurement from the source data .
If both a continuous and categorical result are given in the source data such that both VALUE_AS_NUMBER and VALUE_AS_CONCEPT_ID are both included, store the verbatim value that was mapped to VALUE_AS_CONCEPT_ID here.</rdfs:comment>
    <rdfs:domain rdf:resource="https://w3id.org/omop/ontology/Measurement"/>
    <rdfs:range rdf:resource="http://www.w3.org/2001/XMLSchema#string"/>
    <ns1:omop_cdm_name rdf:datatype="http://www.w3.org/2001/XMLSchema#string">measurement.value_source_value#148 AS str</ns1:omop_cdm_name>
  </rdf:Description>
  <rdf:Description rdf:nodeID="nde7e53d44aa94269b5c0c83d6d8798ccb143">
    <rdf:type rdf:resource="http://www.w3.org/2002/07/owl#Class"/>
    <owl:unionOf rdf:nodeID="nde7e53d44aa94269b5c0c83d6d8798ccb144"/>
  </rdf:Description>
  <rdf:Description rdf:about="https://w3id.org/omop/ontology/ConditionOccurrence">
    <rdf:type rdf:resource="http://www.w3.org/2002/07/owl#Class"/>
    <rdfs:subClassOf rdf:nodeID="nde7e53d44aa94269b5c0c83d6d8798ccb287"/>
    <rdfs:subClassOf rdf:nodeID="nde7e53d44aa94269b5c0c83d6d8798ccb288"/>
    <rdfs:subClassOf rdf:nodeID="nde7e53d44aa94269b5c0c83d6d8798ccb289"/>
    <rdfs:subClassOf rdf:nodeID="nde7e53d44aa94269b5c0c83d6d8798ccb290"/>
    <rdfs:subClassOf rdf:nodeID="nde7e53d44aa94269b5c0c83d6d8798ccb292"/>
    <rdfs:subClassOf rdf:nodeID="nde7e53d44aa94269b5c0c83d6d8798ccb293"/>
    <rdfs:subClassOf rdf:nodeID="nde7e53d44aa94269b5c0c83d6d8798ccb294"/>
    <rdfs:subClassOf rdf:nodeID="nde7e53d44aa94269b5c0c83d6d8798ccb295"/>
    <rdfs:subClassOf rdf:nodeID="nde7e53d44aa94269b5c0c83d6d8798ccb296"/>
    <rdfs:subClassOf rdf:nodeID="nde7e53d44aa94269b5c0c83d6d8798ccb297"/>
    <rdfs:subClassOf rdf:nodeID="nde7e53d44aa94269b5c0c83d6d8798ccb298"/>
    <rdfs:subClassOf rdf:nodeID="nde7e53d44aa94269b5c0c83d6d8798ccb299"/>
    <rdfs:subClassOf rdf:nodeID="nde7e53d44aa94269b5c0c83d6d8798ccb300"/>
    <rdfs:subClassOf rdf:resource="https://w3id.org/omop/ontology/DateDuration"/>
    <rdfs:subClassOf rdf:resource="https://w3id.org/omop/ontology/DatetimeDuration"/>
    <rdfs:subClassOf rdf:resource="https://w3id.org/omop/ontology/Occurrence"/>
    <ns1:omop_cdm_name rdf:datatype="http://www.w3.org/2001/XMLSchema#string">condition_occurrence</ns1:omop_cdm_name>
  </rdf:Description>
  <rdf:Description rdf:about="https://w3id.org/omop/ontology/has_status">
    <rdf:type rdf:resource="http://www.w3.org/2002/07/owl#FunctionalProperty"/>
    <rdf:type rdf:resource="http://www.w3.org/2002/07/owl#ObjectProperty"/>
    <ns2:python_name rdf:datatype="http://www.w3.org/2001/XMLSchema#string">status</ns2:python_name>
    <rdfs:comment xml:lang="en">(for ConditionOccurrence:) This concept represents the point during the visit the diagnosis was given (admitting diagnosis, final diagnosis), whether the diagnosis was determined due to laboratory findings, if the diagnosis was exclusionary, or if it was a preliminary diagnosis, among others.
Choose the Concept in the Condition Status domain that best represents the point during the visit when the diagnosis was given. These can include admitting diagnosis, principal diagnosis, and secondary diagnosis. If not available, set to 0. [Accepted Concepts](https://athena.ohdsi.org/search-terms/terms?domain=Condition+Status&amp;standardConcept=Standard&amp;page=1&amp;pageSize=15&amp;query=).</rdfs:comment>
    <rdfs:domain rdf:resource="https://w3id.org/omop/ontology/ConditionOccurrence"/>
    <rdfs:range rdf:resource="https://w3id.org/omop/ontology/Concept"/>
    <ns1:omop_cdm_name rdf:datatype="http://www.w3.org/2001/XMLSchema#string">condition_occurrence.condition_status_concept_id#69 AS Concept</ns1:omop_cdm_name>
  </rdf:Description>
  <rdf:Description rdf:nodeID="nde7e53d44aa94269b5c0c83d6d8798ccb271">
    <rdf:first rdf:resource="https://w3id.org/omop/ontology/Exposure"/>
    <rdf:rest rdf:nodeID="nde7e53d44aa94269b5c0c83d6d8798ccb272"/>
  </rdf:Description>
  <rdf:Description rdf:nodeID="nde7e53d44aa94269b5c0c83d6d8798ccb85">
    <rdf:type rdf:resource="http://www.w3.org/2002/07/owl#Restriction"/>
    <owl:onProperty rdf:resource="https://w3id.org/omop/ontology/has_descendant"/>
    <owl:someValuesFrom rdf:resource="https://w3id.org/omop/ontology/Concept"/>
  </rdf:Description>
  <rdf:Description rdf:nodeID="nde7e53d44aa94269b5c0c83d6d8798ccb306">
    <rdf:type rdf:resource="http://www.w3.org/2002/07/owl#Restriction"/>
    <owl:allValuesFrom rdf:resource="https://w3id.org/omop/ontology/Concept"/>
    <owl:onProperty rdf:resource="https://w3id.org/omop/ontology/has_modifier"/>
  </rdf:Description>
  <rdf:Description rdf:nodeID="nde7e53d44aa94269b5c0c83d6d8798ccb349">
    <rdf:type rdf:resource="http://www.w3.org/2002/07/owl#Restriction"/>
    <owl:allValuesFrom rdf:resource="http://www.w3.org/2001/XMLSchema#string"/>
    <owl:onProperty rdf:resource="https://w3id.org/omop/ontology/offset"/>
  </rdf:Description>
  <rdf:Description rdf:nodeID="nde7e53d44aa94269b5c0c83d6d8798ccb524">
    <rdf:type rdf:resource="http://www.w3.org/2002/07/owl#Restriction"/>
    <owl:onProperty rdf:nodeID="nde7e53d44aa94269b5c0c83d6d8798ccb525"/>
    <owl:someValuesFrom rdf:resource="https://w3id.org/omop/ontology/Person"/>
  </rdf:Description>
  <rdf:Description rdf:nodeID="nde7e53d44aa94269b5c0c83d6d8798ccb299">
    <rdf:type rdf:resource="http://www.w3.org/2002/07/owl#Restriction"/>
    <owl:allValuesFrom rdf:resource="https://w3id.org/omop/ontology/Concept"/>
    <owl:onProperty rdf:resource="https://w3id.org/omop/ontology/has_concept"/>
  </rdf:Description>
  <rdf:Description rdf:nodeID="nde7e53d44aa94269b5c0c83d6d8798ccb613">
    <rdf:type rdf:resource="http://www.w3.org/2002/07/owl#Restriction"/>
    <owl:allValuesFrom rdf:resource="https://w3id.org/omop/ontology/Provider"/>
    <owl:onProperty rdf:resource="https://w3id.org/omop/ontology/has_provider"/>
  </rdf:Description>
  <rdf:Description rdf:about="https://w3id.org/omop/ontology/has_value_as_concept">
    <rdf:type rdf:resource="http://www.w3.org/2002/07/owl#FunctionalProperty"/>
    <rdf:type rdf:resource="http://www.w3.org/2002/07/owl#ObjectProperty"/>
    <ns2:python_name rdf:datatype="http://www.w3.org/2001/XMLSchema#string">value_as_concept</ns2:python_name>
    <rdfs:comment xml:lang="en">(for Measurement:) If the raw data gives a categorial result for measurements those values are captured and mapped to standard concepts in the 'Meas Value' domain.
If the raw data provides categorial results as well as continuous results for measurements, it is a valid ETL choice to preserve both values. The continuous value should go in the VALUE_AS_NUMBER field and the categorical value should be mapped to a standard concept in the 'Meas Value' domain and put in the VALUE_AS_CONCEPT_ID field. This is also the destination for the 'Maps to value' relationship.</rdfs:comment>
    <rdfs:comment xml:lang="en">(for Observation:) It is possible that some records destined for the Observation table have two clinical ideas represented in one source code. This is common with ICD10 codes that describe a family history of some Condition, for example. In OMOP the Vocabulary breaks these two clinical ideas into two codes; one becomes the OBSERVATION_CONCEPT_ID and the other becomes the VALUE_AS_CONCEPT_ID. It is important when using the Observation table to keep this possibility in mind and to examine the VALUE_AS_CONCEPT_ID field for relevant information.
Note that the value of VALUE_AS_CONCEPT_ID may be provided through mapping from a source Concept which contains the content of the Observation. In those situations, the CONCEPT_RELATIONSHIP table in addition to the 'Maps to' record contains a second record with the relationship_id set to 'Maps to value'. For example, ICD10 [Z82.4](https://athena.ohdsi.org/search-terms/terms/45581076) 'Family history of ischaemic heart disease and other diseases of the circulatory system' has a 'Maps to' relationship to [4167217](https://athena.ohdsi.org/search-terms/terms/4167217) 'Family history of clinical finding' as well as a 'Maps to value' record to [134057](https://athena.ohdsi.org/search-terms/terms/134057) 'Disorder of cardiovascular system'.</rdfs:comment>
    <rdfs:domain rdf:nodeID="nde7e53d44aa94269b5c0c83d6d8798ccb69"/>
    <rdfs:range rdf:resource="https://w3id.org/omop/ontology/Concept"/>
    <ns1:omop_cdm_name rdf:datatype="http://www.w3.org/2001/XMLSchema#string">measurement.value_as_concept_id#138 AS Concept</ns1:omop_cdm_name>
    <ns1:omop_cdm_name rdf:datatype="http://www.w3.org/2001/XMLSchema#string">metadata.value_as_concept_id#349 AS Concept</ns1:omop_cdm_name>
    <ns1:omop_cdm_name rdf:datatype="http://www.w3.org/2001/XMLSchema#string">observation.value_as_concept_id#157 AS Concept</ns1:omop_cdm_name>
  </rdf:Description>
  <rdf:Description rdf:nodeID="nde7e53d44aa94269b5c0c83d6d8798ccb211">
    <rdf:type rdf:resource="http://www.w3.org/2002/07/owl#Restriction"/>
    <owl:onProperty rdf:resource="https://w3id.org/omop/ontology/has_concept"/>
    <owl:someValuesFrom rdf:resource="https://w3id.org/omop/ontology/Concept"/>
  </rdf:Description>
  <rdf:Description rdf:nodeID="nde7e53d44aa94269b5c0c83d6d8798ccb321">
    <rdf:type rdf:resource="http://www.w3.org/2002/07/owl#Restriction"/>
    <owl:onProperty rdf:resource="https://w3id.org/omop/ontology/admitted_from_source_value"/>
    <owl:someValuesFrom rdf:resource="http://www.w3.org/2001/XMLSchema#integer"/>
  </rdf:Description>
  <rdf:Description rdf:nodeID="nde7e53d44aa94269b5c0c83d6d8798ccb57">
    <rdf:type rdf:resource="http://www.w3.org/2002/07/owl#Class"/>
    <owl:unionOf rdf:nodeID="nde7e53d44aa94269b5c0c83d6d8798ccb58"/>
  </rdf:Description>
  <rdf:Description rdf:nodeID="nde7e53d44aa94269b5c0c83d6d8798ccb406">
    <rdf:type rdf:resource="http://www.w3.org/2002/07/owl#Restriction"/>
    <owl:onProperty rdf:resource="https://w3id.org/omop/ontology/has_concept"/>
    <owl:someValuesFrom rdf:resource="https://w3id.org/omop/ontology/Concept"/>
  </rdf:Description>
  <rdf:Description rdf:nodeID="nde7e53d44aa94269b5c0c83d6d8798ccb142">
    <rdf:first rdf:resource="https://w3id.org/omop/ontology/ConceptRelationship"/>
    <rdf:rest rdf:resource="http://www.w3.org/1999/02/22-rdf-syntax-ns#nil"/>
  </rdf:Description>
  <rdf:Description rdf:about="https://w3id.org/omop/ontology/dea">
    <rdf:type rdf:resource="http://www.w3.org/2002/07/owl#DatatypeProperty"/>
    <rdf:type rdf:resource="http://www.w3.org/2002/07/owl#FunctionalProperty"/>
    <rdfs:comment xml:lang="en">(for Provider:) This is the identifier issued by the DEA, a US federal agency, that allows a provider to write prescriptions for controlled substances.</rdfs:comment>
    <rdfs:domain rdf:resource="https://w3id.org/omop/ontology/Provider"/>
    <rdfs:range rdf:resource="http://www.w3.org/2001/XMLSchema#string"/>
    <ns1:omop_cdm_name rdf:datatype="http://www.w3.org/2001/XMLSchema#string">provider.dea#276 AS str</ns1:omop_cdm_name>
  </rdf:Description>
  <rdf:Description rdf:nodeID="nde7e53d44aa94269b5c0c83d6d8798ccb336">
    <rdf:type rdf:resource="http://www.w3.org/2002/07/owl#Restriction"/>
    <owl:allValuesFrom rdf:resource="http://www.w3.org/2001/XMLSchema#integer"/>
    <owl:onProperty rdf:resource="https://w3id.org/omop/ontology/box_size"/>
  </rdf:Description>
  <rdf:Description rdf:nodeID="nde7e53d44aa94269b5c0c83d6d8798ccb218">
    <rdf:type rdf:resource="http://www.w3.org/2002/07/owl#Restriction"/>
    <owl:allValuesFrom rdf:resource="http://www.w3.org/2001/XMLSchema#string"/>
    <owl:onProperty rdf:resource="https://w3id.org/omop/ontology/is_hierarchical"/>
  </rdf:Description>
  <rdf:Description rdf:nodeID="nde7e53d44aa94269b5c0c83d6d8798ccb606">
    <rdf:type rdf:resource="http://www.w3.org/2002/07/owl#Restriction"/>
    <owl:allValuesFrom rdf:resource="http://www.w3.org/2001/XMLSchema#string"/>
    <owl:onProperty rdf:resource="https://w3id.org/omop/ontology/survey_version_number"/>
  </rdf:Description>
  <rdf:Description rdf:nodeID="nde7e53d44aa94269b5c0c83d6d8798ccb585">
    <rdf:first rdf:resource="http://www.w3.org/2001/XMLSchema#integer"/>
    <rdf:rest rdf:nodeID="nde7e53d44aa94269b5c0c83d6d8798ccb586"/>
  </rdf:Description>
  <rdf:Description rdf:nodeID="nde7e53d44aa94269b5c0c83d6d8798ccb419">
    <owl:inverseOf rdf:resource="https://w3id.org/omop/ontology/has_note"/>
  </rdf:Description>
  <rdf:Description rdf:nodeID="nde7e53d44aa94269b5c0c83d6d8798ccb400">
    <rdf:type rdf:resource="http://www.w3.org/2002/07/owl#Restriction"/>
    <owl:allValuesFrom rdf:resource="http://www.w3.org/2001/XMLSchema#string"/>
    <owl:onProperty rdf:resource="https://w3id.org/omop/ontology/version"/>
  </rdf:Description>
  <rdf:Description rdf:about="https://w3id.org/omop/ontology/has_race">
    <rdf:type rdf:resource="http://www.w3.org/2002/07/owl#FunctionalProperty"/>
    <rdf:type rdf:resource="http://www.w3.org/2002/07/owl#ObjectProperty"/>
    <ns2:python_name rdf:datatype="http://www.w3.org/2001/XMLSchema#string">race</ns2:python_name>
    <rdfs:comment xml:lang="en">(for Person:) This field captures race or ethnic background of the person.
Only use this field if you have information about race or ethnic background. The Vocabulary contains Concepts about the main races and ethnic backgrounds in a hierarchical system. Due to the imprecise nature of human races and ethnic backgrounds, this is not a perfect system. Mixed races are not supported. If a clear race or ethnic background cannot be established, use Concept_Id 0. [Accepted Race Concepts](http://athena.ohdsi.org/search-terms/terms?domain=Race&amp;standardConcept=Standard&amp;page=1&amp;pageSize=15&amp;query=).</rdfs:comment>
    <rdfs:domain rdf:resource="https://w3id.org/omop/ontology/Person"/>
    <rdfs:range rdf:resource="https://w3id.org/omop/ontology/Concept"/>
    <ns1:omop_cdm_name rdf:datatype="http://www.w3.org/2001/XMLSchema#string">person.race_concept_id#8 AS Concept</ns1:omop_cdm_name>
  </rdf:Description>
  <rdf:Description rdf:nodeID="nde7e53d44aa94269b5c0c83d6d8798ccb571">
    <rdf:type rdf:resource="http://www.w3.org/2002/07/owl#Class"/>
    <owl:unionOf rdf:nodeID="nde7e53d44aa94269b5c0c83d6d8798ccb572"/>
  </rdf:Description>
  <rdf:Description rdf:nodeID="nde7e53d44aa94269b5c0c83d6d8798ccb452">
    <rdf:type rdf:resource="http://www.w3.org/2002/07/owl#Restriction"/>
    <owl:allValuesFrom rdf:resource="https://w3id.org/omop/ontology/Provider"/>
    <owl:onProperty rdf:resource="https://w3id.org/omop/ontology/has_provider"/>
  </rdf:Description>
  <rdf:Description rdf:about="https://w3id.org/omop/ontology/billed_date">
    <rdf:type rdf:resource="http://www.w3.org/2002/07/owl#DatatypeProperty"/>
    <rdf:type rdf:resource="http://www.w3.org/2002/07/owl#FunctionalProperty"/>
    <rdfs:comment xml:lang="en">(for Cost:) The date a bill was generated for a service or encounter</rdfs:comment>
    <rdfs:domain rdf:resource="https://w3id.org/omop/ontology/Cost"/>
    <rdfs:range rdf:resource="http://www.w3.org/2001/XMLSchema#date"/>
    <ns1:omop_cdm_name rdf:datatype="http://www.w3.org/2001/XMLSchema#string">cost.billed_date#318 AS date</ns1:omop_cdm_name>
  </rdf:Description>
  <rdf:Description rdf:nodeID="nde7e53d44aa94269b5c0c83d6d8798ccb330">
    <rdf:type rdf:resource="http://www.w3.org/2002/07/owl#Restriction"/>
    <owl:allValuesFrom rdf:resource="http://www.w3.org/2001/XMLSchema#string"/>
    <owl:onProperty rdf:resource="https://w3id.org/omop/ontology/invalid_reason"/>
  </rdf:Description>
  <rdf:Description rdf:nodeID="nde7e53d44aa94269b5c0c83d6d8798ccb188">
    <rdf:type rdf:resource="http://www.w3.org/2002/07/owl#Restriction"/>
    <owl:allValuesFrom rdf:resource="https://w3id.org/omop/ontology/Concept"/>
    <owl:onProperty rdf:resource="https://w3id.org/omop/ontology/has_type"/>
  </rdf:Description>
  <rdf:Description rdf:nodeID="nde7e53d44aa94269b5c0c83d6d8798ccb154">
    <rdf:type rdf:resource="http://www.w3.org/2002/07/owl#Restriction"/>
    <owl:onProperty rdf:resource="https://w3id.org/omop/ontology/domain_concept_id_2"/>
    <owl:someValuesFrom rdf:resource="http://www.w3.org/2001/XMLSchema#integer"/>
  </rdf:Description>
  <rdf:Description rdf:nodeID="nde7e53d44aa94269b5c0c83d6d8798ccb208">
    <rdf:type rdf:resource="http://www.w3.org/2002/07/owl#Restriction"/>
    <owl:onProperty rdf:resource="https://w3id.org/omop/ontology/has_concept"/>
    <owl:someValuesFrom rdf:resource="https://w3id.org/omop/ontology/Concept"/>
  </rdf:Description>
  <rdf:Description rdf:nodeID="nde7e53d44aa94269b5c0c83d6d8798ccb331">
    <rdf:type rdf:resource="http://www.w3.org/2002/07/owl#Restriction"/>
    <owl:onProperty rdf:resource="https://w3id.org/omop/ontology/valid_end_date"/>
    <owl:someValuesFrom rdf:resource="http://www.w3.org/2001/XMLSchema#date"/>
  </rdf:Description>
  <rdf:Description rdf:nodeID="nde7e53d44aa94269b5c0c83d6d8798ccb625">
    <rdf:first rdf:resource="https://w3id.org/omop/ontology/Observation"/>
    <rdf:rest rdf:nodeID="nde7e53d44aa94269b5c0c83d6d8798ccb626"/>
  </rdf:Description>
  <rdf:Description rdf:nodeID="nde7e53d44aa94269b5c0c83d6d8798ccb129">
    <rdf:type rdf:resource="http://www.w3.org/2002/07/owl#Class"/>
    <owl:unionOf rdf:nodeID="nde7e53d44aa94269b5c0c83d6d8798ccb130"/>
  </rdf:Description>
  <rdf:Description rdf:nodeID="nde7e53d44aa94269b5c0c83d6d8798ccb232">
    <rdf:type rdf:resource="http://www.w3.org/2002/07/owl#Class"/>
    <owl:unionOf rdf:nodeID="nde7e53d44aa94269b5c0c83d6d8798ccb233"/>
  </rdf:Description>
  <rdf:Description rdf:about="https://w3id.org/omop/ontology/ConceptSynonym">
    <rdf:type rdf:resource="http://www.w3.org/2002/07/owl#Class"/>
    <rdfs:subClassOf rdf:nodeID="nde7e53d44aa94269b5c0c83d6d8798ccb20"/>
    <rdfs:subClassOf rdf:nodeID="nde7e53d44aa94269b5c0c83d6d8798ccb21"/>
    <rdfs:subClassOf rdf:nodeID="nde7e53d44aa94269b5c0c83d6d8798ccb22"/>
    <rdfs:subClassOf rdf:nodeID="nde7e53d44aa94269b5c0c83d6d8798ccb23"/>
    <rdfs:subClassOf rdf:nodeID="nde7e53d44aa94269b5c0c83d6d8798ccb24"/>
    <rdfs:subClassOf rdf:nodeID="nde7e53d44aa94269b5c0c83d6d8798ccb25"/>
    <rdfs:subClassOf rdf:resource="https://w3id.org/omop/ontology/OmopCDMThing"/>
    <ns1:omop_cdm_name rdf:datatype="http://www.w3.org/2001/XMLSchema#string">concept_synonym</ns1:omop_cdm_name>
  </rdf:Description>
  <rdf:Description rdf:about="https://w3id.org/omop/ontology/anatomic_site_source_value">
    <rdf:type rdf:resource="http://www.w3.org/2002/07/owl#DatatypeProperty"/>
    <rdf:type rdf:resource="http://www.w3.org/2002/07/owl#FunctionalProperty"/>
    <rdfs:comment xml:lang="en">(for Specimen:) This is the site on the body where the specimen was taken from, as represented in the source.</rdfs:comment>
    <rdfs:domain rdf:resource="https://w3id.org/omop/ontology/Specimen"/>
    <rdfs:range rdf:resource="http://www.w3.org/2001/XMLSchema#string"/>
    <ns1:omop_cdm_name rdf:datatype="http://www.w3.org/2001/XMLSchema#string">specimen.anatomic_site_source_value#220 AS str</ns1:omop_cdm_name>
  </rdf:Description>
  <rdf:Description rdf:nodeID="nde7e53d44aa94269b5c0c83d6d8798ccb626">
    <rdf:first rdf:resource="https://w3id.org/omop/ontology/Era"/>
    <rdf:rest rdf:nodeID="nde7e53d44aa94269b5c0c83d6d8798ccb627"/>
  </rdf:Description>
  <rdf:Description rdf:nodeID="nde7e53d44aa94269b5c0c83d6d8798ccb136">
    <rdf:first rdf:resource="https://w3id.org/omop/ontology/VisitOccurrence"/>
    <rdf:rest rdf:nodeID="nde7e53d44aa94269b5c0c83d6d8798ccb137"/>
  </rdf:Description>
  <rdf:Description rdf:nodeID="nde7e53d44aa94269b5c0c83d6d8798ccb456">
    <rdf:type rdf:resource="http://www.w3.org/2002/07/owl#Restriction"/>
    <owl:allValuesFrom rdf:resource="https://w3id.org/omop/ontology/Provider"/>
    <owl:onProperty rdf:resource="https://w3id.org/omop/ontology/has_provider"/>
  </rdf:Description>
  <rdf:Description rdf:nodeID="nde7e53d44aa94269b5c0c83d6d8798ccb504">
    <owl:inverseOf rdf:resource="https://w3id.org/omop/ontology/has_cost"/>
  </rdf:Description>
  <rdf:Description rdf:nodeID="nde7e53d44aa94269b5c0c83d6d8798ccb614">
    <rdf:type rdf:resource="http://www.w3.org/2002/07/owl#Restriction"/>
    <owl:allValuesFrom rdf:resource="https://w3id.org/omop/ontology/Concept"/>
    <owl:onProperty rdf:resource="https://w3id.org/omop/ontology/has_assisted"/>
  </rdf:Description>
  <rdf:Description rdf:nodeID="nde7e53d44aa94269b5c0c83d6d8798ccb659">
    <rdf:type rdf:resource="http://www.w3.org/2002/07/owl#Restriction"/>
    <owl:allValuesFrom rdf:resource="http://www.w3.org/2001/XMLSchema#string"/>
    <owl:onProperty rdf:resource="https://w3id.org/omop/ontology/race_source_value"/>
  </rdf:Description>
  <rdf:Description rdf:about="https://w3id.org/omop/ontology/value_as_string">
    <rdf:type rdf:resource="http://www.w3.org/2002/07/owl#DatatypeProperty"/>
    <rdf:type rdf:resource="http://www.w3.org/2002/07/owl#FunctionalProperty"/>
    <rdfs:comment xml:lang="en">(for Observation:) This is the categorical value of the Result of the Observation, if applicable and available.</rdfs:comment>
    <rdfs:domain rdf:nodeID="nde7e53d44aa94269b5c0c83d6d8798ccb17"/>
    <rdfs:range rdf:resource="http://www.w3.org/2001/XMLSchema#string"/>
    <ns1:omop_cdm_name rdf:datatype="http://www.w3.org/2001/XMLSchema#string">metadata.value_as_string#348 AS str</ns1:omop_cdm_name>
    <ns1:omop_cdm_name rdf:datatype="http://www.w3.org/2001/XMLSchema#string">observation.value_as_string#156 AS str</ns1:omop_cdm_name>
  </rdf:Description>
  <rdf:Description rdf:nodeID="nde7e53d44aa94269b5c0c83d6d8798ccb489">
    <rdf:first rdf:resource="https://w3id.org/omop/ontology/BaseVisit"/>
    <rdf:rest rdf:nodeID="nde7e53d44aa94269b5c0c83d6d8798ccb490"/>
  </rdf:Description>
  <rdf:Description rdf:nodeID="nde7e53d44aa94269b5c0c83d6d8798ccb430">
    <rdf:type rdf:resource="http://www.w3.org/2002/07/owl#Restriction"/>
    <owl:allValuesFrom rdf:resource="http://www.w3.org/2001/XMLSchema#string"/>
    <owl:onProperty rdf:resource="https://w3id.org/omop/ontology/text"/>
  </rdf:Description>
  <rdf:Description rdf:nodeID="nde7e53d44aa94269b5c0c83d6d8798ccb4">
    <rdf:type rdf:resource="http://www.w3.org/2002/07/owl#Restriction"/>
    <owl:onProperty rdf:resource="https://w3id.org/omop/ontology/has_definition"/>
    <owl:someValuesFrom rdf:resource="https://w3id.org/omop/ontology/CohortDefinition"/>
  </rdf:Description>
  <rdf:Description rdf:nodeID="nde7e53d44aa94269b5c0c83d6d8798ccb576">
    <rdf:first rdf:resource="https://w3id.org/omop/ontology/Relationship"/>
    <rdf:rest rdf:nodeID="nde7e53d44aa94269b5c0c83d6d8798ccb577"/>
  </rdf:Description>
  <rdf:Description rdf:nodeID="nde7e53d44aa94269b5c0c83d6d8798ccb670">
    <rdf:type rdf:resource="http://www.w3.org/2002/07/owl#Restriction"/>
    <owl:allValuesFrom rdf:resource="http://www.w3.org/2001/XMLSchema#dateTime"/>
    <owl:onProperty rdf:resource="https://w3id.org/omop/ontology/birth_datetime"/>
  </rdf:Description>
  <rdf:Description rdf:nodeID="nde7e53d44aa94269b5c0c83d6d8798ccb313">
    <rdf:type rdf:resource="http://www.w3.org/2002/07/owl#Restriction"/>
    <owl:allValuesFrom rdf:resource="http://www.w3.org/2001/XMLSchema#string"/>
    <owl:onProperty rdf:resource="https://w3id.org/omop/ontology/source_value"/>
  </rdf:Description>
  <rdf:Description rdf:nodeID="nde7e53d44aa94269b5c0c83d6d8798ccb109">
    <rdf:type rdf:resource="http://www.w3.org/2002/07/owl#Restriction"/>
    <owl:onProperty rdf:resource="https://w3id.org/omop/ontology/has_domain"/>
    <owl:someValuesFrom rdf:resource="https://w3id.org/omop/ontology/Domain"/>
  </rdf:Description>
  <rdf:Description rdf:nodeID="nde7e53d44aa94269b5c0c83d6d8798ccb418">
    <rdf:type rdf:resource="http://www.w3.org/2002/07/owl#Restriction"/>
    <owl:onProperty rdf:nodeID="nde7e53d44aa94269b5c0c83d6d8798ccb419"/>
    <owl:someValuesFrom rdf:resource="https://w3id.org/omop/ontology/Person"/>
  </rdf:Description>
  <rdf:Description rdf:about="https://w3id.org/omop/ontology/race_source_value">
    <rdf:type rdf:resource="http://www.w3.org/2002/07/owl#DatatypeProperty"/>
    <rdf:type rdf:resource="http://www.w3.org/2002/07/owl#FunctionalProperty"/>
    <rdfs:comment xml:lang="en">(for Person:) This field is used to store the race of the person from the source data. It is not intended for use in standard analytics but for reference only.
Put the race of the person as it appears in the source data.</rdfs:comment>
    <rdfs:domain rdf:resource="https://w3id.org/omop/ontology/Person"/>
    <rdfs:range rdf:resource="http://www.w3.org/2001/XMLSchema#string"/>
    <ns1:omop_cdm_name rdf:datatype="http://www.w3.org/2001/XMLSchema#string">person.race_source_value#16 AS str</ns1:omop_cdm_name>
  </rdf:Description>
  <rdf:Description rdf:nodeID="nde7e53d44aa94269b5c0c83d6d8798ccb574">
    <rdf:first rdf:resource="https://w3id.org/omop/ontology/Domain"/>
    <rdf:rest rdf:nodeID="nde7e53d44aa94269b5c0c83d6d8798ccb575"/>
  </rdf:Description>
  <rdf:Description rdf:nodeID="nde7e53d44aa94269b5c0c83d6d8798ccb267">
    <rdf:first rdf:resource="https://w3id.org/omop/ontology/ConditionOccurrence"/>
    <rdf:rest rdf:nodeID="nde7e53d44aa94269b5c0c83d6d8798ccb268"/>
  </rdf:Description>
  <rdf:Description rdf:nodeID="nde7e53d44aa94269b5c0c83d6d8798ccb212">
    <rdf:type rdf:resource="http://www.w3.org/2002/07/owl#Restriction"/>
    <owl:allValuesFrom rdf:resource="http://www.w3.org/2002/07/owl#Thing"/>
    <owl:onProperty rdf:resource="https://w3id.org/omop/ontology/has_reverse_relationship"/>
  </rdf:Description>
  <rdf:Description rdf:nodeID="nde7e53d44aa94269b5c0c83d6d8798ccb201">
    <rdf:type rdf:resource="http://www.w3.org/2002/07/owl#Restriction"/>
    <owl:allValuesFrom rdf:resource="https://w3id.org/omop/ontology/Concept"/>
    <owl:onProperty rdf:resource="https://w3id.org/omop/ontology/has_concept"/>
  </rdf:Description>
  <rdf:Description rdf:nodeID="nde7e53d44aa94269b5c0c83d6d8798ccb228">
    <rdf:first rdf:resource="https://w3id.org/omop/ontology/DrugStrength"/>
    <rdf:rest rdf:nodeID="nde7e53d44aa94269b5c0c83d6d8798ccb229"/>
  </rdf:Description>
  <rdf:Description rdf:nodeID="nde7e53d44aa94269b5c0c83d6d8798ccb493">
    <rdf:type rdf:resource="http://www.w3.org/2002/07/owl#Restriction"/>
    <owl:allValuesFrom rdf:resource="https://w3id.org/omop/ontology/Concept"/>
    <owl:onProperty rdf:resource="https://w3id.org/omop/ontology/has_revenue_code"/>
  </rdf:Description>
  <rdf:Description rdf:nodeID="nde7e53d44aa94269b5c0c83d6d8798ccb554">
    <rdf:type rdf:resource="http://www.w3.org/2002/07/owl#Restriction"/>
    <owl:onProperty rdf:resource="https://w3id.org/omop/ontology/has_plan"/>
    <owl:someValuesFrom rdf:resource="https://w3id.org/omop/ontology/Concept"/>
  </rdf:Description>
  <rdf:Description rdf:nodeID="nde7e53d44aa94269b5c0c83d6d8798ccb631">
    <rdf:first rdf:resource="https://w3id.org/omop/ontology/Domain"/>
    <rdf:rest rdf:nodeID="nde7e53d44aa94269b5c0c83d6d8798ccb632"/>
  </rdf:Description>
  <rdf:Description rdf:nodeID="nde7e53d44aa94269b5c0c83d6d8798ccb402">
    <rdf:type rdf:resource="http://www.w3.org/2002/07/owl#Restriction"/>
    <owl:onProperty rdf:resource="https://w3id.org/omop/ontology/reference"/>
    <owl:someValuesFrom rdf:resource="http://www.w3.org/2001/XMLSchema#string"/>
  </rdf:Description>
  <rdf:Description rdf:nodeID="nde7e53d44aa94269b5c0c83d6d8798ccb335">
    <rdf:type rdf:resource="http://www.w3.org/2002/07/owl#Restriction"/>
    <owl:onProperty rdf:resource="https://w3id.org/omop/ontology/has_concept"/>
    <owl:someValuesFrom rdf:resource="https://w3id.org/omop/ontology/Concept"/>
  </rdf:Description>
  <rdf:Description rdf:nodeID="nde7e53d44aa94269b5c0c83d6d8798ccb667">
    <rdf:type rdf:resource="http://www.w3.org/2002/07/owl#Restriction"/>
    <owl:allValuesFrom rdf:resource="https://w3id.org/omop/ontology/VisitDetail"/>
    <owl:onProperty rdf:resource="https://w3id.org/omop/ontology/has_visit_detail"/>
  </rdf:Description>
  <rdf:Description rdf:nodeID="nde7e53d44aa94269b5c0c83d6d8798ccb262">
    <rdf:type rdf:resource="http://www.w3.org/2002/07/owl#Restriction"/>
    <owl:onProperty rdf:resource="https://w3id.org/omop/ontology/valid_end_date"/>
    <owl:someValuesFrom rdf:resource="http://www.w3.org/2001/XMLSchema#date"/>
  </rdf:Description>
  <rdf:Description rdf:nodeID="nde7e53d44aa94269b5c0c83d6d8798ccb470">
    <rdf:type rdf:resource="http://www.w3.org/2002/07/owl#Restriction"/>
    <owl:allValuesFrom rdf:resource="http://www.w3.org/2001/XMLSchema#decimal"/>
    <owl:onProperty rdf:resource="https://w3id.org/omop/ontology/range_high"/>
  </rdf:Description>
  <rdf:Description rdf:about="https://w3id.org/omop/ontology/plan_source_value">
    <rdf:type rdf:resource="http://www.w3.org/2002/07/owl#DatatypeProperty"/>
    <rdf:type rdf:resource="http://www.w3.org/2002/07/owl#FunctionalProperty"/>
    <rdfs:comment xml:lang="en">(for PayerPlanPeriod:) This is the health benefit Plan of the Person as it appears in the source data.</rdfs:comment>
    <rdfs:domain rdf:resource="https://w3id.org/omop/ontology/PayerPlanPeriod"/>
    <rdfs:range rdf:resource="http://www.w3.org/2001/XMLSchema#string"/>
    <ns1:omop_cdm_name rdf:datatype="http://www.w3.org/2001/XMLSchema#string">payer_plan_period.plan_source_value#295 AS str</ns1:omop_cdm_name>
  </rdf:Description>
  <rdf:Description rdf:nodeID="nde7e53d44aa94269b5c0c83d6d8798ccb231">
    <rdf:first rdf:resource="https://w3id.org/omop/ontology/ConceptRelationship"/>
    <rdf:rest rdf:resource="http://www.w3.org/1999/02/22-rdf-syntax-ns#nil"/>
  </rdf:Description>
  <rdf:Description rdf:nodeID="nde7e53d44aa94269b5c0c83d6d8798ccb588">
    <rdf:type rdf:resource="http://www.w3.org/2000/01/rdf-schema#Datatype"/>
    <owl:unionOf rdf:nodeID="nde7e53d44aa94269b5c0c83d6d8798ccb589"/>
  </rdf:Description>
  <rdf:Description rdf:nodeID="nde7e53d44aa94269b5c0c83d6d8798ccb536">
    <rdf:type rdf:resource="http://www.w3.org/2002/07/owl#Restriction"/>
    <owl:onProperty rdf:resource="https://w3id.org/omop/ontology/has_contract"/>
    <owl:someValuesFrom rdf:resource="https://w3id.org/omop/ontology/Concept"/>
  </rdf:Description>
  <rdf:Description rdf:nodeID="nde7e53d44aa94269b5c0c83d6d8798ccb300">
    <rdf:type rdf:resource="http://www.w3.org/2002/07/owl#Restriction"/>
    <owl:allValuesFrom rdf:resource="https://w3id.org/omop/ontology/Concept"/>
    <owl:onProperty rdf:resource="https://w3id.org/omop/ontology/has_type"/>
  </rdf:Description>
  <rdf:Description rdf:nodeID="nde7e53d44aa94269b5c0c83d6d8798ccb137">
    <rdf:first rdf:resource="https://w3id.org/omop/ontology/Person"/>
    <rdf:rest rdf:resource="http://www.w3.org/1999/02/22-rdf-syntax-ns#nil"/>
  </rdf:Description>
  <rdf:Description rdf:nodeID="nde7e53d44aa94269b5c0c83d6d8798ccb433">
    <rdf:type rdf:resource="http://www.w3.org/2002/07/owl#Restriction"/>
    <owl:onProperty rdf:resource="https://w3id.org/omop/ontology/has_type"/>
    <owl:someValuesFrom rdf:resource="https://w3id.org/omop/ontology/Concept"/>
  </rdf:Description>
  <rdf:Description rdf:nodeID="nde7e53d44aa94269b5c0c83d6d8798ccb177">
    <rdf:type rdf:resource="http://www.w3.org/2002/07/owl#Restriction"/>
    <owl:allValuesFrom rdf:resource="http://www.w3.org/2001/XMLSchema#integer"/>
    <owl:onProperty rdf:resource="https://w3id.org/omop/ontology/concept_id_1"/>
  </rdf:Description>
  <rdf:Description rdf:nodeID="nde7e53d44aa94269b5c0c83d6d8798ccb565">
    <rdf:first rdf:resource="https://w3id.org/omop/ontology/Cost"/>
    <rdf:rest rdf:nodeID="nde7e53d44aa94269b5c0c83d6d8798ccb566"/>
  </rdf:Description>
  <rdf:Description rdf:nodeID="nde7e53d44aa94269b5c0c83d6d8798ccb40">
    <rdf:first rdf:resource="https://w3id.org/omop/ontology/BaseVisit"/>
    <rdf:rest rdf:nodeID="nde7e53d44aa94269b5c0c83d6d8798ccb41"/>
  </rdf:Description>
  <rdf:Description rdf:nodeID="nde7e53d44aa94269b5c0c83d6d8798ccb581">
    <rdf:first rdf:resource="https://w3id.org/omop/ontology/Provider"/>
    <rdf:rest rdf:nodeID="nde7e53d44aa94269b5c0c83d6d8798ccb582"/>
  </rdf:Description>
  <rdf:Description rdf:about="https://w3id.org/omop/ontology/range_low">
    <rdf:type rdf:resource="http://www.w3.org/2002/07/owl#DatatypeProperty"/>
    <rdf:type rdf:resource="http://www.w3.org/2002/07/owl#FunctionalProperty"/>
    <rdfs:comment xml:lang="en">(for Measurement:) Ranges have the same unit as the VALUE_AS_NUMBER. These ranges are provided by the source and should remain NULL if not given.
If reference ranges for upper and lower limit of normal as provided (typically by a laboratory) these are stored in the RANGE_HIGH and RANGE_LOW fields. This should be set to NULL if not provided.</rdfs:comment>
    <rdfs:domain rdf:resource="https://w3id.org/omop/ontology/Measurement"/>
    <rdfs:range rdf:resource="http://www.w3.org/2001/XMLSchema#decimal"/>
    <ns1:omop_cdm_name rdf:datatype="http://www.w3.org/2001/XMLSchema#string">measurement.range_low#140 AS float</ns1:omop_cdm_name>
  </rdf:Description>
  <rdf:Description rdf:nodeID="nde7e53d44aa94269b5c0c83d6d8798ccb130">
    <rdf:first rdf:resource="https://w3id.org/omop/ontology/FactRelationship"/>
    <rdf:rest rdf:nodeID="nde7e53d44aa94269b5c0c83d6d8798ccb131"/>
  </rdf:Description>
  <rdf:Description rdf:nodeID="nde7e53d44aa94269b5c0c83d6d8798ccb414">
    <rdf:type rdf:resource="http://www.w3.org/2002/07/owl#Restriction"/>
    <owl:allValuesFrom rdf:resource="http://www.w3.org/2001/XMLSchema#string"/>
    <owl:onProperty rdf:resource="https://w3id.org/omop/ontology/county"/>
  </rdf:Description>
  <rdf:Description rdf:nodeID="nde7e53d44aa94269b5c0c83d6d8798ccb171">
    <rdf:first rdf:resource="https://w3id.org/omop/ontology/Measurement"/>
    <rdf:rest rdf:nodeID="nde7e53d44aa94269b5c0c83d6d8798ccb172"/>
  </rdf:Description>
  <rdf:Description rdf:about="https://w3id.org/omop/ontology/max_levels_of_separation">
    <rdf:type rdf:resource="http://www.w3.org/2002/07/owl#DatatypeProperty"/>
    <rdf:type rdf:resource="http://www.w3.org/2002/07/owl#FunctionalProperty"/>
    <rdfs:comment xml:lang="en">(for ConceptAncestor:) The maximum separation in number of
levels of hierarchy between ancestor and
descendant concepts. This is an attribute
that is used to simplify hierarchic analysis.</rdfs:comment>
    <rdfs:domain rdf:resource="https://w3id.org/omop/ontology/ConceptAncestor"/>
    <rdfs:range rdf:resource="http://www.w3.org/2001/XMLSchema#integer"/>
    <ns1:omop_cdm_name rdf:datatype="http://www.w3.org/2001/XMLSchema#string">concept_ancestor.max_levels_of_separation#401 AS int</ns1:omop_cdm_name>
  </rdf:Description>
  <rdf:Description rdf:nodeID="nde7e53d44aa94269b5c0c83d6d8798ccb242">
    <rdf:type rdf:resource="http://www.w3.org/2002/07/owl#Restriction"/>
    <owl:allValuesFrom rdf:resource="http://www.w3.org/2001/XMLSchema#string"/>
    <owl:onProperty rdf:resource="https://w3id.org/omop/ontology/description"/>
  </rdf:Description>
  <rdf:Description rdf:nodeID="nde7e53d44aa94269b5c0c83d6d8798ccb353">
    <rdf:type rdf:resource="http://www.w3.org/2002/07/owl#Restriction"/>
    <owl:onProperty rdf:resource="https://w3id.org/omop/ontology/has_admitted_from"/>
    <owl:someValuesFrom rdf:resource="https://w3id.org/omop/ontology/Concept"/>
  </rdf:Description>
  <rdf:Description rdf:nodeID="nde7e53d44aa94269b5c0c83d6d8798ccb16">
    <rdf:first rdf:resource="https://w3id.org/omop/ontology/Observation"/>
    <rdf:rest rdf:resource="http://www.w3.org/1999/02/22-rdf-syntax-ns#nil"/>
  </rdf:Description>
  <rdf:Description rdf:nodeID="nde7e53d44aa94269b5c0c83d6d8798ccb366">
    <rdf:first rdf:resource="https://w3id.org/omop/ontology/Location"/>
    <rdf:rest rdf:nodeID="nde7e53d44aa94269b5c0c83d6d8798ccb367"/>
  </rdf:Description>
  <rdf:Description rdf:nodeID="nde7e53d44aa94269b5c0c83d6d8798ccb512">
    <rdf:type rdf:resource="http://www.w3.org/2002/07/owl#Restriction"/>
    <owl:allValuesFrom rdf:resource="https://w3id.org/omop/ontology/Provider"/>
    <owl:onProperty rdf:resource="https://w3id.org/omop/ontology/has_provider"/>
  </rdf:Description>
  <rdf:Description rdf:nodeID="nde7e53d44aa94269b5c0c83d6d8798ccb135">
    <rdf:type rdf:resource="http://www.w3.org/2002/07/owl#Class"/>
    <owl:unionOf rdf:nodeID="nde7e53d44aa94269b5c0c83d6d8798ccb136"/>
  </rdf:Description>
  <rdf:Description rdf:nodeID="nde7e53d44aa94269b5c0c83d6d8798ccb9">
    <rdf:first rdf:resource="http://www.w3.org/2001/XMLSchema#integer"/>
    <rdf:rest rdf:nodeID="nde7e53d44aa94269b5c0c83d6d8798ccb10"/>
  </rdf:Description>
  <rdf:Description rdf:nodeID="nde7e53d44aa94269b5c0c83d6d8798ccb113">
    <rdf:first rdf:resource="https://w3id.org/omop/ontology/Concept"/>
    <rdf:rest rdf:nodeID="nde7e53d44aa94269b5c0c83d6d8798ccb114"/>
  </rdf:Description>
  <rdf:Description rdf:nodeID="nde7e53d44aa94269b5c0c83d6d8798ccb684">
    <rdf:type rdf:resource="http://www.w3.org/2002/07/owl#Restriction"/>
    <owl:onProperty rdf:resource="https://w3id.org/omop/ontology/name"/>
    <owl:someValuesFrom rdf:resource="http://www.w3.org/2001/XMLSchema#string"/>
  </rdf:Description>
  <rdf:Description rdf:nodeID="nde7e53d44aa94269b5c0c83d6d8798ccb277">
    <rdf:type rdf:resource="http://www.w3.org/2002/07/owl#Restriction"/>
    <owl:allValuesFrom rdf:resource="http://www.w3.org/2001/XMLSchema#string"/>
    <owl:onProperty rdf:resource="https://w3id.org/omop/ontology/source_documentation_reference"/>
  </rdf:Description>
  <rdf:Description rdf:nodeID="nde7e53d44aa94269b5c0c83d6d8798ccb653">
    <rdf:type rdf:resource="http://www.w3.org/2002/07/owl#Restriction"/>
    <owl:onProperty rdf:resource="https://w3id.org/omop/ontology/year_of_birth"/>
    <owl:someValuesFrom rdf:resource="http://www.w3.org/2001/XMLSchema#integer"/>
  </rdf:Description>
  <rdf:Description rdf:nodeID="nde7e53d44aa94269b5c0c83d6d8798ccb132">
    <rdf:type rdf:resource="http://www.w3.org/2002/07/owl#Class"/>
    <owl:unionOf rdf:nodeID="nde7e53d44aa94269b5c0c83d6d8798ccb133"/>
  </rdf:Description>
  <rdf:Description rdf:nodeID="nde7e53d44aa94269b5c0c83d6d8798ccb440">
    <rdf:type rdf:resource="http://www.w3.org/2002/07/owl#Restriction"/>
    <owl:allValuesFrom rdf:resource="https://w3id.org/omop/ontology/Concept"/>
    <owl:onProperty rdf:resource="https://w3id.org/omop/ontology/has_source"/>
  </rdf:Description>
  <rdf:Description rdf:nodeID="nde7e53d44aa94269b5c0c83d6d8798ccb285">
    <rdf:type rdf:resource="http://www.w3.org/2002/07/owl#Restriction"/>
    <owl:allValuesFrom rdf:resource="http://www.w3.org/2001/XMLSchema#date"/>
    <owl:onProperty rdf:resource="https://w3id.org/omop/ontology/date"/>
  </rdf:Description>
  <rdf:Description rdf:nodeID="nde7e53d44aa94269b5c0c83d6d8798ccb29">
    <rdf:type rdf:resource="http://www.w3.org/2002/07/owl#Restriction"/>
    <owl:onProperty rdf:nodeID="nde7e53d44aa94269b5c0c83d6d8798ccb30"/>
    <owl:someValuesFrom rdf:resource="https://w3id.org/omop/ontology/Person"/>
  </rdf:Description>
  <rdf:Description rdf:nodeID="nde7e53d44aa94269b5c0c83d6d8798ccb572">
    <rdf:first rdf:resource="https://w3id.org/omop/ontology/CareSite"/>
    <rdf:rest rdf:nodeID="nde7e53d44aa94269b5c0c83d6d8798ccb573"/>
  </rdf:Description>
  <rdf:Description rdf:nodeID="nde7e53d44aa94269b5c0c83d6d8798ccb174">
    <rdf:first rdf:resource="https://w3id.org/omop/ontology/Specimen"/>
    <rdf:rest rdf:resource="http://www.w3.org/1999/02/22-rdf-syntax-ns#nil"/>
  </rdf:Description>
  <rdf:Description rdf:nodeID="nde7e53d44aa94269b5c0c83d6d8798ccb598">
    <rdf:type rdf:resource="http://www.w3.org/2002/07/owl#Restriction"/>
    <owl:allValuesFrom rdf:resource="https://w3id.org/omop/ontology/Concept"/>
    <owl:onProperty rdf:resource="https://w3id.org/omop/ontology/has_survey_source"/>
  </rdf:Description>
  <rdf:Description rdf:nodeID="nde7e53d44aa94269b5c0c83d6d8798ccb48">
    <rdf:type rdf:resource="http://www.w3.org/2002/07/owl#Class"/>
    <owl:unionOf rdf:nodeID="nde7e53d44aa94269b5c0c83d6d8798ccb49"/>
  </rdf:Description>
  <rdf:Description rdf:nodeID="nde7e53d44aa94269b5c0c83d6d8798ccb381">
    <rdf:type rdf:resource="http://www.w3.org/2002/07/owl#Restriction"/>
    <owl:allValuesFrom rdf:resource="http://www.w3.org/2001/XMLSchema#integer"/>
    <owl:onProperty rdf:resource="https://w3id.org/omop/ontology/days_supply"/>
  </rdf:Description>
  <rdf:Description rdf:nodeID="nde7e53d44aa94269b5c0c83d6d8798ccb431">
    <rdf:type rdf:resource="http://www.w3.org/2002/07/owl#Restriction"/>
    <owl:allValuesFrom rdf:resource="https://w3id.org/omop/ontology/Concept"/>
    <owl:onProperty rdf:resource="https://w3id.org/omop/ontology/has_encoding"/>
  </rdf:Description>
  <rdf:Description rdf:nodeID="nde7e53d44aa94269b5c0c83d6d8798ccb608">
    <owl:inverseOf rdf:resource="https://w3id.org/omop/ontology/has_survey_conduct"/>
  </rdf:Description>
  <rdf:Description rdf:nodeID="nde7e53d44aa94269b5c0c83d6d8798ccb51">
    <rdf:type rdf:resource="http://www.w3.org/2002/07/owl#Class"/>
    <owl:unionOf rdf:nodeID="nde7e53d44aa94269b5c0c83d6d8798ccb52"/>
  </rdf:Description>
  <rdf:Description rdf:nodeID="nde7e53d44aa94269b5c0c83d6d8798ccb128">
    <rdf:first rdf:resource="https://w3id.org/omop/ontology/Person"/>
    <rdf:rest rdf:resource="http://www.w3.org/1999/02/22-rdf-syntax-ns#nil"/>
  </rdf:Description>
  <rdf:Description rdf:nodeID="nde7e53d44aa94269b5c0c83d6d8798ccb451">
    <rdf:type rdf:resource="http://www.w3.org/2002/07/owl#Restriction"/>
    <owl:onProperty rdf:resource="https://w3id.org/omop/ontology/has_source"/>
    <owl:someValuesFrom rdf:resource="https://w3id.org/omop/ontology/Concept"/>
  </rdf:Description>
  <rdf:Description rdf:nodeID="nde7e53d44aa94269b5c0c83d6d8798ccb67">
    <rdf:first rdf:resource="https://w3id.org/omop/ontology/VisitOccurrence"/>
    <rdf:rest rdf:nodeID="nde7e53d44aa94269b5c0c83d6d8798ccb68"/>
  </rdf:Description>
  <rdf:Description rdf:about="https://w3id.org/omop/ontology/domain_concept_id_1">
    <rdf:type rdf:resource="http://www.w3.org/2002/07/owl#DatatypeProperty"/>
    <rdf:type rdf:resource="http://www.w3.org/2002/07/owl#FunctionalProperty"/>
    <rdfs:domain rdf:resource="https://w3id.org/omop/ontology/FactRelationship"/>
    <rdfs:range rdf:resource="http://www.w3.org/2001/XMLSchema#integer"/>
    <ns1:omop_cdm_name rdf:datatype="http://www.w3.org/2001/XMLSchema#string">fact_relationship.domain_concept_id_1#222 AS int</ns1:omop_cdm_name>
  </rdf:Description>
  <rdf:Description rdf:about="https://w3id.org/omop/ontology/has_visit_occurrence">
    <rdf:type rdf:resource="http://www.w3.org/2002/07/owl#ObjectProperty"/>
    <ns2:python_name rdf:datatype="http://www.w3.org/2001/XMLSchema#string">visit_occurrences</ns2:python_name>
    <rdfs:domain rdf:resource="https://w3id.org/omop/ontology/Person"/>
    <rdfs:range rdf:resource="https://w3id.org/omop/ontology/VisitOccurrence"/>
    <ns1:omop_cdm_name rdf:datatype="http://www.w3.org/2001/XMLSchema#string">visit_occurrence.person_id#26 AS Person</ns1:omop_cdm_name>
  </rdf:Description>
  <rdf:Description rdf:nodeID="nde7e53d44aa94269b5c0c83d6d8798ccb243">
    <rdf:type rdf:resource="http://www.w3.org/2002/07/owl#Restriction"/>
    <owl:allValuesFrom rdf:resource="https://w3id.org/omop/ontology/Concept"/>
    <owl:onProperty rdf:resource="https://w3id.org/omop/ontology/has_subject"/>
  </rdf:Description>
  <rdf:Description rdf:nodeID="nde7e53d44aa94269b5c0c83d6d8798ccb516">
    <rdf:type rdf:resource="http://www.w3.org/2002/07/owl#Restriction"/>
    <owl:allValuesFrom rdf:resource="http://www.w3.org/2001/XMLSchema#decimal"/>
    <owl:onProperty rdf:resource="https://w3id.org/omop/ontology/value_as_number"/>
  </rdf:Description>
  <rdf:Description rdf:nodeID="nde7e53d44aa94269b5c0c83d6d8798ccb126">
    <rdf:first rdf:resource="https://w3id.org/omop/ontology/CareSite"/>
    <rdf:rest rdf:nodeID="nde7e53d44aa94269b5c0c83d6d8798ccb127"/>
  </rdf:Description>
  <rdf:Description rdf:nodeID="nde7e53d44aa94269b5c0c83d6d8798ccb217">
    <rdf:type rdf:resource="http://www.w3.org/2002/07/owl#Restriction"/>
    <owl:allValuesFrom rdf:resource="http://www.w3.org/2001/XMLSchema#string"/>
    <owl:onProperty rdf:resource="https://w3id.org/omop/ontology/defines_ancestry"/>
  </rdf:Description>
  <rdf:Description rdf:nodeID="nde7e53d44aa94269b5c0c83d6d8798ccb577">
    <rdf:first rdf:resource="https://w3id.org/omop/ontology/CdmSource"/>
    <rdf:rest rdf:nodeID="nde7e53d44aa94269b5c0c83d6d8798ccb578"/>
  </rdf:Description>
  <rdf:Description rdf:nodeID="nde7e53d44aa94269b5c0c83d6d8798ccb341">
    <rdf:type rdf:resource="http://www.w3.org/2002/07/owl#Restriction"/>
    <owl:allValuesFrom rdf:resource="http://www.w3.org/2001/XMLSchema#string"/>
    <owl:onProperty rdf:resource="https://w3id.org/omop/ontology/lexical_variant"/>
  </rdf:Description>
  <rdf:Description rdf:nodeID="nde7e53d44aa94269b5c0c83d6d8798ccb497">
    <rdf:type rdf:resource="http://www.w3.org/2002/07/owl#Restriction"/>
    <owl:allValuesFrom rdf:resource="https://w3id.org/omop/ontology/Concept"/>
    <owl:onProperty rdf:resource="https://w3id.org/omop/ontology/has_currency"/>
  </rdf:Description>
  <rdf:Description rdf:nodeID="nde7e53d44aa94269b5c0c83d6d8798ccb34">
    <rdf:first rdf:resource="https://w3id.org/omop/ontology/VisitOccurrence"/>
    <rdf:rest rdf:nodeID="nde7e53d44aa94269b5c0c83d6d8798ccb35"/>
  </rdf:Description>
  <rdf:Description rdf:about="https://w3id.org/omop/ontology/fact_id_2">
    <rdf:type rdf:resource="http://www.w3.org/2002/07/owl#DatatypeProperty"/>
    <rdf:type rdf:resource="http://www.w3.org/2002/07/owl#FunctionalProperty"/>
    <rdfs:domain rdf:resource="https://w3id.org/omop/ontology/FactRelationship"/>
    <rdfs:range rdf:resource="http://www.w3.org/2001/XMLSchema#integer"/>
    <ns1:omop_cdm_name rdf:datatype="http://www.w3.org/2001/XMLSchema#string">fact_relationship.fact_id_2#225 AS int</ns1:omop_cdm_name>
  </rdf:Description>
  <rdf:Description rdf:nodeID="nde7e53d44aa94269b5c0c83d6d8798ccb295">
    <rdf:type rdf:resource="http://www.w3.org/2002/07/owl#Restriction"/>
    <owl:allValuesFrom rdf:resource="http://www.w3.org/2001/XMLSchema#string"/>
    <owl:onProperty rdf:resource="https://w3id.org/omop/ontology/stop_reason"/>
  </rdf:Description>
  <rdf:Description rdf:nodeID="nde7e53d44aa94269b5c0c83d6d8798ccb350">
    <rdf:type rdf:resource="http://www.w3.org/2002/07/owl#Restriction"/>
    <owl:allValuesFrom rdf:resource="http://www.w3.org/2001/XMLSchema#string"/>
    <owl:onProperty rdf:resource="https://w3id.org/omop/ontology/snippet"/>
  </rdf:Description>
  <rdf:Description rdf:nodeID="nde7e53d44aa94269b5c0c83d6d8798ccb55">
    <rdf:first rdf:resource="https://w3id.org/omop/ontology/BaseVisit"/>
    <rdf:rest rdf:nodeID="nde7e53d44aa94269b5c0c83d6d8798ccb56"/>
  </rdf:Description>
  <rdf:Description rdf:nodeID="nde7e53d44aa94269b5c0c83d6d8798ccb602">
    <rdf:type rdf:resource="http://www.w3.org/2002/07/owl#Restriction"/>
    <owl:onProperty rdf:resource="https://w3id.org/omop/ontology/survey_end_datetime"/>
    <owl:someValuesFrom rdf:resource="http://www.w3.org/2001/XMLSchema#dateTime"/>
  </rdf:Description>
  <rdf:Description rdf:nodeID="nde7e53d44aa94269b5c0c83d6d8798ccb3">
    <rdf:type rdf:resource="http://www.w3.org/2002/07/owl#Restriction"/>
    <owl:onProperty rdf:resource="https://w3id.org/omop/ontology/has_subject"/>
    <owl:someValuesFrom rdf:resource="http://www.w3.org/2002/07/owl#Thing"/>
  </rdf:Description>
  <rdf:Description rdf:nodeID="nde7e53d44aa94269b5c0c83d6d8798ccb658">
    <rdf:type rdf:resource="http://www.w3.org/2002/07/owl#Restriction"/>
    <owl:allValuesFrom rdf:resource="https://w3id.org/omop/ontology/Concept"/>
    <owl:onProperty rdf:resource="https://w3id.org/omop/ontology/has_race_source"/>
  </rdf:Description>
  <rdf:Description rdf:nodeID="nde7e53d44aa94269b5c0c83d6d8798ccb495">
    <rdf:type rdf:resource="http://www.w3.org/2002/07/owl#Restriction"/>
    <owl:allValuesFrom rdf:resource="https://w3id.org/omop/ontology/Concept"/>
    <owl:onProperty rdf:resource="https://w3id.org/omop/ontology/has_event_field"/>
  </rdf:Description>
  <rdf:Description rdf:nodeID="nde7e53d44aa94269b5c0c83d6d8798ccb75">
    <rdf:first rdf:resource="https://w3id.org/omop/ontology/Observation"/>
    <rdf:rest rdf:nodeID="nde7e53d44aa94269b5c0c83d6d8798ccb76"/>
  </rdf:Description>
  <rdf:Description rdf:nodeID="nde7e53d44aa94269b5c0c83d6d8798ccb380">
    <rdf:type rdf:resource="http://www.w3.org/2002/07/owl#Restriction"/>
    <owl:allValuesFrom rdf:resource="http://www.w3.org/2001/XMLSchema#string"/>
    <owl:onProperty rdf:resource="https://w3id.org/omop/ontology/route_source_value"/>
  </rdf:Description>
  <rdf:Description rdf:nodeID="nde7e53d44aa94269b5c0c83d6d8798ccb288">
    <rdf:type rdf:resource="http://www.w3.org/2002/07/owl#Restriction"/>
    <owl:allValuesFrom rdf:resource="https://w3id.org/omop/ontology/Provider"/>
    <owl:onProperty rdf:resource="https://w3id.org/omop/ontology/has_provider"/>
  </rdf:Description>
  <rdf:Description rdf:nodeID="nde7e53d44aa94269b5c0c83d6d8798ccb619">
    <rdf:type rdf:resource="http://www.w3.org/2002/07/owl#Restriction"/>
    <owl:allValuesFrom rdf:resource="https://w3id.org/omop/ontology/Concept"/>
    <owl:onProperty rdf:resource="https://w3id.org/omop/ontology/has_survey"/>
  </rdf:Description>
  <rdf:Description rdf:about="https://w3id.org/omop/ontology/longitude">
    <rdf:type rdf:resource="http://www.w3.org/2002/07/owl#DatatypeProperty"/>
    <rdf:type rdf:resource="http://www.w3.org/2002/07/owl#FunctionalProperty"/>
    <rdfs:comment xml:lang="en">(for Location:) The geocoded longitude.</rdfs:comment>
    <rdfs:domain rdf:resource="https://w3id.org/omop/ontology/Location"/>
    <rdfs:range rdf:resource="http://www.w3.org/2001/XMLSchema#decimal"/>
    <ns1:omop_cdm_name rdf:datatype="http://www.w3.org/2001/XMLSchema#string">location.longitude#260 AS float</ns1:omop_cdm_name>
  </rdf:Description>
  <rdf:Description rdf:about="https://w3id.org/omop/ontology/omop_cdm_name">
    <rdf:type rdf:resource="http://www.w3.org/2002/07/owl#AnnotationProperty"/>
  </rdf:Description>
  <rdf:Description rdf:nodeID="nde7e53d44aa94269b5c0c83d6d8798ccb236">
    <rdf:first rdf:resource="https://w3id.org/omop/ontology/ConceptRelationship"/>
    <rdf:rest rdf:resource="http://www.w3.org/1999/02/22-rdf-syntax-ns#nil"/>
  </rdf:Description>
  <rdf:Description rdf:nodeID="nde7e53d44aa94269b5c0c83d6d8798ccb122">
    <rdf:type rdf:resource="http://www.w3.org/2002/07/owl#Class"/>
    <owl:unionOf rdf:nodeID="nde7e53d44aa94269b5c0c83d6d8798ccb123"/>
  </rdf:Description>
  <rdf:Description rdf:nodeID="nde7e53d44aa94269b5c0c83d6d8798ccb553">
    <rdf:type rdf:resource="http://www.w3.org/2002/07/owl#Restriction"/>
    <owl:allValuesFrom rdf:resource="https://w3id.org/omop/ontology/Concept"/>
    <owl:onProperty rdf:resource="https://w3id.org/omop/ontology/has_stop_reason_concept"/>
  </rdf:Description>
  <rdf:Description rdf:nodeID="nde7e53d44aa94269b5c0c83d6d8798ccb115">
    <rdf:type rdf:resource="http://www.w3.org/2002/07/owl#Class"/>
    <owl:unionOf rdf:nodeID="nde7e53d44aa94269b5c0c83d6d8798ccb116"/>
  </rdf:Description>
  <rdf:Description rdf:nodeID="nde7e53d44aa94269b5c0c83d6d8798ccb427">
    <rdf:type rdf:resource="http://www.w3.org/2002/07/owl#Restriction"/>
    <owl:allValuesFrom rdf:resource="https://w3id.org/omop/ontology/NoteNlp"/>
    <owl:onProperty rdf:resource="https://w3id.org/omop/ontology/has_note_nlp"/>
  </rdf:Description>
  <rdf:Description rdf:nodeID="nde7e53d44aa94269b5c0c83d6d8798ccb25">
    <rdf:type rdf:resource="http://www.w3.org/2002/07/owl#Restriction"/>
    <owl:onProperty rdf:resource="https://w3id.org/omop/ontology/has_concept"/>
    <owl:someValuesFrom rdf:resource="https://w3id.org/omop/ontology/Concept"/>
  </rdf:Description>
  <rdf:Description rdf:nodeID="nde7e53d44aa94269b5c0c83d6d8798ccb604">
    <rdf:type rdf:resource="http://www.w3.org/2002/07/owl#Restriction"/>
    <owl:onProperty rdf:resource="https://w3id.org/omop/ontology/has_survey_source"/>
    <owl:someValuesFrom rdf:resource="https://w3id.org/omop/ontology/Concept"/>
  </rdf:Description>
  <rdf:Description rdf:nodeID="nde7e53d44aa94269b5c0c83d6d8798ccb69">
    <rdf:type rdf:resource="http://www.w3.org/2002/07/owl#Class"/>
    <owl:unionOf rdf:nodeID="nde7e53d44aa94269b5c0c83d6d8798ccb70"/>
  </rdf:Description>
  <rdf:Description rdf:nodeID="nde7e53d44aa94269b5c0c83d6d8798ccb240">
    <rdf:type rdf:resource="http://www.w3.org/2002/07/owl#Restriction"/>
    <owl:allValuesFrom rdf:resource="http://www.w3.org/2001/XMLSchema#date"/>
    <owl:onProperty rdf:resource="https://w3id.org/omop/ontology/cohort_initiation_date"/>
  </rdf:Description>
  <rdf:Description rdf:nodeID="nde7e53d44aa94269b5c0c83d6d8798ccb273">
    <rdf:first rdf:resource="https://w3id.org/omop/ontology/SurveyConduct"/>
    <rdf:rest rdf:resource="http://www.w3.org/1999/02/22-rdf-syntax-ns#nil"/>
  </rdf:Description>
  <rdf:Description rdf:nodeID="nde7e53d44aa94269b5c0c83d6d8798ccb195">
    <rdf:type rdf:resource="http://www.w3.org/2002/07/owl#Restriction"/>
    <owl:allValuesFrom rdf:resource="http://www.w3.org/2001/XMLSchema#string"/>
    <owl:onProperty rdf:resource="https://w3id.org/omop/ontology/gender_source_value"/>
  </rdf:Description>
  <rdf:Description rdf:nodeID="nde7e53d44aa94269b5c0c83d6d8798ccb296">
    <rdf:type rdf:resource="http://www.w3.org/2002/07/owl#Restriction"/>
    <owl:allValuesFrom rdf:resource="https://w3id.org/omop/ontology/Concept"/>
    <owl:onProperty rdf:resource="https://w3id.org/omop/ontology/has_source"/>
  </rdf:Description>
  <rdf:Description rdf:nodeID="nde7e53d44aa94269b5c0c83d6d8798ccb501">
    <rdf:type rdf:resource="http://www.w3.org/2002/07/owl#Restriction"/>
    <owl:allValuesFrom rdf:resource="http://www.w3.org/2001/XMLSchema#date"/>
    <owl:onProperty rdf:resource="https://w3id.org/omop/ontology/billed_date"/>
  </rdf:Description>
  <rdf:Description rdf:nodeID="nde7e53d44aa94269b5c0c83d6d8798ccb8">
    <rdf:type rdf:resource="http://www.w3.org/2000/01/rdf-schema#Datatype"/>
    <owl:unionOf rdf:nodeID="nde7e53d44aa94269b5c0c83d6d8798ccb9"/>
  </rdf:Description>
  <rdf:Description rdf:nodeID="nde7e53d44aa94269b5c0c83d6d8798ccb384">
    <rdf:type rdf:resource="http://www.w3.org/2002/07/owl#Restriction"/>
    <owl:allValuesFrom rdf:resource="http://www.w3.org/2001/XMLSchema#date"/>
    <owl:onProperty rdf:resource="https://w3id.org/omop/ontology/verbatim_end_date"/>
  </rdf:Description>
  <rdf:Description rdf:nodeID="nde7e53d44aa94269b5c0c83d6d8798ccb616">
    <rdf:type rdf:resource="http://www.w3.org/2002/07/owl#Restriction"/>
    <owl:onProperty rdf:resource="https://w3id.org/omop/ontology/has_survey"/>
    <owl:someValuesFrom rdf:resource="https://w3id.org/omop/ontology/Concept"/>
  </rdf:Description>
  <rdf:Description rdf:nodeID="nde7e53d44aa94269b5c0c83d6d8798ccb133">
    <rdf:first rdf:resource="https://w3id.org/omop/ontology/Cohort"/>
    <rdf:rest rdf:nodeID="nde7e53d44aa94269b5c0c83d6d8798ccb134"/>
  </rdf:Description>
  <rdf:Description rdf:nodeID="nde7e53d44aa94269b5c0c83d6d8798ccb662">
    <rdf:type rdf:resource="http://www.w3.org/2002/07/owl#Restriction"/>
    <owl:allValuesFrom rdf:resource="https://w3id.org/omop/ontology/DeviceExposure"/>
    <owl:onProperty rdf:resource="https://w3id.org/omop/ontology/has_device_exposure"/>
  </rdf:Description>
  <rdf:Description rdf:nodeID="nde7e53d44aa94269b5c0c83d6d8798ccb643">
    <rdf:type rdf:resource="http://www.w3.org/2002/07/owl#Restriction"/>
    <owl:allValuesFrom rdf:resource="https://w3id.org/omop/ontology/Location"/>
    <owl:onProperty rdf:resource="https://w3id.org/omop/ontology/has_location"/>
  </rdf:Description>
  <rdf:Description rdf:nodeID="nde7e53d44aa94269b5c0c83d6d8798ccb266">
    <rdf:first rdf:resource="https://w3id.org/omop/ontology/Person"/>
    <rdf:rest rdf:nodeID="nde7e53d44aa94269b5c0c83d6d8798ccb267"/>
  </rdf:Description>
  <rdf:Description rdf:nodeID="nde7e53d44aa94269b5c0c83d6d8798ccb147">
    <rdf:first rdf:resource="https://w3id.org/omop/ontology/Specimen"/>
    <rdf:rest rdf:resource="http://www.w3.org/1999/02/22-rdf-syntax-ns#nil"/>
  </rdf:Description>
  <rdf:Description rdf:nodeID="nde7e53d44aa94269b5c0c83d6d8798ccb484">
    <rdf:first rdf:resource="https://w3id.org/omop/ontology/NoteNlp"/>
    <rdf:rest rdf:nodeID="nde7e53d44aa94269b5c0c83d6d8798ccb485"/>
  </rdf:Description>
  <rdf:Description rdf:nodeID="nde7e53d44aa94269b5c0c83d6d8798ccb315">
    <owl:inverseOf rdf:resource="https://w3id.org/omop/ontology/has_visit_detail"/>
  </rdf:Description>
  <rdf:Description rdf:nodeID="nde7e53d44aa94269b5c0c83d6d8798ccb411">
    <rdf:type rdf:resource="http://www.w3.org/2002/07/owl#Restriction"/>
    <owl:allValuesFrom rdf:resource="http://www.w3.org/2001/XMLSchema#decimal"/>
    <owl:onProperty rdf:resource="https://w3id.org/omop/ontology/latitude"/>
  </rdf:Description>
  <rdf:Description rdf:nodeID="nde7e53d44aa94269b5c0c83d6d8798ccb463">
    <owl:inverseOf rdf:resource="https://w3id.org/omop/ontology/has_measurement"/>
  </rdf:Description>
  <rdf:Description rdf:nodeID="nde7e53d44aa94269b5c0c83d6d8798ccb523">
    <rdf:type rdf:resource="http://www.w3.org/2002/07/owl#Restriction"/>
    <owl:allValuesFrom rdf:resource="http://www.w3.org/2002/07/owl#Thing"/>
    <owl:onProperty rdf:resource="https://w3id.org/omop/ontology/has_event"/>
  </rdf:Description>
  <rdf:Description rdf:nodeID="nde7e53d44aa94269b5c0c83d6d8798ccb76">
    <rdf:first rdf:resource="https://w3id.org/omop/ontology/Specimen"/>
    <rdf:rest rdf:resource="http://www.w3.org/1999/02/22-rdf-syntax-ns#nil"/>
  </rdf:Description>
  <rdf:Description rdf:nodeID="nde7e53d44aa94269b5c0c83d6d8798ccb62">
    <rdf:first rdf:resource="https://w3id.org/omop/ontology/Person"/>
    <rdf:rest rdf:resource="http://www.w3.org/1999/02/22-rdf-syntax-ns#nil"/>
  </rdf:Description>
  <rdf:Description rdf:nodeID="nde7e53d44aa94269b5c0c83d6d8798ccb651">
    <rdf:type rdf:resource="http://www.w3.org/2002/07/owl#Restriction"/>
    <owl:allValuesFrom rdf:resource="https://w3id.org/omop/ontology/PayerPlanPeriod"/>
    <owl:onProperty rdf:resource="https://w3id.org/omop/ontology/has_payer_plan_period"/>
  </rdf:Description>
  <rdf:Description rdf:nodeID="nde7e53d44aa94269b5c0c83d6d8798ccb401">
    <rdf:type rdf:resource="http://www.w3.org/2002/07/owl#Restriction"/>
    <owl:onProperty rdf:resource="https://w3id.org/omop/ontology/name"/>
    <owl:someValuesFrom rdf:resource="http://www.w3.org/2001/XMLSchema#string"/>
  </rdf:Description>
  <rdf:Description rdf:nodeID="nde7e53d44aa94269b5c0c83d6d8798ccb210">
    <rdf:type rdf:resource="http://www.w3.org/2002/07/owl#Restriction"/>
    <owl:allValuesFrom rdf:resource="http://www.w3.org/2001/XMLSchema#string"/>
    <owl:onProperty rdf:resource="https://w3id.org/omop/ontology/source_value"/>
  </rdf:Description>
  <rdf:Description rdf:nodeID="nde7e53d44aa94269b5c0c83d6d8798ccb229">
    <rdf:first rdf:resource="https://w3id.org/omop/ontology/Concept"/>
    <rdf:rest rdf:nodeID="nde7e53d44aa94269b5c0c83d6d8798ccb230"/>
  </rdf:Description>
  <rdf:Description rdf:nodeID="nde7e53d44aa94269b5c0c83d6d8798ccb362">
    <rdf:first rdf:resource="https://w3id.org/omop/ontology/Note"/>
    <rdf:rest rdf:nodeID="nde7e53d44aa94269b5c0c83d6d8798ccb363"/>
  </rdf:Description>
  <rdf:Description rdf:nodeID="nde7e53d44aa94269b5c0c83d6d8798ccb254">
    <rdf:type rdf:resource="http://www.w3.org/2002/07/owl#Restriction"/>
    <owl:onProperty rdf:resource="https://w3id.org/omop/ontology/source_code"/>
    <owl:someValuesFrom rdf:resource="http://www.w3.org/2001/XMLSchema#string"/>
  </rdf:Description>
  <rdf:Description rdf:nodeID="nde7e53d44aa94269b5c0c83d6d8798ccb255">
    <rdf:type rdf:resource="http://www.w3.org/2002/07/owl#Restriction"/>
    <owl:allValuesFrom rdf:resource="http://www.w3.org/2001/XMLSchema#string"/>
    <owl:onProperty rdf:resource="https://w3id.org/omop/ontology/source_code_description"/>
  </rdf:Description>
  <rdf:Description rdf:nodeID="nde7e53d44aa94269b5c0c83d6d8798ccb90">
    <rdf:type rdf:resource="http://www.w3.org/2002/07/owl#Restriction"/>
    <owl:onProperty rdf:resource="https://w3id.org/omop/ontology/name"/>
    <owl:someValuesFrom rdf:resource="http://www.w3.org/2001/XMLSchema#string"/>
  </rdf:Description>
  <rdf:Description rdf:nodeID="nde7e53d44aa94269b5c0c83d6d8798ccb620">
    <rdf:type rdf:resource="http://www.w3.org/2002/07/owl#Restriction"/>
    <owl:onProperty rdf:resource="https://w3id.org/omop/ontology/has_assisted"/>
    <owl:someValuesFrom rdf:resource="https://w3id.org/omop/ontology/Concept"/>
  </rdf:Description>
  <rdf:Description rdf:nodeID="nde7e53d44aa94269b5c0c83d6d8798ccb538">
    <rdf:type rdf:resource="http://www.w3.org/2002/07/owl#Restriction"/>
    <owl:allValuesFrom rdf:resource="https://w3id.org/omop/ontology/Concept"/>
    <owl:onProperty rdf:resource="https://w3id.org/omop/ontology/has_sponsor_source"/>
  </rdf:Description>
  <rdf:Description rdf:nodeID="nde7e53d44aa94269b5c0c83d6d8798ccb634">
    <rdf:first rdf:resource="https://w3id.org/omop/ontology/ConceptSynonym"/>
    <rdf:rest rdf:nodeID="nde7e53d44aa94269b5c0c83d6d8798ccb635"/>
  </rdf:Description>
  <rdf:Description rdf:nodeID="nde7e53d44aa94269b5c0c83d6d8798ccb459">
    <rdf:type rdf:resource="http://www.w3.org/2002/07/owl#Restriction"/>
    <owl:allValuesFrom rdf:resource="http://www.w3.org/2001/XMLSchema#string"/>
    <owl:onProperty rdf:resource="https://w3id.org/omop/ontology/value_source_value"/>
  </rdf:Description>
  <rdf:Description rdf:nodeID="nde7e53d44aa94269b5c0c83d6d8798ccb36">
    <rdf:type rdf:resource="http://www.w3.org/2002/07/owl#Class"/>
    <owl:unionOf rdf:nodeID="nde7e53d44aa94269b5c0c83d6d8798ccb37"/>
  </rdf:Description>
  <rdf:Description rdf:nodeID="nde7e53d44aa94269b5c0c83d6d8798ccb339">
    <rdf:type rdf:resource="http://www.w3.org/2002/07/owl#Restriction"/>
    <owl:allValuesFrom rdf:resource="http://www.w3.org/2001/XMLSchema#string"/>
    <owl:onProperty rdf:resource="https://w3id.org/omop/ontology/system"/>
  </rdf:Description>
  <rdf:Description rdf:nodeID="nde7e53d44aa94269b5c0c83d6d8798ccb60">
    <rdf:type rdf:resource="http://www.w3.org/2002/07/owl#Class"/>
    <owl:unionOf rdf:nodeID="nde7e53d44aa94269b5c0c83d6d8798ccb61"/>
  </rdf:Description>
  <rdf:Description rdf:nodeID="nde7e53d44aa94269b5c0c83d6d8798ccb386">
    <rdf:type rdf:resource="http://www.w3.org/2002/07/owl#Restriction"/>
    <owl:allValuesFrom rdf:resource="http://www.w3.org/2001/XMLSchema#string"/>
    <owl:onProperty rdf:resource="https://w3id.org/omop/ontology/source_value"/>
  </rdf:Description>
  <rdf:Description rdf:nodeID="nde7e53d44aa94269b5c0c83d6d8798ccb566">
    <rdf:first rdf:resource="https://w3id.org/omop/ontology/Observation"/>
    <rdf:rest rdf:nodeID="nde7e53d44aa94269b5c0c83d6d8798ccb567"/>
  </rdf:Description>
  <rdf:Description rdf:nodeID="nde7e53d44aa94269b5c0c83d6d8798ccb462">
    <rdf:type rdf:resource="http://www.w3.org/2002/07/owl#Restriction"/>
    <owl:onProperty rdf:nodeID="nde7e53d44aa94269b5c0c83d6d8798ccb463"/>
    <owl:someValuesFrom rdf:resource="https://w3id.org/omop/ontology/Person"/>
  </rdf:Description>
  <rdf:Description rdf:nodeID="nde7e53d44aa94269b5c0c83d6d8798ccb503">
    <rdf:type rdf:resource="http://www.w3.org/2002/07/owl#Restriction"/>
    <owl:onProperty rdf:nodeID="nde7e53d44aa94269b5c0c83d6d8798ccb504"/>
    <owl:someValuesFrom rdf:resource="https://w3id.org/omop/ontology/Person"/>
  </rdf:Description>
  <rdf:Description rdf:nodeID="nde7e53d44aa94269b5c0c83d6d8798ccb294">
    <rdf:type rdf:resource="http://www.w3.org/2002/07/owl#Restriction"/>
    <owl:allValuesFrom rdf:resource="http://www.w3.org/2001/XMLSchema#string"/>
    <owl:onProperty rdf:resource="https://w3id.org/omop/ontology/status_source_value"/>
  </rdf:Description>
  <rdf:Description rdf:nodeID="nde7e53d44aa94269b5c0c83d6d8798ccb292">
    <rdf:type rdf:resource="http://www.w3.org/2002/07/owl#Restriction"/>
    <owl:onProperty rdf:resource="https://w3id.org/omop/ontology/has_type"/>
    <owl:someValuesFrom rdf:resource="https://w3id.org/omop/ontology/Concept"/>
  </rdf:Description>
  <rdf:Description rdf:nodeID="nde7e53d44aa94269b5c0c83d6d8798ccb64">
    <rdf:first rdf:resource="https://w3id.org/omop/ontology/BaseVisit"/>
    <rdf:rest rdf:nodeID="nde7e53d44aa94269b5c0c83d6d8798ccb65"/>
  </rdf:Description>
  <rdf:Description rdf:nodeID="nde7e53d44aa94269b5c0c83d6d8798ccb611">
    <rdf:type rdf:resource="http://www.w3.org/2002/07/owl#Restriction"/>
    <owl:allValuesFrom rdf:resource="https://w3id.org/omop/ontology/Concept"/>
    <owl:onProperty rdf:resource="https://w3id.org/omop/ontology/has_collection_method"/>
  </rdf:Description>
  <rdf:Description rdf:nodeID="nde7e53d44aa94269b5c0c83d6d8798ccb545">
    <owl:inverseOf rdf:resource="https://w3id.org/omop/ontology/has_payer_plan_period"/>
  </rdf:Description>
  <rdf:Description rdf:nodeID="nde7e53d44aa94269b5c0c83d6d8798ccb225">
    <rdf:type rdf:resource="http://www.w3.org/2002/07/owl#Restriction"/>
    <owl:allValuesFrom rdf:resource="http://www.w3.org/2001/XMLSchema#string"/>
    <owl:onProperty rdf:resource="https://w3id.org/omop/ontology/place_of_service_source_value"/>
  </rdf:Description>
  <rdf:Description rdf:nodeID="nde7e53d44aa94269b5c0c83d6d8798ccb629">
    <rdf:first rdf:resource="https://w3id.org/omop/ontology/ProcedureOccurrence"/>
    <rdf:rest rdf:nodeID="nde7e53d44aa94269b5c0c83d6d8798ccb630"/>
  </rdf:Description>
  <rdf:Description rdf:nodeID="nde7e53d44aa94269b5c0c83d6d8798ccb291">
    <owl:inverseOf rdf:resource="https://w3id.org/omop/ontology/has_condition_occurrence"/>
  </rdf:Description>
  <rdf:Description rdf:nodeID="nde7e53d44aa94269b5c0c83d6d8798ccb422">
    <rdf:type rdf:resource="http://www.w3.org/2002/07/owl#Restriction"/>
    <owl:allValuesFrom rdf:resource="http://www.w3.org/2001/XMLSchema#string"/>
    <owl:onProperty rdf:resource="https://w3id.org/omop/ontology/source_value"/>
  </rdf:Description>
  <rdf:Description rdf:nodeID="nde7e53d44aa94269b5c0c83d6d8798ccb655">
    <rdf:type rdf:resource="http://www.w3.org/2002/07/owl#Restriction"/>
    <owl:allValuesFrom rdf:resource="https://w3id.org/omop/ontology/ConditionOccurrence"/>
    <owl:onProperty rdf:resource="https://w3id.org/omop/ontology/has_condition_occurrence"/>
  </rdf:Description>
  <rdf:Description rdf:nodeID="nde7e53d44aa94269b5c0c83d6d8798ccb364">
    <rdf:first rdf:resource="https://w3id.org/omop/ontology/Specimen"/>
    <rdf:rest rdf:nodeID="nde7e53d44aa94269b5c0c83d6d8798ccb365"/>
  </rdf:Description>
  <rdf:Description rdf:nodeID="nde7e53d44aa94269b5c0c83d6d8798ccb139">
    <rdf:first rdf:resource="https://w3id.org/omop/ontology/DrugStrength"/>
    <rdf:rest rdf:nodeID="nde7e53d44aa94269b5c0c83d6d8798ccb140"/>
  </rdf:Description>
  <rdf:Description rdf:nodeID="nde7e53d44aa94269b5c0c83d6d8798ccb230">
    <rdf:first rdf:resource="https://w3id.org/omop/ontology/SourceToConceptMap"/>
    <rdf:rest rdf:nodeID="nde7e53d44aa94269b5c0c83d6d8798ccb231"/>
  </rdf:Description>
  <rdf:Description rdf:nodeID="nde7e53d44aa94269b5c0c83d6d8798ccb10">
    <rdf:first rdf:resource="http://www.w3.org/2001/XMLSchema#string"/>
    <rdf:rest rdf:resource="http://www.w3.org/1999/02/22-rdf-syntax-ns#nil"/>
  </rdf:Description>
  <rdf:Description rdf:nodeID="nde7e53d44aa94269b5c0c83d6d8798ccb78">
    <rdf:first rdf:resource="https://w3id.org/omop/ontology/Provider"/>
    <rdf:rest rdf:nodeID="nde7e53d44aa94269b5c0c83d6d8798ccb79"/>
  </rdf:Description>
  <rdf:Description rdf:nodeID="nde7e53d44aa94269b5c0c83d6d8798ccb417">
    <rdf:type rdf:resource="http://www.w3.org/2002/07/owl#Restriction"/>
    <owl:allValuesFrom rdf:resource="https://w3id.org/omop/ontology/Concept"/>
    <owl:onProperty rdf:resource="https://w3id.org/omop/ontology/has_event_field"/>
  </rdf:Description>
  <rdf:Description rdf:nodeID="nde7e53d44aa94269b5c0c83d6d8798ccb687">
    <rdf:type rdf:resource="http://www.w3.org/2002/07/owl#Restriction"/>
    <owl:onProperty rdf:resource="https://w3id.org/omop/ontology/has_class"/>
    <owl:someValuesFrom rdf:resource="https://w3id.org/omop/ontology/ConceptClass"/>
  </rdf:Description>
  <rdf:Description rdf:nodeID="nde7e53d44aa94269b5c0c83d6d8798ccb281">
    <rdf:type rdf:resource="http://www.w3.org/2002/07/owl#Restriction"/>
    <owl:allValuesFrom rdf:resource="http://www.w3.org/2001/XMLSchema#string"/>
    <owl:onProperty rdf:resource="https://w3id.org/omop/ontology/cdm_holder"/>
  </rdf:Description>
  <rdf:Description rdf:nodeID="nde7e53d44aa94269b5c0c83d6d8798ccb53">
    <rdf:first rdf:resource="https://w3id.org/omop/ontology/Person"/>
    <rdf:rest rdf:resource="http://www.w3.org/1999/02/22-rdf-syntax-ns#nil"/>
  </rdf:Description>
  <rdf:Description rdf:nodeID="nde7e53d44aa94269b5c0c83d6d8798ccb483">
    <rdf:first rdf:resource="https://w3id.org/omop/ontology/ConditionOccurrence"/>
    <rdf:rest rdf:nodeID="nde7e53d44aa94269b5c0c83d6d8798ccb484"/>
  </rdf:Description>
  <rdf:Description rdf:nodeID="nde7e53d44aa94269b5c0c83d6d8798ccb311">
    <owl:inverseOf rdf:resource="https://w3id.org/omop/ontology/has_procedure_occurrence"/>
  </rdf:Description>
  <rdf:Description rdf:nodeID="nde7e53d44aa94269b5c0c83d6d8798ccb685">
    <rdf:type rdf:resource="http://www.w3.org/2002/07/owl#Restriction"/>
    <owl:allValuesFrom rdf:resource="http://www.w3.org/2001/XMLSchema#string"/>
    <owl:onProperty rdf:resource="https://w3id.org/omop/ontology/name"/>
  </rdf:Description>
  <rdf:Description rdf:nodeID="nde7e53d44aa94269b5c0c83d6d8798ccb639">
    <rdf:first rdf:resource="https://w3id.org/omop/ontology/Measurement"/>
    <rdf:rest rdf:resource="http://www.w3.org/1999/02/22-rdf-syntax-ns#nil"/>
  </rdf:Description>
  <rdf:Description rdf:nodeID="nde7e53d44aa94269b5c0c83d6d8798ccb173">
    <rdf:first rdf:resource="https://w3id.org/omop/ontology/DoseEra"/>
    <rdf:rest rdf:nodeID="nde7e53d44aa94269b5c0c83d6d8798ccb174"/>
  </rdf:Description>
  <rdf:Description rdf:nodeID="nde7e53d44aa94269b5c0c83d6d8798ccb363">
    <rdf:first rdf:resource="https://w3id.org/omop/ontology/ConditionOccurrence"/>
    <rdf:rest rdf:nodeID="nde7e53d44aa94269b5c0c83d6d8798ccb364"/>
  </rdf:Description>
  <rdf:Description rdf:nodeID="nde7e53d44aa94269b5c0c83d6d8798ccb125">
    <rdf:type rdf:resource="http://www.w3.org/2002/07/owl#Class"/>
    <owl:unionOf rdf:nodeID="nde7e53d44aa94269b5c0c83d6d8798ccb126"/>
  </rdf:Description>
  <rdf:Description rdf:nodeID="nde7e53d44aa94269b5c0c83d6d8798ccb579">
    <rdf:first rdf:resource="https://w3id.org/omop/ontology/ConceptSynonym"/>
    <rdf:rest rdf:nodeID="nde7e53d44aa94269b5c0c83d6d8798ccb580"/>
  </rdf:Description>
  <rdf:Description rdf:nodeID="nde7e53d44aa94269b5c0c83d6d8798ccb221">
    <rdf:type rdf:resource="http://www.w3.org/2002/07/owl#Restriction"/>
    <owl:allValuesFrom rdf:resource="http://www.w3.org/2001/XMLSchema#string"/>
    <owl:onProperty rdf:resource="https://w3id.org/omop/ontology/source_value"/>
  </rdf:Description>
  <rdf:Description rdf:nodeID="nde7e53d44aa94269b5c0c83d6d8798ccb119">
    <rdf:first rdf:resource="https://w3id.org/omop/ontology/Note"/>
    <rdf:rest rdf:nodeID="nde7e53d44aa94269b5c0c83d6d8798ccb120"/>
  </rdf:Description>
  <rdf:Description rdf:nodeID="nde7e53d44aa94269b5c0c83d6d8798ccb127">
    <rdf:first rdf:resource="https://w3id.org/omop/ontology/LocationHistory"/>
    <rdf:rest rdf:nodeID="nde7e53d44aa94269b5c0c83d6d8798ccb128"/>
  </rdf:Description>
  <rdf:Description rdf:nodeID="nde7e53d44aa94269b5c0c83d6d8798ccb491">
    <rdf:first rdf:resource="https://w3id.org/omop/ontology/Measurement"/>
    <rdf:rest rdf:resource="http://www.w3.org/1999/02/22-rdf-syntax-ns#nil"/>
  </rdf:Description>
  <rdf:Description rdf:nodeID="nde7e53d44aa94269b5c0c83d6d8798ccb99">
    <owl:inverseOf rdf:resource="https://w3id.org/omop/ontology/has_drug_era"/>
  </rdf:Description>
  <rdf:Description rdf:nodeID="nde7e53d44aa94269b5c0c83d6d8798ccb39">
    <rdf:type rdf:resource="http://www.w3.org/2002/07/owl#Class"/>
    <owl:unionOf rdf:nodeID="nde7e53d44aa94269b5c0c83d6d8798ccb40"/>
  </rdf:Description>
  <rdf:Description rdf:nodeID="nde7e53d44aa94269b5c0c83d6d8798ccb98">
    <rdf:type rdf:resource="http://www.w3.org/2002/07/owl#Restriction"/>
    <owl:onProperty rdf:nodeID="nde7e53d44aa94269b5c0c83d6d8798ccb99"/>
    <owl:someValuesFrom rdf:resource="https://w3id.org/omop/ontology/Person"/>
  </rdf:Description>
  <rdf:Description rdf:nodeID="nde7e53d44aa94269b5c0c83d6d8798ccb191">
    <rdf:type rdf:resource="http://www.w3.org/2002/07/owl#Restriction"/>
    <owl:allValuesFrom rdf:resource="http://www.w3.org/2001/XMLSchema#string"/>
    <owl:onProperty rdf:resource="https://w3id.org/omop/ontology/cause_source_value"/>
  </rdf:Description>
  <rdf:Description rdf:nodeID="nde7e53d44aa94269b5c0c83d6d8798ccb77">
    <rdf:type rdf:resource="http://www.w3.org/2002/07/owl#Class"/>
    <owl:unionOf rdf:nodeID="nde7e53d44aa94269b5c0c83d6d8798ccb78"/>
  </rdf:Description>
  <rdf:Description rdf:nodeID="nde7e53d44aa94269b5c0c83d6d8798ccb6">
    <rdf:first rdf:resource="https://w3id.org/omop/ontology/BaseVisit"/>
    <rdf:rest rdf:nodeID="nde7e53d44aa94269b5c0c83d6d8798ccb7"/>
  </rdf:Description>
  <rdf:Description rdf:nodeID="nde7e53d44aa94269b5c0c83d6d8798ccb247">
    <rdf:type rdf:resource="http://www.w3.org/2002/07/owl#Restriction"/>
    <owl:allValuesFrom rdf:resource="http://www.w3.org/2001/XMLSchema#date"/>
    <owl:onProperty rdf:resource="https://w3id.org/omop/ontology/start_date"/>
  </rdf:Description>
  <rdf:Description rdf:nodeID="nde7e53d44aa94269b5c0c83d6d8798ccb41">
    <rdf:first rdf:resource="https://w3id.org/omop/ontology/Person"/>
    <rdf:rest rdf:resource="http://www.w3.org/1999/02/22-rdf-syntax-ns#nil"/>
  </rdf:Description>
  <rdf:Description rdf:nodeID="nde7e53d44aa94269b5c0c83d6d8798ccb589">
    <rdf:first rdf:resource="http://www.w3.org/2001/XMLSchema#integer"/>
    <rdf:rest rdf:nodeID="nde7e53d44aa94269b5c0c83d6d8798ccb590"/>
  </rdf:Description>
  <rdf:Description rdf:nodeID="nde7e53d44aa94269b5c0c83d6d8798ccb284">
    <rdf:type rdf:resource="http://www.w3.org/2002/07/owl#Restriction"/>
    <owl:allValuesFrom rdf:resource="http://www.w3.org/2001/XMLSchema#date"/>
    <owl:onProperty rdf:resource="https://w3id.org/omop/ontology/source_release_date"/>
  </rdf:Description>
  <rdf:Description rdf:nodeID="nde7e53d44aa94269b5c0c83d6d8798ccb42">
    <rdf:type rdf:resource="http://www.w3.org/2002/07/owl#Class"/>
    <owl:unionOf rdf:nodeID="nde7e53d44aa94269b5c0c83d6d8798ccb43"/>
  </rdf:Description>
  <rdf:Description rdf:nodeID="nde7e53d44aa94269b5c0c83d6d8798ccb675">
    <rdf:type rdf:resource="http://www.w3.org/2002/07/owl#Restriction"/>
    <owl:allValuesFrom rdf:resource="http://www.w3.org/2001/XMLSchema#string"/>
    <owl:onProperty rdf:resource="https://w3id.org/omop/ontology/ethnicity_source_value"/>
  </rdf:Description>
  <rdf:Description rdf:nodeID="nde7e53d44aa94269b5c0c83d6d8798ccb637">
    <rdf:first rdf:resource="https://w3id.org/omop/ontology/Exposure"/>
    <rdf:rest rdf:nodeID="nde7e53d44aa94269b5c0c83d6d8798ccb638"/>
  </rdf:Description>
  <rdf:Description rdf:nodeID="nde7e53d44aa94269b5c0c83d6d8798ccb59">
    <rdf:first rdf:resource="https://w3id.org/omop/ontology/Person"/>
    <rdf:rest rdf:resource="http://www.w3.org/1999/02/22-rdf-syntax-ns#nil"/>
  </rdf:Description>
  <rdf:Description rdf:nodeID="nde7e53d44aa94269b5c0c83d6d8798ccb527">
    <rdf:type rdf:resource="http://www.w3.org/2002/07/owl#Restriction"/>
    <owl:allValuesFrom rdf:resource="http://www.w3.org/2001/XMLSchema#string"/>
    <owl:onProperty rdf:resource="https://w3id.org/omop/ontology/source_value"/>
  </rdf:Description>
  <rdf:Description rdf:nodeID="nde7e53d44aa94269b5c0c83d6d8798ccb632">
    <rdf:first rdf:resource="https://w3id.org/omop/ontology/DrugStrength"/>
    <rdf:rest rdf:nodeID="nde7e53d44aa94269b5c0c83d6d8798ccb633"/>
  </rdf:Description>
  <rdf:Description rdf:nodeID="nde7e53d44aa94269b5c0c83d6d8798ccb68">
    <rdf:first rdf:resource="https://w3id.org/omop/ontology/Person"/>
    <rdf:rest rdf:resource="http://www.w3.org/1999/02/22-rdf-syntax-ns#nil"/>
  </rdf:Description>
  <rdf:Description rdf:nodeID="nde7e53d44aa94269b5c0c83d6d8798ccb567">
    <rdf:first rdf:resource="https://w3id.org/omop/ontology/BaseVisit"/>
    <rdf:rest rdf:nodeID="nde7e53d44aa94269b5c0c83d6d8798ccb568"/>
  </rdf:Description>
  <rdf:Description rdf:nodeID="nde7e53d44aa94269b5c0c83d6d8798ccb213">
    <rdf:type rdf:resource="http://www.w3.org/2002/07/owl#Restriction"/>
    <owl:onProperty rdf:resource="https://w3id.org/omop/ontology/name"/>
    <owl:someValuesFrom rdf:resource="http://www.w3.org/2001/XMLSchema#string"/>
  </rdf:Description>
  <rdf:Description rdf:nodeID="nde7e53d44aa94269b5c0c83d6d8798ccb272">
    <rdf:first rdf:resource="https://w3id.org/omop/ontology/Measurement"/>
    <rdf:rest rdf:nodeID="nde7e53d44aa94269b5c0c83d6d8798ccb273"/>
  </rdf:Description>
  <rdf:Description rdf:nodeID="nde7e53d44aa94269b5c0c83d6d8798ccb481">
    <rdf:type rdf:resource="http://www.w3.org/2002/07/owl#Class"/>
    <owl:unionOf rdf:nodeID="nde7e53d44aa94269b5c0c83d6d8798ccb482"/>
  </rdf:Description>
  <rdf:Description rdf:nodeID="nde7e53d44aa94269b5c0c83d6d8798ccb151">
    <rdf:type rdf:resource="http://www.w3.org/2002/07/owl#Restriction"/>
    <owl:allValuesFrom rdf:resource="http://www.w3.org/2002/07/owl#Thing"/>
    <owl:onProperty rdf:resource="https://w3id.org/omop/ontology/has_unique_device"/>
  </rdf:Description>
  <rdf:Description rdf:nodeID="nde7e53d44aa94269b5c0c83d6d8798ccb371">
    <rdf:first rdf:resource="https://w3id.org/omop/ontology/BasePerson"/>
    <rdf:rest rdf:nodeID="nde7e53d44aa94269b5c0c83d6d8798ccb372"/>
  </rdf:Description>
  <rdf:Description rdf:nodeID="nde7e53d44aa94269b5c0c83d6d8798ccb94">
    <owl:inverseOf rdf:resource="https://w3id.org/omop/ontology/has_dose_era"/>
  </rdf:Description>
  <rdf:Description rdf:nodeID="nde7e53d44aa94269b5c0c83d6d8798ccb650">
    <rdf:type rdf:resource="http://www.w3.org/2002/07/owl#Restriction"/>
    <owl:allValuesFrom rdf:resource="https://w3id.org/omop/ontology/Observation"/>
    <owl:onProperty rdf:resource="https://w3id.org/omop/ontology/has_observation"/>
  </rdf:Description>
  <rdf:Description rdf:nodeID="nde7e53d44aa94269b5c0c83d6d8798ccb30">
    <owl:inverseOf rdf:resource="https://w3id.org/omop/ontology/has_observation_period"/>
  </rdf:Description>
  <rdf:Description rdf:nodeID="nde7e53d44aa94269b5c0c83d6d8798ccb140">
    <rdf:first rdf:resource="https://w3id.org/omop/ontology/Concept"/>
    <rdf:rest rdf:nodeID="nde7e53d44aa94269b5c0c83d6d8798ccb141"/>
  </rdf:Description>
  <rdf:Description rdf:nodeID="nde7e53d44aa94269b5c0c83d6d8798ccb415">
    <rdf:type rdf:resource="http://www.w3.org/2002/07/owl#Restriction"/>
    <owl:allValuesFrom rdf:resource="http://www.w3.org/2001/XMLSchema#string"/>
    <owl:onProperty rdf:resource="https://w3id.org/omop/ontology/source_value"/>
  </rdf:Description>
  <rdf:Description rdf:nodeID="nde7e53d44aa94269b5c0c83d6d8798ccb238">
    <rdf:type rdf:resource="http://www.w3.org/2002/07/owl#Restriction"/>
    <owl:allValuesFrom rdf:resource="http://www.w3.org/2001/XMLSchema#string"/>
    <owl:onProperty rdf:resource="https://w3id.org/omop/ontology/syntax"/>
  </rdf:Description>
  <rdf:Description rdf:nodeID="nde7e53d44aa94269b5c0c83d6d8798ccb449">
    <rdf:type rdf:resource="http://www.w3.org/2002/07/owl#Restriction"/>
    <owl:allValuesFrom rdf:resource="http://www.w3.org/2001/XMLSchema#string"/>
    <owl:onProperty rdf:resource="https://w3id.org/omop/ontology/source_value"/>
  </rdf:Description>
  <rdf:Description rdf:nodeID="nde7e53d44aa94269b5c0c83d6d8798ccb661">
    <rdf:type rdf:resource="http://www.w3.org/2002/07/owl#Restriction"/>
    <owl:allValuesFrom rdf:resource="http://www.w3.org/2001/XMLSchema#dateTime"/>
    <owl:onProperty rdf:resource="https://w3id.org/omop/ontology/death_datetime"/>
  </rdf:Description>
  <rdf:Description rdf:nodeID="nde7e53d44aa94269b5c0c83d6d8798ccb360">
    <rdf:type rdf:resource="http://www.w3.org/2002/07/owl#Class"/>
    <owl:unionOf rdf:nodeID="nde7e53d44aa94269b5c0c83d6d8798ccb361"/>
  </rdf:Description>
  <rdf:Description rdf:nodeID="nde7e53d44aa94269b5c0c83d6d8798ccb627">
    <rdf:first rdf:resource="https://w3id.org/omop/ontology/ConceptClass"/>
    <rdf:rest rdf:nodeID="nde7e53d44aa94269b5c0c83d6d8798ccb628"/>
  </rdf:Description>
  <rdf:Description rdf:nodeID="nde7e53d44aa94269b5c0c83d6d8798ccb52">
    <rdf:first rdf:resource="https://w3id.org/omop/ontology/BaseVisit"/>
    <rdf:rest rdf:nodeID="nde7e53d44aa94269b5c0c83d6d8798ccb53"/>
  </rdf:Description>
  <rdf:Description rdf:nodeID="nde7e53d44aa94269b5c0c83d6d8798ccb226">
    <rdf:type rdf:resource="http://www.w3.org/2002/07/owl#Restriction"/>
    <owl:allValuesFrom rdf:resource="http://www.w3.org/2001/XMLSchema#string"/>
    <owl:onProperty rdf:resource="https://w3id.org/omop/ontology/name"/>
  </rdf:Description>
  <rdf:Description rdf:nodeID="nde7e53d44aa94269b5c0c83d6d8798ccb590">
    <rdf:first rdf:resource="http://www.w3.org/2001/XMLSchema#string"/>
    <rdf:rest rdf:resource="http://www.w3.org/1999/02/22-rdf-syntax-ns#nil"/>
  </rdf:Description>
  <rdf:Description rdf:nodeID="nde7e53d44aa94269b5c0c83d6d8798ccb28">
    <owl:inverseOf rdf:resource="https://w3id.org/omop/ontology/has_condition_era"/>
  </rdf:Description>
  <rdf:Description rdf:nodeID="nde7e53d44aa94269b5c0c83d6d8798ccb345">
    <owl:inverseOf rdf:resource="https://w3id.org/omop/ontology/has_note_nlp"/>
  </rdf:Description>
  <rdf:Description rdf:nodeID="nde7e53d44aa94269b5c0c83d6d8798ccb677">
    <rdf:type rdf:resource="http://www.w3.org/2002/07/owl#Restriction"/>
    <owl:onProperty rdf:resource="https://w3id.org/omop/ontology/has_vocabulary"/>
    <owl:someValuesFrom rdf:resource="https://w3id.org/omop/ontology/Vocabulary"/>
  </rdf:Description>
  <rdf:Description rdf:nodeID="nde7e53d44aa94269b5c0c83d6d8798ccb623">
    <rdf:first rdf:resource="https://w3id.org/omop/ontology/ConditionOccurrence"/>
    <rdf:rest rdf:nodeID="nde7e53d44aa94269b5c0c83d6d8798ccb624"/>
  </rdf:Description>
  <rdf:Description rdf:nodeID="nde7e53d44aa94269b5c0c83d6d8798ccb361">
    <rdf:first rdf:resource="https://w3id.org/omop/ontology/CareSite"/>
    <rdf:rest rdf:nodeID="nde7e53d44aa94269b5c0c83d6d8798ccb362"/>
  </rdf:Description>
  <rdf:Description rdf:nodeID="nde7e53d44aa94269b5c0c83d6d8798ccb394">
    <owl:inverseOf rdf:resource="https://w3id.org/omop/ontology/has_specimen"/>
  </rdf:Description>
  <rdf:Description rdf:nodeID="nde7e53d44aa94269b5c0c83d6d8798ccb66">
    <rdf:type rdf:resource="http://www.w3.org/2002/07/owl#Class"/>
    <owl:unionOf rdf:nodeID="nde7e53d44aa94269b5c0c83d6d8798ccb67"/>
  </rdf:Description>
  <rdf:Description rdf:nodeID="nde7e53d44aa94269b5c0c83d6d8798ccb359">
    <owl:inverseOf rdf:resource="https://w3id.org/omop/ontology/has_visit_occurrence"/>
  </rdf:Description>
  <rdf:Description rdf:nodeID="nde7e53d44aa94269b5c0c83d6d8798ccb17">
    <rdf:type rdf:resource="http://www.w3.org/2002/07/owl#Class"/>
    <owl:unionOf rdf:nodeID="nde7e53d44aa94269b5c0c83d6d8798ccb18"/>
  </rdf:Description>
  <rdf:Description rdf:nodeID="nde7e53d44aa94269b5c0c83d6d8798ccb490">
    <rdf:first rdf:resource="https://w3id.org/omop/ontology/Exposure"/>
    <rdf:rest rdf:nodeID="nde7e53d44aa94269b5c0c83d6d8798ccb491"/>
  </rdf:Description>
  <rdf:Description rdf:nodeID="nde7e53d44aa94269b5c0c83d6d8798ccb377">
    <owl:inverseOf rdf:resource="https://w3id.org/omop/ontology/has_drug_exposure"/>
  </rdf:Description>
  <rdf:Description rdf:nodeID="nde7e53d44aa94269b5c0c83d6d8798ccb172">
    <rdf:first rdf:resource="https://w3id.org/omop/ontology/Observation"/>
    <rdf:rest rdf:nodeID="nde7e53d44aa94269b5c0c83d6d8798ccb173"/>
  </rdf:Description>
  <rdf:Description rdf:nodeID="nde7e53d44aa94269b5c0c83d6d8798ccb562">
    <rdf:first rdf:resource="https://w3id.org/omop/ontology/ConditionOccurrence"/>
    <rdf:rest rdf:nodeID="nde7e53d44aa94269b5c0c83d6d8798ccb563"/>
  </rdf:Description>
</rdf:RDF>
